<?xml version="1.0"?>
<rdf:RDF xmlns="http://www.ease-crc.org/ont/SOMA-HOME.owl#"
     xml:base="http://www.ease-crc.org/ont/SOMA-HOME.owl"
     xmlns:owl="http://www.w3.org/2002/07/owl#"
     xmlns:rdf="http://www.w3.org/1999/02/22-rdf-syntax-ns#"
     xmlns:xml="http://www.w3.org/XML/1998/namespace"
     xmlns:xsd="http://www.w3.org/2001/XMLSchema#"
     xmlns:SOMA="http://www.ease-crc.org/ont/SOMA.owl#"
     xmlns:rdfs="http://www.w3.org/2000/01/rdf-schema#">
    <owl:Ontology rdf:about="http://www.ease-crc.org/ont/SOMA-HOME.owl">
        <owl:imports rdf:resource="http://www.ease-crc.org/ont/DUL.owl"/>
        <owl:imports rdf:resource="http://www.ease-crc.org/ont/SOMA.owl"/>
        <owl:versionInfo>current</owl:versionInfo>
    </owl:Ontology>
    


    <!-- 
    ///////////////////////////////////////////////////////////////////////////////////////
    //
    // Object Properties
    //
    ///////////////////////////////////////////////////////////////////////////////////////
     -->


    


    <!-- http://www.ease-crc.org/ont/SOMA-ACT.owl#causes -->


    <owl:ObjectProperty rdf:about="http://www.ease-crc.org/ont/SOMA-ACT.owl#causes">
        <rdfs:subPropertyOf rdf:resource="http://www.ontologydesignpatterns.org/ont/dul/DUL.owl#precedes"/>
        <rdf:type rdf:resource="http://www.w3.org/2002/07/owl#TransitiveProperty"/>
        <rdfs:isDefinedBy rdf:resource="http://www.ease-crc.org/ont/SOMA-ACT.owl"/>
        <rdfs:label xml:lang="en">Simple relationship between two actions to express that the object (the reaction) would not have occured if it were not for the subject (the cause), e.g., a Communication Action classified as an Querying Task causes another Communication Task classified as an Answering Task and the latter would not have occured without the former. An example without Agents involved would be some domino stone would not have toppled without the first one toppling.

When Agents are involved, the relation might be seen as an abstraction of the execution of some plan that arises from changing the agents goal that is due to perceiving the cause. However, currently it is unclear how to model such a pattern and therefore not included in SOMA.

This relation is seen as transitive.</rdfs:label>
        <rdfs:label xml:lang="en">causes</rdfs:label>
    </owl:ObjectProperty>
    


    <!-- http://www.ease-crc.org/ont/SOMA-ACT.owl#directlyCauses -->


    <owl:ObjectProperty rdf:about="http://www.ease-crc.org/ont/SOMA-ACT.owl#directlyCauses">
        <rdfs:subPropertyOf rdf:resource="http://www.ease-crc.org/ont/SOMA-ACT.owl#causes"/>
        <owl:inverseOf rdf:resource="http://www.ease-crc.org/ont/SOMA-ACT.owl#isDirectReactionTo"/>
        <rdfs:domain rdf:resource="http://www.ontologydesignpatterns.org/ont/dul/DUL.owl#Event"/>
        <rdfs:range rdf:resource="http://www.ontologydesignpatterns.org/ont/dul/DUL.owl#Event"/>
        <rdfs:comment xml:lang="en">Non-transitive version of &quot;causes&quot;.</rdfs:comment>
        <rdfs:isDefinedBy rdf:resource="http://www.ease-crc.org/ont/SOMA-ACT.owl"/>
        <rdfs:label xml:lang="en">directly causes</rdfs:label>
    </owl:ObjectProperty>
    


    <!-- http://www.ease-crc.org/ont/SOMA-ACT.owl#isDirectReactionTo -->


    <owl:ObjectProperty rdf:about="http://www.ease-crc.org/ont/SOMA-ACT.owl#isDirectReactionTo">
        <rdfs:subPropertyOf rdf:resource="http://www.ease-crc.org/ont/SOMA-ACT.owl#isReactionTo"/>
        <rdfs:domain rdf:resource="http://www.ontologydesignpatterns.org/ont/dul/DUL.owl#Event"/>
        <rdfs:range rdf:resource="http://www.ontologydesignpatterns.org/ont/dul/DUL.owl#Event"/>
        <rdfs:comment xml:lang="en">Non-transitive version of &quot;is reaction to&quot;.</rdfs:comment>
        <rdfs:isDefinedBy rdf:resource="http://www.ease-crc.org/ont/SOMA-ACT.owl"/>
        <rdfs:label xml:lang="en">is direct reaction to</rdfs:label>
    </owl:ObjectProperty>
    


    <!-- http://www.ease-crc.org/ont/SOMA-ACT.owl#isReactionTo -->


    <owl:ObjectProperty rdf:about="http://www.ease-crc.org/ont/SOMA-ACT.owl#isReactionTo">
        <rdfs:subPropertyOf rdf:resource="http://www.ontologydesignpatterns.org/ont/dul/DUL.owl#follows"/>
        <rdf:type rdf:resource="http://www.w3.org/2002/07/owl#TransitiveProperty"/>
        <rdfs:domain rdf:resource="http://www.ontologydesignpatterns.org/ont/dul/DUL.owl#Event"/>
        <rdfs:range rdf:resource="http://www.ontologydesignpatterns.org/ont/dul/DUL.owl#Event"/>
        <rdfs:comment xml:lang="en">Simple relationship between two actions to express that the subject (the reaction) would not have occured if it were not for the object (the cause), e.g., a Communication Action classified as an Answering Task is a reaction to another Communication Task classified as a Query Task and would not have occured without the other. An example without Agents involved would be some domino stone would not have toppled without the first one toppling.

When Agents are involved, the relation might be seen as an abstraction of the execution of some plan that arises from changing the agents goal that is due to perceiving the cause. However, currently it is unclear how to model such a pattern and therefore not included in SOMA.

This relation is seen as transitive.</rdfs:comment>
        <rdfs:isDefinedBy rdf:resource="http://www.ease-crc.org/ont/SOMA-ACT.owl"/>
        <rdfs:label>is reaction to</rdfs:label>
    </owl:ObjectProperty>
    


    <!-- http://www.ease-crc.org/ont/SOMA-OBJ.owl#hasChildLink -->


    <owl:ObjectProperty rdf:about="http://www.ease-crc.org/ont/SOMA-OBJ.owl#hasChildLink">
        <rdfs:subPropertyOf rdf:resource="http://www.ontologydesignpatterns.org/ont/dul/DUL.owl#hasConstituent"/>
        <owl:inverseOf rdf:resource="http://www.ease-crc.org/ont/SOMA-OBJ.owl#isChildLinkOf"/>
        <rdfs:domain rdf:resource="http://www.ease-crc.org/ont/SOMA-OBJ.owl#Joint"/>
        <rdfs:range rdf:resource="http://www.ontologydesignpatterns.org/ont/dul/DUL.owl#PhysicalObject"/>
        <rdfs:comment>Relates a joint to the link it connects which is closer to the end of the kinematic chain.</rdfs:comment>
        <rdfs:isDefinedBy rdf:resource="http://www.ease-crc.org/ont/SOMA-OBJ.owl"/>
        <rdfs:label>has child link</rdfs:label>
    </owl:ObjectProperty>
    


    <!-- http://www.ease-crc.org/ont/SOMA-OBJ.owl#hasEndLink -->


    <owl:ObjectProperty rdf:about="http://www.ease-crc.org/ont/SOMA-OBJ.owl#hasEndLink">
        <rdfs:subPropertyOf rdf:resource="http://www.ease-crc.org/ont/SOMA-OBJ.owl#hasLink"/>
        <owl:inverseOf rdf:resource="http://www.ease-crc.org/ont/SOMA-OBJ.owl#isEndLinkOf"/>
        <rdfs:domain rdf:resource="http://www.ontologydesignpatterns.org/ont/dul/DUL.owl#PhysicalObject"/>
        <rdfs:range rdf:resource="http://www.ontologydesignpatterns.org/ont/dul/DUL.owl#PhysicalObject"/>
        <rdfs:comment>Relates an object to kinematic components at the end of the kinematic chain.</rdfs:comment>
        <rdfs:isDefinedBy rdf:resource="http://www.ease-crc.org/ont/SOMA-OBJ.owl"/>
        <rdfs:label>has end link</rdfs:label>
    </owl:ObjectProperty>
    


    <!-- http://www.ease-crc.org/ont/SOMA-OBJ.owl#hasJointLimit -->


    <owl:ObjectProperty rdf:about="http://www.ease-crc.org/ont/SOMA-OBJ.owl#hasJointLimit">
        <rdfs:subPropertyOf rdf:resource="http://www.ontologydesignpatterns.org/ont/dul/DUL.owl#hasRegion"/>
        <owl:inverseOf rdf:resource="http://www.ease-crc.org/ont/SOMA-OBJ.owl#isJointLimitOf"/>
        <rdfs:domain rdf:resource="http://www.ease-crc.org/ont/SOMA-OBJ.owl#Joint"/>
        <rdfs:range rdf:resource="http://www.ease-crc.org/ont/SOMA-OBJ.owl#JointLimit"/>
        <rdfs:comment>Relates a joint to its physical limits.</rdfs:comment>
        <rdfs:isDefinedBy rdf:resource="http://www.ease-crc.org/ont/SOMA-OBJ.owl"/>
        <rdfs:label>has joint limit</rdfs:label>
    </owl:ObjectProperty>
    


    <!-- http://www.ease-crc.org/ont/SOMA-OBJ.owl#hasJointState -->


    <owl:ObjectProperty rdf:about="http://www.ease-crc.org/ont/SOMA-OBJ.owl#hasJointState">
        <rdfs:subPropertyOf rdf:resource="http://www.ontologydesignpatterns.org/ont/dul/DUL.owl#hasRegion"/>
        <owl:inverseOf rdf:resource="http://www.ease-crc.org/ont/SOMA-OBJ.owl#isJointStateOf"/>
        <rdfs:domain rdf:resource="http://www.ease-crc.org/ont/SOMA-OBJ.owl#Joint"/>
        <rdfs:range rdf:resource="http://www.ease-crc.org/ont/SOMA-OBJ.owl#JointState"/>
        <rdfs:comment>Relates a joint to its state.</rdfs:comment>
        <rdfs:isDefinedBy rdf:resource="http://www.ease-crc.org/ont/SOMA-OBJ.owl"/>
        <rdfs:label>has joint state</rdfs:label>
    </owl:ObjectProperty>
    


    <!-- http://www.ease-crc.org/ont/SOMA-OBJ.owl#hasLink -->


    <owl:ObjectProperty rdf:about="http://www.ease-crc.org/ont/SOMA-OBJ.owl#hasLink">
        <rdfs:subPropertyOf rdf:resource="http://www.ontologydesignpatterns.org/ont/dul/DUL.owl#hasComponent"/>
        <owl:inverseOf rdf:resource="http://www.ease-crc.org/ont/SOMA-OBJ.owl#isLinkOf"/>
        <rdfs:domain rdf:resource="http://www.ontologydesignpatterns.org/ont/dul/DUL.owl#PhysicalObject"/>
        <rdfs:range rdf:resource="http://www.ontologydesignpatterns.org/ont/dul/DUL.owl#PhysicalObject"/>
        <rdfs:comment>Relates an object to its kinematic components.</rdfs:comment>
        <rdfs:isDefinedBy rdf:resource="http://www.ease-crc.org/ont/SOMA-OBJ.owl"/>
        <rdfs:label>has link</rdfs:label>
    </owl:ObjectProperty>
    


    <!-- http://www.ease-crc.org/ont/SOMA-OBJ.owl#hasNetForce -->


    <owl:ObjectProperty rdf:about="http://www.ease-crc.org/ont/SOMA-OBJ.owl#hasNetForce">
        <rdfs:subPropertyOf rdf:resource="http://www.ontologydesignpatterns.org/ont/dul/DUL.owl#hasRegion"/>
        <owl:inverseOf rdf:resource="http://www.ease-crc.org/ont/SOMA-OBJ.owl#isNetForceOf"/>
        <rdfs:domain rdf:resource="http://www.ontologydesignpatterns.org/ont/dul/DUL.owl#PhysicalObject"/>
        <rdfs:range rdf:resource="http://www.ease-crc.org/ont/SOMA-OBJ.owl#NetForce"/>
        <rdfs:comment>A relation between a physical object and the total force acting on it.</rdfs:comment>
        <rdfs:isDefinedBy rdf:resource="http://www.ease-crc.org/ont/SOMA-OBJ.owl"/>
        <rdfs:label>has net force</rdfs:label>
    </owl:ObjectProperty>
    


    <!-- http://www.ease-crc.org/ont/SOMA-OBJ.owl#hasParentLink -->


    <owl:ObjectProperty rdf:about="http://www.ease-crc.org/ont/SOMA-OBJ.owl#hasParentLink">
        <rdfs:subPropertyOf rdf:resource="http://www.ontologydesignpatterns.org/ont/dul/DUL.owl#hasConstituent"/>
        <owl:inverseOf rdf:resource="http://www.ease-crc.org/ont/SOMA-OBJ.owl#isParentLinkOf"/>
        <rdfs:domain rdf:resource="http://www.ease-crc.org/ont/SOMA-OBJ.owl#Joint"/>
        <rdfs:range rdf:resource="http://www.ontologydesignpatterns.org/ont/dul/DUL.owl#PhysicalObject"/>
        <rdfs:comment>Relates a joint to the link it connects which is closer to the root of the kinematic chain.</rdfs:comment>
        <rdfs:isDefinedBy rdf:resource="http://www.ease-crc.org/ont/SOMA-OBJ.owl"/>
        <rdfs:label>has parent link</rdfs:label>
    </owl:ObjectProperty>
    


    <!-- http://www.ease-crc.org/ont/SOMA-OBJ.owl#hasRootLink -->


    <owl:ObjectProperty rdf:about="http://www.ease-crc.org/ont/SOMA-OBJ.owl#hasRootLink">
        <rdfs:subPropertyOf rdf:resource="http://www.ease-crc.org/ont/SOMA-OBJ.owl#hasLink"/>
        <owl:inverseOf rdf:resource="http://www.ease-crc.org/ont/SOMA-OBJ.owl#isRootLinkOf"/>
        <rdfs:domain rdf:resource="http://www.ontologydesignpatterns.org/ont/dul/DUL.owl#PhysicalObject"/>
        <rdfs:range rdf:resource="http://www.ontologydesignpatterns.org/ont/dul/DUL.owl#PhysicalObject"/>
        <rdfs:comment>Relates an object to kinematic components at the root of the kinematic chain.</rdfs:comment>
        <rdfs:isDefinedBy rdf:resource="http://www.ease-crc.org/ont/SOMA-OBJ.owl"/>
        <rdfs:label>has root link</rdfs:label>
    </owl:ObjectProperty>
    


    <!-- http://www.ease-crc.org/ont/SOMA-OBJ.owl#isChildLinkOf -->


    <owl:ObjectProperty rdf:about="http://www.ease-crc.org/ont/SOMA-OBJ.owl#isChildLinkOf">
        <rdfs:subPropertyOf rdf:resource="http://www.ontologydesignpatterns.org/ont/dul/DUL.owl#isConstituentOf"/>
        <rdfs:domain rdf:resource="http://www.ontologydesignpatterns.org/ont/dul/DUL.owl#PhysicalObject"/>
        <rdfs:range rdf:resource="http://www.ease-crc.org/ont/SOMA-OBJ.owl#Joint"/>
        <rdfs:comment>Relates a joint to the link it connects which is closer to the end of the kinematic chain.</rdfs:comment>
        <rdfs:isDefinedBy rdf:resource="http://www.ease-crc.org/ont/SOMA-OBJ.owl"/>
        <rdfs:label>is child link of</rdfs:label>
    </owl:ObjectProperty>
    


    <!-- http://www.ease-crc.org/ont/SOMA-OBJ.owl#isEndLinkOf -->


    <owl:ObjectProperty rdf:about="http://www.ease-crc.org/ont/SOMA-OBJ.owl#isEndLinkOf">
        <rdfs:subPropertyOf rdf:resource="http://www.ease-crc.org/ont/SOMA-OBJ.owl#isLinkOf"/>
        <rdfs:domain rdf:resource="http://www.ontologydesignpatterns.org/ont/dul/DUL.owl#PhysicalObject"/>
        <rdfs:range rdf:resource="http://www.ontologydesignpatterns.org/ont/dul/DUL.owl#PhysicalObject"/>
        <rdfs:comment>Relates an object to kinematic components at the end of the kinematic chain.</rdfs:comment>
        <rdfs:isDefinedBy rdf:resource="http://www.ease-crc.org/ont/SOMA-OBJ.owl"/>
        <rdfs:label>is end link of</rdfs:label>
    </owl:ObjectProperty>
    


    <!-- http://www.ease-crc.org/ont/SOMA-OBJ.owl#isJointLimitOf -->


    <owl:ObjectProperty rdf:about="http://www.ease-crc.org/ont/SOMA-OBJ.owl#isJointLimitOf">
        <rdfs:subPropertyOf rdf:resource="http://www.ontologydesignpatterns.org/ont/dul/DUL.owl#isRegionFor"/>
        <rdfs:domain rdf:resource="http://www.ease-crc.org/ont/SOMA-OBJ.owl#JointLimit"/>
        <rdfs:range rdf:resource="http://www.ease-crc.org/ont/SOMA-OBJ.owl#Joint"/>
        <rdfs:comment>Relates a joint to its physical limits.</rdfs:comment>
        <rdfs:isDefinedBy rdf:resource="http://www.ease-crc.org/ont/SOMA-OBJ.owl"/>
        <rdfs:label>is joint limit of</rdfs:label>
    </owl:ObjectProperty>
    


    <!-- http://www.ease-crc.org/ont/SOMA-OBJ.owl#isJointStateOf -->


    <owl:ObjectProperty rdf:about="http://www.ease-crc.org/ont/SOMA-OBJ.owl#isJointStateOf">
        <rdfs:subPropertyOf rdf:resource="http://www.ontologydesignpatterns.org/ont/dul/DUL.owl#isRegionFor"/>
        <rdfs:domain rdf:resource="http://www.ease-crc.org/ont/SOMA-OBJ.owl#JointState"/>
        <rdfs:range rdf:resource="http://www.ease-crc.org/ont/SOMA-OBJ.owl#Joint"/>
        <rdfs:comment>Relates a joint to its state.</rdfs:comment>
        <rdfs:isDefinedBy rdf:resource="http://www.ease-crc.org/ont/SOMA-OBJ.owl"/>
        <rdfs:label>is joint state of</rdfs:label>
    </owl:ObjectProperty>
    


    <!-- http://www.ease-crc.org/ont/SOMA-OBJ.owl#isLinkOf -->


    <owl:ObjectProperty rdf:about="http://www.ease-crc.org/ont/SOMA-OBJ.owl#isLinkOf">
        <rdfs:subPropertyOf rdf:resource="http://www.ontologydesignpatterns.org/ont/dul/DUL.owl#isComponentOf"/>
        <rdfs:domain rdf:resource="http://www.ontologydesignpatterns.org/ont/dul/DUL.owl#PhysicalObject"/>
        <rdfs:range rdf:resource="http://www.ontologydesignpatterns.org/ont/dul/DUL.owl#PhysicalObject"/>
        <rdfs:comment>Relates an object to its kinematic components.</rdfs:comment>
        <rdfs:isDefinedBy rdf:resource="http://www.ease-crc.org/ont/SOMA-OBJ.owl"/>
        <rdfs:label>is link of</rdfs:label>
    </owl:ObjectProperty>
    


    <!-- http://www.ease-crc.org/ont/SOMA-OBJ.owl#isMassAttributeOf -->


    <owl:ObjectProperty rdf:about="http://www.ease-crc.org/ont/SOMA-OBJ.owl#isMassAttributeOf">
        <rdfs:subPropertyOf rdf:resource="http://www.ontologydesignpatterns.org/ont/dul/DUL.owl#isRegionFor"/>
        <owl:inverseOf rdf:resource="http://www.ease-crc.org/ont/SOMA.owl#hasMassAttribute"/>
        <rdfs:domain rdf:resource="http://www.ease-crc.org/ont/SOMA.owl#MassAttribute"/>
        <rdfs:range rdf:resource="http://www.ontologydesignpatterns.org/ont/dul/DUL.owl#PhysicalObject"/>
        <rdfs:comment>A relation between physical objects and their mass.</rdfs:comment>
        <rdfs:isDefinedBy rdf:resource="http://www.ease-crc.org/ont/SOMA-OBJ.owl"/>
        <rdfs:label>is mass attribute of</rdfs:label>
    </owl:ObjectProperty>
    


    <!-- http://www.ease-crc.org/ont/SOMA-OBJ.owl#isNetForceOf -->


    <owl:ObjectProperty rdf:about="http://www.ease-crc.org/ont/SOMA-OBJ.owl#isNetForceOf">
        <rdfs:subPropertyOf rdf:resource="http://www.ontologydesignpatterns.org/ont/dul/DUL.owl#isRegionFor"/>
        <rdfs:domain rdf:resource="http://www.ease-crc.org/ont/SOMA-OBJ.owl#NetForce"/>
        <rdfs:range rdf:resource="http://www.ontologydesignpatterns.org/ont/dul/DUL.owl#PhysicalObject"/>
        <rdfs:comment>A relation between a physical object and the total force acting on it.</rdfs:comment>
        <rdfs:isDefinedBy rdf:resource="http://www.ease-crc.org/ont/SOMA-OBJ.owl"/>
        <rdfs:label>is net force of</rdfs:label>
    </owl:ObjectProperty>
    


    <!-- http://www.ease-crc.org/ont/SOMA-OBJ.owl#isParentLinkOf -->


    <owl:ObjectProperty rdf:about="http://www.ease-crc.org/ont/SOMA-OBJ.owl#isParentLinkOf">
        <rdfs:subPropertyOf rdf:resource="http://www.ontologydesignpatterns.org/ont/dul/DUL.owl#isConstituentOf"/>
        <rdfs:domain rdf:resource="http://www.ontologydesignpatterns.org/ont/dul/DUL.owl#PhysicalObject"/>
        <rdfs:range rdf:resource="http://www.ease-crc.org/ont/SOMA-OBJ.owl#Joint"/>
        <rdfs:comment>Relates a joint to the link it connects which is closer to the root of the kinematic chain.</rdfs:comment>
        <rdfs:isDefinedBy rdf:resource="http://www.ease-crc.org/ont/SOMA-OBJ.owl"/>
        <rdfs:label>is parent link of</rdfs:label>
    </owl:ObjectProperty>
    


    <!-- http://www.ease-crc.org/ont/SOMA-OBJ.owl#isRootLinkOf -->


    <owl:ObjectProperty rdf:about="http://www.ease-crc.org/ont/SOMA-OBJ.owl#isRootLinkOf">
        <rdfs:subPropertyOf rdf:resource="http://www.ease-crc.org/ont/SOMA-OBJ.owl#isLinkOf"/>
        <rdfs:domain rdf:resource="http://www.ontologydesignpatterns.org/ont/dul/DUL.owl#PhysicalObject"/>
        <rdfs:range rdf:resource="http://www.ontologydesignpatterns.org/ont/dul/DUL.owl#PhysicalObject"/>
        <rdfs:comment>Relates an object to kinematic components at the root of the kinematic chain.</rdfs:comment>
        <rdfs:isDefinedBy rdf:resource="http://www.ease-crc.org/ont/SOMA-OBJ.owl"/>
        <rdfs:label>is root link of</rdfs:label>
    </owl:ObjectProperty>
    


    <!-- http://www.ease-crc.org/ont/SOMA-SAY.owl#isInitialSceneOf -->


    <owl:ObjectProperty rdf:about="http://www.ease-crc.org/ont/SOMA-SAY.owl#isInitialSceneOf">
        <rdfs:subPropertyOf rdf:resource="http://www.ontologydesignpatterns.org/ont/dul/DUL.owl#isObjectIncludedIn"/>
        <owl:inverseOf rdf:resource="http://www.ease-crc.org/ont/SOMA.owl#hasInitialScene"/>
        <rdfs:domain rdf:resource="http://www.ease-crc.org/ont/SOMA.owl#Scene"/>
        <rdfs:range rdf:resource="http://www.ease-crc.org/ont/SOMA.owl#StateTransition"/>
        <rdfs:comment>A relation between StateTransitions and Scenes, which identifies the scene the transition starts from.</rdfs:comment>
        <rdfs:isDefinedBy rdf:resource="http://www.ease-crc.org/ont/SOMA-SAY.owl"/>
    </owl:ObjectProperty>
    


    <!-- http://www.ease-crc.org/ont/SOMA-SAY.owl#isTerminalSceneOf -->


    <owl:ObjectProperty rdf:about="http://www.ease-crc.org/ont/SOMA-SAY.owl#isTerminalSceneOf">
        <rdfs:subPropertyOf rdf:resource="http://www.ontologydesignpatterns.org/ont/dul/DUL.owl#isObjectIncludedIn"/>
        <owl:inverseOf rdf:resource="http://www.ease-crc.org/ont/SOMA.owl#hasTerminalScene"/>
        <rdfs:domain rdf:resource="http://www.ease-crc.org/ont/SOMA.owl#Scene"/>
        <rdfs:range rdf:resource="http://www.ease-crc.org/ont/SOMA.owl#StateTransition"/>
        <rdfs:comment>A relation between StateTransitions and Scenes, which identifies the scene the transition is expected to end at.</rdfs:comment>
        <rdfs:isDefinedBy rdf:resource="http://www.ease-crc.org/ont/SOMA-SAY.owl"/>
    </owl:ObjectProperty>
    


    <!-- http://www.ease-crc.org/ont/SOMA-WF.owl#hasPreviousStep -->


    <owl:ObjectProperty rdf:about="http://www.ease-crc.org/ont/SOMA-WF.owl#hasPreviousStep">
        <rdfs:subPropertyOf rdf:resource="http://www.ontologydesignpatterns.org/ont/dul/DUL.owl#directlyFollows"/>
        <owl:inverseOf rdf:resource="http://www.ease-crc.org/ont/SOMA.owl#hasNextStep"/>
        <rdfs:domain rdf:resource="http://www.ontologydesignpatterns.org/ont/dul/DUL.owl#Task"/>
        <rdfs:range rdf:resource="http://www.ontologydesignpatterns.org/ont/dul/DUL.owl#Task"/>
        <rdfs:comment>An ordering relation between tasks in some workflow, stating that a task is preceded by another.</rdfs:comment>
        <rdfs:isDefinedBy rdf:resource="http://www.ease-crc.org/ont/SOMA-WF.owl"/>
        <rdfs:label>has previous step</rdfs:label>
    </owl:ObjectProperty>
    


    <!-- http://www.ease-crc.org/ont/SOMA-WF.owl#isFirstStepOf -->


    <owl:ObjectProperty rdf:about="http://www.ease-crc.org/ont/SOMA-WF.owl#isFirstStepOf">
        <rdfs:subPropertyOf rdf:resource="http://www.ease-crc.org/ont/SOMA-WF.owl#isStepOf"/>
        <owl:inverseOf rdf:resource="http://www.ease-crc.org/ont/SOMA.owl#hasFirstStep"/>
        <rdfs:domain rdf:resource="http://www.ontologydesignpatterns.org/ont/dul/DUL.owl#Task"/>
        <rdfs:range rdf:resource="http://www.ontologydesignpatterns.org/ont/dul/DUL.owl#Workflow"/>
        <rdfs:comment>A relation stating that some task is the first one in a workflow.</rdfs:comment>
        <rdfs:isDefinedBy rdf:resource="http://www.ease-crc.org/ont/SOMA-WF.owl"/>
        <rdfs:label>is first step of</rdfs:label>
    </owl:ObjectProperty>
    


    <!-- http://www.ease-crc.org/ont/SOMA-WF.owl#isStepOf -->


    <owl:ObjectProperty rdf:about="http://www.ease-crc.org/ont/SOMA-WF.owl#isStepOf">
        <rdfs:subPropertyOf rdf:resource="http://www.ontologydesignpatterns.org/ont/dul/DUL.owl#isTaskDefinedIn"/>
        <owl:inverseOf rdf:resource="http://www.ease-crc.org/ont/SOMA.owl#hasStep"/>
        <rdfs:domain rdf:resource="http://www.ontologydesignpatterns.org/ont/dul/DUL.owl#Task"/>
        <rdfs:range rdf:resource="http://www.ontologydesignpatterns.org/ont/dul/DUL.owl#Workflow"/>
        <rdfs:comment>A relation stating that a task is a step in a workflow.</rdfs:comment>
        <rdfs:isDefinedBy rdf:resource="http://www.ease-crc.org/ont/SOMA-WF.owl"/>
        <rdfs:label>is step of</rdfs:label>
    </owl:ObjectProperty>
    


    <!-- http://www.ease-crc.org/ont/SOMA.owl#affordanceDefines -->


    <owl:ObjectProperty rdf:about="http://www.ease-crc.org/ont/SOMA.owl#affordanceDefines">
        <rdfs:subPropertyOf rdf:resource="http://www.ontologydesignpatterns.org/ont/dul/DUL.owl#defines"/>
        <owl:inverseOf rdf:resource="http://www.ease-crc.org/ont/SOMA.owl#isDefinedInAffordance"/>
        <rdfs:domain rdf:resource="http://www.ease-crc.org/ont/SOMA.owl#Affordance"/>
        <rdfs:range rdf:resource="http://www.ontologydesignpatterns.org/ont/dul/DUL.owl#Concept"/>
        <rdfs:comment>A relation between an Affordance and a Concept (often an EventType).</rdfs:comment>
        <rdfs:isDefinedBy rdf:resource="http://www.ease-crc.org/ont/SOMA-OBJ.owl"/>
        <rdfs:label>affordance defines</rdfs:label>
    </owl:ObjectProperty>
    


    <!-- http://www.ease-crc.org/ont/SOMA.owl#affordanceDefinesTask -->


    <owl:ObjectProperty rdf:about="http://www.ease-crc.org/ont/SOMA.owl#affordanceDefinesTask">
        <rdfs:subPropertyOf rdf:resource="http://www.ease-crc.org/ont/SOMA.owl#affordanceDefines"/>
        <rdfs:subPropertyOf rdf:resource="http://www.ontologydesignpatterns.org/ont/dul/DUL.owl#definesTask"/>
        <owl:inverseOf rdf:resource="http://www.ease-crc.org/ont/SOMA.owl#isTaskDefinedInAffordance"/>
        <rdfs:domain rdf:resource="http://www.ease-crc.org/ont/SOMA.owl#Affordance"/>
        <rdfs:range rdf:resource="http://www.ontologydesignpatterns.org/ont/dul/DUL.owl#Task"/>
        <rdfs:comment>A relation between an Affordance and a Task</rdfs:comment>
        <rdfs:isDefinedBy rdf:resource="http://www.ease-crc.org/ont/SOMA-OBJ.owl"/>
        <rdfs:label>affordance defines task</rdfs:label>
    </owl:ObjectProperty>
    


    <!-- http://www.ease-crc.org/ont/SOMA.owl#affordsBearer -->


    <owl:ObjectProperty rdf:about="http://www.ease-crc.org/ont/SOMA.owl#affordsBearer">
        <rdfs:subPropertyOf rdf:resource="http://www.ease-crc.org/ont/SOMA.owl#affordsConcept"/>
        <owl:inverseOf rdf:resource="http://www.ease-crc.org/ont/SOMA.owl#isBearerAffordedBy"/>
        <rdfs:domain rdf:resource="http://www.ease-crc.org/ont/SOMA.owl#Disposition"/>
        <rdfs:range rdf:resource="http://www.ontologydesignpatterns.org/ont/dul/DUL.owl#Role"/>
        <owl:propertyChainAxiom rdf:parseType="Collection">
            <rdf:Description rdf:about="http://www.ontologydesignpatterns.org/ont/dul/DUL.owl#isDescribedBy"/>
            <rdf:Description rdf:about="http://www.ease-crc.org/ont/SOMA.owl#definesBearer"/>
        </owl:propertyChainAxiom>
        <rdfs:comment>Relates a disposition to the bearer role defined by the affordance describing the disposition.</rdfs:comment>
        <rdfs:isDefinedBy rdf:resource="http://www.ease-crc.org/ont/SOMA-OBJ.owl"/>
        <rdfs:label>affords bearer</rdfs:label>
    </owl:ObjectProperty>
    


    <!-- http://www.ease-crc.org/ont/SOMA.owl#affordsConcept -->


    <owl:ObjectProperty rdf:about="http://www.ease-crc.org/ont/SOMA.owl#affordsConcept">
        <rdfs:subPropertyOf rdf:resource="http://www.ontologydesignpatterns.org/ont/dul/DUL.owl#associatedWith"/>
        <owl:inverseOf rdf:resource="http://www.ease-crc.org/ont/SOMA.owl#isConceptAffordedBy"/>
        <rdfs:domain rdf:resource="http://www.ease-crc.org/ont/SOMA.owl#Disposition"/>
        <rdfs:range rdf:resource="http://www.ontologydesignpatterns.org/ont/dul/DUL.owl#Concept"/>
        <owl:propertyChainAxiom rdf:parseType="Collection">
            <rdf:Description rdf:about="http://www.ontologydesignpatterns.org/ont/dul/DUL.owl#isDescribedBy"/>
            <rdf:Description rdf:about="http://www.ease-crc.org/ont/SOMA.owl#affordanceDefines"/>
        </owl:propertyChainAxiom>
        <rdfs:comment>A relation between a disposition and a concept defined in the affordance that describes the disposition.</rdfs:comment>
        <rdfs:isDefinedBy rdf:resource="http://www.ease-crc.org/ont/SOMA-OBJ.owl"/>
        <rdfs:label>affords concept</rdfs:label>
    </owl:ObjectProperty>
    


    <!-- http://www.ease-crc.org/ont/SOMA.owl#affordsSetpoint -->


    <owl:ObjectProperty rdf:about="http://www.ease-crc.org/ont/SOMA.owl#affordsSetpoint">
        <rdfs:subPropertyOf rdf:resource="http://www.ease-crc.org/ont/SOMA.owl#affordsConcept"/>
        <owl:inverseOf rdf:resource="http://www.ease-crc.org/ont/SOMA.owl#isSetpointAffordedBy"/>
        <rdfs:domain rdf:resource="http://www.ease-crc.org/ont/SOMA.owl#Disposition"/>
        <rdfs:range rdf:resource="http://www.ease-crc.org/ont/SOMA.owl#Setpoint"/>
        <owl:propertyChainAxiom rdf:parseType="Collection">
            <rdf:Description rdf:about="http://www.ontologydesignpatterns.org/ont/dul/DUL.owl#isDescribedBy"/>
            <rdf:Description rdf:about="http://www.ease-crc.org/ont/SOMA.owl#definesSetpoint"/>
        </owl:propertyChainAxiom>
        <rdfs:comment>Relates a disposition to the setpoint parameter defined by the affordance describing the disposition.</rdfs:comment>
        <rdfs:isDefinedBy rdf:resource="http://www.ease-crc.org/ont/SOMA-OBJ.owl"/>
        <rdfs:label>affords setpoint</rdfs:label>
    </owl:ObjectProperty>
    


    <!-- http://www.ease-crc.org/ont/SOMA.owl#affordsTask -->


    <owl:ObjectProperty rdf:about="http://www.ease-crc.org/ont/SOMA.owl#affordsTask">
        <rdfs:subPropertyOf rdf:resource="http://www.ease-crc.org/ont/SOMA.owl#affordsConcept"/>
        <owl:inverseOf rdf:resource="http://www.ease-crc.org/ont/SOMA.owl#isTaskAffordedBy"/>
        <rdfs:domain rdf:resource="http://www.ease-crc.org/ont/SOMA.owl#Disposition"/>
        <rdfs:range rdf:resource="http://www.ontologydesignpatterns.org/ont/dul/DUL.owl#Task"/>
        <owl:propertyChainAxiom rdf:parseType="Collection">
            <rdf:Description rdf:about="http://www.ontologydesignpatterns.org/ont/dul/DUL.owl#isDescribedBy"/>
            <rdf:Description rdf:about="http://www.ease-crc.org/ont/SOMA.owl#affordanceDefinesTask"/>
        </owl:propertyChainAxiom>
        <rdfs:comment>Relates a disposition to the task defined by the affordance describing the disposition.</rdfs:comment>
        <rdfs:isDefinedBy rdf:resource="http://www.ease-crc.org/ont/SOMA-OBJ.owl"/>
        <rdfs:label>affords task</rdfs:label>
    </owl:ObjectProperty>
    


    <!-- http://www.ease-crc.org/ont/SOMA.owl#affordsTrigger -->


    <owl:ObjectProperty rdf:about="http://www.ease-crc.org/ont/SOMA.owl#affordsTrigger">
        <rdfs:subPropertyOf rdf:resource="http://www.ease-crc.org/ont/SOMA.owl#affordsConcept"/>
        <owl:inverseOf rdf:resource="http://www.ease-crc.org/ont/SOMA.owl#isTriggerAffordedBy"/>
        <rdfs:domain rdf:resource="http://www.ease-crc.org/ont/SOMA.owl#Disposition"/>
        <rdfs:range rdf:resource="http://www.ontologydesignpatterns.org/ont/dul/DUL.owl#Role"/>
        <owl:propertyChainAxiom rdf:parseType="Collection">
            <rdf:Description rdf:about="http://www.ontologydesignpatterns.org/ont/dul/DUL.owl#isDescribedBy"/>
            <rdf:Description rdf:about="http://www.ease-crc.org/ont/SOMA.owl#definesTrigger"/>
        </owl:propertyChainAxiom>
        <rdfs:comment>Relates a disposition to the trigger role defined by the affordance describing the disposition.</rdfs:comment>
        <rdfs:isDefinedBy rdf:resource="http://www.ease-crc.org/ont/SOMA-HOME.owl"/>
        <rdfs:isDefinedBy rdf:resource="http://www.ease-crc.org/ont/SOMA-OBJ.owl"/>
        <rdfs:label>affords trigger</rdfs:label>
    </owl:ObjectProperty>
    


    <!-- http://www.ease-crc.org/ont/SOMA.owl#answers -->


    <owl:ObjectProperty rdf:about="http://www.ease-crc.org/ont/SOMA.owl#answers">
        <rdfs:subPropertyOf rdf:resource="http://www.ease-crc.org/ont/SOMA.owl#relatesToAnotherRole"/>
        <rdfs:domain rdf:resource="http://www.ease-crc.org/ont/SOMA.owl#Message"/>
        <rdfs:range rdf:resource="http://www.ease-crc.org/ont/SOMA.owl#Message"/>
        <rdfs:isDefinedBy rdf:resource="http://www.ease-crc.org/ont/SOMA-ACT.owl"/>
        <rdfs:label>The relation between an answering message and the message it answers.</rdfs:label>
        <rdfs:label>answers</rdfs:label>
    </owl:ObjectProperty>
    


    <!-- http://www.ease-crc.org/ont/SOMA.owl#containsObject -->


    <owl:ObjectProperty rdf:about="http://www.ease-crc.org/ont/SOMA.owl#containsObject">
        <rdfs:subPropertyOf rdf:resource="http://www.ease-crc.org/ont/SOMA.owl#contains"/>
        <rdfs:subPropertyOf rdf:resource="http://www.ontologydesignpatterns.org/ont/dul/DUL.owl#isLocationOf"/>
        <owl:inverseOf rdf:resource="http://www.ease-crc.org/ont/SOMA.owl#isInsideOf"/>
        <rdf:type rdf:resource="http://www.w3.org/2002/07/owl#TransitiveProperty"/>
        <rdfs:domain rdf:resource="http://www.ontologydesignpatterns.org/ont/dul/DUL.owl#PhysicalObject"/>
        <rdfs:range rdf:resource="http://www.ontologydesignpatterns.org/ont/dul/DUL.owl#PhysicalObject"/>
        <rdfs:comment>A spatial relation holding between a container, and objects it contains.</rdfs:comment>
        <rdfs:isDefinedBy rdf:resource="http://www.ease-crc.org/ont/SOMA-OBJ.owl"/>
        <rdfs:label>contains object</rdfs:label>
    </owl:ObjectProperty>
    


    <!-- http://www.ease-crc.org/ont/SOMA.owl#coversObject -->


    <owl:ObjectProperty rdf:about="http://www.ease-crc.org/ont/SOMA.owl#coversObject">
        <rdfs:subPropertyOf rdf:resource="http://www.ease-crc.org/ont/SOMA.owl#interactsWith"/>
        <owl:inverseOf rdf:resource="http://www.ease-crc.org/ont/SOMA.owl#isCoveredByObject"/>
        <rdf:type rdf:resource="http://www.w3.org/2002/07/owl#AsymmetricProperty"/>
        <rdf:type rdf:resource="http://www.w3.org/2002/07/owl#IrreflexiveProperty"/>
        <rdfs:domain rdf:resource="http://www.ontologydesignpatterns.org/ont/dul/DUL.owl#PhysicalObject"/>
        <rdfs:range rdf:resource="http://www.ontologydesignpatterns.org/ont/dul/DUL.owl#PhysicalObject"/>
        <rdfs:comment>A relationship from an object (the coverer) that blocks access to another or its interior (the coveree).</rdfs:comment>
        <rdfs:isDefinedBy rdf:resource="http://www.ease-crc.org/ont/SOMA-SAY.owl"/>
    </owl:ObjectProperty>
    


    <!-- http://www.ease-crc.org/ont/SOMA.owl#definesBearer -->


    <owl:ObjectProperty rdf:about="http://www.ease-crc.org/ont/SOMA.owl#definesBearer">
        <rdfs:subPropertyOf rdf:resource="http://www.ontologydesignpatterns.org/ont/dul/DUL.owl#definesRole"/>
        <owl:inverseOf rdf:resource="http://www.ease-crc.org/ont/SOMA.owl#isBearerDefinedIn"/>
        <rdfs:domain rdf:resource="http://www.ease-crc.org/ont/SOMA.owl#Affordance"/>
        <rdfs:range rdf:resource="http://www.ontologydesignpatterns.org/ont/dul/DUL.owl#Role"/>
        <rdfs:comment>Relates an affordance which is a relation between a bearer and a trigger, to the role of the bearer when the affordance is manifested.</rdfs:comment>
        <rdfs:isDefinedBy rdf:resource="http://www.ease-crc.org/ont/SOMA-OBJ.owl"/>
        <rdfs:label>defines bearer</rdfs:label>
    </owl:ObjectProperty>
    


    <!-- http://www.ease-crc.org/ont/SOMA.owl#definesInput -->


    <owl:ObjectProperty rdf:about="http://www.ease-crc.org/ont/SOMA.owl#definesInput">
        <rdfs:subPropertyOf rdf:resource="http://www.ease-crc.org/ont/SOMA.owl#definesParticipant"/>
        <rdfs:domain rdf:resource="http://www.ontologydesignpatterns.org/ont/dul/DUL.owl#Description"/>
        <rdfs:range>
            <owl:Class>
                <owl:unionOf rdf:parseType="Collection">
                    <rdf:Description rdf:about="http://www.ontologydesignpatterns.org/ont/dul/DUL.owl#Parameter"/>
                    <rdf:Description rdf:about="http://www.ontologydesignpatterns.org/ont/dul/DUL.owl#Role"/>
                </owl:unionOf>
            </owl:Class>
        </rdfs:range>
        <rdfs:comment>The defined participant is an &quot;input&quot;: 

- some object existing at the beginning of a Task&apos;s execution, and that will be acted on during the execution of the task;
- some region/value which informs the way in which the Task will be executed.</rdfs:comment>
        <rdfs:isDefinedBy rdf:resource="http://www.ease-crc.org/ont/SOMA-WF.owl"/>
    </owl:ObjectProperty>
    


    <!-- http://www.ease-crc.org/ont/SOMA.owl#definesOutput -->


    <owl:ObjectProperty rdf:about="http://www.ease-crc.org/ont/SOMA.owl#definesOutput">
        <rdfs:subPropertyOf rdf:resource="http://www.ease-crc.org/ont/SOMA.owl#definesParticipant"/>
        <rdfs:domain rdf:resource="http://www.ontologydesignpatterns.org/ont/dul/DUL.owl#Description"/>
        <rdfs:range>
            <owl:Class>
                <owl:unionOf rdf:parseType="Collection">
                    <rdf:Description rdf:about="http://www.ontologydesignpatterns.org/ont/dul/DUL.owl#Parameter"/>
                    <rdf:Description rdf:about="http://www.ontologydesignpatterns.org/ont/dul/DUL.owl#Role"/>
                </owl:unionOf>
            </owl:Class>
        </rdfs:range>
        <rdfs:comment>Defines an &quot;output&quot; participant:

- an Entity (Object or state of affairs) that exists as a result of the execution of a Task;
- a Region/value that has been demarcated/computed as a result of the execution of a Task.</rdfs:comment>
        <rdfs:isDefinedBy rdf:resource="http://www.ease-crc.org/ont/SOMA-WF.owl"/>
    </owl:ObjectProperty>
    


    <!-- http://www.ease-crc.org/ont/SOMA.owl#definesParameter -->


    <owl:ObjectProperty rdf:about="http://www.ease-crc.org/ont/SOMA.owl#definesParameter">
        <rdfs:subPropertyOf rdf:resource="http://www.ontologydesignpatterns.org/ont/dul/DUL.owl#defines"/>
        <owl:inverseOf rdf:resource="http://www.ease-crc.org/ont/SOMA.owl#isParameterDefinedIn"/>
        <rdfs:domain rdf:resource="http://www.ontologydesignpatterns.org/ont/dul/DUL.owl#Description"/>
        <rdfs:range rdf:resource="http://www.ontologydesignpatterns.org/ont/dul/DUL.owl#Parameter"/>
        <rdfs:comment>A relation between a description and a parameter.</rdfs:comment>
        <rdfs:isDefinedBy rdf:resource="http://www.ease-crc.org/ont/SOMA-OBJ.owl"/>
        <rdfs:label>defines parameter</rdfs:label>
    </owl:ObjectProperty>
    


    <!-- http://www.ease-crc.org/ont/SOMA.owl#definesParticipant -->


    <owl:ObjectProperty rdf:about="http://www.ease-crc.org/ont/SOMA.owl#definesParticipant">
        <rdfs:subPropertyOf rdf:resource="http://www.ontologydesignpatterns.org/ont/dul/DUL.owl#defines"/>
        <rdfs:domain rdf:resource="http://www.ontologydesignpatterns.org/ont/dul/DUL.owl#Description"/>
        <rdfs:range rdf:resource="http://www.ontologydesignpatterns.org/ont/dul/DUL.owl#Concept"/>
        <rdfs:comment>A Description definesParticipant a Concept to classify participants in Events associated to that Description.

The prototypical example is a Task, which is a concept to classify Actions (a form of Event). A Task may define several Roles, with which to classify participants in the event of that Task&apos;s execution.</rdfs:comment>
        <rdfs:isDefinedBy rdf:resource="http://www.ease-crc.org/ont/SOMA-WF.owl"/>
    </owl:ObjectProperty>
    


    <!-- http://www.ease-crc.org/ont/SOMA.owl#definesProcess -->


    <owl:ObjectProperty rdf:about="http://www.ease-crc.org/ont/SOMA.owl#definesProcess">
        <rdfs:subPropertyOf rdf:resource="http://www.ontologydesignpatterns.org/ont/dul/DUL.owl#defines"/>
        <owl:inverseOf rdf:resource="http://www.ease-crc.org/ont/SOMA.owl#isProcessDefinedIn"/>
        <rdfs:domain rdf:resource="http://www.ontologydesignpatterns.org/ont/dul/DUL.owl#Description"/>
        <rdfs:range rdf:resource="http://www.ease-crc.org/ont/SOMA.owl#ProcessType"/>
        <rdfs:comment>A relation between a description and a process type.</rdfs:comment>
        <rdfs:isDefinedBy rdf:resource="http://www.ease-crc.org/ont/SOMA-PROC.owl"/>
        <rdfs:label>defines process</rdfs:label>
    </owl:ObjectProperty>
    


    <!-- http://www.ease-crc.org/ont/SOMA.owl#definesSetpoint -->


    <owl:ObjectProperty rdf:about="http://www.ease-crc.org/ont/SOMA.owl#definesSetpoint">
        <rdfs:subPropertyOf rdf:resource="http://www.ease-crc.org/ont/SOMA.owl#definesParameter"/>
        <owl:inverseOf rdf:resource="http://www.ease-crc.org/ont/SOMA.owl#isSetpointDefinedIn"/>
        <rdfs:domain rdf:resource="http://www.ontologydesignpatterns.org/ont/dul/DUL.owl#Description"/>
        <rdfs:range rdf:resource="http://www.ease-crc.org/ont/SOMA.owl#Setpoint"/>
        <rdfs:comment>Defines the dedicated goal region of a description.</rdfs:comment>
        <rdfs:isDefinedBy rdf:resource="http://www.ease-crc.org/ont/SOMA-OBJ.owl"/>
        <rdfs:label>defines setpoint</rdfs:label>
    </owl:ObjectProperty>
    


    <!-- http://www.ease-crc.org/ont/SOMA.owl#definesTrigger -->


    <owl:ObjectProperty rdf:about="http://www.ease-crc.org/ont/SOMA.owl#definesTrigger">
        <rdfs:subPropertyOf rdf:resource="http://www.ontologydesignpatterns.org/ont/dul/DUL.owl#definesRole"/>
        <owl:inverseOf rdf:resource="http://www.ease-crc.org/ont/SOMA.owl#isTriggerDefinedIn"/>
        <rdfs:domain rdf:resource="http://www.ease-crc.org/ont/SOMA.owl#Affordance"/>
        <rdfs:range rdf:resource="http://www.ontologydesignpatterns.org/ont/dul/DUL.owl#Role"/>
        <rdfs:comment>Relates an affordance which is a relation between a bearer and a trigger, to the role of the trigger when the affordance is manifested.</rdfs:comment>
        <rdfs:isDefinedBy rdf:resource="http://www.ease-crc.org/ont/SOMA-OBJ.owl"/>
        <rdfs:label>defines trigger</rdfs:label>
    </owl:ObjectProperty>
    


    <!-- http://www.ease-crc.org/ont/SOMA.owl#describesQuality -->


    <owl:ObjectProperty rdf:about="http://www.ease-crc.org/ont/SOMA.owl#describesQuality">
        <rdfs:subPropertyOf rdf:resource="http://www.ontologydesignpatterns.org/ont/dul/DUL.owl#describes"/>
        <owl:inverseOf rdf:resource="http://www.ease-crc.org/ont/SOMA.owl#isQualityDescribedBy"/>
        <rdfs:domain rdf:resource="http://www.ontologydesignpatterns.org/ont/dul/DUL.owl#Description"/>
        <rdfs:range rdf:resource="http://www.ontologydesignpatterns.org/ont/dul/DUL.owl#Quality"/>
        <rdfs:comment>Relates a description to a quality that it describes.</rdfs:comment>
        <rdfs:isDefinedBy rdf:resource="http://www.ease-crc.org/ont/SOMA-OBJ.owl"/>
        <rdfs:label>describes quality</rdfs:label>
    </owl:ObjectProperty>
    


    <!-- http://www.ease-crc.org/ont/SOMA.owl#encodes -->


    <owl:ObjectProperty rdf:about="http://www.ease-crc.org/ont/SOMA.owl#encodes">
        <rdfs:subPropertyOf rdf:resource="http://www.ontologydesignpatterns.org/ont/dul/DUL.owl#associatedWith"/>
        <rdf:type rdf:resource="http://www.w3.org/2002/07/owl#SymmetricProperty"/>
        <rdfs:domain rdf:resource="http://www.ontologydesignpatterns.org/ont/dul/DUL.owl#InformationObject"/>
        <rdfs:range rdf:resource="http://www.ontologydesignpatterns.org/ont/dul/DUL.owl#InformationObject"/>
        <rdfs:comment xml:lang="en">The relation between two Information Objects that have the same meaning, but are formatted differently. E.g., a text written in UTF-8 encodes a text in a natural writing system (letters) and vice versa.</rdfs:comment>
        <rdfs:isDefinedBy rdf:resource="http://www.ease-crc.org/ont/SOMA-IO.owl"/>
    </owl:ObjectProperty>
    


    <!-- http://www.ease-crc.org/ont/SOMA.owl#givesMeaningTo -->


    <owl:ObjectProperty rdf:about="http://www.ease-crc.org/ont/SOMA.owl#givesMeaningTo">
        <rdfs:subPropertyOf rdf:resource="http://www.ontologydesignpatterns.org/ont/dul/DUL.owl#associatedWith"/>
        <owl:inverseOf rdf:resource="http://www.ease-crc.org/ont/SOMA.owl#isGivenMeaningBy"/>
        <rdfs:domain rdf:resource="http://www.ease-crc.org/ont/SOMA.owl#System"/>
        <rdfs:range rdf:resource="http://www.ontologydesignpatterns.org/ont/dul/DUL.owl#InformationObject"/>
        <rdfs:isDefinedBy rdf:resource="http://www.ease-crc.org/ont/SOMA-IO.owl"/>
        <rdfs:label xml:lang="en">The relation between a System and Information Object that is given meaning to by said system, e.g., a Language might give meaning to some word, sentence, text, etc., but without the knowledge of said System (Language), the text will not make sense to a reader.</rdfs:label>
        <rdfs:label xml:lang="en">gives meaning to</rdfs:label>
    </owl:ObjectProperty>
    


    <!-- http://www.ease-crc.org/ont/SOMA.owl#hasAction -->


    <owl:ObjectProperty rdf:about="http://www.ease-crc.org/ont/SOMA.owl#hasAction">
        <rdfs:subPropertyOf rdf:resource="http://www.ontologydesignpatterns.org/ont/dul/DUL.owl#hasConstituent"/>
        <rdfs:domain rdf:resource="http://www.ontologydesignpatterns.org/ont/dul/DUL.owl#Action"/>
        <rdfs:range rdf:resource="http://www.ontologydesignpatterns.org/ont/dul/DUL.owl#Action"/>
        <rdfs:comment>A relation from an Action to a component Action.</rdfs:comment>
        <rdfs:isDefinedBy rdf:resource="http://www.ease-crc.org/ont/SOMA-ACT.owl"/>
        <rdfs:label>has action</rdfs:label>
    </owl:ObjectProperty>
    


    <!-- http://www.ease-crc.org/ont/SOMA.owl#hasAlterationResult -->


    <owl:ObjectProperty rdf:about="http://www.ease-crc.org/ont/SOMA.owl#hasAlterationResult">
        <rdfs:subPropertyOf rdf:resource="http://www.ontologydesignpatterns.org/ont/dul/DUL.owl#hasRegion"/>
        <owl:inverseOf rdf:resource="http://www.ease-crc.org/ont/SOMA.owl#isAlterationResultOf"/>
        <rdfs:domain rdf:resource="http://www.ontologydesignpatterns.org/ont/dul/DUL.owl#Action"/>
        <rdfs:range rdf:resource="http://www.ontologydesignpatterns.org/ont/dul/DUL.owl#Region"/>
        <rdfs:comment>Relates an action that alters an object to the region that the alteration reached during the action.</rdfs:comment>
        <rdfs:isDefinedBy rdf:resource="http://www.ease-crc.org/ont/SOMA-OBJ.owl"/>
        <rdfs:label>has alteration result</rdfs:label>
    </owl:ObjectProperty>
    


    <!-- http://www.ease-crc.org/ont/SOMA.owl#hasAnswer -->


    <owl:ObjectProperty rdf:about="http://www.ease-crc.org/ont/SOMA.owl#hasAnswer">
        <rdfs:subPropertyOf rdf:resource="http://www.ease-crc.org/ont/SOMA.owl#relatesToAnotherRole"/>
        <rdfs:comment>The relation between a message and its answer.</rdfs:comment>
        <rdfs:isDefinedBy rdf:resource="http://www.ease-crc.org/ont/SOMA-ACT.owl"/>
        <rdfs:label>has answer</rdfs:label>
    </owl:ObjectProperty>
    


    <!-- http://www.ease-crc.org/ont/SOMA.owl#hasBinding -->


    <owl:ObjectProperty rdf:about="http://www.ease-crc.org/ont/SOMA.owl#hasBinding">
        <rdfs:subPropertyOf rdf:resource="http://www.ontologydesignpatterns.org/ont/dul/DUL.owl#hasPart"/>
        <rdfs:domain rdf:resource="http://www.ontologydesignpatterns.org/ont/dul/DUL.owl#Description"/>
        <rdfs:range rdf:resource="http://www.ease-crc.org/ont/SOMA.owl#Binding"/>
        <rdfs:comment>Asserts that in a context described by Description, a Binding relation holds.</rdfs:comment>
        <rdfs:isDefinedBy rdf:resource="http://www.ease-crc.org/ont/SOMA-WF.owl"/>
        <rdfs:label xml:lang="en">has binding</rdfs:label>
    </owl:ObjectProperty>
    


    <!-- http://www.ease-crc.org/ont/SOMA.owl#hasBindingFiller -->


    <owl:ObjectProperty rdf:about="http://www.ease-crc.org/ont/SOMA.owl#hasBindingFiller">
        <rdfs:subPropertyOf rdf:resource="http://www.ontologydesignpatterns.org/ont/dul/DUL.owl#describes"/>
        <rdfs:domain rdf:resource="http://www.ease-crc.org/ont/SOMA.owl#Binding"/>
        <rdfs:range rdf:resource="http://www.ontologydesignpatterns.org/ont/dul/DUL.owl#Entity"/>
        <rdfs:comment>Indicates that an Entity is described by a Binding, in that it is associated with the Role/Parameter that the Binding binds it to. The Binding is only valid in some descriptive context such as a Workflow or Narrative.

Note, the filler can be a Role/Parameter as well, and there are two distinct interpretations, depending on whether the Binding is a RoleRoleBinding or a RoleFillerBinding. See the comments on Binding for more details.

Only RoleFillerBindings can have general Entities as fillers. RoleRoleBindings can only connect to Roles or Parameters via this property.</rdfs:comment>
        <rdfs:isDefinedBy rdf:resource="http://www.ease-crc.org/ont/SOMA-WF.owl"/>
        <rdfs:label xml:lang="en">has binding filler</rdfs:label>
    </owl:ObjectProperty>
    


    <!-- http://www.ease-crc.org/ont/SOMA.owl#hasBindingRole -->


    <owl:ObjectProperty rdf:about="http://www.ease-crc.org/ont/SOMA.owl#hasBindingRole">
        <rdfs:subPropertyOf rdf:resource="http://www.ontologydesignpatterns.org/ont/dul/DUL.owl#hasPart"/>
        <rdfs:domain rdf:resource="http://www.ease-crc.org/ont/SOMA.owl#Binding"/>
        <rdfs:range>
            <owl:Class>
                <owl:unionOf rdf:parseType="Collection">
                    <rdf:Description rdf:about="http://www.ontologydesignpatterns.org/ont/dul/DUL.owl#Parameter"/>
                    <rdf:Description rdf:about="http://www.ontologydesignpatterns.org/ont/dul/DUL.owl#Role"/>
                </owl:unionOf>
            </owl:Class>
        </rdfs:range>
        <rdfs:comment>Indicates that a Role/Parameter is going to be associated to some filler, or other Role/Parameter, by a Binding. The Binding is only valid in some descriptive context such as a Narrative or Workflow.</rdfs:comment>
        <rdfs:isDefinedBy rdf:resource="http://www.ease-crc.org/ont/SOMA-WF.owl"/>
        <rdfs:label xml:lang="en">has binding role</rdfs:label>
    </owl:ObjectProperty>
    


    <!-- http://www.ease-crc.org/ont/SOMA.owl#hasColor -->


    <owl:ObjectProperty rdf:about="http://www.ease-crc.org/ont/SOMA.owl#hasColor">
        <rdfs:subPropertyOf rdf:resource="http://www.ontologydesignpatterns.org/ont/dul/DUL.owl#hasQuality"/>
        <owl:inverseOf rdf:resource="http://www.ease-crc.org/ont/SOMA.owl#isColorOf"/>
        <rdfs:domain rdf:resource="http://www.ontologydesignpatterns.org/ont/dul/DUL.owl#PhysicalObject"/>
        <rdfs:range rdf:resource="http://www.ease-crc.org/ont/SOMA.owl#Color"/>
        <rdfs:comment>Relates an object to its color quality.</rdfs:comment>
        <rdfs:isDefinedBy rdf:resource="http://www.ease-crc.org/ont/SOMA-OBJ.owl"/>
        <rdfs:label>has color</rdfs:label>
    </owl:ObjectProperty>
    


    <!-- http://www.ease-crc.org/ont/SOMA.owl#hasDesign -->


    <owl:ObjectProperty rdf:about="http://www.ease-crc.org/ont/SOMA.owl#hasDesign">
        <rdfs:subPropertyOf rdf:resource="http://www.ontologydesignpatterns.org/ont/dul/DUL.owl#isDescribedBy"/>
        <owl:inverseOf rdf:resource="http://www.ease-crc.org/ont/SOMA.owl#isDesignOf"/>
        <rdfs:domain rdf:resource="http://www.ontologydesignpatterns.org/ont/dul/DUL.owl#Object"/>
        <rdfs:range rdf:resource="http://www.ontologydesignpatterns.org/ont/dul/DUL.owl#Design"/>
        <rdfs:comment>Relates an object to the design according to which it was constructed.</rdfs:comment>
        <rdfs:isDefinedBy rdf:resource="http://www.ease-crc.org/ont/SOMA-OBJ.owl"/>
        <rdfs:label>has design</rdfs:label>
    </owl:ObjectProperty>
    


    <!-- http://www.ease-crc.org/ont/SOMA.owl#hasDisposition -->


    <owl:ObjectProperty rdf:about="http://www.ease-crc.org/ont/SOMA.owl#hasDisposition">
        <rdfs:subPropertyOf rdf:resource="http://www.ontologydesignpatterns.org/ont/dul/DUL.owl#hasQuality"/>
        <owl:inverseOf rdf:resource="http://www.ease-crc.org/ont/SOMA.owl#isDispositionOf"/>
        <rdfs:domain rdf:resource="http://www.ontologydesignpatterns.org/ont/dul/DUL.owl#Object"/>
        <rdfs:range rdf:resource="http://www.ease-crc.org/ont/SOMA.owl#Disposition"/>
        <rdfs:comment>Associates an object to one of its dispositions.</rdfs:comment>
        <rdfs:isDefinedBy rdf:resource="http://www.ease-crc.org/ont/SOMA-HOME.owl"/>
        <rdfs:isDefinedBy rdf:resource="http://www.ease-crc.org/ont/SOMA-OBJ.owl"/>
        <rdfs:label>has disposition</rdfs:label>
    </owl:ObjectProperty>
    


    <!-- http://www.ease-crc.org/ont/SOMA.owl#hasExecutionState -->


    <owl:ObjectProperty rdf:about="http://www.ease-crc.org/ont/SOMA.owl#hasExecutionState">
        <rdfs:subPropertyOf rdf:resource="http://www.ontologydesignpatterns.org/ont/dul/DUL.owl#hasRegion"/>
        <rdfs:domain rdf:resource="http://www.ontologydesignpatterns.org/ont/dul/DUL.owl#Action"/>
        <rdfs:range rdf:resource="http://www.ease-crc.org/ont/SOMA.owl#ExecutionStateRegion"/>
        <rdfs:comment>A relation from an Action to its execution state.</rdfs:comment>
        <rdfs:isDefinedBy rdf:resource="http://www.ease-crc.org/ont/SOMA-ACT.owl"/>
        <rdfs:label>has execution state</rdfs:label>
    </owl:ObjectProperty>
    


    <!-- http://www.ease-crc.org/ont/SOMA.owl#hasFeature -->


    <owl:ObjectProperty rdf:about="http://www.ease-crc.org/ont/SOMA.owl#hasFeature">
        <rdfs:subPropertyOf rdf:resource="http://www.ontologydesignpatterns.org/ont/dul/DUL.owl#hasConstituent"/>
        <owl:inverseOf rdf:resource="http://www.ease-crc.org/ont/SOMA.owl#isFeatureOf"/>
        <rdfs:domain rdf:resource="http://www.ontologydesignpatterns.org/ont/dul/DUL.owl#PhysicalObject"/>
        <rdfs:range rdf:resource="http://www.ease-crc.org/ont/SOMA.owl#Feature"/>
        <rdfs:comment>Associates a physical object to one of its features.</rdfs:comment>
        <rdfs:isDefinedBy rdf:resource="http://www.ease-crc.org/ont/SOMA-OBJ.owl"/>
        <rdfs:label>has feature</rdfs:label>
    </owl:ObjectProperty>
    


    <!-- http://www.ease-crc.org/ont/SOMA.owl#hasFirstStep -->


    <owl:ObjectProperty rdf:about="http://www.ease-crc.org/ont/SOMA.owl#hasFirstStep">
        <rdfs:subPropertyOf rdf:resource="http://www.ease-crc.org/ont/SOMA.owl#hasStep"/>
        <rdfs:domain rdf:resource="http://www.ontologydesignpatterns.org/ont/dul/DUL.owl#Workflow"/>
        <rdfs:range rdf:resource="http://www.ontologydesignpatterns.org/ont/dul/DUL.owl#Task"/>
        <rdfs:comment>A relation from a Workflow to its first Task.</rdfs:comment>
        <rdfs:isDefinedBy rdf:resource="http://www.ease-crc.org/ont/SOMA-WF.owl"/>
        <rdfs:label>has first step</rdfs:label>
    </owl:ObjectProperty>
    


    <!-- http://www.ease-crc.org/ont/SOMA.owl#hasFrictionAttribute -->


    <owl:ObjectProperty rdf:about="http://www.ease-crc.org/ont/SOMA.owl#hasFrictionAttribute">
        <rdfs:subPropertyOf rdf:resource="http://www.ontologydesignpatterns.org/ont/dul/DUL.owl#hasRegion"/>
        <rdfs:domain rdf:resource="http://www.ontologydesignpatterns.org/ont/dul/DUL.owl#PhysicalObject"/>
        <rdfs:range rdf:resource="http://www.ease-crc.org/ont/SOMA.owl#FrictionAttribute"/>
        <rdfs:comment>A relation between physical objects and their friction attribute.</rdfs:comment>
        <rdfs:isDefinedBy rdf:resource="http://www.ease-crc.org/ont/SOMA-OBJ.owl"/>
        <rdfs:label>has friction attribute</rdfs:label>
    </owl:ObjectProperty>
    


    <!-- http://www.ease-crc.org/ont/SOMA.owl#hasInitialScene -->


    <owl:ObjectProperty rdf:about="http://www.ease-crc.org/ont/SOMA.owl#hasInitialScene">
        <rdfs:subPropertyOf rdf:resource="http://www.ontologydesignpatterns.org/ont/dul/DUL.owl#includesObject"/>
        <rdf:type rdf:resource="http://www.w3.org/2002/07/owl#AsymmetricProperty"/>
        <rdf:type rdf:resource="http://www.w3.org/2002/07/owl#IrreflexiveProperty"/>
        <rdfs:domain rdf:resource="http://www.ease-crc.org/ont/SOMA.owl#StateTransition"/>
        <rdfs:range rdf:resource="http://www.ease-crc.org/ont/SOMA.owl#Scene"/>
        <rdfs:comment>A relation between StateTransitions and Scenes, which identifies the scene the transition starts from.</rdfs:comment>
        <rdfs:isDefinedBy rdf:resource="http://www.ease-crc.org/ont/SOMA-SAY.owl"/>
    </owl:ObjectProperty>
    


    <!-- http://www.ease-crc.org/ont/SOMA.owl#hasInitialSituation -->


    <owl:ObjectProperty rdf:about="http://www.ease-crc.org/ont/SOMA.owl#hasInitialSituation">
        <rdfs:subPropertyOf rdf:resource="http://www.ontologydesignpatterns.org/ont/dul/DUL.owl#includesObject"/>
        <owl:inverseOf rdf:resource="http://www.ease-crc.org/ont/SOMA.owl#isInitialSituationOf"/>
        <rdf:type rdf:resource="http://www.w3.org/2002/07/owl#AsymmetricProperty"/>
        <rdf:type rdf:resource="http://www.w3.org/2002/07/owl#IrreflexiveProperty"/>
        <rdfs:domain rdf:resource="http://www.ease-crc.org/ont/SOMA.owl#SituationTransition"/>
        <rdfs:range rdf:resource="http://www.ontologydesignpatterns.org/ont/dul/DUL.owl#Situation"/>
        <rdfs:range rdf:nodeID="genid20"/>
        <rdfs:comment>A relation between SituationTransitions and Situations, which identifies the Situation the transition starts from.</rdfs:comment>
        <rdfs:isDefinedBy rdf:resource="http://www.ease-crc.org/ont/SOMA-ACT.owl"/>
    </owl:ObjectProperty>
    <owl:Class rdf:nodeID="genid20">
        <owl:complementOf rdf:resource="http://www.ease-crc.org/ont/SOMA.owl/NonmanifestedSituation"/>
    </owl:Class>
    <owl:Axiom>
        <owl:annotatedSource rdf:resource="http://www.ease-crc.org/ont/SOMA.owl#hasInitialSituation"/>
        <owl:annotatedProperty rdf:resource="http://www.w3.org/2000/01/rdf-schema#range"/>
        <owl:annotatedTarget rdf:nodeID="genid20"/>
        <rdfs:comment>If something is an initial situation of some transition, then it must manifest.</rdfs:comment>
    </owl:Axiom>
    


    <!-- http://www.ease-crc.org/ont/SOMA.owl#hasLocalization -->


    <owl:ObjectProperty rdf:about="http://www.ease-crc.org/ont/SOMA.owl#hasLocalization">
        <rdfs:subPropertyOf rdf:resource="http://www.ontologydesignpatterns.org/ont/dul/DUL.owl#hasQuality"/>
        <owl:inverseOf rdf:resource="http://www.ease-crc.org/ont/SOMA.owl#isLocalizationOf"/>
        <rdfs:domain rdf:resource="http://www.ontologydesignpatterns.org/ont/dul/DUL.owl#PhysicalObject"/>
        <rdfs:range rdf:resource="http://www.ease-crc.org/ont/SOMA.owl#Localization"/>
        <rdfs:comment>Relates an object to its localization quality.</rdfs:comment>
        <rdfs:isDefinedBy rdf:resource="http://www.ease-crc.org/ont/SOMA-OBJ.owl"/>
        <rdfs:label>has localization</rdfs:label>
    </owl:ObjectProperty>
    


    <!-- http://www.ease-crc.org/ont/SOMA.owl#hasMassAttribute -->


    <owl:ObjectProperty rdf:about="http://www.ease-crc.org/ont/SOMA.owl#hasMassAttribute">
        <rdfs:subPropertyOf rdf:resource="http://www.ontologydesignpatterns.org/ont/dul/DUL.owl#hasRegion"/>
        <rdfs:domain rdf:resource="http://www.ontologydesignpatterns.org/ont/dul/DUL.owl#PhysicalObject"/>
        <rdfs:range rdf:resource="http://www.ease-crc.org/ont/SOMA.owl#MassAttribute"/>
        <rdfs:comment>A relation between physical objects and their mass.</rdfs:comment>
        <rdfs:isDefinedBy rdf:resource="http://www.ease-crc.org/ont/SOMA-OBJ.owl"/>
        <rdfs:label>has mass attribute</rdfs:label>
    </owl:ObjectProperty>
    


    <!-- http://www.ease-crc.org/ont/SOMA.owl#hasNextStep -->


    <owl:ObjectProperty rdf:about="http://www.ease-crc.org/ont/SOMA.owl#hasNextStep">
        <rdfs:subPropertyOf rdf:resource="http://www.ontologydesignpatterns.org/ont/dul/DUL.owl#directlyPrecedes"/>
        <rdfs:domain rdf:resource="http://www.ontologydesignpatterns.org/ont/dul/DUL.owl#Task"/>
        <rdfs:range rdf:resource="http://www.ontologydesignpatterns.org/ont/dul/DUL.owl#Task"/>
        <rdfs:comment>An ordering relation between tasks in a workflow, saying that a task is followed by another.</rdfs:comment>
        <rdfs:isDefinedBy rdf:resource="http://www.ease-crc.org/ont/SOMA-WF.owl"/>
        <rdfs:label>has next step</rdfs:label>
    </owl:ObjectProperty>
    


    <!-- http://www.ease-crc.org/ont/SOMA.owl#hasPhysicalComponent -->


    <owl:ObjectProperty rdf:about="http://www.ease-crc.org/ont/SOMA.owl#hasPhysicalComponent">
        <rdfs:isDefinedBy rdf:resource="http://www.ease-crc.org/ont/SOMA-HOME.owl"/>
        <rdfs:isDefinedBy rdf:resource="http://www.ease-crc.org/ont/SOMA-OBJ.owl"/>
    </owl:ObjectProperty>
    


    <!-- http://www.ease-crc.org/ont/SOMA.owl#hasPredecessor -->


    <owl:ObjectProperty rdf:about="http://www.ease-crc.org/ont/SOMA.owl#hasPredecessor">
        <rdfs:subPropertyOf rdf:resource="http://www.ontologydesignpatterns.org/ont/dul/DUL.owl#hasPart"/>
        <rdfs:domain rdf:resource="http://www.ease-crc.org/ont/SOMA.owl#Succedence"/>
        <rdfs:range rdf:resource="http://www.ontologydesignpatterns.org/ont/dul/DUL.owl#Workflow"/>
        <rdfs:comment>Indicates that a Task is the predecessor in a Succedence Relation; that is, this is the task to execute first.</rdfs:comment>
        <rdfs:isDefinedBy rdf:resource="http://www.ease-crc.org/ont/SOMA-WF.owl"/>
        <rdfs:label xml:lang="en">has predecessor</rdfs:label>
    </owl:ObjectProperty>
    


    <!-- http://www.ease-crc.org/ont/SOMA.owl#hasProcessType -->


    <owl:ObjectProperty rdf:about="http://www.ease-crc.org/ont/SOMA.owl#hasProcessType">
        <rdfs:subPropertyOf rdf:resource="http://www.ontologydesignpatterns.org/ont/dul/DUL.owl#isRelatedToConcept"/>
        <owl:inverseOf rdf:resource="http://www.ease-crc.org/ont/SOMA.owl#isProcessTypeOf"/>
        <rdfs:domain rdf:resource="http://www.ontologydesignpatterns.org/ont/dul/DUL.owl#Role"/>
        <rdfs:range rdf:resource="http://www.ease-crc.org/ont/SOMA.owl#ProcessType"/>
        <rdfs:comment>A relation between roles and process types, e.g. a catalysator is needed to trigger some chemical reaction.</rdfs:comment>
        <rdfs:isDefinedBy rdf:resource="http://www.ease-crc.org/ont/SOMA-PROC.owl"/>
        <rdfs:label>has process type</rdfs:label>
    </owl:ObjectProperty>
    


    <!-- http://www.ease-crc.org/ont/SOMA.owl#hasQuale -->


    <owl:ObjectProperty rdf:about="http://www.ease-crc.org/ont/SOMA.owl#hasQuale">
        <rdfs:subPropertyOf rdf:resource="http://www.ontologydesignpatterns.org/ont/dul/DUL.owl#hasRegion"/>
        <owl:inverseOf rdf:resource="http://www.ease-crc.org/ont/SOMA.owl#isQualeOf"/>
        <rdfs:domain rdf:resource="http://www.ontologydesignpatterns.org/ont/dul/DUL.owl#Quality"/>
        <rdfs:range rdf:resource="http://www.ontologydesignpatterns.org/ont/dul/DUL.owl#Region"/>
        <rdfs:comment>Relates a quality to its &quot;value&quot;, called quale, which is an atomic quality region.</rdfs:comment>
        <rdfs:isDefinedBy rdf:resource="http://www.ease-crc.org/ont/SOMA-OBJ.owl"/>
        <rdfs:label>has quale</rdfs:label>
    </owl:ObjectProperty>
    


    <!-- http://www.ease-crc.org/ont/SOMA.owl#hasShape -->


    <owl:ObjectProperty rdf:about="http://www.ease-crc.org/ont/SOMA.owl#hasShape">
        <rdfs:subPropertyOf rdf:resource="http://www.ontologydesignpatterns.org/ont/dul/DUL.owl#hasQuality"/>
        <owl:inverseOf rdf:resource="http://www.ease-crc.org/ont/SOMA.owl#isShapeOf"/>
        <rdfs:domain rdf:resource="http://www.ontologydesignpatterns.org/ont/dul/DUL.owl#PhysicalObject"/>
        <rdfs:range rdf:resource="http://www.ease-crc.org/ont/SOMA.owl#Shape"/>
        <rdfs:comment>Relates an object to its shape quality.</rdfs:comment>
        <rdfs:isDefinedBy rdf:resource="http://www.ease-crc.org/ont/SOMA-OBJ.owl"/>
        <rdfs:label>has shape</rdfs:label>
    </owl:ObjectProperty>
    


    <!-- http://www.ease-crc.org/ont/SOMA.owl#hasShapeRegion -->


    <owl:ObjectProperty rdf:about="http://www.ease-crc.org/ont/SOMA.owl#hasShapeRegion">
        <rdfs:subPropertyOf rdf:resource="http://www.ontologydesignpatterns.org/ont/dul/DUL.owl#hasRegion"/>
        <owl:inverseOf rdf:resource="http://www.ease-crc.org/ont/SOMA.owl#isShapeRegionOf"/>
        <rdfs:domain>
            <owl:Class>
                <owl:unionOf rdf:parseType="Collection">
                    <rdf:Description rdf:about="http://www.ease-crc.org/ont/SOMA.owl#Shape"/>
                    <rdf:Description rdf:about="http://www.ontologydesignpatterns.org/ont/dul/DUL.owl#PhysicalObject"/>
                </owl:unionOf>
            </owl:Class>
        </rdfs:domain>
        <rdfs:range rdf:resource="http://www.ease-crc.org/ont/SOMA.owl#ShapeRegion"/>
        <rdfs:comment>A relation between physical objects and their shape attribute.</rdfs:comment>
        <rdfs:isDefinedBy rdf:resource="http://www.ease-crc.org/ont/SOMA-HOME.owl"/>
        <rdfs:isDefinedBy rdf:resource="http://www.ease-crc.org/ont/SOMA-OBJ.owl"/>
        <rdfs:label>has shape region</rdfs:label>
    </owl:ObjectProperty>
    


    <!-- http://www.ease-crc.org/ont/SOMA.owl#hasSoftwareAgent -->


    <rdf:Description rdf:about="http://www.ease-crc.org/ont/SOMA.owl#hasSoftwareAgent">
        <rdfs:range rdf:resource="http://www.ease-crc.org/ont/SOMA.owl#SoftwareInstance"/>
    </rdf:Description>
    


    <!-- http://www.ease-crc.org/ont/SOMA.owl#hasSpaceRegion -->


    <owl:ObjectProperty rdf:about="http://www.ease-crc.org/ont/SOMA.owl#hasSpaceRegion">
        <rdfs:subPropertyOf rdf:resource="http://www.ontologydesignpatterns.org/ont/dul/DUL.owl#hasRegion"/>
        <owl:inverseOf rdf:resource="http://www.ease-crc.org/ont/SOMA.owl#isSpaceRegionFor"/>
        <rdfs:domain>
            <owl:Class>
                <owl:unionOf rdf:parseType="Collection">
                    <rdf:Description rdf:about="http://www.ease-crc.org/ont/SOMA.owl#Localization"/>
                    <rdf:Description rdf:about="http://www.ease-crc.org/ont/SOMA.owl#ShapeRegion"/>
                    <rdf:Description rdf:about="http://www.ontologydesignpatterns.org/ont/dul/DUL.owl#PhysicalObject"/>
                </owl:unionOf>
            </owl:Class>
        </rdfs:domain>
        <rdfs:range rdf:resource="http://www.ontologydesignpatterns.org/ont/dul/DUL.owl#SpaceRegion"/>
        <rdfs:comment>Relates an entity to a space region.</rdfs:comment>
        <rdfs:isDefinedBy rdf:resource="http://www.ease-crc.org/ont/SOMA-OBJ.owl"/>
        <rdfs:label>has space region</rdfs:label>
    </owl:ObjectProperty>
    


    <!-- http://www.ease-crc.org/ont/SOMA.owl#hasStateType -->


    <owl:ObjectProperty rdf:about="http://www.ease-crc.org/ont/SOMA.owl#hasStateType">
        <rdfs:subPropertyOf rdf:resource="http://www.ontologydesignpatterns.org/ont/dul/DUL.owl#isRelatedToConcept"/>
        <owl:inverseOf rdf:resource="http://www.ease-crc.org/ont/SOMA.owl#isStateTypeOf"/>
        <rdfs:domain rdf:resource="http://www.ontologydesignpatterns.org/ont/dul/DUL.owl#Role"/>
        <rdfs:range rdf:resource="http://www.ease-crc.org/ont/SOMA.owl#StateType"/>
        <rdfs:comment>A relation between roles and state types, e.g. &apos;the chair is the supporter of the person sitting on it&apos;.</rdfs:comment>
        <rdfs:isDefinedBy rdf:resource="http://www.ease-crc.org/ont/SOMA-STATE.owl"/>
        <rdfs:label>has state type</rdfs:label>
    </owl:ObjectProperty>
    


    <!-- http://www.ease-crc.org/ont/SOMA.owl#hasStep -->


    <owl:ObjectProperty rdf:about="http://www.ease-crc.org/ont/SOMA.owl#hasStep">
        <rdfs:subPropertyOf rdf:resource="http://www.ontologydesignpatterns.org/ont/dul/DUL.owl#definesTask"/>
        <rdfs:domain rdf:resource="http://www.ontologydesignpatterns.org/ont/dul/DUL.owl#Workflow"/>
        <rdfs:range rdf:resource="http://www.ontologydesignpatterns.org/ont/dul/DUL.owl#Task"/>
        <rdfs:comment>A relation between a Workflow and a Task it contains.</rdfs:comment>
        <rdfs:isDefinedBy rdf:resource="http://www.ease-crc.org/ont/SOMA-WF.owl"/>
        <rdfs:label>has step</rdfs:label>
    </owl:ObjectProperty>
    


    <!-- http://www.ease-crc.org/ont/SOMA.owl#hasSuccedence -->


    <owl:ObjectProperty rdf:about="http://www.ease-crc.org/ont/SOMA.owl#hasSuccedence">
        <rdfs:subPropertyOf rdf:resource="http://www.ontologydesignpatterns.org/ont/dul/DUL.owl#hasPart"/>
        <rdfs:domain rdf:resource="http://www.ontologydesignpatterns.org/ont/dul/DUL.owl#Workflow"/>
        <rdfs:range rdf:resource="http://www.ease-crc.org/ont/SOMA.owl#Succedence"/>
        <rdfs:comment>A relation between a Workflow and a Succedence that appears in it.</rdfs:comment>
        <rdfs:isDefinedBy rdf:resource="http://www.ease-crc.org/ont/SOMA-WF.owl"/>
        <rdfs:label xml:lang="en">has succedence</rdfs:label>
    </owl:ObjectProperty>
    


    <!-- http://www.ease-crc.org/ont/SOMA.owl#hasSuccessor -->


    <owl:ObjectProperty rdf:about="http://www.ease-crc.org/ont/SOMA.owl#hasSuccessor">
        <rdfs:subPropertyOf rdf:resource="http://www.ontologydesignpatterns.org/ont/dul/DUL.owl#hasPart"/>
        <rdfs:domain rdf:resource="http://www.ease-crc.org/ont/SOMA.owl#Succedence"/>
        <rdfs:range rdf:resource="http://www.ontologydesignpatterns.org/ont/dul/DUL.owl#Workflow"/>
        <rdfs:comment>Indicates that a Task is the successor in a Succedence Relation: that is, it is the Task to execute last.</rdfs:comment>
        <rdfs:isDefinedBy rdf:resource="http://www.ease-crc.org/ont/SOMA-WF.owl"/>
        <rdfs:label xml:lang="en">has successor</rdfs:label>
    </owl:ObjectProperty>
    


    <!-- http://www.ease-crc.org/ont/SOMA.owl#hasTask -->


    <owl:ObjectProperty rdf:about="http://www.ease-crc.org/ont/SOMA.owl#hasTask">
        <rdfs:subPropertyOf rdf:resource="http://www.ontologydesignpatterns.org/ont/dul/DUL.owl#hasPart"/>
        <rdfs:domain>
            <owl:Class>
                <owl:unionOf rdf:parseType="Collection">
                    <rdf:Description rdf:about="http://www.ontologydesignpatterns.org/ont/dul/DUL.owl#Relation"/>
                    <rdf:Description rdf:about="http://www.ontologydesignpatterns.org/ont/dul/DUL.owl#Workflow"/>
                </owl:unionOf>
            </owl:Class>
        </rdfs:domain>
        <rdfs:range rdf:resource="http://www.ontologydesignpatterns.org/ont/dul/DUL.owl#Task"/>
        <rdfs:comment>A relation to indicate that a Task is part of a Workflow or ordering Relation: that is, the task may be executed during the execution of the Workflow, or there exists some Relation between the Tasks that informs how their executions are to be located in time.</rdfs:comment>
        <rdfs:isDefinedBy rdf:resource="http://www.ease-crc.org/ont/SOMA-WF.owl"/>
        <rdfs:label xml:lang="en">has task</rdfs:label>
    </owl:ObjectProperty>
    


    <!-- http://www.ease-crc.org/ont/SOMA.owl#hasTerminalScene -->


    <owl:ObjectProperty rdf:about="http://www.ease-crc.org/ont/SOMA.owl#hasTerminalScene">
        <rdfs:subPropertyOf rdf:resource="http://www.ontologydesignpatterns.org/ont/dul/DUL.owl#includesObject"/>
        <rdf:type rdf:resource="http://www.w3.org/2002/07/owl#AsymmetricProperty"/>
        <rdf:type rdf:resource="http://www.w3.org/2002/07/owl#IrreflexiveProperty"/>
        <rdfs:domain rdf:resource="http://www.ease-crc.org/ont/SOMA.owl#StateTransition"/>
        <rdfs:range rdf:resource="http://www.ease-crc.org/ont/SOMA.owl#Scene"/>
        <rdfs:comment>A relation between StateTransitions and Scenes, which identifies the scene the transition is expected to end at.</rdfs:comment>
        <rdfs:isDefinedBy rdf:resource="http://www.ease-crc.org/ont/SOMA-SAY.owl"/>
    </owl:ObjectProperty>
    


    <!-- http://www.ease-crc.org/ont/SOMA.owl#hasTerminalSituation -->


    <owl:ObjectProperty rdf:about="http://www.ease-crc.org/ont/SOMA.owl#hasTerminalSituation">
        <rdfs:subPropertyOf rdf:resource="http://www.ontologydesignpatterns.org/ont/dul/DUL.owl#includesObject"/>
        <owl:inverseOf rdf:resource="http://www.ease-crc.org/ont/SOMA.owl#isTerminalSituationOf"/>
        <rdf:type rdf:resource="http://www.w3.org/2002/07/owl#AsymmetricProperty"/>
        <rdf:type rdf:resource="http://www.w3.org/2002/07/owl#IrreflexiveProperty"/>
        <rdfs:domain rdf:resource="http://www.ease-crc.org/ont/SOMA.owl#SituationTransition"/>
        <rdfs:range rdf:resource="http://www.ontologydesignpatterns.org/ont/dul/DUL.owl#Situation"/>
        <rdfs:range rdf:nodeID="genid32"/>
        <rdfs:comment>A relation between SituationTransitions and Situations, which identifies the Situation the transition ends at.</rdfs:comment>
        <rdfs:isDefinedBy rdf:resource="http://www.ease-crc.org/ont/SOMA-ACT.owl"/>
    </owl:ObjectProperty>
    <owl:Class rdf:nodeID="genid32">
        <owl:complementOf rdf:resource="http://www.ease-crc.org/ont/SOMA.owl/NonmanifestedSituation"/>
    </owl:Class>
    <owl:Axiom>
        <owl:annotatedSource rdf:resource="http://www.ease-crc.org/ont/SOMA.owl#hasTerminalSituation"/>
        <owl:annotatedProperty rdf:resource="http://www.w3.org/2000/01/rdf-schema#range"/>
        <owl:annotatedTarget rdf:nodeID="genid32"/>
        <rdfs:comment>If something is a terminal situation then it must be a manifested situation (regardless of whether it was expected or not).</rdfs:comment>
    </owl:Axiom>
    


    <!-- http://www.ease-crc.org/ont/SOMA.owl#interactsWith -->


    <owl:ObjectProperty rdf:about="http://www.ease-crc.org/ont/SOMA.owl#interactsWith">
        <rdfs:subPropertyOf rdf:resource="http://www.ontologydesignpatterns.org/ont/dul/DUL.owl#associatedWith"/>
        <rdf:type rdf:resource="http://www.w3.org/2002/07/owl#SymmetricProperty"/>
        <rdfs:domain rdf:resource="http://www.ontologydesignpatterns.org/ont/dul/DUL.owl#PhysicalObject"/>
        <rdfs:range rdf:resource="http://www.ontologydesignpatterns.org/ont/dul/DUL.owl#PhysicalObject"/>
        <rdfs:comment>A relation between objects that interact with each other.</rdfs:comment>
        <rdfs:isDefinedBy rdf:resource="http://www.ease-crc.org/ont/SOMA-PROC.owl"/>
        <rdfs:isDefinedBy rdf:resource="http://www.ease-crc.org/ont/SOMA-SAY.owl"/>
        <rdfs:label>interacts with</rdfs:label>
    </owl:ObjectProperty>
    


    <!-- http://www.ease-crc.org/ont/SOMA.owl#involvesEffector -->


    <owl:ObjectProperty rdf:about="http://www.ease-crc.org/ont/SOMA.owl#involvesEffector">
        <rdfs:subPropertyOf rdf:resource="http://www.ontologydesignpatterns.org/ont/dul/DUL.owl#hasParticipant"/>
        <owl:inverseOf rdf:resource="http://www.ease-crc.org/ont/SOMA.owl#isEffectorInvolvedIn"/>
        <rdfs:domain rdf:resource="http://www.ontologydesignpatterns.org/ont/dul/DUL.owl#Event"/>
        <rdfs:range rdf:resource="http://www.ease-crc.org/ont/SOMA.owl#PhysicalEffector"/>
        <rdfs:comment>Effector participation.</rdfs:comment>
        <rdfs:isDefinedBy rdf:resource="http://www.ease-crc.org/ont/SOMA-OBJ.owl"/>
        <rdfs:label>involves effector</rdfs:label>
    </owl:ObjectProperty>
    


    <!-- http://www.ease-crc.org/ont/SOMA.owl#isAlterationResultOf -->


    <owl:ObjectProperty rdf:about="http://www.ease-crc.org/ont/SOMA.owl#isAlterationResultOf">
        <rdfs:subPropertyOf rdf:resource="http://www.ontologydesignpatterns.org/ont/dul/DUL.owl#isRegionFor"/>
        <rdfs:domain rdf:resource="http://www.ontologydesignpatterns.org/ont/dul/DUL.owl#Region"/>
        <rdfs:range rdf:resource="http://www.ontologydesignpatterns.org/ont/dul/DUL.owl#Action"/>
        <rdfs:comment>Relates an action that alters an object to the region that the alteration reached during the action.</rdfs:comment>
        <rdfs:isDefinedBy rdf:resource="http://www.ease-crc.org/ont/SOMA-OBJ.owl"/>
        <rdfs:label>is alteration result of</rdfs:label>
    </owl:ObjectProperty>
    


    <!-- http://www.ease-crc.org/ont/SOMA.owl#isAnsweredBy -->


    <owl:ObjectProperty rdf:about="http://www.ease-crc.org/ont/SOMA.owl#isAnsweredBy">
        <rdfs:subPropertyOf rdf:resource="http://www.ontologydesignpatterns.org/ont/dul/DUL.owl#involvesAgent"/>
        <rdfs:domain rdf:resource="http://www.ontologydesignpatterns.org/ont/dul/DUL.owl#Event"/>
        <rdfs:range rdf:resource="http://www.ontologydesignpatterns.org/ont/dul/DUL.owl#Agent"/>
        <rdfs:comment>A relation from a Query to an Agent who answers it.</rdfs:comment>
        <rdfs:isDefinedBy rdf:resource="http://www.ease-crc.org/ont/SOMA-SAY.owl"/>
        <rdfs:label>is answered by</rdfs:label>
    </owl:ObjectProperty>
    


    <!-- http://www.ease-crc.org/ont/SOMA.owl#isAskedBy -->


    <owl:ObjectProperty rdf:about="http://www.ease-crc.org/ont/SOMA.owl#isAskedBy">
        <rdfs:subPropertyOf rdf:resource="http://www.ontologydesignpatterns.org/ont/dul/DUL.owl#involvesAgent"/>
        <rdfs:domain rdf:resource="http://www.ease-crc.org/ont/SOMA.owl#QueryingTask"/>
        <rdfs:range rdf:resource="http://www.ontologydesignpatterns.org/ont/dul/DUL.owl#Agent"/>
        <rdfs:comment>A relation from a Query to the Agent who asks it.</rdfs:comment>
        <rdfs:isDefinedBy rdf:resource="http://www.ease-crc.org/ont/SOMA-ACT.owl"/>
        <rdfs:label>is asked by</rdfs:label>
    </owl:ObjectProperty>
    


    <!-- http://www.ease-crc.org/ont/SOMA.owl#isBearerAffordedBy -->


    <owl:ObjectProperty rdf:about="http://www.ease-crc.org/ont/SOMA.owl#isBearerAffordedBy">
        <rdfs:subPropertyOf rdf:resource="http://www.ease-crc.org/ont/SOMA.owl#isConceptAffordedBy"/>
        <rdfs:domain rdf:resource="http://www.ontologydesignpatterns.org/ont/dul/DUL.owl#Role"/>
        <rdfs:range rdf:resource="http://www.ease-crc.org/ont/SOMA.owl#Disposition"/>
        <owl:propertyChainAxiom rdf:parseType="Collection">
            <rdf:Description rdf:about="http://www.ease-crc.org/ont/SOMA.owl#isBearerDefinedIn"/>
            <rdf:Description rdf:about="http://www.ontologydesignpatterns.org/ont/dul/DUL.owl#describes"/>
        </owl:propertyChainAxiom>
        <rdfs:comment>Relates a disposition to the bearer role defined by the affordance describing the disposition.</rdfs:comment>
        <rdfs:isDefinedBy rdf:resource="http://www.ease-crc.org/ont/SOMA-OBJ.owl"/>
        <rdfs:label>is bearer afforded by</rdfs:label>
    </owl:ObjectProperty>
    


    <!-- http://www.ease-crc.org/ont/SOMA.owl#isBearerDefinedIn -->


    <owl:ObjectProperty rdf:about="http://www.ease-crc.org/ont/SOMA.owl#isBearerDefinedIn">
        <rdfs:subPropertyOf rdf:resource="http://www.ontologydesignpatterns.org/ont/dul/DUL.owl#isRoleDefinedIn"/>
        <rdfs:domain rdf:resource="http://www.ontologydesignpatterns.org/ont/dul/DUL.owl#Role"/>
        <rdfs:range rdf:resource="http://www.ease-crc.org/ont/SOMA.owl#Affordance"/>
        <rdfs:comment>Relates an affordance which is a relation between a bearer and a trigger, to the role of the bearer when the affordance is manifested.</rdfs:comment>
        <rdfs:isDefinedBy rdf:resource="http://www.ease-crc.org/ont/SOMA-OBJ.owl"/>
        <rdfs:label>is bearer defined in</rdfs:label>
    </owl:ObjectProperty>
    


    <!-- http://www.ease-crc.org/ont/SOMA.owl#isColorOf -->


    <owl:ObjectProperty rdf:about="http://www.ease-crc.org/ont/SOMA.owl#isColorOf">
        <rdfs:subPropertyOf rdf:resource="http://www.ontologydesignpatterns.org/ont/dul/DUL.owl#isQualityOf"/>
        <rdfs:domain rdf:resource="http://www.ease-crc.org/ont/SOMA.owl#Color"/>
        <rdfs:range rdf:resource="http://www.ontologydesignpatterns.org/ont/dul/DUL.owl#PhysicalObject"/>
        <rdfs:comment>Relates a color quality to the object the color belongs to.</rdfs:comment>
        <rdfs:isDefinedBy rdf:resource="http://www.ease-crc.org/ont/SOMA-OBJ.owl"/>
        <rdfs:label>is color of</rdfs:label>
    </owl:ObjectProperty>
    


    <!-- http://www.ease-crc.org/ont/SOMA.owl#isConceptAffordedBy -->


    <owl:ObjectProperty rdf:about="http://www.ease-crc.org/ont/SOMA.owl#isConceptAffordedBy">
        <rdfs:subPropertyOf rdf:resource="http://www.ontologydesignpatterns.org/ont/dul/DUL.owl#associatedWith"/>
        <rdfs:domain rdf:resource="http://www.ontologydesignpatterns.org/ont/dul/DUL.owl#Concept"/>
        <rdfs:range rdf:resource="http://www.ease-crc.org/ont/SOMA.owl#Disposition"/>
        <owl:propertyChainAxiom rdf:parseType="Collection">
            <rdf:Description rdf:about="http://www.ease-crc.org/ont/SOMA.owl#isDefinedInAffordance"/>
            <rdf:Description rdf:about="http://www.ontologydesignpatterns.org/ont/dul/DUL.owl#describes"/>
        </owl:propertyChainAxiom>
        <rdfs:comment>A relation between a disposition and a concept defined in the affordance that describes the disposition.</rdfs:comment>
        <rdfs:isDefinedBy rdf:resource="http://www.ease-crc.org/ont/SOMA-OBJ.owl"/>
        <rdfs:label>is concept afforded by</rdfs:label>
    </owl:ObjectProperty>
    


    <!-- http://www.ease-crc.org/ont/SOMA.owl#isCoveredByObject -->


    <owl:ObjectProperty rdf:about="http://www.ease-crc.org/ont/SOMA.owl#isCoveredByObject">
        <rdfs:subPropertyOf rdf:resource="http://www.ease-crc.org/ont/SOMA.owl#interactsWith"/>
        <rdf:type rdf:resource="http://www.w3.org/2002/07/owl#AsymmetricProperty"/>
        <rdf:type rdf:resource="http://www.w3.org/2002/07/owl#IrreflexiveProperty"/>
        <rdfs:domain rdf:resource="http://www.ontologydesignpatterns.org/ont/dul/DUL.owl#PhysicalObject"/>
        <rdfs:range rdf:resource="http://www.ontologydesignpatterns.org/ont/dul/DUL.owl#PhysicalObject"/>
        <rdfs:comment>A relation from an object (the coveree) which is itself, or has its interior, prevented from being accessed from outside by a coverer.</rdfs:comment>
        <rdfs:isDefinedBy rdf:resource="http://www.ease-crc.org/ont/SOMA-SAY.owl"/>
    </owl:ObjectProperty>
    


    <!-- http://www.ease-crc.org/ont/SOMA.owl#isDefinedInAffordance -->


    <owl:ObjectProperty rdf:about="http://www.ease-crc.org/ont/SOMA.owl#isDefinedInAffordance">
        <rdfs:subPropertyOf rdf:resource="http://www.ontologydesignpatterns.org/ont/dul/DUL.owl#isDefinedIn"/>
        <rdfs:domain rdf:resource="http://www.ontologydesignpatterns.org/ont/dul/DUL.owl#Concept"/>
        <rdfs:range rdf:resource="http://www.ease-crc.org/ont/SOMA.owl#Affordance"/>
        <rdfs:comment>A relation between a Concept and an Affordance.</rdfs:comment>
        <rdfs:isDefinedBy rdf:resource="http://www.ease-crc.org/ont/SOMA-OBJ.owl"/>
        <rdfs:label>is defined in affordance</rdfs:label>
    </owl:ObjectProperty>
    


    <!-- http://www.ease-crc.org/ont/SOMA.owl#isDepositOf -->


    <owl:ObjectProperty rdf:about="http://www.ease-crc.org/ont/SOMA.owl#isDepositOf">
        <rdfs:subPropertyOf rdf:resource="http://www.ontologydesignpatterns.org/ont/dul/DUL.owl#isLocationOf"/>
        <owl:inverseOf rdf:resource="http://www.ease-crc.org/ont/SOMA.owl#isOntopOf"/>
        <rdfs:domain rdf:resource="http://www.ontologydesignpatterns.org/ont/dul/DUL.owl#PhysicalObject"/>
        <rdfs:range rdf:resource="http://www.ontologydesignpatterns.org/ont/dul/DUL.owl#PhysicalObject"/>
        <rdfs:comment>A spatial relation holding between an object (the deposit), and objects that are located ontop of it.</rdfs:comment>
        <rdfs:isDefinedBy rdf:resource="http://www.ease-crc.org/ont/SOMA-OBJ.owl"/>
        <rdfs:label>is deposit of</rdfs:label>
    </owl:ObjectProperty>
    


    <!-- http://www.ease-crc.org/ont/SOMA.owl#isDesignFor -->


    <owl:ObjectProperty rdf:about="http://www.ease-crc.org/ont/SOMA.owl#isDesignFor">
        <rdfs:subPropertyOf rdf:resource="http://www.ontologydesignpatterns.org/ont/dul/DUL.owl#describes"/>
        <owl:inverseOf rdf:resource="http://www.ease-crc.org/ont/SOMA.owl#isDesignedBy"/>
        <rdfs:domain rdf:resource="http://www.ontologydesignpatterns.org/ont/dul/DUL.owl#Design"/>
        <rdfs:range rdf:resource="http://www.ontologydesignpatterns.org/ont/dul/DUL.owl#DesignedArtifact"/>
        <rdfs:comment xml:lang="en">A special relation between a Design and a DesignedArtifact, to indicate that the Design describes a way to construct the DesignedArtifact.</rdfs:comment>
        <rdfs:isDefinedBy rdf:resource="http://www.ease-crc.org/ont/SOMA-IO.owl"/>
        <rdfs:label xml:lang="en">is design for</rdfs:label>
    </owl:ObjectProperty>
    


    <!-- http://www.ease-crc.org/ont/SOMA.owl#isDesignOf -->


    <owl:ObjectProperty rdf:about="http://www.ease-crc.org/ont/SOMA.owl#isDesignOf">
        <rdfs:subPropertyOf rdf:resource="http://www.ontologydesignpatterns.org/ont/dul/DUL.owl#describes"/>
        <rdfs:domain rdf:resource="http://www.ontologydesignpatterns.org/ont/dul/DUL.owl#Design"/>
        <rdfs:range rdf:resource="http://www.ontologydesignpatterns.org/ont/dul/DUL.owl#Object"/>
        <rdfs:comment>Relates a design to an object that was constructed according to it.</rdfs:comment>
        <rdfs:isDefinedBy rdf:resource="http://www.ease-crc.org/ont/SOMA-OBJ.owl"/>
        <rdfs:label>is design of</rdfs:label>
    </owl:ObjectProperty>
    


    <!-- http://www.ease-crc.org/ont/SOMA.owl#isDesignedBy -->


    <owl:ObjectProperty rdf:about="http://www.ease-crc.org/ont/SOMA.owl#isDesignedBy">
        <rdfs:subPropertyOf rdf:resource="http://www.ontologydesignpatterns.org/ont/dul/DUL.owl#isDescribedBy"/>
        <rdfs:domain rdf:resource="http://www.ontologydesignpatterns.org/ont/dul/DUL.owl#DesignedArtifact"/>
        <rdfs:range rdf:resource="http://www.ontologydesignpatterns.org/ont/dul/DUL.owl#Design"/>
        <rdfs:comment xml:lang="en">A special relation between a Design and a Designed Artifact, to indicate that the Designed Artifact is described by the Design.</rdfs:comment>
        <rdfs:isDefinedBy rdf:resource="http://www.ease-crc.org/ont/SOMA-IO.owl"/>
        <rdfs:label xml:lang="en">is designed by</rdfs:label>
    </owl:ObjectProperty>
    


    <!-- http://www.ease-crc.org/ont/SOMA.owl#isDispositionOf -->


    <owl:ObjectProperty rdf:about="http://www.ease-crc.org/ont/SOMA.owl#isDispositionOf">
        <rdfs:subPropertyOf rdf:resource="http://www.ontologydesignpatterns.org/ont/dul/DUL.owl#isQualityOf"/>
        <rdfs:domain rdf:resource="http://www.ease-crc.org/ont/SOMA.owl#Disposition"/>
        <rdfs:range rdf:resource="http://www.ontologydesignpatterns.org/ont/dul/DUL.owl#Object"/>
        <rdfs:comment>Associates a disposition quality to the object holding it.</rdfs:comment>
        <rdfs:isDefinedBy rdf:resource="http://www.ease-crc.org/ont/SOMA-OBJ.owl"/>
        <rdfs:label>is disposition of</rdfs:label>
    </owl:ObjectProperty>
    


    <!-- http://www.ease-crc.org/ont/SOMA.owl#isEffectorInvolvedIn -->


    <owl:ObjectProperty rdf:about="http://www.ease-crc.org/ont/SOMA.owl#isEffectorInvolvedIn">
        <rdfs:subPropertyOf rdf:resource="http://www.ontologydesignpatterns.org/ont/dul/DUL.owl#isParticipantIn"/>
        <rdfs:domain rdf:resource="http://www.ease-crc.org/ont/SOMA.owl#PhysicalEffector"/>
        <rdfs:range rdf:resource="http://www.ontologydesignpatterns.org/ont/dul/DUL.owl#Event"/>
        <rdfs:comment>Effector participation.</rdfs:comment>
        <rdfs:isDefinedBy rdf:resource="http://www.ease-crc.org/ont/SOMA-OBJ.owl"/>
        <rdfs:label>is effector involved in</rdfs:label>
    </owl:ObjectProperty>
    


    <!-- http://www.ease-crc.org/ont/SOMA.owl#isFeatureOf -->


    <owl:ObjectProperty rdf:about="http://www.ease-crc.org/ont/SOMA.owl#isFeatureOf">
        <rdfs:subPropertyOf rdf:resource="http://www.ontologydesignpatterns.org/ont/dul/DUL.owl#isConstituentOf"/>
        <rdfs:domain rdf:resource="http://www.ease-crc.org/ont/SOMA.owl#Feature"/>
        <rdfs:range rdf:resource="http://www.ontologydesignpatterns.org/ont/dul/DUL.owl#PhysicalObject"/>
        <rdfs:comment>Associates a feature to the physical object it belongs to.</rdfs:comment>
        <rdfs:isDefinedBy rdf:resource="http://www.ease-crc.org/ont/SOMA-OBJ.owl"/>
        <rdfs:label>is feature of</rdfs:label>
    </owl:ObjectProperty>
    


    <!-- http://www.ease-crc.org/ont/SOMA.owl#isGivenMeaningBy -->


    <owl:ObjectProperty rdf:about="http://www.ease-crc.org/ont/SOMA.owl#isGivenMeaningBy">
        <rdfs:subPropertyOf rdf:resource="http://www.ontologydesignpatterns.org/ont/dul/DUL.owl#associatedWith"/>
        <rdfs:domain rdf:resource="http://www.ontologydesignpatterns.org/ont/dul/DUL.owl#InformationObject"/>
        <rdfs:range rdf:resource="http://www.ease-crc.org/ont/SOMA.owl#System"/>
        <rdfs:comment xml:lang="en">The relation between an Information Object and a System that gives meaning to said object, e.g., a word, sentence, text, etc. might be given meaning by a Language and without the knowledge of said System (Language), the text will not make sense to a reader.</rdfs:comment>
        <rdfs:isDefinedBy rdf:resource="http://www.ease-crc.org/ont/SOMA-IO.owl"/>
        <rdfs:label xml:lang="en">is given meaning by</rdfs:label>
    </owl:ObjectProperty>
    


    <!-- http://www.ease-crc.org/ont/SOMA.owl#isInitialSituationOf -->


    <owl:ObjectProperty rdf:about="http://www.ease-crc.org/ont/SOMA.owl#isInitialSituationOf">
        <rdfs:subPropertyOf rdf:resource="http://www.ontologydesignpatterns.org/ont/dul/DUL.owl#isObjectIncludedIn"/>
        <rdfs:domain rdf:resource="http://www.ontologydesignpatterns.org/ont/dul/DUL.owl#Situation"/>
        <rdfs:range rdf:resource="http://www.ease-crc.org/ont/SOMA.owl#SituationTransition"/>
        <rdfs:comment>A relation between SituationTransitions and Situations, which identifies the Situation the transition starts from.</rdfs:comment>
        <rdfs:isDefinedBy rdf:resource="http://www.ease-crc.org/ont/SOMA-ACT.owl"/>
        <rdfs:label xml:lang="en">is initial situation of</rdfs:label>
    </owl:ObjectProperty>
    


    <!-- http://www.ease-crc.org/ont/SOMA.owl#isInsideOf -->


    <owl:ObjectProperty rdf:about="http://www.ease-crc.org/ont/SOMA.owl#isInsideOf">
        <rdfs:subPropertyOf rdf:resource="http://www.ease-crc.org/ont/SOMA.owl#isContainedIn"/>
        <rdfs:subPropertyOf rdf:resource="http://www.ontologydesignpatterns.org/ont/dul/DUL.owl#hasLocation"/>
        <rdf:type rdf:resource="http://www.w3.org/2002/07/owl#TransitiveProperty"/>
        <rdfs:domain rdf:resource="http://www.ontologydesignpatterns.org/ont/dul/DUL.owl#PhysicalObject"/>
        <rdfs:range rdf:resource="http://www.ontologydesignpatterns.org/ont/dul/DUL.owl#PhysicalObject"/>
        <rdfs:comment>A spatial relation holding between an object (the container), and objects it contains.</rdfs:comment>
        <rdfs:isDefinedBy rdf:resource="http://www.ease-crc.org/ont/SOMA-OBJ.owl"/>
        <rdfs:label>is inside of</rdfs:label>
    </owl:ObjectProperty>
    


    <!-- http://www.ease-crc.org/ont/SOMA.owl#isLinkedTo -->


    <owl:ObjectProperty rdf:about="http://www.ease-crc.org/ont/SOMA.owl#isLinkedTo">
        <rdfs:subPropertyOf rdf:resource="http://www.ontologydesignpatterns.org/ont/dul/DUL.owl#hasLocation"/>
        <rdf:type rdf:resource="http://www.w3.org/2002/07/owl#SymmetricProperty"/>
        <rdfs:domain rdf:resource="http://www.ontologydesignpatterns.org/ont/dul/DUL.owl#PhysicalObject"/>
        <rdfs:range rdf:resource="http://www.ontologydesignpatterns.org/ont/dul/DUL.owl#PhysicalObject"/>
        <rdfs:comment>A spatial relation holding between objects that are linked with each other such that they resist spatial separation.</rdfs:comment>
        <rdfs:isDefinedBy rdf:resource="http://www.ease-crc.org/ont/SOMA-OBJ.owl"/>
        <rdfs:label>is linked to</rdfs:label>
    </owl:ObjectProperty>
    


    <!-- http://www.ease-crc.org/ont/SOMA.owl#isLocalizationOf -->


    <owl:ObjectProperty rdf:about="http://www.ease-crc.org/ont/SOMA.owl#isLocalizationOf">
        <rdfs:subPropertyOf rdf:resource="http://www.ontologydesignpatterns.org/ont/dul/DUL.owl#isQualityOf"/>
        <rdfs:domain rdf:resource="http://www.ease-crc.org/ont/SOMA.owl#Localization"/>
        <rdfs:range rdf:resource="http://www.ontologydesignpatterns.org/ont/dul/DUL.owl#PhysicalObject"/>
        <rdfs:comment>Relates a localization quality to the object the localization belongs to.</rdfs:comment>
        <rdfs:isDefinedBy rdf:resource="http://www.ease-crc.org/ont/SOMA-OBJ.owl"/>
        <rdfs:label>is localization of</rdfs:label>
    </owl:ObjectProperty>
    


    <!-- http://www.ease-crc.org/ont/SOMA.owl#isMovedByAgent -->


    <owl:ObjectProperty rdf:about="http://www.ease-crc.org/ont/SOMA.owl#isMovedByAgent">
        <rdfs:subPropertyOf rdf:resource="http://www.ease-crc.org/ont/SOMA.owl#interactsWith"/>
        <owl:inverseOf rdf:resource="http://www.ease-crc.org/ont/SOMA.owl#movesObject"/>
        <rdfs:domain rdf:resource="http://www.ontologydesignpatterns.org/ont/dul/DUL.owl#PhysicalObject"/>
        <rdfs:range rdf:resource="http://www.ontologydesignpatterns.org/ont/dul/DUL.owl#Agent"/>
        <rdfs:comment>A relation from an object to an agent who causes it to move.</rdfs:comment>
        <rdfs:isDefinedBy rdf:resource="http://www.ease-crc.org/ont/SOMA-SAY.owl"/>
    </owl:ObjectProperty>
    


    <!-- http://www.ease-crc.org/ont/SOMA.owl#isOntopOf -->


    <owl:ObjectProperty rdf:about="http://www.ease-crc.org/ont/SOMA.owl#isOntopOf">
        <rdfs:subPropertyOf rdf:resource="http://www.ontologydesignpatterns.org/ont/dul/DUL.owl#hasLocation"/>
        <rdfs:domain rdf:resource="http://www.ontologydesignpatterns.org/ont/dul/DUL.owl#PhysicalObject"/>
        <rdfs:range rdf:resource="http://www.ontologydesignpatterns.org/ont/dul/DUL.owl#PhysicalObject"/>
        <rdfs:comment>A spatial relation holding between an object (the deposit), and objects that are located ontop of it.</rdfs:comment>
        <rdfs:isDefinedBy rdf:resource="http://www.ease-crc.org/ont/SOMA-OBJ.owl"/>
        <rdfs:label>is ontop of</rdfs:label>
    </owl:ObjectProperty>
    


    <!-- http://www.ease-crc.org/ont/SOMA.owl#isParameterDefinedIn -->


    <owl:ObjectProperty rdf:about="http://www.ease-crc.org/ont/SOMA.owl#isParameterDefinedIn">
        <rdfs:subPropertyOf rdf:resource="http://www.ontologydesignpatterns.org/ont/dul/DUL.owl#isDefinedIn"/>
        <rdfs:domain rdf:resource="http://www.ontologydesignpatterns.org/ont/dul/DUL.owl#Parameter"/>
        <rdfs:range rdf:resource="http://www.ontologydesignpatterns.org/ont/dul/DUL.owl#Description"/>
        <rdfs:comment>A relation between a description and a parameter.</rdfs:comment>
        <rdfs:isDefinedBy rdf:resource="http://www.ease-crc.org/ont/SOMA-OBJ.owl"/>
        <rdfs:label>is parameter defined in</rdfs:label>
    </owl:ObjectProperty>
    


    <!-- http://www.ease-crc.org/ont/SOMA.owl#isPerformedBy -->


    <owl:ObjectProperty rdf:about="http://www.ease-crc.org/ont/SOMA.owl#isPerformedBy">
        <rdfs:subPropertyOf rdf:resource="http://www.ontologydesignpatterns.org/ont/dul/DUL.owl#involvesAgent"/>
        <rdfs:domain rdf:resource="http://www.ontologydesignpatterns.org/ont/dul/DUL.owl#Action"/>
        <rdfs:range rdf:resource="http://www.ontologydesignpatterns.org/ont/dul/DUL.owl#Agent"/>
        <rdfs:comment>A relation from an Action to the Agent who performs it.</rdfs:comment>
        <rdfs:isDefinedBy rdf:resource="http://www.ease-crc.org/ont/SOMA-ACT.owl"/>
        <rdfs:label>is performed by</rdfs:label>
    </owl:ObjectProperty>
    


    <!-- http://www.ease-crc.org/ont/SOMA.owl#isPhysicallyContainedIn -->


    <owl:ObjectProperty rdf:about="http://www.ease-crc.org/ont/SOMA.owl#isPhysicallyContainedIn">
        <rdfs:subPropertyOf rdf:resource="http://www.ontologydesignpatterns.org/ont/dul/DUL.owl#isLocationOf"/>
        <rdfs:domain rdf:resource="http://www.ontologydesignpatterns.org/ont/dul/DUL.owl#Entity"/>
        <rdfs:range rdf:resource="http://www.ontologydesignpatterns.org/ont/dul/DUL.owl#Entity"/>
        <rdfs:comment>A spatial relation holding between an object (the container), and objects it contains.</rdfs:comment>
        <rdfs:isDefinedBy rdf:resource="http://www.ease-crc.org/ont/SOMA-OBJ.owl"/>
        <rdfs:label>is physically contained in</rdfs:label>
    </owl:ObjectProperty>
    


    <!-- http://www.ease-crc.org/ont/SOMA.owl#isPlanFor -->


    <owl:ObjectProperty rdf:about="http://www.ease-crc.org/ont/SOMA.owl#isPlanFor">
        <rdfs:isDefinedBy rdf:resource="http://www.ease-crc.org/ont/SOMA-WF.owl"/>
    </owl:ObjectProperty>
    


    <!-- http://www.ease-crc.org/ont/SOMA.owl#isProcessDefinedIn -->


    <owl:ObjectProperty rdf:about="http://www.ease-crc.org/ont/SOMA.owl#isProcessDefinedIn">
        <rdfs:subPropertyOf rdf:resource="http://www.ontologydesignpatterns.org/ont/dul/DUL.owl#isDefinedIn"/>
        <rdfs:domain rdf:resource="http://www.ease-crc.org/ont/SOMA.owl#ProcessType"/>
        <rdfs:range rdf:resource="http://www.ontologydesignpatterns.org/ont/dul/DUL.owl#Description"/>
        <rdfs:comment>A relation between a process type and a description that defines it.</rdfs:comment>
        <rdfs:isDefinedBy rdf:resource="http://www.ease-crc.org/ont/SOMA-PROC.owl"/>
        <rdfs:label>is process defined in</rdfs:label>
    </owl:ObjectProperty>
    


    <!-- http://www.ease-crc.org/ont/SOMA.owl#isProcessTypeOf -->


    <owl:ObjectProperty rdf:about="http://www.ease-crc.org/ont/SOMA.owl#isProcessTypeOf">
        <rdfs:subPropertyOf rdf:resource="http://www.ontologydesignpatterns.org/ont/dul/DUL.owl#isRelatedToConcept"/>
        <rdfs:domain rdf:resource="http://www.ease-crc.org/ont/SOMA.owl#ProcessType"/>
        <rdfs:range rdf:resource="http://www.ontologydesignpatterns.org/ont/dul/DUL.owl#Role"/>
        <rdfs:comment>A relation between roles and process types, e.g. a catalysator is needed to trigger some chemical reaction.</rdfs:comment>
        <rdfs:isDefinedBy rdf:resource="http://www.ease-crc.org/ont/SOMA-PROC.owl"/>
        <rdfs:label>is process type of</rdfs:label>
    </owl:ObjectProperty>
    


    <!-- http://www.ease-crc.org/ont/SOMA.owl#isQualeOf -->


    <owl:ObjectProperty rdf:about="http://www.ease-crc.org/ont/SOMA.owl#isQualeOf">
        <rdfs:subPropertyOf rdf:resource="http://www.ontologydesignpatterns.org/ont/dul/DUL.owl#isRegionFor"/>
        <rdfs:domain rdf:resource="http://www.ontologydesignpatterns.org/ont/dul/DUL.owl#Region"/>
        <rdfs:range rdf:resource="http://www.ontologydesignpatterns.org/ont/dul/DUL.owl#Quality"/>
        <rdfs:comment>Relates a quality to its &quot;value&quot;, called quale, which is an atomic quality region.</rdfs:comment>
        <rdfs:isDefinedBy rdf:resource="http://www.ease-crc.org/ont/SOMA-OBJ.owl"/>
        <rdfs:label>is quale of</rdfs:label>
    </owl:ObjectProperty>
    


    <!-- http://www.ease-crc.org/ont/SOMA.owl#isQualityDescribedBy -->


    <owl:ObjectProperty rdf:about="http://www.ease-crc.org/ont/SOMA.owl#isQualityDescribedBy">
        <rdfs:subPropertyOf rdf:resource="http://www.ontologydesignpatterns.org/ont/dul/DUL.owl#isDescribedBy"/>
        <rdfs:domain rdf:resource="http://www.ontologydesignpatterns.org/ont/dul/DUL.owl#Quality"/>
        <rdfs:range rdf:resource="http://www.ontologydesignpatterns.org/ont/dul/DUL.owl#Description"/>
        <rdfs:comment>Relates a description to a quality it describes.</rdfs:comment>
        <rdfs:isDefinedBy rdf:resource="http://www.ease-crc.org/ont/SOMA-OBJ.owl"/>
        <rdfs:label>is quality described by</rdfs:label>
    </owl:ObjectProperty>
    


    <!-- http://www.ease-crc.org/ont/SOMA.owl#isSetpointAffordedBy -->


    <owl:ObjectProperty rdf:about="http://www.ease-crc.org/ont/SOMA.owl#isSetpointAffordedBy">
        <rdfs:subPropertyOf rdf:resource="http://www.ease-crc.org/ont/SOMA.owl#isConceptAffordedBy"/>
        <rdfs:domain rdf:resource="http://www.ease-crc.org/ont/SOMA.owl#Setpoint"/>
        <rdfs:range rdf:resource="http://www.ease-crc.org/ont/SOMA.owl#Disposition"/>
        <owl:propertyChainAxiom rdf:parseType="Collection">
            <rdf:Description rdf:about="http://www.ease-crc.org/ont/SOMA.owl#isSetpointDefinedIn"/>
            <rdf:Description rdf:about="http://www.ontologydesignpatterns.org/ont/dul/DUL.owl#describes"/>
        </owl:propertyChainAxiom>
        <rdfs:comment>Relates a disposition to the setpoint parameter defined by the affordance describing the disposition.</rdfs:comment>
        <rdfs:isDefinedBy rdf:resource="http://www.ease-crc.org/ont/SOMA-OBJ.owl"/>
        <rdfs:label>is setpoint afforded by</rdfs:label>
    </owl:ObjectProperty>
    


    <!-- http://www.ease-crc.org/ont/SOMA.owl#isSetpointDefinedIn -->


    <owl:ObjectProperty rdf:about="http://www.ease-crc.org/ont/SOMA.owl#isSetpointDefinedIn">
        <rdfs:subPropertyOf rdf:resource="http://www.ease-crc.org/ont/SOMA.owl#isParameterDefinedIn"/>
        <rdfs:domain rdf:resource="http://www.ease-crc.org/ont/SOMA.owl#Setpoint"/>
        <rdfs:range rdf:resource="http://www.ontologydesignpatterns.org/ont/dul/DUL.owl#Description"/>
        <rdfs:comment>Defines the dedicated goal region of a description.</rdfs:comment>
        <rdfs:isDefinedBy rdf:resource="http://www.ease-crc.org/ont/SOMA-OBJ.owl"/>
        <rdfs:label>is setpoint defined in</rdfs:label>
    </owl:ObjectProperty>
    


    <!-- http://www.ease-crc.org/ont/SOMA.owl#isShapeOf -->


    <owl:ObjectProperty rdf:about="http://www.ease-crc.org/ont/SOMA.owl#isShapeOf">
        <rdfs:subPropertyOf rdf:resource="http://www.ontologydesignpatterns.org/ont/dul/DUL.owl#isQualityOf"/>
        <rdfs:domain rdf:resource="http://www.ease-crc.org/ont/SOMA.owl#Shape"/>
        <rdfs:range rdf:resource="http://www.ontologydesignpatterns.org/ont/dul/DUL.owl#PhysicalObject"/>
        <rdfs:comment>Relates a shape quality to the object the shape belongs to.</rdfs:comment>
        <rdfs:isDefinedBy rdf:resource="http://www.ease-crc.org/ont/SOMA-OBJ.owl"/>
        <rdfs:label>is shape of</rdfs:label>
    </owl:ObjectProperty>
    


    <!-- http://www.ease-crc.org/ont/SOMA.owl#isShapeRegionOf -->


    <owl:ObjectProperty rdf:about="http://www.ease-crc.org/ont/SOMA.owl#isShapeRegionOf">
        <rdfs:subPropertyOf rdf:resource="http://www.ontologydesignpatterns.org/ont/dul/DUL.owl#isRegionFor"/>
        <rdfs:domain rdf:resource="http://www.ease-crc.org/ont/SOMA.owl#ShapeRegion"/>
        <rdfs:range>
            <owl:Class>
                <owl:unionOf rdf:parseType="Collection">
                    <rdf:Description rdf:about="http://www.ease-crc.org/ont/SOMA.owl#Shape"/>
                    <rdf:Description rdf:about="http://www.ontologydesignpatterns.org/ont/dul/DUL.owl#PhysicalObject"/>
                </owl:unionOf>
            </owl:Class>
        </rdfs:range>
        <rdfs:comment>Relates a shape to a physical object that has it.</rdfs:comment>
        <rdfs:isDefinedBy rdf:resource="http://www.ease-crc.org/ont/SOMA-OBJ.owl"/>
        <rdfs:label>is shape region of</rdfs:label>
    </owl:ObjectProperty>
    


    <!-- http://www.ease-crc.org/ont/SOMA.owl#isSpaceRegionFor -->


    <owl:ObjectProperty rdf:about="http://www.ease-crc.org/ont/SOMA.owl#isSpaceRegionFor">
        <rdfs:subPropertyOf rdf:resource="http://www.ontologydesignpatterns.org/ont/dul/DUL.owl#isRegionFor"/>
        <rdfs:domain rdf:resource="http://www.ontologydesignpatterns.org/ont/dul/DUL.owl#SpaceRegion"/>
        <rdfs:range>
            <owl:Class>
                <owl:unionOf rdf:parseType="Collection">
                    <rdf:Description rdf:about="http://www.ease-crc.org/ont/SOMA.owl#Localization"/>
                    <rdf:Description rdf:about="http://www.ontologydesignpatterns.org/ont/dul/DUL.owl#PhysicalObject"/>
                </owl:unionOf>
            </owl:Class>
        </rdfs:range>
        <rdfs:comment>Relates a space region to an entity.</rdfs:comment>
        <rdfs:isDefinedBy rdf:resource="http://www.ease-crc.org/ont/SOMA-OBJ.owl"/>
        <rdfs:label>is space region for</rdfs:label>
    </owl:ObjectProperty>
    


    <!-- http://www.ease-crc.org/ont/SOMA.owl#isStateTypeOf -->


    <owl:ObjectProperty rdf:about="http://www.ease-crc.org/ont/SOMA.owl#isStateTypeOf">
        <rdfs:subPropertyOf rdf:resource="http://www.ontologydesignpatterns.org/ont/dul/DUL.owl#isRelatedToConcept"/>
        <rdfs:domain rdf:resource="http://www.ease-crc.org/ont/SOMA.owl#StateType"/>
        <rdfs:range rdf:resource="http://www.ontologydesignpatterns.org/ont/dul/DUL.owl#Role"/>
        <rdfs:comment>A relation between roles and state types, e.g. &apos;the chair is the supporter of the person sitting on it&apos;.</rdfs:comment>
        <rdfs:isDefinedBy rdf:resource="http://www.ease-crc.org/ont/SOMA-STATE.owl"/>
        <rdfs:label>is state type of</rdfs:label>
    </owl:ObjectProperty>
    


    <!-- http://www.ease-crc.org/ont/SOMA.owl#isSupportedBy -->


    <owl:ObjectProperty rdf:about="http://www.ease-crc.org/ont/SOMA.owl#isSupportedBy">
        <rdfs:subPropertyOf rdf:resource="http://www.ease-crc.org/ont/SOMA.owl#interactsWith"/>
        <rdfs:subPropertyOf rdf:resource="http://www.ontologydesignpatterns.org/ont/dul/DUL.owl#hasCommonBoundary"/>
        <owl:inverseOf rdf:resource="http://www.ease-crc.org/ont/SOMA.owl#supports"/>
        <rdfs:domain rdf:resource="http://www.ontologydesignpatterns.org/ont/dul/DUL.owl#Entity"/>
        <rdfs:range rdf:resource="http://www.ontologydesignpatterns.org/ont/dul/DUL.owl#Entity"/>
        <rdfs:comment>A relation between an object (the supporter) and another object (the supportee) where the supporter cancels the effect of gravity on the supportee.</rdfs:comment>
        <rdfs:comment>Relates a supportee to one of its supporters.</rdfs:comment>
        <rdfs:isDefinedBy rdf:resource="http://www.ease-crc.org/ont/SOMA-OBJ.owl"/>
        <rdfs:isDefinedBy rdf:resource="http://www.ease-crc.org/ont/SOMA-PROC.owl"/>
        <rdfs:label>is supported by</rdfs:label>
    </owl:ObjectProperty>
    


    <!-- http://www.ease-crc.org/ont/SOMA.owl#isTaskAffordedBy -->


    <owl:ObjectProperty rdf:about="http://www.ease-crc.org/ont/SOMA.owl#isTaskAffordedBy">
        <rdfs:subPropertyOf rdf:resource="http://www.ease-crc.org/ont/SOMA.owl#isConceptAffordedBy"/>
        <rdfs:domain rdf:resource="http://www.ontologydesignpatterns.org/ont/dul/DUL.owl#Task"/>
        <rdfs:range rdf:resource="http://www.ease-crc.org/ont/SOMA.owl#Disposition"/>
        <owl:propertyChainAxiom rdf:parseType="Collection">
            <rdf:Description rdf:about="http://www.ease-crc.org/ont/SOMA.owl#isTaskDefinedInAffordance"/>
            <rdf:Description rdf:about="http://www.ontologydesignpatterns.org/ont/dul/DUL.owl#describes"/>
        </owl:propertyChainAxiom>
        <rdfs:comment>Relates a disposition to the task defined by the affordance describing the disposition.</rdfs:comment>
        <rdfs:isDefinedBy rdf:resource="http://www.ease-crc.org/ont/SOMA-OBJ.owl"/>
        <rdfs:label>is task afforded by</rdfs:label>
    </owl:ObjectProperty>
    


    <!-- http://www.ease-crc.org/ont/SOMA.owl#isTaskDefinedInAffordance -->


    <owl:ObjectProperty rdf:about="http://www.ease-crc.org/ont/SOMA.owl#isTaskDefinedInAffordance">
        <rdfs:subPropertyOf rdf:resource="http://www.ease-crc.org/ont/SOMA.owl#isDefinedInAffordance"/>
        <rdfs:subPropertyOf rdf:resource="http://www.ontologydesignpatterns.org/ont/dul/DUL.owl#isTaskDefinedIn"/>
        <rdfs:domain rdf:resource="http://www.ontologydesignpatterns.org/ont/dul/DUL.owl#Task"/>
        <rdfs:range rdf:resource="http://www.ease-crc.org/ont/SOMA.owl#Affordance"/>
        <rdfs:comment>A relation between a Task and an Affordance, such that the task is defined in terms of using the affordance.</rdfs:comment>
        <rdfs:isDefinedBy rdf:resource="http://www.ease-crc.org/ont/SOMA-OBJ.owl"/>
        <rdfs:label>is task defined in affordance</rdfs:label>
    </owl:ObjectProperty>
    


    <!-- http://www.ease-crc.org/ont/SOMA.owl#isTerminalSituationOf -->


    <owl:ObjectProperty rdf:about="http://www.ease-crc.org/ont/SOMA.owl#isTerminalSituationOf">
        <rdfs:subPropertyOf rdf:resource="http://www.ontologydesignpatterns.org/ont/dul/DUL.owl#isObjectIncludedIn"/>
        <rdfs:domain rdf:resource="http://www.ontologydesignpatterns.org/ont/dul/DUL.owl#Situation"/>
        <rdfs:range rdf:resource="http://www.ease-crc.org/ont/SOMA.owl#SituationTransition"/>
        <rdfs:comment>A relation between SituationTransitions and Situations, which identifies the Situation the transition ends at.</rdfs:comment>
        <rdfs:isDefinedBy rdf:resource="http://www.ease-crc.org/ont/SOMA-ACT.owl"/>
        <rdfs:label xml:lang="en">is terminal situation of</rdfs:label>
    </owl:ObjectProperty>
    


    <!-- http://www.ease-crc.org/ont/SOMA.owl#isTriggerAffordedBy -->


    <owl:ObjectProperty rdf:about="http://www.ease-crc.org/ont/SOMA.owl#isTriggerAffordedBy">
        <rdfs:subPropertyOf rdf:resource="http://www.ease-crc.org/ont/SOMA.owl#isConceptAffordedBy"/>
        <rdfs:domain rdf:resource="http://www.ontologydesignpatterns.org/ont/dul/DUL.owl#Role"/>
        <rdfs:range rdf:resource="http://www.ease-crc.org/ont/SOMA.owl#Disposition"/>
        <owl:propertyChainAxiom rdf:parseType="Collection">
            <rdf:Description rdf:about="http://www.ease-crc.org/ont/SOMA.owl#isTriggerDefinedIn"/>
            <rdf:Description rdf:about="http://www.ontologydesignpatterns.org/ont/dul/DUL.owl#describes"/>
        </owl:propertyChainAxiom>
        <rdfs:comment>Relates a disposition to the trigger role defined by the affordance describing the disposition.</rdfs:comment>
        <rdfs:isDefinedBy rdf:resource="http://www.ease-crc.org/ont/SOMA-OBJ.owl"/>
        <rdfs:label>is trigger afforded by</rdfs:label>
    </owl:ObjectProperty>
    


    <!-- http://www.ease-crc.org/ont/SOMA.owl#isTriggerDefinedIn -->


    <owl:ObjectProperty rdf:about="http://www.ease-crc.org/ont/SOMA.owl#isTriggerDefinedIn">
        <rdfs:subPropertyOf rdf:resource="http://www.ontologydesignpatterns.org/ont/dul/DUL.owl#isRoleDefinedIn"/>
        <rdfs:domain rdf:resource="http://www.ontologydesignpatterns.org/ont/dul/DUL.owl#Role"/>
        <rdfs:range rdf:resource="http://www.ease-crc.org/ont/SOMA.owl#Affordance"/>
        <rdfs:comment>Relates an affordance which is a relation between a bearer and a trigger, to the role of the trigger when the affordance is manifested.</rdfs:comment>
        <rdfs:isDefinedBy rdf:resource="http://www.ease-crc.org/ont/SOMA-OBJ.owl"/>
        <rdfs:label>is trigger defined in</rdfs:label>
    </owl:ObjectProperty>
    


    <!-- http://www.ease-crc.org/ont/SOMA.owl#movesObject -->


    <owl:ObjectProperty rdf:about="http://www.ease-crc.org/ont/SOMA.owl#movesObject">
        <rdfs:subPropertyOf rdf:resource="http://www.ease-crc.org/ont/SOMA.owl#interactsWith"/>
        <rdfs:domain rdf:resource="http://www.ontologydesignpatterns.org/ont/dul/DUL.owl#Agent"/>
        <rdfs:range rdf:resource="http://www.ontologydesignpatterns.org/ont/dul/DUL.owl#PhysicalObject"/>
        <rdfs:comment>A relation from an agent to an object that the agent causes to move.</rdfs:comment>
        <rdfs:isDefinedBy rdf:resource="http://www.ease-crc.org/ont/SOMA-SAY.owl"/>
    </owl:ObjectProperty>
    


    <!-- http://www.ease-crc.org/ont/SOMA.owl#relatesToAnotherRole -->


    <owl:ObjectProperty rdf:about="http://www.ease-crc.org/ont/SOMA.owl#relatesToAnotherRole">
        <rdfs:subPropertyOf rdf:resource="http://www.ontologydesignpatterns.org/ont/dul/DUL.owl#associatedWith"/>
        <rdf:type rdf:resource="http://www.w3.org/2002/07/owl#SymmetricProperty"/>
        <rdfs:domain rdf:resource="http://www.ontologydesignpatterns.org/ont/dul/DUL.owl#Role"/>
        <rdfs:range rdf:resource="http://www.ontologydesignpatterns.org/ont/dul/DUL.owl#Role"/>
        <rdfs:comment>Simple top-level property for relations between two roles.</rdfs:comment>
        <rdfs:isDefinedBy rdf:resource="http://www.ease-crc.org/ont/SOMA-ACT.owl"/>
        <rdfs:label>relates to another role</rdfs:label>
    </owl:ObjectProperty>
    


    <!-- http://www.ease-crc.org/ont/SOMA.owl#supports -->


    <owl:ObjectProperty rdf:about="http://www.ease-crc.org/ont/SOMA.owl#supports">
        <rdfs:subPropertyOf rdf:resource="http://www.ease-crc.org/ont/SOMA.owl#interactsWith"/>
        <rdfs:subPropertyOf rdf:resource="http://www.ontologydesignpatterns.org/ont/dul/DUL.owl#hasCommonBoundary"/>
        <rdfs:domain rdf:resource="http://www.ontologydesignpatterns.org/ont/dul/DUL.owl#Entity"/>
        <rdfs:range rdf:resource="http://www.ontologydesignpatterns.org/ont/dul/DUL.owl#Entity"/>
        <rdfs:comment>A relation between an object (the supporter) and another object (the supportee) where the supporter cancels the effect of gravity on the supportee.</rdfs:comment>
        <rdfs:comment>Relates a supportee to one of its supporters.</rdfs:comment>
        <rdfs:isDefinedBy rdf:resource="http://www.ease-crc.org/ont/SOMA-OBJ.owl"/>
        <rdfs:isDefinedBy rdf:resource="http://www.ease-crc.org/ont/SOMA-PROC.owl"/>
    </owl:ObjectProperty>
    


    <!-- http://www.ease-crc.org/ont/SOMA.owl#transitionsBack -->


    <owl:ObjectProperty rdf:about="http://www.ease-crc.org/ont/SOMA.owl#transitionsBack">
        <rdfs:subPropertyOf rdf:resource="http://www.ease-crc.org/ont/SOMA.owl#transitionsFrom"/>
        <rdfs:subPropertyOf rdf:resource="http://www.ease-crc.org/ont/SOMA.owl#transitionsTo"/>
        <rdfs:domain rdf:resource="http://www.ease-crc.org/ont/SOMA.owl#Transient"/>
        <rdfs:range rdf:resource="http://www.ontologydesignpatterns.org/ont/dul/DUL.owl#Object"/>
        <rdfs:comment>A property which relates a Transient to an Object it both changes from and changes into. This is useful to model objects which, through participation in a process, transform themselves so that an ontological reclassification is necessary, however this transformation is reversible and at the end of the process the objects revert to their previous kind. An example of this is catalysts in chemistry.</rdfs:comment>
        <rdfs:isDefinedBy rdf:resource="http://www.ease-crc.org/ont/SOMA-OBJ.owl"/>
        <rdfs:label xml:lang="en">transitions back</rdfs:label>
    </owl:ObjectProperty>
    


    <!-- http://www.ease-crc.org/ont/SOMA.owl#transitionsFrom -->


    <owl:ObjectProperty rdf:about="http://www.ease-crc.org/ont/SOMA.owl#transitionsFrom">
        <rdfs:subPropertyOf rdf:resource="http://www.ontologydesignpatterns.org/ont/dul/DUL.owl#hasCommonBoundary"/>
        <rdfs:domain rdf:resource="http://www.ease-crc.org/ont/SOMA.owl#Transient"/>
        <rdfs:range rdf:resource="http://www.ontologydesignpatterns.org/ont/dul/DUL.owl#Object"/>
        <rdfs:comment>A property which relates a Transient to an Object it changes from. This is useful to model objects which, through participation in a process, transform themselves so that an ontological reclassification is necessary. An example of this is dough undergoing the Maillard reaction through baking.</rdfs:comment>
        <rdfs:isDefinedBy rdf:resource="http://www.ease-crc.org/ont/SOMA-OBJ.owl"/>
        <rdfs:label xml:lang="en">transitions from</rdfs:label>
    </owl:ObjectProperty>
    


    <!-- http://www.ease-crc.org/ont/SOMA.owl#transitionsTo -->


    <owl:ObjectProperty rdf:about="http://www.ease-crc.org/ont/SOMA.owl#transitionsTo">
        <rdfs:subPropertyOf rdf:resource="http://www.ontologydesignpatterns.org/ont/dul/DUL.owl#hasCommonBoundary"/>
        <rdfs:domain rdf:resource="http://www.ease-crc.org/ont/SOMA.owl#Transient"/>
        <rdfs:range rdf:resource="http://www.ontologydesignpatterns.org/ont/dul/DUL.owl#Object"/>
        <rdfs:comment>A property which relates a Transient to an Object it changes into. This is useful to model objects which, through participation in a process, transform themselves so that an ontological reclassification is necessary. An example of this is baked dough eventually becoming bread by completing a baking process.</rdfs:comment>
        <rdfs:isDefinedBy rdf:resource="http://www.ease-crc.org/ont/SOMA-OBJ.owl"/>
        <rdfs:label xml:lang="en">transitions to</rdfs:label>
    </owl:ObjectProperty>
    


    <!-- http://www.ease-crc.org/ont/SOMA.owl/hasExpectedTerminalSituation -->


    <owl:ObjectProperty rdf:about="http://www.ease-crc.org/ont/SOMA.owl/hasExpectedTerminalSituation">
        <rdfs:subPropertyOf rdf:resource="http://www.ease-crc.org/ont/SOMA.owl#hasTerminalSituation"/>
        <rdfs:subPropertyOf rdf:resource="http://www.ontologydesignpatterns.org/ont/dul/DUL.owl#hasPostcondition"/>
        <rdfs:comment>A relation between a Transition and the Situation it is expected to, and does actually, end at. You can assert this relationship when the observed outcome of a transition matches expectations.</rdfs:comment>
        <rdfs:isDefinedBy rdf:resource="http://www.ease-crc.org/ont/SOMA-ACT.owl"/>
    </owl:ObjectProperty>
    


    <!-- http://www.ease-crc.org/ont/SOMA.owl/hasRequiredInitialSituation -->


    <owl:ObjectProperty rdf:about="http://www.ease-crc.org/ont/SOMA.owl/hasRequiredInitialSituation">
        <rdfs:subPropertyOf rdf:resource="http://www.ease-crc.org/ont/SOMA.owl#hasInitialSituation"/>
        <rdfs:subPropertyOf rdf:resource="http://www.ontologydesignpatterns.org/ont/dul/DUL.owl#hasPrecondition"/>
        <rdfs:comment>A relationship between a Situation x and another Situation y that precedes it, such that without y manifesting, it would be impossible for x to manifest.</rdfs:comment>
        <rdfs:isDefinedBy rdf:resource="http://www.ease-crc.org/ont/SOMA-ACT.owl"/>
        <rdfs:label xml:lang="en">has required initial situation</rdfs:label>
    </owl:ObjectProperty>
    


    <!-- http://www.ease-crc.org/ont/SOMA.owl/manifestsIn -->


    <owl:ObjectProperty rdf:about="http://www.ease-crc.org/ont/SOMA.owl/manifestsIn">
        <rdfs:subPropertyOf rdf:resource="http://www.ontologydesignpatterns.org/ont/dul/DUL.owl#includesEvent"/>
        <rdfs:comment>A relationship indicating that a Situation is realized in an Event that actually happened.</rdfs:comment>
        <rdfs:isDefinedBy rdf:resource="http://www.ease-crc.org/ont/SOMA-ACT.owl"/>
        <rdfs:label>manifests in</rdfs:label>
    </owl:ObjectProperty>
    


    <!-- http://www.ease-crc.org/ont/SOMA.owl/preventedBy -->


    <owl:ObjectProperty rdf:about="http://www.ease-crc.org/ont/SOMA.owl/preventedBy">
        <rdfs:subPropertyOf rdf:resource="http://www.ontologydesignpatterns.org/ont/dul/DUL.owl#hasSetting"/>
        <owl:inverseOf rdf:resource="http://www.ease-crc.org/ont/SOMA.owl/prevents"/>
        <rdfs:domain rdf:resource="http://www.ontologydesignpatterns.org/ont/dul/DUL.owl#Situation"/>
        <rdfs:range rdf:resource="http://www.ontologydesignpatterns.org/ont/dul/DUL.owl#Situation"/>
        <rdfs:comment>A relationship indicating a Situation is prevented by another from manifesting.</rdfs:comment>
        <rdfs:isDefinedBy rdf:resource="http://www.ease-crc.org/ont/SOMA-ACT.owl"/>
        <rdfs:label>prevented by</rdfs:label>
    </owl:ObjectProperty>
    


    <!-- http://www.ease-crc.org/ont/SOMA.owl/prevents -->


    <owl:ObjectProperty rdf:about="http://www.ease-crc.org/ont/SOMA.owl/prevents">
        <rdfs:subPropertyOf rdf:resource="http://www.ontologydesignpatterns.org/ont/dul/DUL.owl#isSettingFor"/>
        <rdfs:domain rdf:resource="http://www.ontologydesignpatterns.org/ont/dul/DUL.owl#Situation"/>
        <rdfs:range rdf:resource="http://www.ontologydesignpatterns.org/ont/dul/DUL.owl#Situation"/>
        <rdfs:comment>A relationship indicating that a situation does or would prevent another from manifesting. Useful for reasoning about planning (what to do to avoid some bad outcome) and failure recovery (what aspects of the world state prevent continuing the plan?).</rdfs:comment>
        <rdfs:isDefinedBy rdf:resource="http://www.ease-crc.org/ont/SOMA-ACT.owl"/>
        <rdfs:label>prevents</rdfs:label>
    </owl:ObjectProperty>
    


    <!-- http://www.ontologydesignpatterns.org/ont/dul/DUL.owl#associatedWith -->


    <owl:ObjectProperty rdf:about="http://www.ontologydesignpatterns.org/ont/dul/DUL.owl#associatedWith">
        <rdfs:isDefinedBy rdf:resource="http://www.ease-crc.org/ont/SOMA-PROC.owl"/>
    </owl:ObjectProperty>
    


    <!-- http://www.ontologydesignpatterns.org/ont/dul/DUL.owl#classifies -->


    <owl:ObjectProperty rdf:about="http://www.ontologydesignpatterns.org/ont/dul/DUL.owl#classifies">
        <rdfs:isDefinedBy rdf:resource="http://www.ease-crc.org/ont/SOMA-HOME.owl"/>
        <rdfs:isDefinedBy rdf:resource="http://www.ease-crc.org/ont/SOMA-PROC.owl"/>
        <rdfs:isDefinedBy rdf:resource="http://www.ease-crc.org/ont/SOMA-STATE.owl"/>
    </owl:ObjectProperty>
    


    <!-- http://www.ontologydesignpatterns.org/ont/dul/DUL.owl#defines -->


    <owl:ObjectProperty rdf:about="http://www.ontologydesignpatterns.org/ont/dul/DUL.owl#defines">
        <rdfs:isDefinedBy rdf:resource="http://www.ease-crc.org/ont/SOMA-PROC.owl"/>
        <rdfs:isDefinedBy rdf:resource="http://www.ease-crc.org/ont/SOMA-WF.owl"/>
    </owl:ObjectProperty>
    


    <!-- http://www.ontologydesignpatterns.org/ont/dul/DUL.owl#definesRole -->


    <owl:ObjectProperty rdf:about="http://www.ontologydesignpatterns.org/ont/dul/DUL.owl#definesRole">
        <rdfs:isDefinedBy rdf:resource="http://www.ease-crc.org/ont/SOMA-STATE.owl"/>
    </owl:ObjectProperty>
    


    <!-- http://www.ontologydesignpatterns.org/ont/dul/DUL.owl#describes -->


    <owl:ObjectProperty rdf:about="http://www.ontologydesignpatterns.org/ont/dul/DUL.owl#describes">
        <rdfs:isDefinedBy rdf:resource="http://www.ease-crc.org/ont/SOMA-STATE.owl"/>
        <rdfs:isDefinedBy rdf:resource="http://www.ease-crc.org/ont/SOMA-WF.owl"/>
    </owl:ObjectProperty>
    


    <!-- http://www.ontologydesignpatterns.org/ont/dul/DUL.owl#expresses -->


    <rdf:Description rdf:about="http://www.ontologydesignpatterns.org/ont/dul/DUL.owl#expresses">
        <rdfs:subPropertyOf rdf:resource="http://www.ontologydesignpatterns.org/ont/dul/DUL.owl#isAbout"/>
    </rdf:Description>
    


    <!-- http://www.ontologydesignpatterns.org/ont/dul/DUL.owl#hasPart -->


    <owl:ObjectProperty rdf:about="http://www.ontologydesignpatterns.org/ont/dul/DUL.owl#hasPart">
        <rdfs:isDefinedBy rdf:resource="http://www.ease-crc.org/ont/SOMA-PROC.owl"/>
        <rdfs:isDefinedBy rdf:resource="http://www.ease-crc.org/ont/SOMA-STATE.owl"/>
        <rdfs:isDefinedBy rdf:resource="http://www.ease-crc.org/ont/SOMA-WF.owl"/>
    </owl:ObjectProperty>
    


    <!-- http://www.ontologydesignpatterns.org/ont/dul/DUL.owl#hasParticipant -->


    <owl:ObjectProperty rdf:about="http://www.ontologydesignpatterns.org/ont/dul/DUL.owl#hasParticipant">
        <rdfs:isDefinedBy rdf:resource="http://www.ease-crc.org/ont/SOMA-PROC.owl"/>
        <rdfs:isDefinedBy rdf:resource="http://www.ease-crc.org/ont/SOMA-STATE.owl"/>
    </owl:ObjectProperty>
    


    <!-- http://www.ontologydesignpatterns.org/ont/dul/DUL.owl#hasPostcondition -->


    <rdf:Description rdf:about="http://www.ontologydesignpatterns.org/ont/dul/DUL.owl#hasPostcondition">
        <rdfs:comment>This should be taken to mean that the postcondition is the situation expected to follow the current situation. Whether the expectation is met is another issue.</rdfs:comment>
    </rdf:Description>
    


    <!-- http://www.ontologydesignpatterns.org/ont/dul/DUL.owl#hasPrecondition -->


    <rdf:Description rdf:about="http://www.ontologydesignpatterns.org/ont/dul/DUL.owl#hasPrecondition">
        <rdfs:comment>This should be taken to mean: a precondition is a situation without which the current situation would not be possible.</rdfs:comment>
    </rdf:Description>
    


    <!-- http://www.ontologydesignpatterns.org/ont/dul/DUL.owl#hasQuality -->


    <owl:ObjectProperty rdf:about="http://www.ontologydesignpatterns.org/ont/dul/DUL.owl#hasQuality">
        <rdfs:isDefinedBy rdf:resource="http://www.ease-crc.org/ont/SOMA-HOME.owl"/>
        <rdfs:isDefinedBy rdf:resource="http://www.ease-crc.org/ont/SOMA-OBJ.owl"/>
    </owl:ObjectProperty>
    


    <!-- http://www.ontologydesignpatterns.org/ont/dul/DUL.owl#isDefinedIn -->


    <owl:ObjectProperty rdf:about="http://www.ontologydesignpatterns.org/ont/dul/DUL.owl#isDefinedIn">
        <rdfs:isDefinedBy rdf:resource="http://www.ease-crc.org/ont/SOMA-PROC.owl"/>
    </owl:ObjectProperty>
    


    <!-- http://www.ontologydesignpatterns.org/ont/dul/DUL.owl#isDescribedBy -->


    <owl:ObjectProperty rdf:about="http://www.ontologydesignpatterns.org/ont/dul/DUL.owl#isDescribedBy">
        <rdfs:isDefinedBy rdf:resource="http://www.ease-crc.org/ont/SOMA-OBJ.owl"/>
        <rdfs:isDefinedBy rdf:resource="http://www.ease-crc.org/ont/SOMA-STATE.owl"/>
    </owl:ObjectProperty>
    


    <!-- http://www.ontologydesignpatterns.org/ont/dul/DUL.owl#isExpressedBy -->


    <rdf:Description rdf:about="http://www.ontologydesignpatterns.org/ont/dul/DUL.owl#isExpressedBy">
        <rdfs:subPropertyOf rdf:resource="http://www.ontologydesignpatterns.org/ont/dul/DUL.owl#isReferenceOf"/>
    </rdf:Description>
    


    <!-- http://www.ontologydesignpatterns.org/ont/dul/DUL.owl#isPartOf -->


    <owl:ObjectProperty rdf:about="http://www.ontologydesignpatterns.org/ont/dul/DUL.owl#isPartOf">
        <rdfs:isDefinedBy rdf:resource="http://www.ease-crc.org/ont/SOMA-PROC.owl"/>
    </owl:ObjectProperty>
    


    <!-- http://www.ontologydesignpatterns.org/ont/dul/DUL.owl#isQualityOf -->


    <owl:ObjectProperty rdf:about="http://www.ontologydesignpatterns.org/ont/dul/DUL.owl#isQualityOf">
        <rdfs:isDefinedBy rdf:resource="http://www.ease-crc.org/ont/SOMA-HOME.owl"/>
    </owl:ObjectProperty>
    


    <!-- http://www.ontologydesignpatterns.org/ont/dul/DUL.owl#isRelatedToConcept -->


    <owl:ObjectProperty rdf:about="http://www.ontologydesignpatterns.org/ont/dul/DUL.owl#isRelatedToConcept">
        <rdfs:isDefinedBy rdf:resource="http://www.ease-crc.org/ont/SOMA-PROC.owl"/>
        <rdfs:isDefinedBy rdf:resource="http://www.ease-crc.org/ont/SOMA-STATE.owl"/>
    </owl:ObjectProperty>
    


    <!-- http://www.ontologydesignpatterns.org/ont/dul/DUL.owl#satisfies -->


    <owl:ObjectProperty rdf:about="http://www.ontologydesignpatterns.org/ont/dul/DUL.owl#satisfies">
        <rdfs:isDefinedBy rdf:resource="http://www.ease-crc.org/ont/SOMA-PROC.owl"/>
    </owl:ObjectProperty>
    


    <!-- 
    ///////////////////////////////////////////////////////////////////////////////////////
    //
    // Data properties
    //
    ///////////////////////////////////////////////////////////////////////////////////////
     -->


    


    <!-- http://www.ease-crc.org/ont/SOMA-OBJ.owl#hasForceValue -->


    <owl:DatatypeProperty rdf:about="http://www.ease-crc.org/ont/SOMA-OBJ.owl#hasForceValue">
        <rdfs:subPropertyOf rdf:resource="http://www.ontologydesignpatterns.org/ont/dul/DUL.owl#hasRegionDataValue"/>
        <rdfs:domain rdf:resource="http://www.ease-crc.org/ont/SOMA-OBJ.owl#ForceAttribute"/>
        <rdfs:range rdf:resource="http://www.ease-crc.org/ont/SOMA.owl#array_double"/>
        <rdfs:comment>A value that quantifies a force given in Newton.</rdfs:comment>
        <rdfs:isDefinedBy rdf:resource="http://www.ease-crc.org/ont/SOMA-OBJ.owl"/>
        <rdfs:label>has force value</rdfs:label>
    </owl:DatatypeProperty>
    


    <!-- http://www.ease-crc.org/ont/SOMA-OBJ.owl#hasJointEffort -->


    <owl:DatatypeProperty rdf:about="http://www.ease-crc.org/ont/SOMA-OBJ.owl#hasJointEffort">
        <rdfs:subPropertyOf rdf:resource="http://www.ease-crc.org/ont/SOMA-OBJ.owl#hasJointParameter"/>
        <rdfs:domain rdf:resource="http://www.ease-crc.org/ont/SOMA-OBJ.owl#JointState"/>
        <rdfs:range rdf:resource="http://www.w3.org/2001/XMLSchema#double"/>
        <rdfs:comment>The effort applied in a joint given in N (prismatic joint) or N*m (hinged joints).</rdfs:comment>
        <rdfs:isDefinedBy rdf:resource="http://www.ease-crc.org/ont/SOMA-OBJ.owl"/>
        <rdfs:label>has joint effort</rdfs:label>
    </owl:DatatypeProperty>
    


    <!-- http://www.ease-crc.org/ont/SOMA-OBJ.owl#hasJointEffortLimit -->


    <owl:DatatypeProperty rdf:about="http://www.ease-crc.org/ont/SOMA-OBJ.owl#hasJointEffortLimit">
        <rdfs:subPropertyOf rdf:resource="http://www.ease-crc.org/ont/SOMA-OBJ.owl#hasJointParameter"/>
        <rdfs:domain rdf:resource="http://www.ease-crc.org/ont/SOMA-OBJ.owl#JointLimit"/>
        <rdfs:range rdf:resource="http://www.w3.org/2001/XMLSchema#double"/>
        <rdfs:comment>The maximum effort applied in a joint given in N (prismatic joint) or N*m (hinged joints).</rdfs:comment>
        <rdfs:isDefinedBy rdf:resource="http://www.ease-crc.org/ont/SOMA-OBJ.owl"/>
        <rdfs:label>has joint effort limit</rdfs:label>
    </owl:DatatypeProperty>
    


    <!-- http://www.ease-crc.org/ont/SOMA-OBJ.owl#hasJointParameter -->


    <owl:DatatypeProperty rdf:about="http://www.ease-crc.org/ont/SOMA-OBJ.owl#hasJointParameter">
        <rdfs:subPropertyOf rdf:resource="http://www.ontologydesignpatterns.org/ont/dul/DUL.owl#hasRegionDataValue"/>
        <rdfs:domain rdf:resource="http://www.ontologydesignpatterns.org/ont/dul/DUL.owl#PhysicalAttribute"/>
        <rdfs:range rdf:resource="http://www.w3.org/2001/XMLSchema#double"/>
        <rdfs:comment>Assigns a value for an attribute of a joint.</rdfs:comment>
        <rdfs:isDefinedBy rdf:resource="http://www.ease-crc.org/ont/SOMA-OBJ.owl"/>
        <rdfs:label>has joint parameter</rdfs:label>
    </owl:DatatypeProperty>
    


    <!-- http://www.ease-crc.org/ont/SOMA-OBJ.owl#hasJointPosition -->


    <owl:DatatypeProperty rdf:about="http://www.ease-crc.org/ont/SOMA-OBJ.owl#hasJointPosition">
        <rdfs:subPropertyOf rdf:resource="http://www.ease-crc.org/ont/SOMA-OBJ.owl#hasJointParameter"/>
        <rdfs:domain rdf:resource="http://www.ease-crc.org/ont/SOMA-OBJ.owl#JointState"/>
        <rdfs:range rdf:resource="http://www.w3.org/2001/XMLSchema#double"/>
        <rdfs:comment>The position of a joint given in m (prismatic joints) or rad (hinged joints).</rdfs:comment>
        <rdfs:isDefinedBy rdf:resource="http://www.ease-crc.org/ont/SOMA-OBJ.owl"/>
        <rdfs:label>has joint position</rdfs:label>
    </owl:DatatypeProperty>
    


    <!-- http://www.ease-crc.org/ont/SOMA-OBJ.owl#hasJointPositionMax -->


    <owl:DatatypeProperty rdf:about="http://www.ease-crc.org/ont/SOMA-OBJ.owl#hasJointPositionMax">
        <rdfs:subPropertyOf rdf:resource="http://www.ease-crc.org/ont/SOMA-OBJ.owl#hasJointParameter"/>
        <rdfs:domain rdf:resource="http://www.ease-crc.org/ont/SOMA-OBJ.owl#JointLimit"/>
        <rdfs:range rdf:resource="http://www.w3.org/2001/XMLSchema#double"/>
        <rdfs:comment>The maximum position of a joint given in m (prismatic joints) or rad (hinged joints).</rdfs:comment>
        <rdfs:isDefinedBy rdf:resource="http://www.ease-crc.org/ont/SOMA-OBJ.owl"/>
        <rdfs:label>has joint position max</rdfs:label>
    </owl:DatatypeProperty>
    


    <!-- http://www.ease-crc.org/ont/SOMA-OBJ.owl#hasJointPositionMin -->


    <owl:DatatypeProperty rdf:about="http://www.ease-crc.org/ont/SOMA-OBJ.owl#hasJointPositionMin">
        <rdfs:subPropertyOf rdf:resource="http://www.ease-crc.org/ont/SOMA-OBJ.owl#hasJointParameter"/>
        <rdfs:domain rdf:resource="http://www.ease-crc.org/ont/SOMA-OBJ.owl#JointLimit"/>
        <rdfs:range rdf:resource="http://www.w3.org/2001/XMLSchema#double"/>
        <rdfs:comment>The minimum position of a joint given in m (prismatic joints) or rad (hinged joints).</rdfs:comment>
        <rdfs:isDefinedBy rdf:resource="http://www.ease-crc.org/ont/SOMA-OBJ.owl"/>
        <rdfs:label>has joint position min</rdfs:label>
    </owl:DatatypeProperty>
    


    <!-- http://www.ease-crc.org/ont/SOMA-OBJ.owl#hasJointVelocity -->


    <owl:DatatypeProperty rdf:about="http://www.ease-crc.org/ont/SOMA-OBJ.owl#hasJointVelocity">
        <rdfs:subPropertyOf rdf:resource="http://www.ease-crc.org/ont/SOMA-OBJ.owl#hasJointParameter"/>
        <rdfs:domain rdf:resource="http://www.ease-crc.org/ont/SOMA-OBJ.owl#JointState"/>
        <rdfs:range rdf:resource="http://www.w3.org/2001/XMLSchema#double"/>
        <rdfs:comment>The velocity of a joint given in m/s (prismatic joints) or rad/s (hinged joints).</rdfs:comment>
        <rdfs:isDefinedBy rdf:resource="http://www.ease-crc.org/ont/SOMA-OBJ.owl"/>
        <rdfs:label>has joint velocity</rdfs:label>
    </owl:DatatypeProperty>
    


    <!-- http://www.ease-crc.org/ont/SOMA-OBJ.owl#hasJointVelocityLimit -->


    <owl:DatatypeProperty rdf:about="http://www.ease-crc.org/ont/SOMA-OBJ.owl#hasJointVelocityLimit">
        <rdfs:subPropertyOf rdf:resource="http://www.ease-crc.org/ont/SOMA-OBJ.owl#hasJointParameter"/>
        <rdfs:domain rdf:resource="http://www.ease-crc.org/ont/SOMA-OBJ.owl#JointLimit"/>
        <rdfs:range rdf:resource="http://www.w3.org/2001/XMLSchema#double"/>
        <rdfs:comment>The maximum velocity of a joint given in m/s (prismatic joints) or rad/s (hinged joints).</rdfs:comment>
        <rdfs:isDefinedBy rdf:resource="http://www.ease-crc.org/ont/SOMA-OBJ.owl"/>
        <rdfs:label>has joint velocity limit</rdfs:label>
    </owl:DatatypeProperty>
    


    <!-- http://www.ease-crc.org/ont/SOMA-OBJ.owl#hasShapeScale -->


    <owl:DatatypeProperty rdf:about="http://www.ease-crc.org/ont/SOMA-OBJ.owl#hasShapeScale">
        <rdfs:subPropertyOf rdf:resource="http://www.ease-crc.org/ont/SOMA.owl#hasShapeParameter"/>
        <rdfs:domain rdf:resource="http://www.ease-crc.org/ont/SOMA.owl#ShapeRegion"/>
        <rdfs:range rdf:resource="http://www.ease-crc.org/ont/SOMA.owl#array_double"/>
        <rdfs:comment>The scale of a shape, given as a vector of three real numbers to adjust x, y, z components of vertex vectors. In cases where a shape needs to be flipped compared to the shape described by a mesh, one of the scale components will be negative. 

It is often the case that shapes need to be altered from their description in a shape file, and a typical example of this is scaling a mesh. 

In robotics, it is not uncommon to encounter shapes that are flipped compared to the shape in a mesh file. This is because robots often have bilateral symmetry, thus it makes sense to reuse the same meshes for corresponding links of the left and right arms.</rdfs:comment>
        <rdfs:isDefinedBy rdf:resource="http://www.ease-crc.org/ont/SOMA-OBJ.owl"/>
        <rdfs:label>has shape scale</rdfs:label>
    </owl:DatatypeProperty>
    


    <!-- http://www.ease-crc.org/ont/SOMA.owl#hasColorValue -->


    <owl:DatatypeProperty rdf:about="http://www.ease-crc.org/ont/SOMA.owl#hasColorValue">
        <rdfs:subPropertyOf rdf:resource="http://www.ontologydesignpatterns.org/ont/dul/DUL.owl#hasRegionDataValue"/>
        <rdfs:domain rdf:resource="http://www.ease-crc.org/ont/SOMA.owl#ColorRegion"/>
        <rdfs:comment>Associates a ColorRegion to numerical data describing the color.</rdfs:comment>
        <rdfs:isDefinedBy rdf:resource="http://www.ease-crc.org/ont/SOMA-OBJ.owl"/>
        <rdfs:label>has color value</rdfs:label>
    </owl:DatatypeProperty>
    


    <!-- http://www.ease-crc.org/ont/SOMA.owl#hasDepth -->


    <owl:DatatypeProperty rdf:about="http://www.ease-crc.org/ont/SOMA.owl#hasDepth">
        <rdfs:subPropertyOf rdf:resource="http://www.ease-crc.org/ont/SOMA.owl#hasShapeParameter"/>
        <rdfs:domain rdf:resource="http://www.ease-crc.org/ont/SOMA.owl#ShapeRegion"/>
        <rdfs:range rdf:resource="http://www.w3.org/2001/XMLSchema#float"/>
        <rdfs:comment>The depth of a shape.</rdfs:comment>
        <rdfs:isDefinedBy rdf:resource="http://www.ease-crc.org/ont/SOMA-OBJ.owl"/>
        <rdfs:label>has depth</rdfs:label>
    </owl:DatatypeProperty>
    


    <!-- http://www.ease-crc.org/ont/SOMA.owl#hasFilePath -->


    <owl:DatatypeProperty rdf:about="http://www.ease-crc.org/ont/SOMA.owl#hasFilePath">
        <rdfs:subPropertyOf rdf:resource="http://www.ontologydesignpatterns.org/ont/dul/DUL.owl#hasDataValue"/>
        <rdfs:domain rdf:resource="http://www.ontologydesignpatterns.org/ont/dul/DUL.owl#Entity"/>
        <rdfs:range rdf:resource="http://www.w3.org/2001/XMLSchema#string"/>
        <rdfs:comment>Associates an entity to some file containing data about it. For example, can be used to describe physical objects via a mesh file.</rdfs:comment>
        <rdfs:isDefinedBy rdf:resource="http://www.ease-crc.org/ont/SOMA-OBJ.owl"/>
        <rdfs:label>has file path</rdfs:label>
    </owl:DatatypeProperty>
    


    <!-- http://www.ease-crc.org/ont/SOMA.owl#hasFrictionValue -->


    <owl:DatatypeProperty rdf:about="http://www.ease-crc.org/ont/SOMA.owl#hasFrictionValue">
        <rdfs:subPropertyOf rdf:resource="http://www.ontologydesignpatterns.org/ont/dul/DUL.owl#hasRegionDataValue"/>
        <rdfs:domain rdf:resource="http://www.ease-crc.org/ont/SOMA.owl#FrictionAttribute"/>
        <rdfs:range rdf:resource="http://www.w3.org/2001/XMLSchema#double"/>
        <rdfs:comment>The coefficient of friction denotes the ratio of friction force between touching objects. The coefficient is dimensionless.</rdfs:comment>
        <rdfs:isDefinedBy rdf:resource="http://www.ease-crc.org/ont/SOMA-OBJ.owl"/>
        <rdfs:label>has friction value</rdfs:label>
    </owl:DatatypeProperty>
    


    <!-- http://www.ease-crc.org/ont/SOMA.owl#hasHSVValue -->


    <owl:DatatypeProperty rdf:about="http://www.ease-crc.org/ont/SOMA.owl#hasHSVValue">
        <rdfs:subPropertyOf rdf:resource="http://www.ease-crc.org/ont/SOMA.owl#hasColorValue"/>
        <rdfs:domain rdf:resource="http://www.ease-crc.org/ont/SOMA.owl#ColorRegion"/>
        <rdfs:range rdf:resource="http://www.w3.org/2001/XMLSchema#string"/>
        <rdfs:comment>Associates a ColorRegion to numerical data describing the color. This data uses the Hue-Saturation-Value color space.</rdfs:comment>
        <rdfs:isDefinedBy rdf:resource="http://www.ease-crc.org/ont/SOMA-OBJ.owl"/>
        <rdfs:label>has hsv value</rdfs:label>
    </owl:DatatypeProperty>
    


    <!-- http://www.ease-crc.org/ont/SOMA.owl#hasHeight -->


    <owl:DatatypeProperty rdf:about="http://www.ease-crc.org/ont/SOMA.owl#hasHeight">
        <rdfs:subPropertyOf rdf:resource="http://www.ease-crc.org/ont/SOMA.owl#hasShapeParameter"/>
        <rdfs:domain rdf:resource="http://www.ease-crc.org/ont/SOMA.owl#ShapeRegion"/>
        <rdfs:range rdf:resource="http://www.w3.org/2001/XMLSchema#float"/>
        <rdfs:comment>The height of a shape.</rdfs:comment>
        <rdfs:isDefinedBy rdf:resource="http://www.ease-crc.org/ont/SOMA-OBJ.owl"/>
        <rdfs:label>has height</rdfs:label>
    </owl:DatatypeProperty>
    


    <!-- http://www.ease-crc.org/ont/SOMA.owl#hasLength -->


    <owl:DatatypeProperty rdf:about="http://www.ease-crc.org/ont/SOMA.owl#hasLength">
        <rdfs:subPropertyOf rdf:resource="http://www.ease-crc.org/ont/SOMA.owl#hasShapeParameter"/>
        <rdfs:domain rdf:resource="http://www.ease-crc.org/ont/SOMA.owl#ShapeRegion"/>
        <rdfs:range rdf:resource="http://www.w3.org/2001/XMLSchema#float"/>
        <rdfs:comment>The length of a shape.</rdfs:comment>
        <rdfs:isDefinedBy rdf:resource="http://www.ease-crc.org/ont/SOMA-OBJ.owl"/>
        <rdfs:label>has length</rdfs:label>
    </owl:DatatypeProperty>
    


    <!-- http://www.ease-crc.org/ont/SOMA.owl#hasMassValue -->


    <owl:DatatypeProperty rdf:about="http://www.ease-crc.org/ont/SOMA.owl#hasMassValue">
        <rdfs:subPropertyOf rdf:resource="http://www.ontologydesignpatterns.org/ont/dul/DUL.owl#hasRegionDataValue"/>
        <rdfs:domain rdf:resource="http://www.ease-crc.org/ont/SOMA.owl#MassAttribute"/>
        <rdfs:range rdf:resource="http://www.w3.org/2001/XMLSchema#double"/>
        <rdfs:comment>The mass value of a physical object in kilogram.</rdfs:comment>
        <rdfs:isDefinedBy rdf:resource="http://www.ease-crc.org/ont/SOMA-OBJ.owl"/>
        <rdfs:label>has mass value</rdfs:label>
    </owl:DatatypeProperty>
    


    <!-- http://www.ease-crc.org/ont/SOMA.owl#hasPositionData -->


    <owl:DatatypeProperty rdf:about="http://www.ease-crc.org/ont/SOMA.owl#hasPositionData">
        <rdfs:subPropertyOf rdf:resource="http://www.ease-crc.org/ont/SOMA.owl#hasSpaceParameter"/>
        <rdfs:domain rdf:resource="http://www.ontologydesignpatterns.org/ont/dul/DUL.owl#SpaceRegion"/>
        <rdfs:range rdf:resource="http://www.w3.org/2001/XMLSchema#string"/>
        <rdfs:comment>Associates a spatial region to a position.</rdfs:comment>
        <rdfs:isDefinedBy rdf:resource="http://www.ease-crc.org/ont/SOMA-OBJ.owl"/>
        <rdfs:label>has position data</rdfs:label>
    </owl:DatatypeProperty>
    


    <!-- http://www.ease-crc.org/ont/SOMA.owl#hasPriority -->


    <owl:DatatypeProperty rdf:about="http://www.ease-crc.org/ont/SOMA.owl#hasPriority">
        <rdfs:subPropertyOf rdf:resource="http://www.ontologydesignpatterns.org/ont/dul/DUL.owl#hasDataValue"/>
        <rdfs:domain rdf:resource="http://www.ontologydesignpatterns.org/ont/dul/DUL.owl#Task"/>
        <rdfs:comment>A relation asserting some entity has a particular priority.</rdfs:comment>
        <rdfs:isDefinedBy rdf:resource="http://www.ease-crc.org/ont/SOMA-WF.owl"/>
    </owl:DatatypeProperty>
    


    <!-- http://www.ease-crc.org/ont/SOMA.owl#hasRGBValue -->


    <owl:DatatypeProperty rdf:about="http://www.ease-crc.org/ont/SOMA.owl#hasRGBValue">
        <rdfs:subPropertyOf rdf:resource="http://www.ease-crc.org/ont/SOMA.owl#hasColorValue"/>
        <rdfs:domain rdf:resource="http://www.ease-crc.org/ont/SOMA.owl#ColorRegion"/>
        <rdfs:range rdf:resource="http://www.w3.org/2001/XMLSchema#string"/>
        <rdfs:comment>Associates a ColorRegion to numerical data describing the color. This data uses the Red-Green-Blue color space.</rdfs:comment>
        <rdfs:isDefinedBy rdf:resource="http://www.ease-crc.org/ont/SOMA-OBJ.owl"/>
        <rdfs:label>has rgb value</rdfs:label>
    </owl:DatatypeProperty>
    


    <!-- http://www.ease-crc.org/ont/SOMA.owl#hasRadius -->


    <owl:DatatypeProperty rdf:about="http://www.ease-crc.org/ont/SOMA.owl#hasRadius">
        <rdfs:subPropertyOf rdf:resource="http://www.ease-crc.org/ont/SOMA.owl#hasShapeParameter"/>
        <rdfs:domain rdf:resource="http://www.ease-crc.org/ont/SOMA.owl#ShapeRegion"/>
        <rdfs:range rdf:resource="http://www.w3.org/2001/XMLSchema#float"/>
        <rdfs:comment>The radius of a circular or oval shape.</rdfs:comment>
        <rdfs:isDefinedBy rdf:resource="http://www.ease-crc.org/ont/SOMA-OBJ.owl"/>
        <rdfs:label>has radius</rdfs:label>
    </owl:DatatypeProperty>
    


    <!-- http://www.ease-crc.org/ont/SOMA.owl#hasReferenceFrame -->


    <owl:DatatypeProperty rdf:about="http://www.ease-crc.org/ont/SOMA.owl#hasReferenceFrame">
        <rdfs:subPropertyOf rdf:resource="http://www.ease-crc.org/ont/SOMA.owl#hasSpaceParameter"/>
        <rdfs:domain rdf:resource="http://www.ontologydesignpatterns.org/ont/dul/DUL.owl#SpaceRegion"/>
        <rdfs:range rdf:resource="http://www.w3.org/2001/XMLSchema#string"/>
        <rdfs:comment>Gives the name associated to the local coordinate frame of a SpaceRegion.</rdfs:comment>
        <rdfs:isDefinedBy rdf:resource="http://www.ease-crc.org/ont/SOMA-OBJ.owl"/>
        <rdfs:label>has reference frame</rdfs:label>
    </owl:DatatypeProperty>
    


    <!-- http://www.ease-crc.org/ont/SOMA.owl#hasShapeParameter -->


    <owl:DatatypeProperty rdf:about="http://www.ease-crc.org/ont/SOMA.owl#hasShapeParameter">
        <rdfs:subPropertyOf rdf:resource="http://www.ontologydesignpatterns.org/ont/dul/DUL.owl#hasRegionDataValue"/>
        <rdfs:domain rdf:resource="http://www.ease-crc.org/ont/SOMA.owl#ShapeRegion"/>
        <rdfs:range>
            <rdfs:Datatype>
                <owl:unionOf rdf:parseType="Collection">
                    <rdf:Description rdf:about="http://www.ease-crc.org/ont/SOMA.owl#array_double"/>
                    <rdf:Description rdf:about="http://www.w3.org/2001/XMLSchema#double"/>
                    <rdf:Description rdf:about="http://www.w3.org/2001/XMLSchema#float"/>
                    <rdf:Description rdf:about="http://www.w3.org/2001/XMLSchema#string"/>
                </owl:unionOf>
            </rdfs:Datatype>
        </rdfs:range>
        <rdfs:comment>Associates a SpaceRegion to some parameter value describing its shape. This is a fairly generic property, and to capture the semantics of the information associated to the SpaceRegion, its more specific subproperties should be used.</rdfs:comment>
        <rdfs:isDefinedBy rdf:resource="http://www.ease-crc.org/ont/SOMA-OBJ.owl"/>
        <rdfs:label>has shape parameter</rdfs:label>
    </owl:DatatypeProperty>
    


    <!-- http://www.ease-crc.org/ont/SOMA.owl#hasSpaceParameter -->


    <owl:DatatypeProperty rdf:about="http://www.ease-crc.org/ont/SOMA.owl#hasSpaceParameter">
        <rdfs:subPropertyOf rdf:resource="http://www.ontologydesignpatterns.org/ont/dul/DUL.owl#hasRegionDataValue"/>
        <rdfs:domain rdf:resource="http://www.ontologydesignpatterns.org/ont/dul/DUL.owl#SpaceRegion"/>
        <rdfs:comment>Associates a SpaceRegion to some parameter value describing it. This is a fairly generic property, and to capture the semantics of the information associated to the SpaceRegion, its more specific subproperties should be used.</rdfs:comment>
        <rdfs:isDefinedBy rdf:resource="http://www.ease-crc.org/ont/SOMA-OBJ.owl"/>
        <rdfs:label>has space parameter</rdfs:label>
    </owl:DatatypeProperty>
    


    <!-- http://www.ease-crc.org/ont/SOMA.owl#hasWidth -->


    <owl:DatatypeProperty rdf:about="http://www.ease-crc.org/ont/SOMA.owl#hasWidth">
        <rdfs:subPropertyOf rdf:resource="http://www.ease-crc.org/ont/SOMA.owl#hasShapeParameter"/>
        <rdfs:domain rdf:resource="http://www.ease-crc.org/ont/SOMA.owl#ShapeRegion"/>
        <rdfs:range rdf:resource="http://www.w3.org/2001/XMLSchema#float"/>
        <rdfs:comment>The width of a shape.</rdfs:comment>
        <rdfs:isDefinedBy rdf:resource="http://www.ease-crc.org/ont/SOMA-OBJ.owl"/>
        <rdfs:label>has width</rdfs:label>
    </owl:DatatypeProperty>
    


    <!-- 
    ///////////////////////////////////////////////////////////////////////////////////////
    //
    // Classes
    //
    ///////////////////////////////////////////////////////////////////////////////////////
     -->


    


    <!-- http://www.ease-crc.org/ont/SOMA-ACT.owl#AnsweringTask -->


    <owl:Class rdf:about="http://www.ease-crc.org/ont/SOMA-ACT.owl#AnsweringTask">
        <owl:equivalentClass>
            <owl:Class>
                <owl:intersectionOf rdf:parseType="Collection">
                    <rdf:Description rdf:about="http://www.ease-crc.org/ont/SOMA.owl#IllocutionaryTask"/>
                    <owl:Restriction>
                        <owl:onProperty rdf:resource="http://www.ontologydesignpatterns.org/ont/dul/DUL.owl#classifies"/>
                        <owl:allValuesFrom>
                            <owl:Restriction>
                                <owl:onProperty rdf:resource="http://www.ease-crc.org/ont/SOMA-ACT.owl#isReactionTo"/>
                                <owl:allValuesFrom>
                                    <owl:Restriction>
                                        <owl:onProperty rdf:resource="http://www.ontologydesignpatterns.org/ont/dul/DUL.owl#isClassifiedBy"/>
                                        <owl:someValuesFrom rdf:resource="http://www.ease-crc.org/ont/SOMA.owl#CommandingTask"/>
                                    </owl:Restriction>
                                </owl:allValuesFrom>
                            </owl:Restriction>
                        </owl:allValuesFrom>
                    </owl:Restriction>
                </owl:intersectionOf>
            </owl:Class>
        </owl:equivalentClass>
        <owl:equivalentClass>
            <owl:Restriction>
                <owl:onProperty rdf:resource="http://www.ontologydesignpatterns.org/ont/dul/DUL.owl#isTaskOf"/>
                <owl:someValuesFrom rdf:resource="http://www.ease-crc.org/ont/SOMA.owl#Answer"/>
            </owl:Restriction>
        </owl:equivalentClass>
        <rdfs:comment xml:lang="en">An Illocutionary act where the Sender emits some Message to the Receiver as a reaction to some previous Communication task where the Roles where switched, i.e., the Sender (Receiver) of the Answering task has been the Sender (Sender) for the cause.</rdfs:comment>
        <rdfs:isDefinedBy rdf:resource="http://www.ease-crc.org/ont/SOMA-ACT.owl"/>
        <rdfs:label xml:lang="en">Answering task</rdfs:label>
    </owl:Class>
    


    <!-- http://www.ease-crc.org/ont/SOMA-ACT.owl#QueryAnsweringTask -->


    <owl:Class rdf:about="http://www.ease-crc.org/ont/SOMA-ACT.owl#QueryAnsweringTask">
        <owl:equivalentClass>
            <owl:Class>
                <owl:intersectionOf rdf:parseType="Collection">
                    <rdf:Description rdf:about="http://www.ease-crc.org/ont/SOMA-ACT.owl#AnsweringTask"/>
                    <owl:Restriction>
                        <owl:onProperty rdf:resource="http://www.ontologydesignpatterns.org/ont/dul/DUL.owl#classifies"/>
                        <owl:allValuesFrom>
                            <owl:Restriction>
                                <owl:onProperty rdf:resource="http://www.ease-crc.org/ont/SOMA-ACT.owl#isReactionTo"/>
                                <owl:allValuesFrom>
                                    <owl:Restriction>
                                        <owl:onProperty rdf:resource="http://www.ontologydesignpatterns.org/ont/dul/DUL.owl#isClassifiedBy"/>
                                        <owl:someValuesFrom rdf:resource="http://www.ease-crc.org/ont/SOMA.owl#QueryingTask"/>
                                    </owl:Restriction>
                                </owl:allValuesFrom>
                            </owl:Restriction>
                        </owl:allValuesFrom>
                    </owl:Restriction>
                </owl:intersectionOf>
            </owl:Class>
        </owl:equivalentClass>
        <rdfs:comment xml:lang="en">An Answering task that is the reaction to some Query answering task.

In a lot of cases, such a task is also an Assertion task, e.g., in the following discourse:

&quot;How will the weather be tomorrow?&quot;
&quot;It is going to rain in the morning.&quot;

However, sometimes this might be not the case, e.g., with counterquestions.</rdfs:comment>
        <rdfs:isDefinedBy rdf:resource="http://www.ease-crc.org/ont/SOMA-ACT.owl"/>
        <rdfs:label>Query answering task</rdfs:label>
    </owl:Class>
    


    <!-- http://www.ease-crc.org/ont/SOMA-HOME.owl#Box -->


    <owl:Class rdf:about="http://www.ease-crc.org/ont/SOMA-HOME.owl#Box">
        <rdfs:subClassOf rdf:resource="http://www.ease-crc.org/ont/SOMA.owl#DesignedContainer"/>
        <rdfs:subClassOf>
            <owl:Restriction>
                <owl:onProperty rdf:resource="http://www.ease-crc.org/ont/SOMA.owl#hasShapeRegion"/>
                <owl:someValuesFrom rdf:resource="http://www.ease-crc.org/ont/SOMA.owl#BoxShape"/>
            </owl:Restriction>
        </rdfs:subClassOf>
        <rdfs:comment>A cuboid-shaped container.</rdfs:comment>
        <rdfs:isDefinedBy rdf:resource="http://www.ease-crc.org/ont/SOMA-HOME.owl"/>
    </owl:Class>
    


    <!-- http://www.ease-crc.org/ont/SOMA-HOME.owl#BreadKnife -->


    <owl:Class rdf:about="http://www.ease-crc.org/ont/SOMA-HOME.owl#BreadKnife">
        <rdfs:subClassOf rdf:resource="http://www.ease-crc.org/ont/SOMA-HOME.owl#KitchenKnife"/>
        <rdfs:comment>A knife to cut bread.</rdfs:comment>
        <rdfs:isDefinedBy rdf:resource="http://www.ease-crc.org/ont/SOMA-HOME.owl"/>
    </owl:Class>
    


    <!-- http://www.ease-crc.org/ont/SOMA-HOME.owl#BreakfastPlate -->


    <owl:Class rdf:about="http://www.ease-crc.org/ont/SOMA-HOME.owl#BreakfastPlate">
        <rdfs:subClassOf rdf:resource="http://www.ease-crc.org/ont/SOMA.owl#Plate"/>
        <rdfs:comment>A smaller plate used for serving bread at the dining table with the main meal or to serve breakfast.</rdfs:comment>
        <rdfs:isDefinedBy rdf:resource="http://www.ease-crc.org/ont/SOMA-HOME.owl"/>
    </owl:Class>
    


    <!-- http://www.ease-crc.org/ont/SOMA-HOME.owl#Carafe -->


    <owl:Class rdf:about="http://www.ease-crc.org/ont/SOMA-HOME.owl#Carafe">
        <rdfs:subClassOf rdf:resource="http://www.ease-crc.org/ont/SOMA.owl#DesignedContainer"/>
        <rdfs:comment>A container used to hold and pour some beverage.</rdfs:comment>
        <rdfs:isDefinedBy rdf:resource="http://www.ease-crc.org/ont/SOMA-HOME.owl"/>
    </owl:Class>
    


    <!-- http://www.ease-crc.org/ont/SOMA-HOME.owl#CerealBox -->


    <owl:Class rdf:about="http://www.ease-crc.org/ont/SOMA-HOME.owl#CerealBox">
        <rdfs:subClassOf rdf:resource="http://www.ease-crc.org/ont/SOMA-HOME.owl#Box"/>
        <rdfs:comment>A box which holds, or at least is intended to usually hold, cereal flakes.</rdfs:comment>
        <rdfs:isDefinedBy rdf:resource="http://www.ease-crc.org/ont/SOMA-HOME.owl"/>
    </owl:Class>
    


    <!-- http://www.ease-crc.org/ont/SOMA-HOME.owl#ClosingDisposition -->


    <owl:Class rdf:about="http://www.ease-crc.org/ont/SOMA-HOME.owl#ClosingDisposition">
        <rdfs:subClassOf rdf:resource="http://www.ease-crc.org/ont/SOMA.owl#Linkage"/>
        <rdfs:comment>The disposition of an object to connect with some other, so that a region of space becomes fully enclosed by the object and separate from the exterior. 

Often this connection is between parts of the same object.

Because of the existence of a separation between some interior and exterior space regions, objects that can close are also objects that can contain.</rdfs:comment>
        <rdfs:isDefinedBy rdf:resource="http://www.ease-crc.org/ont/SOMA-HOME.owl"/>
    </owl:Class>
    


    <!-- http://www.ease-crc.org/ont/SOMA-HOME.owl#CoffeeCarafe -->


    <owl:Class rdf:about="http://www.ease-crc.org/ont/SOMA-HOME.owl#CoffeeCarafe">
        <rdfs:subClassOf rdf:resource="http://www.ease-crc.org/ont/SOMA-HOME.owl#Carafe"/>
        <rdfs:comment>A carafe which holds, or at least is intended to usually hold, coffee.</rdfs:comment>
        <rdfs:isDefinedBy rdf:resource="http://www.ease-crc.org/ont/SOMA-HOME.owl"/>
    </owl:Class>
    


    <!-- http://www.ease-crc.org/ont/SOMA-HOME.owl#Cup -->


    <owl:Class rdf:about="http://www.ease-crc.org/ont/SOMA-HOME.owl#Cup">
        <rdfs:subClassOf rdf:resource="http://www.ease-crc.org/ont/SOMA.owl#Crockery"/>
        <rdfs:subClassOf>
            <owl:Restriction>
                <owl:onProperty rdf:resource="http://www.ease-crc.org/ont/SOMA.owl#hasPhysicalComponent"/>
                <owl:someValuesFrom rdf:resource="http://www.ease-crc.org/ont/SOMA.owl#DesignedHandle"/>
            </owl:Restriction>
        </rdfs:subClassOf>
        <rdfs:comment>A round shaped container used for storing liquid and drinking out of it, typically has  a handle for grasping.</rdfs:comment>
        <rdfs:isDefinedBy rdf:resource="http://www.ease-crc.org/ont/SOMA-HOME.owl"/>
    </owl:Class>
    


    <!-- http://www.ease-crc.org/ont/SOMA-HOME.owl#DessertFork -->


    <owl:Class rdf:about="http://www.ease-crc.org/ont/SOMA-HOME.owl#DessertFork">
        <rdfs:subClassOf rdf:resource="http://www.ease-crc.org/ont/SOMA.owl#Fork"/>
        <rdfs:comment>A smallar fork for eating desserts e.g. cake.</rdfs:comment>
        <rdfs:isDefinedBy rdf:resource="http://www.ease-crc.org/ont/SOMA-HOME.owl"/>
    </owl:Class>
    


    <!-- http://www.ease-crc.org/ont/SOMA-HOME.owl#DinnerPlate -->


    <owl:Class rdf:about="http://www.ease-crc.org/ont/SOMA-HOME.owl#DinnerPlate">
        <rdfs:subClassOf rdf:resource="http://www.ease-crc.org/ont/SOMA.owl#Plate"/>
        <rdfs:comment>A regular size plate for eating a main meals.</rdfs:comment>
        <rdfs:isDefinedBy rdf:resource="http://www.ease-crc.org/ont/SOMA-HOME.owl"/>
    </owl:Class>
    


    <!-- http://www.ease-crc.org/ont/SOMA-HOME.owl#Dispenser -->


    <owl:Class rdf:about="http://www.ease-crc.org/ont/SOMA-HOME.owl#Dispenser">
        <rdfs:subClassOf rdf:resource="http://www.ease-crc.org/ont/SOMA.owl#DesignedContainer"/>
        <rdfs:comment>A small container used to store and serve some flavoring substance for a dish or beverage.</rdfs:comment>
        <rdfs:isDefinedBy rdf:resource="http://www.ease-crc.org/ont/SOMA-HOME.owl"/>
    </owl:Class>
    


    <!-- http://www.ease-crc.org/ont/SOMA-HOME.owl#Glass -->


    <owl:Class rdf:about="http://www.ease-crc.org/ont/SOMA-HOME.owl#Glass">
        <rdfs:subClassOf rdf:resource="http://www.ease-crc.org/ont/SOMA.owl#Crockery"/>
        <rdfs:comment>A container made usually from glass or transparent plastic which is used to hold, typically cold, beverages.</rdfs:comment>
        <rdfs:isDefinedBy rdf:resource="http://www.ease-crc.org/ont/SOMA-HOME.owl"/>
    </owl:Class>
    


    <!-- http://www.ease-crc.org/ont/SOMA-HOME.owl#JamJar -->


    <owl:Class rdf:about="http://www.ease-crc.org/ont/SOMA-HOME.owl#JamJar">
        <rdfs:subClassOf rdf:resource="http://www.ease-crc.org/ont/SOMA-HOME.owl#Jar"/>
        <rdfs:comment>A jar which holds, or at least is intended to usually hold, jam.</rdfs:comment>
        <rdfs:isDefinedBy rdf:resource="http://www.ease-crc.org/ont/SOMA-HOME.owl"/>
    </owl:Class>
    


    <!-- http://www.ease-crc.org/ont/SOMA-HOME.owl#Jar -->


    <owl:Class rdf:about="http://www.ease-crc.org/ont/SOMA-HOME.owl#Jar">
        <rdfs:subClassOf rdf:resource="http://www.ease-crc.org/ont/SOMA.owl#DesignedContainer"/>
        <rdfs:comment>A container used for long-term storage of some liquid or viscous dish.</rdfs:comment>
        <rdfs:isDefinedBy rdf:resource="http://www.ease-crc.org/ont/SOMA-HOME.owl"/>
    </owl:Class>
    


    <!-- http://www.ease-crc.org/ont/SOMA-HOME.owl#Kitchen -->


    <owl:Class rdf:about="http://www.ease-crc.org/ont/SOMA-HOME.owl#Kitchen">
        <rdfs:subClassOf rdf:resource="http://www.ease-crc.org/ont/SOMA.owl#Room"/>
        <rdfs:subClassOf>
            <owl:Restriction>
                <owl:onProperty rdf:resource="http://www.ease-crc.org/ont/SOMA.owl#hasDisposition"/>
                <owl:someValuesFrom rdf:resource="http://www.ease-crc.org/ont/SOMA.owl#Containment"/>
            </owl:Restriction>
        </rdfs:subClassOf>
        <rdfs:comment>A designated room to perform the task of cooking.</rdfs:comment>
        <rdfs:isDefinedBy rdf:resource="http://www.ease-crc.org/ont/SOMA-HOME.owl"/>
    </owl:Class>
    


    <!-- http://www.ease-crc.org/ont/SOMA-HOME.owl#KitchenKnife -->


    <owl:Class rdf:about="http://www.ease-crc.org/ont/SOMA-HOME.owl#KitchenKnife">
        <rdfs:subClassOf rdf:resource="http://www.ease-crc.org/ont/SOMA.owl#Knife"/>
        <rdfs:comment>A tool designed to be used for kitchen related common tasks. Such as smearing a bread or cutting a cucumber.</rdfs:comment>
        <rdfs:isDefinedBy rdf:resource="http://www.ease-crc.org/ont/SOMA-HOME.owl"/>
    </owl:Class>
    


    <!-- http://www.ease-crc.org/ont/SOMA-HOME.owl#MilkBottle -->


    <owl:Class rdf:about="http://www.ease-crc.org/ont/SOMA-HOME.owl#MilkBottle">
        <rdfs:subClassOf rdf:resource="http://www.ease-crc.org/ont/SOMA.owl#Bottle"/>
        <rdfs:comment>A bottle which holds, or at least is intended to usually hold, milk.</rdfs:comment>
        <rdfs:isDefinedBy rdf:resource="http://www.ease-crc.org/ont/SOMA-HOME.owl"/>
    </owl:Class>
    


    <!-- http://www.ease-crc.org/ont/SOMA-HOME.owl#MilkPack -->


    <owl:Class rdf:about="http://www.ease-crc.org/ont/SOMA-HOME.owl#MilkPack">
        <rdfs:subClassOf rdf:resource="http://www.ease-crc.org/ont/SOMA.owl#Pack"/>
        <rdfs:comment>A pack which holds, or at least is intended to usually hold, milk.</rdfs:comment>
        <rdfs:isDefinedBy rdf:resource="http://www.ease-crc.org/ont/SOMA-HOME.owl"/>
    </owl:Class>
    


    <!-- http://www.ease-crc.org/ont/SOMA-HOME.owl#NutellaJar -->


    <owl:Class rdf:about="http://www.ease-crc.org/ont/SOMA-HOME.owl#NutellaJar">
        <rdfs:subClassOf rdf:resource="http://www.ease-crc.org/ont/SOMA-HOME.owl#Jar"/>
        <rdfs:comment>A jar which holds, or at least is intended to usually hold, Nutella.</rdfs:comment>
        <rdfs:isDefinedBy rdf:resource="http://www.ease-crc.org/ont/SOMA-HOME.owl"/>
    </owl:Class>
    


    <!-- http://www.ease-crc.org/ont/SOMA-HOME.owl#Oven -->


    <owl:Class rdf:about="http://www.ease-crc.org/ont/SOMA-HOME.owl#Oven">
        <rdfs:subClassOf rdf:resource="http://www.ease-crc.org/ont/SOMA.owl#Appliance"/>
        <rdfs:subClassOf rdf:resource="http://www.ease-crc.org/ont/SOMA.owl#DesignedContainer"/>
        <rdfs:subClassOf>
            <owl:Restriction>
                <owl:onProperty rdf:resource="http://www.ease-crc.org/ont/SOMA.owl#hasDisposition"/>
                <owl:someValuesFrom rdf:resource="http://www.ease-crc.org/ont/SOMA-HOME.owl#TemperingByHeating"/>
            </owl:Restriction>
        </rdfs:subClassOf>
        <rdfs:comment>An appliance with an enclosed compartment that exposes food to heat</rdfs:comment>
        <rdfs:isDefinedBy rdf:resource="http://www.ease-crc.org/ont/SOMA-HOME.owl"/>
    </owl:Class>
    


    <!-- http://www.ease-crc.org/ont/SOMA-HOME.owl#PastaBowl -->


    <owl:Class rdf:about="http://www.ease-crc.org/ont/SOMA-HOME.owl#PastaBowl">
        <rdfs:subClassOf rdf:resource="http://www.ease-crc.org/ont/SOMA.owl#Bowl"/>
        <rdfs:comment>A bowl which holds, or at least is intended to usually hold, pasta.</rdfs:comment>
        <rdfs:isDefinedBy rdf:resource="http://www.ease-crc.org/ont/SOMA-HOME.owl"/>
    </owl:Class>
    


    <!-- http://www.ease-crc.org/ont/SOMA-HOME.owl#PepperShaker -->


    <owl:Class rdf:about="http://www.ease-crc.org/ont/SOMA-HOME.owl#PepperShaker">
        <rdfs:subClassOf rdf:resource="http://www.ease-crc.org/ont/SOMA-HOME.owl#Shaker"/>
        <rdfs:comment>A shaker which holds, or at least is intended to usually hold, pepper.</rdfs:comment>
        <rdfs:isDefinedBy rdf:resource="http://www.ease-crc.org/ont/SOMA-HOME.owl"/>
    </owl:Class>
    


    <!-- http://www.ease-crc.org/ont/SOMA-HOME.owl#RaspberryJamJar -->


    <owl:Class rdf:about="http://www.ease-crc.org/ont/SOMA-HOME.owl#RaspberryJamJar">
        <rdfs:subClassOf rdf:resource="http://www.ease-crc.org/ont/SOMA-HOME.owl#JamJar"/>
        <rdfs:comment>A jar which holds, or at least is intended to usually hold, raspberry jam.</rdfs:comment>
        <rdfs:isDefinedBy rdf:resource="http://www.ease-crc.org/ont/SOMA-HOME.owl"/>
    </owl:Class>
    


    <!-- http://www.ease-crc.org/ont/SOMA-HOME.owl#SaladBowl -->


    <owl:Class rdf:about="http://www.ease-crc.org/ont/SOMA-HOME.owl#SaladBowl">
        <rdfs:subClassOf rdf:resource="http://www.ease-crc.org/ont/SOMA.owl#Bowl"/>
        <rdfs:comment>A bowl which holds, or at least is intended to usually hold, salad.</rdfs:comment>
        <rdfs:isDefinedBy rdf:resource="http://www.ease-crc.org/ont/SOMA-HOME.owl"/>
    </owl:Class>
    


    <!-- http://www.ease-crc.org/ont/SOMA-HOME.owl#SaltShaker -->


    <owl:Class rdf:about="http://www.ease-crc.org/ont/SOMA-HOME.owl#SaltShaker">
        <rdfs:subClassOf rdf:resource="http://www.ease-crc.org/ont/SOMA-HOME.owl#Shaker"/>
        <rdfs:comment>A shaker which holds, or at least is intended to usually hold, salt.</rdfs:comment>
        <rdfs:isDefinedBy rdf:resource="http://www.ease-crc.org/ont/SOMA-HOME.owl"/>
    </owl:Class>
    


    <!-- http://www.ease-crc.org/ont/SOMA-HOME.owl#Shaker -->


    <owl:Class rdf:about="http://www.ease-crc.org/ont/SOMA-HOME.owl#Shaker">
        <rdfs:subClassOf rdf:resource="http://www.ease-crc.org/ont/SOMA.owl#DesignedContainer"/>
        <rdfs:comment>A container used for storing fine grained substances such as salt or paper.</rdfs:comment>
        <rdfs:isDefinedBy rdf:resource="http://www.ease-crc.org/ont/SOMA-HOME.owl"/>
    </owl:Class>
    


    <!-- http://www.ease-crc.org/ont/SOMA-HOME.owl#SoupPot -->


    <owl:Class rdf:about="http://www.ease-crc.org/ont/SOMA-HOME.owl#SoupPot">
        <rdfs:subClassOf rdf:resource="http://www.ease-crc.org/ont/SOMA.owl#Pot"/>
        <rdfs:comment>A pot which holds, or at least is intended to usually hold, soup.</rdfs:comment>
        <rdfs:isDefinedBy rdf:resource="http://www.ease-crc.org/ont/SOMA-HOME.owl"/>
    </owl:Class>
    


    <!-- http://www.ease-crc.org/ont/SOMA-HOME.owl#Spoon -->


    <owl:Class rdf:about="http://www.ease-crc.org/ont/SOMA-HOME.owl#Spoon">
        <rdfs:subClassOf rdf:resource="http://www.ease-crc.org/ont/SOMA.owl#Cutlery"/>
        <rdfs:subClassOf>
            <owl:Restriction>
                <owl:onProperty rdf:resource="http://www.ease-crc.org/ont/SOMA.owl#hasDisposition"/>
                <owl:someValuesFrom rdf:resource="http://www.ease-crc.org/ont/SOMA.owl#Containment"/>
            </owl:Restriction>
        </rdfs:subClassOf>
        <rdfs:subClassOf>
            <owl:Restriction>
                <owl:onProperty rdf:resource="http://www.ease-crc.org/ont/SOMA.owl#hasPhysicalComponent"/>
                <owl:someValuesFrom rdf:resource="http://www.ease-crc.org/ont/SOMA.owl#Bowl"/>
            </owl:Restriction>
        </rdfs:subClassOf>
        <rdfs:subClassOf>
            <owl:Restriction>
                <owl:onProperty rdf:resource="http://www.ease-crc.org/ont/SOMA.owl#hasPhysicalComponent"/>
                <owl:someValuesFrom rdf:resource="http://www.ease-crc.org/ont/SOMA.owl#DesignedHandle"/>
            </owl:Restriction>
        </rdfs:subClassOf>
        <rdfs:subClassOf>
            <owl:Restriction>
                <owl:onProperty rdf:resource="http://www.ease-crc.org/ont/SOMA.owl#hasDisposition"/>
                <owl:qualifiedCardinality rdf:datatype="http://www.w3.org/2001/XMLSchema#nonNegativeInteger">1</owl:qualifiedCardinality>
                <owl:onClass rdf:resource="http://www.ease-crc.org/ont/SOMA.owl#Insertion"/>
            </owl:Restriction>
        </rdfs:subClassOf>
        <rdfs:subClassOf>
            <owl:Restriction>
                <owl:onProperty rdf:resource="http://www.ease-crc.org/ont/SOMA.owl#hasDisposition"/>
                <owl:qualifiedCardinality rdf:datatype="http://www.w3.org/2001/XMLSchema#nonNegativeInteger">1</owl:qualifiedCardinality>
                <owl:onClass>
                    <owl:Class>
                        <owl:intersectionOf rdf:parseType="Collection">
                            <rdf:Description rdf:about="http://www.ease-crc.org/ont/SOMA.owl#Insertion"/>
                            <owl:Restriction>
                                <owl:onProperty rdf:resource="http://www.ease-crc.org/ont/SOMA.owl#affordsTrigger"/>
                                <owl:allValuesFrom>
                                    <owl:Restriction>
                                        <owl:onProperty rdf:resource="http://www.ontologydesignpatterns.org/ont/dul/DUL.owl#classifies"/>
                                        <owl:allValuesFrom rdf:resource="http://www.ontologydesignpatterns.org/ont/dul/DUL.owl#Substance"/>
                                    </owl:Restriction>
                                </owl:allValuesFrom>
                            </owl:Restriction>
                        </owl:intersectionOf>
                    </owl:Class>
                </owl:onClass>
            </owl:Restriction>
        </rdfs:subClassOf>
        <rdfs:comment>An eating or cooking implement consisting of a small shallow bowl with a relatively long handle.</rdfs:comment>
        <rdfs:isDefinedBy rdf:resource="http://www.ease-crc.org/ont/SOMA-HOME.owl"/>
    </owl:Class>
    


    <!-- http://www.ease-crc.org/ont/SOMA-HOME.owl#SugarDispenser -->


    <owl:Class rdf:about="http://www.ease-crc.org/ont/SOMA-HOME.owl#SugarDispenser">
        <rdfs:subClassOf rdf:resource="http://www.ease-crc.org/ont/SOMA-HOME.owl#Dispenser"/>
        <rdfs:comment>A dispenser used to hold, or at least is intended to usually hold and serve, sugar.</rdfs:comment>
        <rdfs:isDefinedBy rdf:resource="http://www.ease-crc.org/ont/SOMA-HOME.owl"/>
    </owl:Class>
    


    <!-- http://www.ease-crc.org/ont/SOMA-HOME.owl#TableFork -->


    <owl:Class rdf:about="http://www.ease-crc.org/ont/SOMA-HOME.owl#TableFork">
        <rdfs:subClassOf rdf:resource="http://www.ease-crc.org/ont/SOMA.owl#Fork"/>
        <rdfs:comment>A regular size fork used for eating meals, e.g. for Spaghetti.</rdfs:comment>
        <rdfs:isDefinedBy rdf:resource="http://www.ease-crc.org/ont/SOMA-HOME.owl"/>
    </owl:Class>
    


    <!-- http://www.ease-crc.org/ont/SOMA-HOME.owl#TableKnife -->


    <owl:Class rdf:about="http://www.ease-crc.org/ont/SOMA-HOME.owl#TableKnife">
        <rdfs:subClassOf rdf:resource="http://www.ease-crc.org/ont/SOMA-HOME.owl#KitchenKnife"/>
        <rdfs:comment>A knife used for eating or speading butter on bread.</rdfs:comment>
        <rdfs:isDefinedBy rdf:resource="http://www.ease-crc.org/ont/SOMA-HOME.owl"/>
    </owl:Class>
    


    <!-- http://www.ease-crc.org/ont/SOMA-HOME.owl#TableSpoon -->


    <owl:Class rdf:about="http://www.ease-crc.org/ont/SOMA-HOME.owl#TableSpoon">
        <rdfs:subClassOf rdf:resource="http://www.ease-crc.org/ont/SOMA-HOME.owl#Spoon"/>
        <owl:disjointWith rdf:resource="http://www.ease-crc.org/ont/SOMA-HOME.owl#TeaSpoon"/>
        <rdfs:comment>A spoon usually refered as larger spoon used for serving. However in some regions it is the largest spoon used for eating.</rdfs:comment>
        <rdfs:isDefinedBy rdf:resource="http://www.ease-crc.org/ont/SOMA-HOME.owl"/>
    </owl:Class>
    


    <!-- http://www.ease-crc.org/ont/SOMA-HOME.owl#TeaSpoon -->


    <owl:Class rdf:about="http://www.ease-crc.org/ont/SOMA-HOME.owl#TeaSpoon">
        <rdfs:subClassOf rdf:resource="http://www.ease-crc.org/ont/SOMA-HOME.owl#Spoon"/>
        <rdfs:comment>A spoon relatively smaller in size used for string a cup of tea or measuring a volume. Specifically for cooking or medicine purposes, the volume is defined as 5ml.</rdfs:comment>
        <rdfs:isDefinedBy rdf:resource="http://www.ease-crc.org/ont/SOMA-HOME.owl"/>
    </owl:Class>
    


    <!-- http://www.ease-crc.org/ont/SOMA-HOME.owl#TemperingByCooling -->


    <owl:Class rdf:about="http://www.ease-crc.org/ont/SOMA-HOME.owl#TemperingByCooling">
        <rdfs:subClassOf rdf:resource="http://www.ease-crc.org/ont/SOMA.owl#Tempering"/>
        <rdfs:comment>A disposition of an object to change others by removing heat energy from them.</rdfs:comment>
        <rdfs:isDefinedBy rdf:resource="http://www.ease-crc.org/ont/SOMA-HOME.owl"/>
    </owl:Class>
    


    <!-- http://www.ease-crc.org/ont/SOMA-HOME.owl#TemperingByHeating -->


    <owl:Class rdf:about="http://www.ease-crc.org/ont/SOMA-HOME.owl#TemperingByHeating">
        <rdfs:subClassOf rdf:resource="http://www.ease-crc.org/ont/SOMA.owl#Tempering"/>
        <rdfs:comment>A disposition of an object to change others by applying heat energy to them.</rdfs:comment>
        <rdfs:isDefinedBy rdf:resource="http://www.ease-crc.org/ont/SOMA-HOME.owl"/>
    </owl:Class>
    


    <!-- http://www.ease-crc.org/ont/SOMA-HOME.owl#TrashContainer -->


    <owl:Class rdf:about="http://www.ease-crc.org/ont/SOMA-HOME.owl#TrashContainer">
        <rdfs:subClassOf rdf:resource="http://www.ease-crc.org/ont/SOMA.owl#DesignedContainer"/>
        <rdfs:comment>An item designed to hold trash. Typically equipped with a mechanism to close or open it, to prevent smells from the trash from propagating out and insects and other pests to get in.</rdfs:comment>
        <rdfs:isDefinedBy rdf:resource="http://www.ease-crc.org/ont/SOMA-HOME.owl"/>
    </owl:Class>
    


    <!-- http://www.ease-crc.org/ont/SOMA-HOME.owl#WaterBottle -->


    <owl:Class rdf:about="http://www.ease-crc.org/ont/SOMA-HOME.owl#WaterBottle">
        <rdfs:subClassOf rdf:resource="http://www.ease-crc.org/ont/SOMA.owl#Bottle"/>
        <rdfs:comment>A bottle which holds, or at least is intended to usually hold, water.</rdfs:comment>
        <rdfs:isDefinedBy rdf:resource="http://www.ease-crc.org/ont/SOMA-HOME.owl"/>
    </owl:Class>
    


    <!-- http://www.ease-crc.org/ont/SOMA-HOME.owl#WaterGlass -->


    <owl:Class rdf:about="http://www.ease-crc.org/ont/SOMA-HOME.owl#WaterGlass">
        <rdfs:subClassOf rdf:resource="http://www.ease-crc.org/ont/SOMA-HOME.owl#Glass"/>
        <rdfs:comment>A glass which holds, or at least is intended to usually hold, water. Also affords drinking from it.</rdfs:comment>
        <rdfs:isDefinedBy rdf:resource="http://www.ease-crc.org/ont/SOMA-HOME.owl"/>
    </owl:Class>
    


    <!-- http://www.ease-crc.org/ont/SOMA-HOME.owl#WineBottle -->


    <owl:Class rdf:about="http://www.ease-crc.org/ont/SOMA-HOME.owl#WineBottle">
        <rdfs:subClassOf rdf:resource="http://www.ease-crc.org/ont/SOMA.owl#Bottle"/>
        <rdfs:comment>A bottle which holds, or at least is intended to usually hold, wine.</rdfs:comment>
        <rdfs:isDefinedBy rdf:resource="http://www.ease-crc.org/ont/SOMA-HOME.owl"/>
    </owl:Class>
    


    <!-- http://www.ease-crc.org/ont/SOMA-HOME.owl#WineGlass -->


    <owl:Class rdf:about="http://www.ease-crc.org/ont/SOMA-HOME.owl#WineGlass">
        <rdfs:subClassOf rdf:resource="http://www.ease-crc.org/ont/SOMA-HOME.owl#Glass"/>
        <rdfs:comment>A glass which holds, or at least is intended to usually hold, wine. Also affords drinking from it.</rdfs:comment>
        <rdfs:isDefinedBy rdf:resource="http://www.ease-crc.org/ont/SOMA-HOME.owl"/>
    </owl:Class>
    


    <!-- http://www.ease-crc.org/ont/SOMA-OBJ.owl#ArtificialAgent -->


    <owl:Class rdf:about="http://www.ease-crc.org/ont/SOMA-OBJ.owl#ArtificialAgent">
        <rdfs:subClassOf rdf:resource="http://www.ontologydesignpatterns.org/ont/dul/DUL.owl#PhysicalAgent"/>
        <rdfs:comment>A physical object with artificial characteristics, which can perform actions to achieve desired goals, and typically has sensors and/or actuators.

There can be non-physical artificial agents such as software programs but they are not considered here in the scope of artificial agent.</rdfs:comment>
        <rdfs:isDefinedBy rdf:resource="http://www.ease-crc.org/ont/SOMA-OBJ.owl"/>
        <rdfs:label>Artificial agent</rdfs:label>
    </owl:Class>
    


    <!-- http://www.ease-crc.org/ont/SOMA-OBJ.owl#CanCut -->


    <owl:Class rdf:about="http://www.ease-crc.org/ont/SOMA-OBJ.owl#CanCut">
        <rdfs:subClassOf rdf:resource="http://www.ease-crc.org/ont/SOMA.owl#Variability"/>
        <rdfs:subClassOf>
            <owl:Restriction>
                <owl:onProperty rdf:resource="http://www.ease-crc.org/ont/SOMA.owl#affordsBearer"/>
                <owl:allValuesFrom rdf:resource="http://www.ease-crc.org/ont/SOMA-OBJ.owl#Cutter"/>
            </owl:Restriction>
        </rdfs:subClassOf>
        <rdfs:subClassOf>
            <owl:Restriction>
                <owl:onProperty rdf:resource="http://www.ease-crc.org/ont/SOMA.owl#affordsTrigger"/>
                <owl:allValuesFrom rdf:resource="http://www.ease-crc.org/ont/SOMA-OBJ.owl#CutObject"/>
            </owl:Restriction>
        </rdfs:subClassOf>
        <rdfs:comment>The disposition of an object (the tool) to cut other objects. Such as a knife has cutting ability to cut a cucumber into pieces.</rdfs:comment>
        <rdfs:isDefinedBy rdf:resource="http://www.ease-crc.org/ont/SOMA-OBJ.owl"/>
    </owl:Class>
    


    <!-- http://www.ease-crc.org/ont/SOMA-OBJ.owl#ContinuousJoint -->


    <owl:Class rdf:about="http://www.ease-crc.org/ont/SOMA-OBJ.owl#ContinuousJoint">
        <rdfs:subClassOf rdf:resource="http://www.ease-crc.org/ont/SOMA-OBJ.owl#HingeJoint"/>
        <rdfs:comment>A continuous hinge joint that rotates around an axis and has no upper and lower limits.</rdfs:comment>
        <rdfs:isDefinedBy rdf:resource="http://www.ease-crc.org/ont/SOMA-OBJ.owl"/>
        <rdfs:label>Continuous joint</rdfs:label>
    </owl:Class>
    


    <!-- http://www.ease-crc.org/ont/SOMA-OBJ.owl#CutObject -->


    <owl:Class rdf:about="http://www.ease-crc.org/ont/SOMA-OBJ.owl#CutObject">
        <rdfs:subClassOf rdf:resource="http://www.ease-crc.org/ont/SOMA.owl#AlteredObject"/>
        <rdfs:comment>An object being cut down into pieces.</rdfs:comment>
        <rdfs:isDefinedBy rdf:resource="http://www.ease-crc.org/ont/SOMA-OBJ.owl"/>
    </owl:Class>
    


    <!-- http://www.ease-crc.org/ont/SOMA-OBJ.owl#Cuttability -->


    <owl:Class rdf:about="http://www.ease-crc.org/ont/SOMA-OBJ.owl#Cuttability">
        <rdfs:subClassOf rdf:resource="http://www.ease-crc.org/ont/SOMA.owl#Disposition"/>
        <rdfs:subClassOf>
            <owl:Restriction>
                <owl:onProperty rdf:resource="http://www.ease-crc.org/ont/SOMA.owl#affordsBearer"/>
                <owl:allValuesFrom rdf:resource="http://www.ease-crc.org/ont/SOMA-OBJ.owl#CutObject"/>
            </owl:Restriction>
        </rdfs:subClassOf>
        <rdfs:subClassOf>
            <owl:Restriction>
                <owl:onProperty rdf:resource="http://www.ease-crc.org/ont/SOMA.owl#affordsTrigger"/>
                <owl:allValuesFrom rdf:resource="http://www.ease-crc.org/ont/SOMA-OBJ.owl#Cutter"/>
            </owl:Restriction>
        </rdfs:subClassOf>
        <rdfs:comment>The disposition of an object (the barrier) which makes it able to be cut down (into pieces) usually by some other object with role as a Cutter. Such as a cucumber has cuttability disposition which can be cut by a knife.</rdfs:comment>
        <rdfs:isDefinedBy rdf:resource="http://www.ease-crc.org/ont/SOMA-OBJ.owl"/>
    </owl:Class>
    


    <!-- http://www.ease-crc.org/ont/SOMA-OBJ.owl#Cutter -->


    <owl:Class rdf:about="http://www.ease-crc.org/ont/SOMA-OBJ.owl#Cutter">
        <rdfs:subClassOf rdf:resource="http://www.ease-crc.org/ont/SOMA.owl#Tool"/>
        <rdfs:comment>A role to classify an object used to cut other objects. Usually should poses sharpness as a quality. Execptions are not considered in this context. Such as a wind, water, or other natural agents cutting(eroding) the rocks.</rdfs:comment>
        <rdfs:isDefinedBy rdf:resource="http://www.ease-crc.org/ont/SOMA-OBJ.owl"/>
    </owl:Class>
    


    <!-- http://www.ease-crc.org/ont/SOMA-OBJ.owl#FixedJoint -->


    <owl:Class rdf:about="http://www.ease-crc.org/ont/SOMA-OBJ.owl#FixedJoint">
        <rdfs:subClassOf rdf:resource="http://www.ease-crc.org/ont/SOMA-OBJ.owl#Joint"/>
        <rdfs:subClassOf>
            <owl:Restriction>
                <owl:onProperty rdf:resource="http://www.ease-crc.org/ont/SOMA-OBJ.owl#hasJointState"/>
                <owl:qualifiedCardinality rdf:datatype="http://www.w3.org/2001/XMLSchema#nonNegativeInteger">0</owl:qualifiedCardinality>
                <owl:onClass rdf:resource="http://www.ontologydesignpatterns.org/ont/dul/DUL.owl#Entity"/>
            </owl:Restriction>
        </rdfs:subClassOf>
        <owl:disjointWith rdf:resource="http://www.ease-crc.org/ont/SOMA-OBJ.owl#MovableJoint"/>
        <rdfs:comment>A joint that cannot move, designed to fixiate links.</rdfs:comment>
        <rdfs:isDefinedBy rdf:resource="http://www.ease-crc.org/ont/SOMA-OBJ.owl"/>
        <rdfs:label>Fixed joint</rdfs:label>
    </owl:Class>
    


    <!-- http://www.ease-crc.org/ont/SOMA-OBJ.owl#FloatingJoint -->


    <owl:Class rdf:about="http://www.ease-crc.org/ont/SOMA-OBJ.owl#FloatingJoint">
        <rdfs:subClassOf rdf:resource="http://www.ease-crc.org/ont/SOMA-OBJ.owl#MovableJoint"/>
        <rdfs:comment>A joint that allows motion for all 6 degrees of freedom.</rdfs:comment>
        <rdfs:isDefinedBy rdf:resource="http://www.ease-crc.org/ont/SOMA-OBJ.owl"/>
        <rdfs:label>Floating joint</rdfs:label>
    </owl:Class>
    


    <!-- http://www.ease-crc.org/ont/SOMA-OBJ.owl#ForceAttribute -->


    <owl:Class rdf:about="http://www.ease-crc.org/ont/SOMA-OBJ.owl#ForceAttribute">
        <rdfs:subClassOf rdf:resource="http://www.ontologydesignpatterns.org/ont/dul/DUL.owl#PhysicalAttribute"/>
        <rdfs:subClassOf>
            <owl:Restriction>
                <owl:onProperty rdf:resource="http://www.ease-crc.org/ont/SOMA-OBJ.owl#hasForceValue"/>
                <owl:qualifiedCardinality rdf:datatype="http://www.w3.org/2001/XMLSchema#nonNegativeInteger">1</owl:qualifiedCardinality>
                <owl:onDataRange rdf:resource="http://www.ease-crc.org/ont/SOMA.owl#array_double"/>
            </owl:Restriction>
        </rdfs:subClassOf>
        <rdfs:comment>The value of a force dynamical characteristic. An example is the force exerted on another object when pushing it.</rdfs:comment>
        <rdfs:isDefinedBy rdf:resource="http://www.ease-crc.org/ont/SOMA-OBJ.owl"/>
        <rdfs:label>Force attribute</rdfs:label>
    </owl:Class>
    


    <!-- http://www.ease-crc.org/ont/SOMA-OBJ.owl#HingeJoint -->


    <owl:Class rdf:about="http://www.ease-crc.org/ont/SOMA-OBJ.owl#HingeJoint">
        <rdfs:subClassOf rdf:resource="http://www.ease-crc.org/ont/SOMA-OBJ.owl#MovableJoint"/>
        <rdfs:comment>A joint that rotates along an axis.</rdfs:comment>
        <rdfs:isDefinedBy rdf:resource="http://www.ease-crc.org/ont/SOMA-OBJ.owl"/>
        <rdfs:label>Hinge joint</rdfs:label>
    </owl:Class>
    


    <!-- http://www.ease-crc.org/ont/SOMA-OBJ.owl#Joint -->


    <owl:Class rdf:about="http://www.ease-crc.org/ont/SOMA-OBJ.owl#Joint">
        <owl:equivalentClass>
            <owl:Class>
                <owl:unionOf rdf:parseType="Collection">
                    <rdf:Description rdf:about="http://www.ease-crc.org/ont/SOMA-OBJ.owl#FixedJoint"/>
                    <rdf:Description rdf:about="http://www.ease-crc.org/ont/SOMA-OBJ.owl#MovableJoint"/>
                </owl:unionOf>
            </owl:Class>
        </owl:equivalentClass>
        <rdfs:subClassOf rdf:resource="http://www.ontologydesignpatterns.org/ont/dul/DUL.owl#PhysicalBody"/>
        <rdfs:subClassOf>
            <owl:Restriction>
                <owl:onProperty rdf:resource="http://www.ease-crc.org/ont/SOMA-OBJ.owl#hasChildLink"/>
                <owl:qualifiedCardinality rdf:datatype="http://www.w3.org/2001/XMLSchema#nonNegativeInteger">1</owl:qualifiedCardinality>
                <owl:onClass rdf:resource="http://www.ontologydesignpatterns.org/ont/dul/DUL.owl#PhysicalObject"/>
            </owl:Restriction>
        </rdfs:subClassOf>
        <rdfs:subClassOf>
            <owl:Restriction>
                <owl:onProperty rdf:resource="http://www.ease-crc.org/ont/SOMA-OBJ.owl#hasParentLink"/>
                <owl:qualifiedCardinality rdf:datatype="http://www.w3.org/2001/XMLSchema#nonNegativeInteger">1</owl:qualifiedCardinality>
                <owl:onClass rdf:resource="http://www.ontologydesignpatterns.org/ont/dul/DUL.owl#PhysicalObject"/>
            </owl:Restriction>
        </rdfs:subClassOf>
        <rdfs:subClassOf>
            <owl:Restriction>
                <owl:onProperty rdf:resource="http://www.ease-crc.org/ont/SOMA-OBJ.owl#hasJointState"/>
                <owl:maxQualifiedCardinality rdf:datatype="http://www.w3.org/2001/XMLSchema#nonNegativeInteger">1</owl:maxQualifiedCardinality>
                <owl:onClass rdf:resource="http://www.ease-crc.org/ont/SOMA-OBJ.owl#JointState"/>
            </owl:Restriction>
        </rdfs:subClassOf>
        <rdfs:comment>An object that is used to articulate links in a kinematic structure.</rdfs:comment>
        <rdfs:isDefinedBy rdf:resource="http://www.ease-crc.org/ont/SOMA-OBJ.owl"/>
    </owl:Class>
    


    <!-- http://www.ease-crc.org/ont/SOMA-OBJ.owl#JointLimit -->


    <owl:Class rdf:about="http://www.ease-crc.org/ont/SOMA-OBJ.owl#JointLimit">
        <rdfs:subClassOf rdf:resource="http://www.ontologydesignpatterns.org/ont/dul/DUL.owl#PhysicalAttribute"/>
        <rdfs:comment>The physical limits of a joint.</rdfs:comment>
        <rdfs:isDefinedBy rdf:resource="http://www.ease-crc.org/ont/SOMA-OBJ.owl"/>
        <rdfs:label>Joint limit</rdfs:label>
    </owl:Class>
    


    <!-- http://www.ease-crc.org/ont/SOMA-OBJ.owl#JointState -->


    <owl:Class rdf:about="http://www.ease-crc.org/ont/SOMA-OBJ.owl#JointState">
        <rdfs:subClassOf rdf:resource="http://www.ontologydesignpatterns.org/ont/dul/DUL.owl#PhysicalAttribute"/>
        <rdfs:subClassOf>
            <owl:Restriction>
                <owl:onProperty rdf:resource="http://www.ease-crc.org/ont/SOMA-OBJ.owl#hasJointPosition"/>
                <owl:qualifiedCardinality rdf:datatype="http://www.w3.org/2001/XMLSchema#nonNegativeInteger">1</owl:qualifiedCardinality>
                <owl:onDataRange rdf:resource="http://www.w3.org/2001/XMLSchema#double"/>
            </owl:Restriction>
        </rdfs:subClassOf>
        <rdfs:subClassOf>
            <owl:Restriction>
                <owl:onProperty rdf:resource="http://www.ease-crc.org/ont/SOMA-OBJ.owl#hasJointVelocity"/>
                <owl:qualifiedCardinality rdf:datatype="http://www.w3.org/2001/XMLSchema#nonNegativeInteger">1</owl:qualifiedCardinality>
                <owl:onDataRange rdf:resource="http://www.w3.org/2001/XMLSchema#double"/>
            </owl:Restriction>
        </rdfs:subClassOf>
        <rdfs:subClassOf>
            <owl:Restriction>
                <owl:onProperty rdf:resource="http://www.ease-crc.org/ont/SOMA-OBJ.owl#hasJointEffort"/>
                <owl:maxQualifiedCardinality rdf:datatype="http://www.w3.org/2001/XMLSchema#nonNegativeInteger">1</owl:maxQualifiedCardinality>
                <owl:onDataRange rdf:resource="http://www.w3.org/2001/XMLSchema#double"/>
            </owl:Restriction>
        </rdfs:subClassOf>
        <rdfs:comment>The state of a joint in terms of position, velocity of the joint and effort applied to it.</rdfs:comment>
        <rdfs:isDefinedBy rdf:resource="http://www.ease-crc.org/ont/SOMA-OBJ.owl"/>
        <rdfs:label>Joint state</rdfs:label>
    </owl:Class>
    


    <!-- http://www.ease-crc.org/ont/SOMA-OBJ.owl#MovableJoint -->


    <owl:Class rdf:about="http://www.ease-crc.org/ont/SOMA-OBJ.owl#MovableJoint">
        <rdfs:subClassOf rdf:resource="http://www.ease-crc.org/ont/SOMA-OBJ.owl#Joint"/>
        <rdfs:subClassOf>
            <owl:Restriction>
                <owl:onProperty rdf:resource="http://www.ease-crc.org/ont/SOMA-OBJ.owl#hasJointState"/>
                <owl:qualifiedCardinality rdf:datatype="http://www.w3.org/2001/XMLSchema#nonNegativeInteger">1</owl:qualifiedCardinality>
                <owl:onClass rdf:resource="http://www.ease-crc.org/ont/SOMA-OBJ.owl#JointState"/>
            </owl:Restriction>
        </rdfs:subClassOf>
        <rdfs:comment>A joint where the two connected links can move relative to each other in some dimension.</rdfs:comment>
        <rdfs:isDefinedBy rdf:resource="http://www.ease-crc.org/ont/SOMA-OBJ.owl"/>
        <rdfs:label>Movable joint</rdfs:label>
    </owl:Class>
    


    <!-- http://www.ease-crc.org/ont/SOMA-OBJ.owl#NetForce -->


    <owl:Class rdf:about="http://www.ease-crc.org/ont/SOMA-OBJ.owl#NetForce">
        <rdfs:subClassOf rdf:resource="http://www.ease-crc.org/ont/SOMA-OBJ.owl#ForceAttribute"/>
        <rdfs:comment>The accumulated force acting upon an object.</rdfs:comment>
        <rdfs:isDefinedBy rdf:resource="http://www.ease-crc.org/ont/SOMA-OBJ.owl"/>
        <rdfs:label>Net force</rdfs:label>
    </owl:Class>
    


    <!-- http://www.ease-crc.org/ont/SOMA-OBJ.owl#PlanarJoint -->


    <owl:Class rdf:about="http://www.ease-crc.org/ont/SOMA-OBJ.owl#PlanarJoint">
        <rdfs:subClassOf rdf:resource="http://www.ease-crc.org/ont/SOMA-OBJ.owl#MovableJoint"/>
        <rdfs:comment>A joint that allows motion in a plane perpendicular to an axis.</rdfs:comment>
        <rdfs:isDefinedBy rdf:resource="http://www.ease-crc.org/ont/SOMA-OBJ.owl"/>
        <rdfs:label>Planar joint</rdfs:label>
    </owl:Class>
    


    <!-- http://www.ease-crc.org/ont/SOMA-OBJ.owl#Pourable -->


    <owl:Class rdf:about="http://www.ease-crc.org/ont/SOMA-OBJ.owl#Pourable">
        <rdfs:subClassOf rdf:resource="http://www.ease-crc.org/ont/SOMA.owl#Disposition"/>
        <rdfs:subClassOf>
            <owl:Restriction>
                <owl:onProperty rdf:resource="http://www.ease-crc.org/ont/SOMA.owl#affordsBearer"/>
                <owl:allValuesFrom rdf:resource="http://www.ease-crc.org/ont/SOMA-OBJ.owl#PouredObject"/>
            </owl:Restriction>
        </rdfs:subClassOf>
        <rdfs:comment>The disposition of a fluid or substance which makes it possible to pour it out of a container and into or onto other objects.</rdfs:comment>
        <rdfs:isDefinedBy rdf:resource="http://www.ease-crc.org/ont/SOMA-OBJ.owl"/>
    </owl:Class>
    


    <!-- http://www.ease-crc.org/ont/SOMA-OBJ.owl#PouredObject -->


    <owl:Class rdf:about="http://www.ease-crc.org/ont/SOMA-OBJ.owl#PouredObject">
        <rdfs:subClassOf rdf:resource="http://www.ease-crc.org/ont/SOMA.owl#Patient"/>
        <rdfs:comment>An object being poured into or onto some other object. A role of some fluid or substance that is the patient of pouring task.</rdfs:comment>
        <rdfs:isDefinedBy rdf:resource="http://www.ease-crc.org/ont/SOMA-OBJ.owl"/>
    </owl:Class>
    


    <!-- http://www.ease-crc.org/ont/SOMA-OBJ.owl#PrismaticJoint -->


    <owl:Class rdf:about="http://www.ease-crc.org/ont/SOMA-OBJ.owl#PrismaticJoint">
        <rdfs:subClassOf rdf:resource="http://www.ease-crc.org/ont/SOMA-OBJ.owl#MovableJoint"/>
        <rdfs:subClassOf>
            <owl:Restriction>
                <owl:onProperty rdf:resource="http://www.ease-crc.org/ont/SOMA-OBJ.owl#hasJointLimit"/>
                <owl:qualifiedCardinality rdf:datatype="http://www.w3.org/2001/XMLSchema#nonNegativeInteger">1</owl:qualifiedCardinality>
                <owl:onClass rdf:resource="http://www.ease-crc.org/ont/SOMA-OBJ.owl#JointLimit"/>
            </owl:Restriction>
        </rdfs:subClassOf>
        <rdfs:comment>A sliding joint that slides along an axis, and has a limited range specified by the upper and lower limits.</rdfs:comment>
        <rdfs:isDefinedBy rdf:resource="http://www.ease-crc.org/ont/SOMA-OBJ.owl"/>
        <rdfs:label>Prismatic joint</rdfs:label>
    </owl:Class>
    


    <!-- http://www.ease-crc.org/ont/SOMA-OBJ.owl#RevoluteJoint -->


    <owl:Class rdf:about="http://www.ease-crc.org/ont/SOMA-OBJ.owl#RevoluteJoint">
        <rdfs:subClassOf rdf:resource="http://www.ease-crc.org/ont/SOMA-OBJ.owl#HingeJoint"/>
        <rdfs:subClassOf>
            <owl:Restriction>
                <owl:onProperty rdf:resource="http://www.ease-crc.org/ont/SOMA-OBJ.owl#hasJointLimit"/>
                <owl:qualifiedCardinality rdf:datatype="http://www.w3.org/2001/XMLSchema#nonNegativeInteger">1</owl:qualifiedCardinality>
                <owl:onClass rdf:resource="http://www.ease-crc.org/ont/SOMA-OBJ.owl#JointLimit"/>
            </owl:Restriction>
        </rdfs:subClassOf>
        <rdfs:comment>A hinge joint that rotates along an axis and has a limited range specified by the upper and lower limits.</rdfs:comment>
        <rdfs:isDefinedBy rdf:resource="http://www.ease-crc.org/ont/SOMA-OBJ.owl"/>
        <rdfs:label>Revolute joint</rdfs:label>
    </owl:Class>
    


    <!-- http://www.ease-crc.org/ont/SOMA-OBJ.owl#Storage -->


    <owl:Class rdf:about="http://www.ease-crc.org/ont/SOMA-OBJ.owl#Storage">
        <rdfs:subClassOf rdf:resource="http://www.ease-crc.org/ont/SOMA.owl#Enclosing"/>
        <rdfs:subClassOf>
            <owl:Restriction>
                <owl:onProperty rdf:resource="http://www.ease-crc.org/ont/SOMA.owl#affordsTrigger"/>
                <owl:allValuesFrom rdf:resource="http://www.ease-crc.org/ont/SOMA-OBJ.owl#StoredObject"/>
            </owl:Restriction>
        </rdfs:subClassOf>
        <rdfs:comment>The disposition of an object (the container) to store other objects. Storage of an object would facilitate several objectives; such as to store objects in a safe or usual place, to prevent the substances e.g. prevention of milk going bad by storing them in a refrigrator.</rdfs:comment>
        <rdfs:isDefinedBy rdf:resource="http://www.ease-crc.org/ont/SOMA-OBJ.owl"/>
    </owl:Class>
    


    <!-- http://www.ease-crc.org/ont/SOMA-OBJ.owl#StoredObject -->


    <owl:Class rdf:about="http://www.ease-crc.org/ont/SOMA-OBJ.owl#StoredObject">
        <rdfs:subClassOf rdf:resource="http://www.ease-crc.org/ont/SOMA.owl#EnclosedObject"/>
        <rdfs:comment>An object being stored into some other object, usually inside a container.</rdfs:comment>
        <rdfs:isDefinedBy rdf:resource="http://www.ease-crc.org/ont/SOMA-OBJ.owl"/>
    </owl:Class>
    


    <!-- http://www.ease-crc.org/ont/SOMA-STATE.owl#ContainmentState -->


    <owl:Class rdf:about="http://www.ease-crc.org/ont/SOMA-STATE.owl#ContainmentState">
        <rdfs:subClassOf rdf:resource="http://www.ease-crc.org/ont/SOMA.owl#FunctionalControl"/>
        <rdfs:subClassOf>
            <owl:Restriction>
                <owl:onProperty rdf:resource="http://www.ease-crc.org/ont/SOMA.owl#isStateTypeOf"/>
                <owl:someValuesFrom>
                    <owl:Class>
                        <owl:intersectionOf rdf:parseType="Collection">
                            <rdf:Description rdf:about="http://www.ease-crc.org/ont/SOMA.owl#Container"/>
                            <owl:Restriction>
                                <owl:onProperty rdf:resource="http://www.ontologydesignpatterns.org/ont/dul/DUL.owl#classifies"/>
                                <owl:allValuesFrom>
                                    <owl:Restriction>
                                        <owl:onProperty rdf:resource="http://www.ease-crc.org/ont/SOMA.owl#hasDisposition"/>
                                        <owl:someValuesFrom rdf:resource="http://www.ease-crc.org/ont/SOMA.owl#Containment"/>
                                    </owl:Restriction>
                                </owl:allValuesFrom>
                            </owl:Restriction>
                        </owl:intersectionOf>
                    </owl:Class>
                </owl:someValuesFrom>
            </owl:Restriction>
        </rdfs:subClassOf>
        <rdfs:comment>Classifies States in which an object is kept inside another object.</rdfs:comment>
        <rdfs:isDefinedBy rdf:resource="http://www.ease-crc.org/ont/SOMA-STATE.owl"/>
        <rdfs:label xml:lang="en">Containment state</rdfs:label>
    </owl:Class>
    


    <!-- http://www.ease-crc.org/ont/SOMA.owl#API_Specification -->


    <owl:Class rdf:about="http://www.ease-crc.org/ont/SOMA.owl#API_Specification">
        <rdfs:subClassOf rdf:resource="http://www.ease-crc.org/ont/SOMA.owl#InterfaceSpecification"/>
        <rdfs:comment xml:lang="en">An application programming interface (API) is a way for two or more computer programs to communicate with each other. It is a type of software interface, offering a service to other pieces of software. A document or standard that describes how to build or use an API is called an API specification.

Source: https://en.wikipedia.org/wiki/API</rdfs:comment>
        <rdfs:isDefinedBy rdf:resource="http://www.ease-crc.org/ont/SOMA-IO.owl"/>
        <rdfs:label xml:lang="en">API Specification</rdfs:label>
    </owl:Class>
    


    <!-- http://www.ease-crc.org/ont/SOMA.owl#AbductiveReasoning -->


    <owl:Class rdf:about="http://www.ease-crc.org/ont/SOMA.owl#AbductiveReasoning">
        <rdfs:subClassOf rdf:resource="http://www.ease-crc.org/ont/SOMA.owl#Reasoning"/>
        <rdfs:comment>A task in which the Agent proceeds from some set of statements about a world, and attempts to obtain an explanation for these statements. This explanation is often an inferred cause, such as a final cause or intention. Further, it is often required that there be some guarantees that the explanation produced by AbductiveReasoning have some desirable property, such as being the simplest or most likely given the set of statements to explain.</rdfs:comment>
        <rdfs:isDefinedBy rdf:resource="http://www.ease-crc.org/ont/SOMA-ACT.owl"/>
        <rdfs:label xml:lang="en">Abductive reasoning</rdfs:label>
    </owl:Class>
    


    <!-- http://www.ease-crc.org/ont/SOMA.owl#Accessor -->


    <owl:Class rdf:about="http://www.ease-crc.org/ont/SOMA.owl#Accessor">
        <rdfs:subClassOf rdf:resource="http://www.ease-crc.org/ont/SOMA.owl#Instrument"/>
        <rdfs:comment>A role classifying an object used to gain access to some other entity.</rdfs:comment>
        <rdfs:isDefinedBy rdf:resource="http://www.ease-crc.org/ont/SOMA-OBJ.owl"/>
    </owl:Class>
    


    <!-- http://www.ease-crc.org/ont/SOMA.owl#Actuating -->


    <owl:Class rdf:about="http://www.ease-crc.org/ont/SOMA.owl#Actuating">
        <rdfs:subClassOf rdf:resource="http://www.ease-crc.org/ont/SOMA.owl#PhysicalTask"/>
        <rdfs:comment>Tasks where the goal is to move an object.

Usually, an agent will use their prehensile effectors, ie. hands, for this purpose, so there is a lot of conceptual overlap between Actuating and Manipulating.

However, these categories are nonetheless distinguished in that there are more ways to actuate objects than simply manipulating them; for example, some tool like a net or frying pan might be used to catch an object.

Another way to look at the difference between Actuating and Manipulating is in what they &quot;profile&quot;, ie. focus on as important.

For Actuating, it is the object&apos;s motion that is paramount.

For Manipulating, it is the movement of the hand(s) and the change in functional relationships (such as kinematic control) between the hand(s) and the manipulated object(s).</rdfs:comment>
        <rdfs:comment>todo: think about use of tools. force events are generated between artifacts then. also not only the tool would be the &apos;salient artifact&apos; here.</rdfs:comment>
        <rdfs:isDefinedBy rdf:resource="http://www.ease-crc.org/ont/SOMA-ACT.owl"/>
    </owl:Class>
    


    <!-- http://www.ease-crc.org/ont/SOMA.owl#AestheticDesign -->


    <owl:Class rdf:about="http://www.ease-crc.org/ont/SOMA.owl#AestheticDesign">
        <rdfs:subClassOf rdf:resource="http://www.ontologydesignpatterns.org/ont/dul/DUL.owl#Design"/>
        <rdfs:comment>A design that describes an aesthetic quality of an object.

Aesthetics is the philosophical study of beauty and taste. The term stems from the Greek word &apos;aisthetikos&apos;, meaning &apos;of sense perception&apos;, and is related to the study of sensory values. From design point of view, aesthetics refers to the visual attractiveness of an object. Visual aesthetics have these key elements: Color, Shape, Pattern, Line, Texture, Visual weight, Balance, Scale, Proximity and Movement.</rdfs:comment>
        <rdfs:isDefinedBy rdf:resource="http://www.ease-crc.org/ont/SOMA-OBJ.owl"/>
        <rdfs:label>Aesthetic Design</rdfs:label>
    </owl:Class>
    


    <!-- http://www.ease-crc.org/ont/SOMA.owl#Affordance -->


    <owl:Class rdf:about="http://www.ease-crc.org/ont/SOMA.owl#Affordance">
        <rdfs:subClassOf rdf:resource="http://www.ontologydesignpatterns.org/ont/dul/DUL.owl#Relation"/>
        <rdfs:subClassOf>
            <owl:Restriction>
                <owl:onProperty rdf:resource="http://www.ontologydesignpatterns.org/ont/dul/DUL.owl#describes"/>
                <owl:allValuesFrom rdf:resource="http://www.ease-crc.org/ont/SOMA.owl#Disposition"/>
            </owl:Restriction>
        </rdfs:subClassOf>
        <rdfs:subClassOf>
            <owl:Restriction>
                <owl:onProperty rdf:resource="http://www.ease-crc.org/ont/SOMA.owl#definesBearer"/>
                <owl:qualifiedCardinality rdf:datatype="http://www.w3.org/2001/XMLSchema#nonNegativeInteger">1</owl:qualifiedCardinality>
                <owl:onClass rdf:resource="http://www.ontologydesignpatterns.org/ont/dul/DUL.owl#Role"/>
            </owl:Restriction>
        </rdfs:subClassOf>
        <rdfs:subClassOf>
            <owl:Restriction>
                <owl:onProperty rdf:resource="http://www.ease-crc.org/ont/SOMA.owl#definesTrigger"/>
                <owl:qualifiedCardinality rdf:datatype="http://www.w3.org/2001/XMLSchema#nonNegativeInteger">1</owl:qualifiedCardinality>
                <owl:onClass rdf:resource="http://www.ontologydesignpatterns.org/ont/dul/DUL.owl#Role"/>
            </owl:Restriction>
        </rdfs:subClassOf>
        <rdfs:subClassOf>
            <owl:Restriction>
                <owl:onProperty rdf:resource="http://www.ontologydesignpatterns.org/ont/dul/DUL.owl#definesTask"/>
                <owl:qualifiedCardinality rdf:datatype="http://www.w3.org/2001/XMLSchema#nonNegativeInteger">1</owl:qualifiedCardinality>
                <owl:onClass rdf:resource="http://www.ontologydesignpatterns.org/ont/dul/DUL.owl#Task"/>
            </owl:Restriction>
        </rdfs:subClassOf>
        <rdfs:comment>A relation between an object (the bearer) and others (the triggers) that describes the disposition of the bearer to be involved in an action execution that also involves some trigger object.</rdfs:comment>
        <rdfs:isDefinedBy rdf:resource="http://www.ease-crc.org/ont/SOMA-OBJ.owl"/>
    </owl:Class>
    


    <!-- http://www.ease-crc.org/ont/SOMA.owl#AgentRole -->


    <owl:Class rdf:about="http://www.ease-crc.org/ont/SOMA.owl#AgentRole">
        <rdfs:subClassOf rdf:resource="http://www.ease-crc.org/ont/SOMA.owl#CausativeRole"/>
        <rdfs:subClassOf>
            <owl:Restriction>
                <owl:onProperty rdf:resource="http://www.ontologydesignpatterns.org/ont/dul/DUL.owl#classifies"/>
                <owl:allValuesFrom rdf:resource="http://www.ontologydesignpatterns.org/ont/dul/DUL.owl#Agent"/>
            </owl:Restriction>
        </rdfs:subClassOf>
        <rdfs:comment>A role classifying an Agent responsible for performing an Action.

The entity playing an AgentRole is endowed with sentience and the capacity to deliberately choose actions in pursuit of goals. This distinguishes Agents from other causes that could bring an event about.</rdfs:comment>
        <rdfs:isDefinedBy rdf:resource="http://www.ease-crc.org/ont/SOMA-OBJ.owl"/>
        <rdfs:label xml:lang="en">Agent role</rdfs:label>
    </owl:Class>
    


    <!-- http://www.ease-crc.org/ont/SOMA.owl#Agonist -->


    <owl:Class rdf:about="http://www.ease-crc.org/ont/SOMA.owl#Agonist">
        <rdfs:subClassOf rdf:resource="http://www.ease-crc.org/ont/SOMA.owl#Patient"/>
        <rdfs:comment>A role that classifies entities with a tendency to either cause an alteration or to preserve some state.</rdfs:comment>
        <rdfs:isDefinedBy rdf:resource="http://www.ease-crc.org/ont/SOMA-PROC.owl"/>
    </owl:Class>
    


    <!-- http://www.ease-crc.org/ont/SOMA.owl#Algorithm -->


    <owl:Class rdf:about="http://www.ease-crc.org/ont/SOMA.owl#Algorithm">
        <rdfs:subClassOf rdf:resource="http://www.ontologydesignpatterns.org/ont/dul/DUL.owl#Plan"/>
        <rdfs:comment xml:lang="en">An Algorithm is a finite sequence of well-defined instructions, typically used to solve a class of specific problems or to perform a computation.

From Wikipedia: https://en.wikipedia.org/wiki/Algorithm</rdfs:comment>
        <rdfs:isDefinedBy rdf:resource="http://www.ease-crc.org/ont/SOMA-IO.owl"/>
        <rdfs:label xml:lang="en">Algorithm</rdfs:label>
    </owl:Class>
    


    <!-- http://www.ease-crc.org/ont/SOMA.owl#Alteration -->


    <owl:Class rdf:about="http://www.ease-crc.org/ont/SOMA.owl#Alteration">
        <rdfs:subClassOf rdf:resource="http://www.ease-crc.org/ont/SOMA.owl#ProcessType"/>
        <rdfs:comment>A process by which an aspect of some object changes such as ice cream melting in the sun.</rdfs:comment>
        <rdfs:isDefinedBy rdf:resource="http://www.ease-crc.org/ont/SOMA-PROC.owl"/>
    </owl:Class>
    


    <!-- http://www.ease-crc.org/ont/SOMA.owl#AlterativeInteraction -->


    <owl:Class rdf:about="http://www.ease-crc.org/ont/SOMA.owl#AlterativeInteraction">
        <rdfs:subClassOf rdf:resource="http://www.ease-crc.org/ont/SOMA.owl#ForceInteraction"/>
        <owl:disjointWith rdf:resource="http://www.ease-crc.org/ont/SOMA.owl#PreservativeInteraction"/>
        <rdfs:comment>A force interaction where the agonist has the tendency to set another object into motion. An example is &apos;opening a door&apos; where some object interacts with the door such that it moves out of its frame.</rdfs:comment>
        <rdfs:isDefinedBy rdf:resource="http://www.ease-crc.org/ont/SOMA-PROC.owl"/>
        <rdfs:label>Alterative interaction</rdfs:label>
    </owl:Class>
    


    <!-- http://www.ease-crc.org/ont/SOMA.owl#AlteredObject -->


    <owl:Class rdf:about="http://www.ease-crc.org/ont/SOMA.owl#AlteredObject">
        <rdfs:subClassOf rdf:resource="http://www.ease-crc.org/ont/SOMA.owl#Patient"/>
        <rdfs:comment>An object undergoing modifications.</rdfs:comment>
        <rdfs:isDefinedBy rdf:resource="http://www.ease-crc.org/ont/SOMA-OBJ.owl"/>
        <rdfs:isDefinedBy rdf:resource="http://www.ease-crc.org/ont/SOMA-PROC.owl"/>
        <rdfs:label xml:lang="en">Altered object</rdfs:label>
    </owl:Class>
    


    <!-- http://www.ease-crc.org/ont/SOMA.owl#Answer -->


    <owl:Class rdf:about="http://www.ease-crc.org/ont/SOMA.owl#Answer">
        <rdfs:subClassOf rdf:resource="http://www.ease-crc.org/ont/SOMA.owl#Message"/>
        <rdfs:comment>A role that is played by an Information Realization answering some query.</rdfs:comment>
        <rdfs:isDefinedBy rdf:resource="http://www.ease-crc.org/ont/SOMA-ACT.owl"/>
        <rdfs:label>Answer</rdfs:label>
    </owl:Class>
    


    <!-- http://www.ease-crc.org/ont/SOMA.owl#Antagonist -->


    <owl:Class rdf:about="http://www.ease-crc.org/ont/SOMA.owl#Antagonist">
        <rdfs:subClassOf rdf:resource="http://www.ease-crc.org/ont/SOMA.owl#Patient"/>
        <rdfs:comment>A role that classifies entities that are opposed to the tendency of some agonist.</rdfs:comment>
        <rdfs:isDefinedBy rdf:resource="http://www.ease-crc.org/ont/SOMA-PROC.owl"/>
    </owl:Class>
    


    <!-- http://www.ease-crc.org/ont/SOMA.owl#Appliance -->


    <owl:Class rdf:about="http://www.ease-crc.org/ont/SOMA.owl#Appliance">
        <rdfs:subClassOf rdf:resource="http://www.ontologydesignpatterns.org/ont/dul/DUL.owl#DesignedArtifact"/>
        <rdfs:comment>A device designed to perform a specific task, and that can be operated in some way.</rdfs:comment>
        <rdfs:isDefinedBy rdf:resource="http://www.ease-crc.org/ont/SOMA-HOME.owl"/>
        <rdfs:isDefinedBy rdf:resource="http://www.ease-crc.org/ont/SOMA-OBJ.owl"/>
    </owl:Class>
    


    <!-- http://www.ease-crc.org/ont/SOMA.owl#Approaching -->


    <owl:Class rdf:about="http://www.ease-crc.org/ont/SOMA.owl#Approaching">
        <rdfs:subClassOf rdf:resource="http://www.ease-crc.org/ont/SOMA.owl#Locomotion"/>
        <rdfs:comment>A process type to classify motions by which a body approaches some object or location.</rdfs:comment>
        <rdfs:isDefinedBy rdf:resource="http://www.ease-crc.org/ont/SOMA-PROC.owl"/>
    </owl:Class>
    


    <!-- http://www.ease-crc.org/ont/SOMA.owl#ArchiveFile -->


    <owl:Class rdf:about="http://www.ease-crc.org/ont/SOMA.owl#ArchiveFile">
        <owl:equivalentClass>
            <owl:Class>
                <owl:intersectionOf rdf:parseType="Collection">
                    <rdf:Description rdf:about="http://www.ease-crc.org/ont/SOMA.owl#Digital_File"/>
                    <owl:Restriction>
                        <owl:onProperty rdf:resource="http://www.ontologydesignpatterns.org/ont/dul/DUL.owl#realizes"/>
                        <owl:someValuesFrom rdf:resource="http://www.ease-crc.org/ont/SOMA.owl#ArchiveText"/>
                    </owl:Restriction>
                </owl:intersectionOf>
            </owl:Class>
        </owl:equivalentClass>
        <rdfs:subClassOf rdf:resource="http://www.ease-crc.org/ont/SOMA.owl#Digital_File"/>
        <rdfs:comment xml:lang="en">An archive file is a computer file that is composed of one or more files along with metadata.

Source: https://en.wikipedia.org/wiki/Archive_file</rdfs:comment>
        <rdfs:isDefinedBy rdf:resource="http://www.ease-crc.org/ont/SOMA-IO.owl"/>
        <rdfs:label>Archive File</rdfs:label>
    </owl:Class>
    


    <!-- http://www.ease-crc.org/ont/SOMA.owl#ArchiveFormat -->


    <owl:Class rdf:about="http://www.ease-crc.org/ont/SOMA.owl#ArchiveFormat">
        <rdfs:subClassOf rdf:resource="http://www.ease-crc.org/ont/SOMA.owl#File_format"/>
        <rdfs:subClassOf>
            <owl:Restriction>
                <owl:onProperty rdf:resource="http://www.ease-crc.org/ont/SOMA.owl#givesMeaningTo"/>
                <owl:allValuesFrom rdf:resource="http://www.ease-crc.org/ont/SOMA.owl#ArchiveText"/>
            </owl:Restriction>
        </rdfs:subClassOf>
        <rdfs:comment xml:lang="en">An Archive Format is the file format of an archive file.

Source: https://en.wikipedia.org/wiki/Archive_file#Archive_formats</rdfs:comment>
        <rdfs:isDefinedBy rdf:resource="http://www.ease-crc.org/ont/SOMA-IO.owl"/>
        <rdfs:label xml:lang="en">Archive Format</rdfs:label>
    </owl:Class>
    


    <!-- http://www.ease-crc.org/ont/SOMA.owl#ArchiveText -->


    <owl:Class rdf:about="http://www.ease-crc.org/ont/SOMA.owl#ArchiveText">
        <owl:equivalentClass>
            <owl:Class>
                <owl:intersectionOf rdf:parseType="Collection">
                    <rdf:Description rdf:about="http://www.ease-crc.org/ont/SOMA.owl#Structured_Text"/>
                    <owl:Restriction>
                        <owl:onProperty rdf:resource="http://www.ontologydesignpatterns.org/ont/dul/DUL.owl#expresses"/>
                        <owl:someValuesFrom rdf:resource="http://www.ease-crc.org/ont/SOMA.owl#FileConfiguration"/>
                    </owl:Restriction>
                </owl:intersectionOf>
            </owl:Class>
        </owl:equivalentClass>
        <owl:equivalentClass>
            <owl:Restriction>
                <owl:onProperty rdf:resource="http://www.ease-crc.org/ont/SOMA.owl#isGivenMeaningBy"/>
                <owl:someValuesFrom rdf:resource="http://www.ease-crc.org/ont/SOMA.owl#ArchiveFormat"/>
            </owl:Restriction>
        </owl:equivalentClass>
        <rdfs:comment xml:lang="en">An Archive is a Structured Text that is composed of one or more Structured Texts along with metadata. Archives are used to collect multiple texts together into a single text for easier portability and storage as Archive Files, or simply to compress text to use less storage space as Computer Files. Archive often store directory structures, error detection and correction information, arbitrary comments, and sometimes use built-in encryption.

Source: https://en.wikipedia.org/wiki/Archive_file</rdfs:comment>
        <rdfs:isDefinedBy rdf:resource="http://www.ease-crc.org/ont/SOMA-IO.owl"/>
        <rdfs:label xml:lang="en">Archive Text</rdfs:label>
    </owl:Class>
    


    <!-- http://www.ease-crc.org/ont/SOMA.owl#AreaSurveying -->


    <owl:Class rdf:about="http://www.ease-crc.org/ont/SOMA.owl#AreaSurveying">
        <rdfs:subClassOf rdf:resource="http://www.ease-crc.org/ont/SOMA.owl#Perceiving"/>
        <rdfs:comment>A task in which an Agent uses its perception apparatus to gain information about some location.</rdfs:comment>
        <rdfs:isDefinedBy rdf:resource="http://www.ease-crc.org/ont/SOMA-ACT.owl"/>
        <rdfs:label xml:lang="en">Area surveying</rdfs:label>
    </owl:Class>
    


    <!-- http://www.ease-crc.org/ont/SOMA.owl#Arm -->


    <owl:Class rdf:about="http://www.ease-crc.org/ont/SOMA.owl#Arm">
        <rdfs:subClassOf rdf:resource="http://www.ease-crc.org/ont/SOMA.owl#Limb"/>
        <rdfs:comment>A limb used to reach for objects.</rdfs:comment>
        <rdfs:isDefinedBy rdf:resource="http://www.ease-crc.org/ont/SOMA-OBJ.owl"/>
    </owl:Class>
    


    <!-- http://www.ease-crc.org/ont/SOMA.owl#Arranging -->


    <owl:Class rdf:about="http://www.ease-crc.org/ont/SOMA.owl#Arranging">
        <rdfs:subClassOf rdf:resource="http://www.ease-crc.org/ont/SOMA.owl#Constructing"/>
        <rdfs:comment>A task in which an Agent places a collection of objects at some set of relative poses to each other.</rdfs:comment>
        <rdfs:isDefinedBy rdf:resource="http://www.ease-crc.org/ont/SOMA-ACT.owl"/>
    </owl:Class>
    


    <!-- http://www.ease-crc.org/ont/SOMA.owl#ArtificialAgent -->


    <owl:Class rdf:about="http://www.ease-crc.org/ont/SOMA.owl#ArtificialAgent">
        <rdfs:subClassOf rdf:resource="http://www.ontologydesignpatterns.org/ont/dul/DUL.owl#PhysicalAgent"/>
        <rdfs:comment xml:lang="en">Any constructed agent with physical embodiment that has intentions on its own, e.g., a robot.</rdfs:comment>
        <rdfs:isDefinedBy rdf:resource="http://www.ease-crc.org/ont/SOMA-IO.owl"/>
        <rdfs:label xml:lang="en">Artificial agent</rdfs:label>
    </owl:Class>
    


    <!-- http://www.ease-crc.org/ont/SOMA.owl#Assembling -->


    <owl:Class rdf:about="http://www.ease-crc.org/ont/SOMA.owl#Assembling">
        <rdfs:subClassOf rdf:resource="http://www.ease-crc.org/ont/SOMA.owl#Constructing"/>
        <rdfs:comment>A task in which an Agent connects some objects such that they form a cohesive whole, and which also imposes constraints on the objects&apos; relative motions. Often, the objects that make up an assemblage can also be separated again.</rdfs:comment>
        <rdfs:isDefinedBy rdf:resource="http://www.ease-crc.org/ont/SOMA-ACT.owl"/>
    </owl:Class>
    


    <!-- http://www.ease-crc.org/ont/SOMA.owl#AssertionTask -->


    <owl:Class rdf:about="http://www.ease-crc.org/ont/SOMA.owl#AssertionTask">
        <rdfs:subClassOf rdf:resource="http://www.ease-crc.org/ont/SOMA.owl#IllocutionaryTask"/>
        <rdfs:subClassOf>
            <owl:Restriction>
                <owl:onProperty rdf:resource="http://www.ontologydesignpatterns.org/ont/dul/DUL.owl#classifies"/>
                <owl:allValuesFrom>
                    <owl:Restriction>
                        <owl:onProperty rdf:resource="http://www.ontologydesignpatterns.org/ont/dul/DUL.owl#hasParticipant"/>
                        <owl:someValuesFrom rdf:resource="http://www.ease-crc.org/ont/SOMA.owl#DeclarativeClause"/>
                    </owl:Restriction>
                </owl:allValuesFrom>
            </owl:Restriction>
        </rdfs:subClassOf>
        <rdfs:comment xml:lang="en">An Illocutionary Act where the Sender emits some Message with the intent to change what the Receiver believes to be true in some context. Often, assertions are of facts about the real world, but this need not be the case. Assertions can communicate what someone believes, or refer to a world that is entirely fictional. In all these cases however, assertions are intended to update the listener&apos;s model (of the real world, or of the speaker&apos;s beliefs, or of the fictional world etc.).</rdfs:comment>
        <rdfs:isDefinedBy rdf:resource="http://www.ease-crc.org/ont/SOMA-ACT.owl"/>
        <rdfs:label xml:lang="en">Assertion task</rdfs:label>
    </owl:Class>
    


    <!-- http://www.ease-crc.org/ont/SOMA.owl#AssumingArmPose -->


    <owl:Class rdf:about="http://www.ease-crc.org/ont/SOMA.owl#AssumingArmPose">
        <rdfs:subClassOf rdf:resource="http://www.ease-crc.org/ont/SOMA.owl#AssumingPose"/>
        <rdfs:comment>A task by which an Agent arranges one/some/all of its arms according to some configuration.</rdfs:comment>
        <rdfs:isDefinedBy rdf:resource="http://www.ease-crc.org/ont/SOMA-ACT.owl"/>
        <rdfs:label xml:lang="en">Assuming arm pose</rdfs:label>
    </owl:Class>
    


    <!-- http://www.ease-crc.org/ont/SOMA.owl#AssumingPose -->


    <owl:Class rdf:about="http://www.ease-crc.org/ont/SOMA.owl#AssumingPose">
        <rdfs:subClassOf rdf:resource="http://www.ease-crc.org/ont/SOMA.owl#PhysicalTask"/>
        <rdfs:comment>A task by which an Agent arranges its body, or part of it, according to some configuration.</rdfs:comment>
        <rdfs:isDefinedBy rdf:resource="http://www.ease-crc.org/ont/SOMA-ACT.owl"/>
        <rdfs:label xml:lang="en">Assuming pose</rdfs:label>
    </owl:Class>
    


    <!-- http://www.ease-crc.org/ont/SOMA.owl#AvoidedObject -->


    <owl:Class rdf:about="http://www.ease-crc.org/ont/SOMA.owl#AvoidedObject">
        <rdfs:subClassOf rdf:resource="http://www.ease-crc.org/ont/SOMA.owl#Patient"/>
        <rdfs:comment>An object that is avoided.</rdfs:comment>
        <rdfs:isDefinedBy rdf:resource="http://www.ease-crc.org/ont/SOMA-OBJ.owl"/>
        <rdfs:label xml:lang="en">Avoided object</rdfs:label>
    </owl:Class>
    


    <!-- http://www.ease-crc.org/ont/SOMA.owl#Avoiding -->


    <owl:Class rdf:about="http://www.ease-crc.org/ont/SOMA.owl#Avoiding">
        <rdfs:subClassOf rdf:resource="http://www.ease-crc.org/ont/SOMA.owl#Navigating"/>
        <rdfs:comment>A task in which an Agent moves so as to not enter or pass through a location.</rdfs:comment>
        <rdfs:isDefinedBy rdf:resource="http://www.ease-crc.org/ont/SOMA-ACT.owl"/>
    </owl:Class>
    


    <!-- http://www.ease-crc.org/ont/SOMA.owl#BakedGood -->


    <owl:Class rdf:about="http://www.ease-crc.org/ont/SOMA.owl#BakedGood">
        <rdfs:subClassOf rdf:resource="http://www.ease-crc.org/ont/SOMA.owl#Dish"/>
        <rdfs:isDefinedBy rdf:resource="http://www.ease-crc.org/ont/SOMA-HOME.owl"/>
    </owl:Class>
    


    <!-- http://www.ease-crc.org/ont/SOMA.owl#Barrier -->


    <owl:Class rdf:about="http://www.ease-crc.org/ont/SOMA.owl#Barrier">
        <rdfs:subClassOf rdf:resource="http://www.ease-crc.org/ont/SOMA.owl#Restrictor"/>
        <rdfs:comment>A role classifying an object used to prevent others from entering or leaving a restricted space or group.</rdfs:comment>
        <rdfs:isDefinedBy rdf:resource="http://www.ease-crc.org/ont/SOMA-OBJ.owl"/>
    </owl:Class>
    


    <!-- http://www.ease-crc.org/ont/SOMA.owl#BeneficiaryRole -->


    <owl:Class rdf:about="http://www.ease-crc.org/ont/SOMA.owl#BeneficiaryRole">
        <rdfs:subClassOf rdf:resource="http://www.ease-crc.org/ont/SOMA.owl#GoalRole"/>
        <rdfs:comment>A role classifying an agent for whose benefit an action is performed.</rdfs:comment>
        <rdfs:isDefinedBy rdf:resource="http://www.ease-crc.org/ont/SOMA-OBJ.owl"/>
        <rdfs:label xml:lang="en">Beneficiary role</rdfs:label>
    </owl:Class>
    


    <!-- http://www.ease-crc.org/ont/SOMA.owl#Binding -->


    <owl:Class rdf:about="http://www.ease-crc.org/ont/SOMA.owl#Binding">
        <rdfs:subClassOf rdf:resource="http://www.ontologydesignpatterns.org/ont/dul/DUL.owl#Relation"/>
        <rdfs:subClassOf>
            <owl:Class>
                <owl:unionOf rdf:parseType="Collection">
                    <rdf:Description rdf:about="http://www.ease-crc.org/ont/SOMA.owl#CounterfactualBinding"/>
                    <rdf:Description rdf:about="http://www.ease-crc.org/ont/SOMA.owl#FactualBinding"/>
                </owl:unionOf>
            </owl:Class>
        </rdfs:subClassOf>
        <rdfs:subClassOf>
            <owl:Class>
                <owl:unionOf rdf:parseType="Collection">
                    <rdf:Description rdf:about="http://www.ease-crc.org/ont/SOMA.owl#RoleFillerBinding"/>
                    <rdf:Description rdf:about="http://www.ease-crc.org/ont/SOMA.owl#RoleRoleBinding"/>
                </owl:unionOf>
            </owl:Class>
        </rdfs:subClassOf>
        <rdfs:subClassOf>
            <owl:Restriction>
                <owl:onProperty>
                    <rdf:Description>
                        <owl:inverseOf rdf:resource="http://www.ease-crc.org/ont/SOMA.owl#hasBinding"/>
                    </rdf:Description>
                </owl:onProperty>
                <owl:someValuesFrom rdf:resource="http://www.ontologydesignpatterns.org/ont/dul/DUL.owl#Description"/>
            </owl:Restriction>
        </rdfs:subClassOf>
        <rdfs:subClassOf>
            <owl:Restriction>
                <owl:onProperty rdf:resource="http://www.ease-crc.org/ont/SOMA.owl#hasBindingFiller"/>
                <owl:qualifiedCardinality rdf:datatype="http://www.w3.org/2001/XMLSchema#nonNegativeInteger">1</owl:qualifiedCardinality>
                <owl:onClass rdf:resource="http://www.ontologydesignpatterns.org/ont/dul/DUL.owl#Entity"/>
            </owl:Restriction>
        </rdfs:subClassOf>
        <rdfs:subClassOf>
            <owl:Restriction>
                <owl:onProperty rdf:resource="http://www.ease-crc.org/ont/SOMA.owl#hasBindingRole"/>
                <owl:qualifiedCardinality rdf:datatype="http://www.w3.org/2001/XMLSchema#nonNegativeInteger">1</owl:qualifiedCardinality>
                <owl:onClass>
                    <owl:Class>
                        <owl:unionOf rdf:parseType="Collection">
                            <rdf:Description rdf:about="http://www.ontologydesignpatterns.org/ont/dul/DUL.owl#Parameter"/>
                            <rdf:Description rdf:about="http://www.ontologydesignpatterns.org/ont/dul/DUL.owl#Role"/>
                        </owl:unionOf>
                    </owl:Class>
                </owl:onClass>
            </owl:Restriction>
        </rdfs:subClassOf>
        <rdfs:comment>A Relation between Roles/Parameters and their fillers that holds in a particular descriptive context, such as a Workflow or Narrative.

It covers two conceptually related, but somewhat ontologically distinct situations:

-- a binding between two Roles, or two Parameters, with the meaning that in the particular descriptive context where the Binding holds, a filler for one Role/Parameter is also a filler for the other
-- a binding between a Role/Parameter and an Entity able to fill that Role/Parameter, with the meaning that in the particular descriptive context where the Binding holds, the Entity fills the Role/Parameter.

Note: in the second case, the Entity filling the Role/Parameter may be a Role or Parameter itself. This however does NOT reduce to the first case. Consider these examples:

-- (first situation) The accountant is also the lawyer. In this case, there are two roles, and there is a person filling both of them. This is a factual, role-role binding.
-- (second situation, linking to a generic Entity) The accountant is Bob. In this case, there is a factual, role-filler binding asserting who fills the accountant role.
-- (second situation, linking to a role) The newly opened job is accountant. In this case, there is a factual, role-filler binding asserting that some role is filled by another, without making any assertion about the filler of this second role. It is not known, and not important, whether an accountant exists at this time.

There is a further, orthogonal distinction made between:
-- factual: the Binding is asserted to hold in the descriptive context
-- counterfactual: the Binding is used to express conditions in the descriptive context. A counterfactual Binding is not meant as an assertion that the Binding actually holds.</rdfs:comment>
        <rdfs:isDefinedBy rdf:resource="http://www.ease-crc.org/ont/SOMA-WF.owl"/>
    </owl:Class>
    


    <!-- http://www.ease-crc.org/ont/SOMA.owl#Blade -->


    <owl:Class rdf:about="http://www.ease-crc.org/ont/SOMA.owl#Blade">
        <rdfs:subClassOf rdf:resource="http://www.ease-crc.org/ont/SOMA.owl#DesignedComponent"/>
        <rdfs:comment>A flat cutting edge of an object used to cut through other objects, such as the blade of a ventilator cutting through the air.</rdfs:comment>
        <rdfs:isDefinedBy rdf:resource="http://www.ease-crc.org/ont/SOMA-HOME.owl"/>
    </owl:Class>
    


    <!-- http://www.ease-crc.org/ont/SOMA.owl#Blockage -->


    <owl:Class rdf:about="http://www.ease-crc.org/ont/SOMA.owl#Blockage">
        <rdfs:subClassOf rdf:resource="http://www.ease-crc.org/ont/SOMA.owl#Disposition"/>
        <rdfs:subClassOf>
            <owl:Restriction>
                <owl:onProperty rdf:resource="http://www.ease-crc.org/ont/SOMA.owl#affordsBearer"/>
                <owl:allValuesFrom rdf:resource="http://www.ease-crc.org/ont/SOMA.owl#Barrier"/>
            </owl:Restriction>
        </rdfs:subClassOf>
        <rdfs:subClassOf>
            <owl:Restriction>
                <owl:onProperty rdf:resource="http://www.ease-crc.org/ont/SOMA.owl#affordsTrigger"/>
                <owl:allValuesFrom rdf:resource="http://www.ease-crc.org/ont/SOMA.owl#BlockedObject"/>
            </owl:Restriction>
        </rdfs:subClassOf>
        <rdfs:comment>The disposition of an object (the barrier) to prevent others from accessing, leaving, or seeing a restricted space, or group.</rdfs:comment>
        <rdfs:isDefinedBy rdf:resource="http://www.ease-crc.org/ont/SOMA-OBJ.owl"/>
    </owl:Class>
    


    <!-- http://www.ease-crc.org/ont/SOMA.owl#BlockedObject -->


    <owl:Class rdf:about="http://www.ease-crc.org/ont/SOMA.owl#BlockedObject">
        <rdfs:subClassOf rdf:resource="http://www.ease-crc.org/ont/SOMA.owl#Patient"/>
        <rdfs:comment>An object that is blocked from accessing something.</rdfs:comment>
        <rdfs:isDefinedBy rdf:resource="http://www.ease-crc.org/ont/SOMA-OBJ.owl"/>
        <rdfs:label xml:lang="en">Blocked object</rdfs:label>
    </owl:Class>
    


    <!-- http://www.ease-crc.org/ont/SOMA.owl#BodyMovement -->


    <owl:Class rdf:about="http://www.ease-crc.org/ont/SOMA.owl#BodyMovement">
        <rdfs:subClassOf rdf:resource="http://www.ease-crc.org/ont/SOMA.owl#Motion"/>
        <rdfs:subClassOf>
            <owl:Restriction>
                <owl:onProperty rdf:resource="http://www.ontologydesignpatterns.org/ont/dul/DUL.owl#classifies"/>
                <owl:allValuesFrom>
                    <owl:Class>
                        <owl:unionOf rdf:parseType="Collection">
                            <owl:Restriction>
                                <owl:onProperty rdf:resource="http://www.ontologydesignpatterns.org/ont/dul/DUL.owl#hasParticipant"/>
                                <owl:someValuesFrom rdf:resource="http://www.ontologydesignpatterns.org/ont/dul/DUL.owl#PhysicalAgent"/>
                            </owl:Restriction>
                            <owl:Restriction>
                                <owl:onProperty rdf:resource="http://www.ontologydesignpatterns.org/ont/dul/DUL.owl#hasParticipant"/>
                                <owl:someValuesFrom>
                                    <owl:Class>
                                        <owl:intersectionOf rdf:parseType="Collection">
                                            <rdf:Description rdf:about="http://www.ontologydesignpatterns.org/ont/dul/DUL.owl#PhysicalObject"/>
                                            <owl:Restriction>
                                                <owl:onProperty rdf:resource="http://www.ontologydesignpatterns.org/ont/dul/DUL.owl#isPartOf"/>
                                                <owl:someValuesFrom rdf:resource="http://www.ontologydesignpatterns.org/ont/dul/DUL.owl#PhysicalAgent"/>
                                            </owl:Restriction>
                                        </owl:intersectionOf>
                                    </owl:Class>
                                </owl:someValuesFrom>
                            </owl:Restriction>
                        </owl:unionOf>
                    </owl:Class>
                </owl:allValuesFrom>
            </owl:Restriction>
        </rdfs:subClassOf>
        <rdfs:comment>Motion described in terms of how parts of an Agent&apos;s body move.

As such, this concept can be applied only to motions involving some PhysicalAgent, or body parts of a PhysicalAgent.</rdfs:comment>
        <rdfs:isDefinedBy rdf:resource="http://www.ease-crc.org/ont/SOMA-PROC.owl"/>
    </owl:Class>
    


    <!-- http://www.ease-crc.org/ont/SOMA.owl#Boiling -->


    <owl:Class rdf:about="http://www.ease-crc.org/ont/SOMA.owl#Boiling">
        <rdfs:subClassOf rdf:resource="http://www.ease-crc.org/ont/SOMA.owl#Vaporizing"/>
        <rdfs:comment>In each instance of this collection some liquid matter is raised to its boilingPoint and is thereby changed from being in the Liquid-StateOfMatter to being in the Gaseous-StateOfMatter.</rdfs:comment>
        <rdfs:isDefinedBy rdf:resource="http://www.ease-crc.org/ont/SOMA-PROC.owl"/>
    </owl:Class>
    


    <!-- http://www.ease-crc.org/ont/SOMA.owl#Bottle -->


    <owl:Class rdf:about="http://www.ease-crc.org/ont/SOMA.owl#Bottle">
        <rdfs:subClassOf rdf:resource="http://www.ease-crc.org/ont/SOMA.owl#DesignedContainer"/>
        <rdfs:comment>A container with a narrow neck used to store fluids.</rdfs:comment>
        <rdfs:isDefinedBy rdf:resource="http://www.ease-crc.org/ont/SOMA-HOME.owl"/>
    </owl:Class>
    


    <!-- http://www.ease-crc.org/ont/SOMA.owl#Bowl -->


    <owl:Class rdf:about="http://www.ease-crc.org/ont/SOMA.owl#Bowl">
        <rdfs:subClassOf rdf:resource="http://www.ease-crc.org/ont/SOMA.owl#Crockery"/>
        <rdfs:comment>A round, deep object used to contain food or liquid.</rdfs:comment>
        <rdfs:isDefinedBy rdf:resource="http://www.ease-crc.org/ont/SOMA-HOME.owl"/>
    </owl:Class>
    


    <!-- http://www.ease-crc.org/ont/SOMA.owl#BoxShape -->


    <owl:Class rdf:about="http://www.ease-crc.org/ont/SOMA.owl#BoxShape">
        <rdfs:subClassOf rdf:resource="http://www.ease-crc.org/ont/SOMA.owl#ShapeRegion"/>
        <rdfs:subClassOf>
            <owl:Restriction>
                <owl:onProperty rdf:resource="http://www.ease-crc.org/ont/SOMA.owl#hasHeight"/>
                <owl:qualifiedCardinality rdf:datatype="http://www.w3.org/2001/XMLSchema#nonNegativeInteger">1</owl:qualifiedCardinality>
                <owl:onDataRange rdf:resource="http://www.w3.org/2001/XMLSchema#float"/>
            </owl:Restriction>
        </rdfs:subClassOf>
        <rdfs:subClassOf>
            <owl:Restriction>
                <owl:onProperty rdf:resource="http://www.ease-crc.org/ont/SOMA.owl#hasLength"/>
                <owl:qualifiedCardinality rdf:datatype="http://www.w3.org/2001/XMLSchema#nonNegativeInteger">1</owl:qualifiedCardinality>
                <owl:onDataRange rdf:resource="http://www.w3.org/2001/XMLSchema#float"/>
            </owl:Restriction>
        </rdfs:subClassOf>
        <rdfs:subClassOf>
            <owl:Restriction>
                <owl:onProperty rdf:resource="http://www.ease-crc.org/ont/SOMA.owl#hasWidth"/>
                <owl:qualifiedCardinality rdf:datatype="http://www.w3.org/2001/XMLSchema#nonNegativeInteger">1</owl:qualifiedCardinality>
                <owl:onDataRange rdf:resource="http://www.w3.org/2001/XMLSchema#float"/>
            </owl:Restriction>
        </rdfs:subClassOf>
        <rdfs:comment>A symmetrical shape, either solid or hollow, contained by six rectangles.</rdfs:comment>
        <rdfs:isDefinedBy rdf:resource="http://www.ease-crc.org/ont/SOMA-HOME.owl"/>
        <rdfs:isDefinedBy rdf:resource="http://www.ease-crc.org/ont/SOMA-OBJ.owl"/>
        <rdfs:label>Box shape</rdfs:label>
    </owl:Class>
    


    <!-- http://www.ease-crc.org/ont/SOMA.owl#Bread -->


    <owl:Class rdf:about="http://www.ease-crc.org/ont/SOMA.owl#Bread">
        <rdfs:subClassOf rdf:resource="http://www.ease-crc.org/ont/SOMA.owl#BakedGood"/>
        <rdfs:isDefinedBy rdf:resource="http://www.ease-crc.org/ont/SOMA-HOME.owl"/>
    </owl:Class>
    


    <!-- http://www.ease-crc.org/ont/SOMA.owl#Building -->


    <owl:Class rdf:about="http://www.ease-crc.org/ont/SOMA.owl#Building">
        <rdfs:subClassOf rdf:resource="http://www.ease-crc.org/ont/SOMA.owl#DesignedContainer"/>
        <rdfs:comment>A structure with a roof and walls.</rdfs:comment>
        <rdfs:isDefinedBy rdf:resource="http://www.ease-crc.org/ont/SOMA-HOME.owl"/>
    </owl:Class>
    


    <!-- http://www.ease-crc.org/ont/SOMA.owl#Capacity -->


    <owl:Class rdf:about="http://www.ease-crc.org/ont/SOMA.owl#Capacity">
        <rdfs:subClassOf rdf:resource="http://www.ease-crc.org/ont/SOMA.owl#Intrinsic"/>
        <rdfs:comment>The maximum amount an object can contain.</rdfs:comment>
        <rdfs:isDefinedBy rdf:resource="http://www.ease-crc.org/ont/SOMA-OBJ.owl"/>
    </owl:Class>
    


    <!-- http://www.ease-crc.org/ont/SOMA.owl#Catching -->


    <owl:Class rdf:about="http://www.ease-crc.org/ont/SOMA.owl#Catching">
        <rdfs:subClassOf rdf:resource="http://www.ease-crc.org/ont/SOMA.owl#Actuating"/>
        <owl:disjointWith rdf:resource="http://www.ease-crc.org/ont/SOMA.owl#PickingUp"/>
        <rdfs:comment>A task by which an Agent stops a moving object and gains kinematic control over it, usually by grasping.</rdfs:comment>
        <rdfs:isDefinedBy rdf:resource="http://www.ease-crc.org/ont/SOMA-ACT.owl"/>
    </owl:Class>
    


    <!-- http://www.ease-crc.org/ont/SOMA.owl#CausalEventRole -->


    <owl:Class rdf:about="http://www.ease-crc.org/ont/SOMA.owl#CausalEventRole">
        <rdfs:subClassOf rdf:resource="http://www.ease-crc.org/ont/SOMA.owl#CausativeRole"/>
        <rdfs:comment>A role filled by a description of some action or process that brings about a motion.

As an example, consider the utterance &quot;the tennisman served the ball by hitting it with the racket.&quot; In this utterance, the filler of the CausalEventRole is expressed by the &quot;by hitting it with the racket&quot; constituent.</rdfs:comment>
        <rdfs:isDefinedBy rdf:resource="http://www.ease-crc.org/ont/SOMA-OBJ.owl"/>
        <rdfs:label xml:lang="en">Causal event role</rdfs:label>
    </owl:Class>
    


    <!-- http://www.ease-crc.org/ont/SOMA.owl#CausativeRole -->


    <owl:Class rdf:about="http://www.ease-crc.org/ont/SOMA.owl#CausativeRole">
        <rdfs:subClassOf rdf:resource="http://www.ease-crc.org/ont/SOMA.owl#EventAdjacentRole"/>
        <rdfs:comment>A role classifying objects that are responsible in bringing about an event.

The paradigmatic example is the Agent performing an Action -- the Agent is the effective cause of the Action it performs. However, not all objects causing events are agents.</rdfs:comment>
        <rdfs:isDefinedBy rdf:resource="http://www.ease-crc.org/ont/SOMA-OBJ.owl"/>
        <rdfs:label xml:lang="en">Causative role</rdfs:label>
    </owl:Class>
    


    <!-- http://www.ease-crc.org/ont/SOMA.owl#CausedMotionTheory -->


    <owl:Class rdf:about="http://www.ease-crc.org/ont/SOMA.owl#CausedMotionTheory">
        <rdfs:subClassOf rdf:resource="http://www.ease-crc.org/ont/SOMA.owl#ImageSchemaTheory"/>
        <rdfs:subClassOf>
            <owl:Restriction>
                <owl:onProperty rdf:resource="http://www.ontologydesignpatterns.org/ont/dul/DUL.owl#defines"/>
                <owl:someValuesFrom rdf:resource="http://www.ease-crc.org/ont/SOMA.owl#AgentRole"/>
            </owl:Restriction>
        </rdfs:subClassOf>
        <rdfs:subClassOf>
            <owl:Restriction>
                <owl:onProperty rdf:resource="http://www.ontologydesignpatterns.org/ont/dul/DUL.owl#defines"/>
                <owl:someValuesFrom rdf:resource="http://www.ease-crc.org/ont/SOMA.owl#CausalEventRole"/>
            </owl:Restriction>
        </rdfs:subClassOf>
        <rdfs:subClassOf>
            <owl:Restriction>
                <owl:onProperty rdf:resource="http://www.ontologydesignpatterns.org/ont/dul/DUL.owl#defines"/>
                <owl:someValuesFrom rdf:resource="http://www.ease-crc.org/ont/SOMA.owl#Instrument"/>
            </owl:Restriction>
        </rdfs:subClassOf>
        <rdfs:subClassOf>
            <owl:Restriction>
                <owl:onProperty rdf:resource="http://www.ontologydesignpatterns.org/ont/dul/DUL.owl#defines"/>
                <owl:someValuesFrom rdf:resource="http://www.ease-crc.org/ont/SOMA.owl#Patient"/>
            </owl:Restriction>
        </rdfs:subClassOf>
        <rdfs:subClassOf>
            <owl:Restriction>
                <owl:onProperty rdf:resource="http://www.ontologydesignpatterns.org/ont/dul/DUL.owl#hasPart"/>
                <owl:someValuesFrom rdf:resource="http://www.ease-crc.org/ont/SOMA.owl#SourcePathGoalTheory"/>
            </owl:Restriction>
        </rdfs:subClassOf>
        <rdfs:comment>A schematic theory describing a situation in which an agent performs an action which causes an object to move along a certain path. A popular example being &quot;He sneezed the napkin off the table.&quot; (Goldberg 1995)

Let xA, xP be objects filling the agent, patient roles of this schema. Then one can infer that xA movesObject xP.</rdfs:comment>
        <rdfs:isDefinedBy rdf:resource="http://www.ease-crc.org/ont/SOMA-SAY.owl"/>
        <rdfs:label xml:lang="en">Caused motion theory</rdfs:label>
    </owl:Class>
    


    <!-- http://www.ease-crc.org/ont/SOMA.owl#Ceiling -->


    <owl:Class rdf:about="http://www.ease-crc.org/ont/SOMA.owl#Ceiling">
        <rdfs:subClassOf rdf:resource="http://www.ease-crc.org/ont/SOMA.owl#RoomSurface"/>
        <owl:disjointWith rdf:resource="http://www.ease-crc.org/ont/SOMA.owl#Floor"/>
        <owl:disjointWith rdf:resource="http://www.ease-crc.org/ont/SOMA.owl#Wall"/>
        <rdfs:comment>The upper interior surface of a room.</rdfs:comment>
        <rdfs:isDefinedBy rdf:resource="http://www.ease-crc.org/ont/SOMA-HOME.owl"/>
    </owl:Class>
    


    <!-- http://www.ease-crc.org/ont/SOMA.owl#Channel -->


    <owl:Class rdf:about="http://www.ease-crc.org/ont/SOMA.owl#Channel">
        <rdfs:subClassOf rdf:resource="http://www.ease-crc.org/ont/SOMA.owl#PathRole"/>
        <rdfs:subClassOf>
            <owl:Restriction>
                <owl:onProperty rdf:resource="http://www.ontologydesignpatterns.org/ont/dul/DUL.owl#hasTask"/>
                <owl:someValuesFrom rdf:resource="http://www.ease-crc.org/ont/SOMA.owl#CommunicationTask"/>
            </owl:Restriction>
        </rdfs:subClassOf>
        <rdfs:comment xml:lang="en">A Channel in a Communication Task is the path of travel by a Message, e.g., via WLAN, air (in the case of a Message classifying soundwaves) or a telephone cable.</rdfs:comment>
        <rdfs:isDefinedBy rdf:resource="http://www.ease-crc.org/ont/SOMA-ACT.owl"/>
        <rdfs:label xml:lang="en">Channel</rdfs:label>
    </owl:Class>
    


    <!-- http://www.ease-crc.org/ont/SOMA.owl#CheckingObjectPresence -->


    <owl:Class rdf:about="http://www.ease-crc.org/ont/SOMA.owl#CheckingObjectPresence">
        <rdfs:subClassOf rdf:resource="http://www.ease-crc.org/ont/SOMA.owl#Perceiving"/>
        <rdfs:comment>A task by which an Agent uses its sensors to check for the presence of a specific object and to obtain some other information about it, e.g. pose.</rdfs:comment>
        <rdfs:isDefinedBy rdf:resource="http://www.ease-crc.org/ont/SOMA-ACT.owl"/>
        <rdfs:label xml:lang="en">Checking object presence</rdfs:label>
    </owl:Class>
    


    <!-- http://www.ease-crc.org/ont/SOMA.owl#ChemicalProcess -->


    <owl:Class rdf:about="http://www.ease-crc.org/ont/SOMA.owl#ChemicalProcess">
        <rdfs:subClassOf rdf:resource="http://www.ontologydesignpatterns.org/ont/dul/DUL.owl#Process"/>
        <rdfs:comment>A process by which the chemical constituency of an Entity or set of Entities changes.

In some sense any process that results in entities being created or destroyed might trivially fit here, however this concept is intended specifically for Events where the occuring chemical reactions are of importance.</rdfs:comment>
        <rdfs:isDefinedBy rdf:resource="http://www.ease-crc.org/ont/SOMA-PROC.owl"/>
        <rdfs:label>Chemical process</rdfs:label>
    </owl:Class>
    


    <!-- http://www.ease-crc.org/ont/SOMA.owl#CircularCylinder -->


    <owl:Class rdf:about="http://www.ease-crc.org/ont/SOMA.owl#CircularCylinder">
        <rdfs:subClassOf rdf:resource="http://www.ease-crc.org/ont/SOMA.owl#CylinderShape"/>
        <rdfs:subClassOf>
            <owl:Restriction>
                <owl:onProperty rdf:resource="http://www.ease-crc.org/ont/SOMA.owl#hasRadius"/>
                <owl:qualifiedCardinality rdf:datatype="http://www.w3.org/2001/XMLSchema#nonNegativeInteger">1</owl:qualifiedCardinality>
                <owl:onDataRange rdf:resource="http://www.w3.org/2001/XMLSchema#float"/>
            </owl:Restriction>
        </rdfs:subClassOf>
        <rdfs:comment>A cylinder figure with circular cross section.</rdfs:comment>
        <rdfs:isDefinedBy rdf:resource="http://www.ease-crc.org/ont/SOMA-OBJ.owl"/>
        <rdfs:label>Circular cylinder</rdfs:label>
    </owl:Class>
    


    <!-- http://www.ease-crc.org/ont/SOMA.owl#Classifier -->


    <owl:Class rdf:about="http://www.ease-crc.org/ont/SOMA.owl#Classifier">
        <rdfs:subClassOf rdf:resource="http://www.ease-crc.org/ont/SOMA.owl#StatisticalReasoner"/>
        <rdfs:isDefinedBy rdf:resource="http://www.ease-crc.org/ont/SOMA-IO.owl"/>
        <rdfs:label xml:lang="en">Classifier</rdfs:label>
    </owl:Class>
    


    <!-- http://www.ease-crc.org/ont/SOMA.owl#ClausalObject -->


    <owl:Class rdf:about="http://www.ease-crc.org/ont/SOMA.owl#ClausalObject">
        <rdfs:subClassOf rdf:resource="http://www.ease-crc.org/ont/SOMA.owl#Phrase"/>
        <rdfs:comment>A clause is a phrase containing a subject and a predicate.</rdfs:comment>
        <rdfs:isDefinedBy rdf:resource="http://www.ease-crc.org/ont/SOMA-SAY.owl"/>
        <rdfs:label>Clausal object</rdfs:label>
    </owl:Class>
    


    <!-- http://www.ease-crc.org/ont/SOMA.owl#Clean -->


    <owl:Class rdf:about="http://www.ease-crc.org/ont/SOMA.owl#Clean">
        <rdfs:subClassOf rdf:resource="http://www.ease-crc.org/ont/SOMA.owl#CleanlinessRegion"/>
        <rdfs:comment>A cleanliness region with values considered as clean.</rdfs:comment>
        <rdfs:isDefinedBy rdf:resource="http://www.ease-crc.org/ont/SOMA-OBJ.owl"/>
    </owl:Class>
    


    <!-- http://www.ease-crc.org/ont/SOMA.owl#Cleanliness -->


    <owl:Class rdf:about="http://www.ease-crc.org/ont/SOMA.owl#Cleanliness">
        <rdfs:subClassOf rdf:resource="http://www.ease-crc.org/ont/SOMA.owl#SocialQuality"/>
        <rdfs:subClassOf>
            <owl:Restriction>
                <owl:onProperty rdf:resource="http://www.ontologydesignpatterns.org/ont/dul/DUL.owl#hasRegion"/>
                <owl:someValuesFrom rdf:resource="http://www.ease-crc.org/ont/SOMA.owl#CleanlinessRegion"/>
            </owl:Restriction>
        </rdfs:subClassOf>
        <rdfs:subClassOf>
            <owl:Restriction>
                <owl:onProperty rdf:resource="http://www.ontologydesignpatterns.org/ont/dul/DUL.owl#hasRegion"/>
                <owl:allValuesFrom rdf:resource="http://www.ease-crc.org/ont/SOMA.owl#CleanlinessRegion"/>
            </owl:Restriction>
        </rdfs:subClassOf>
        <rdfs:comment>The quality of being clean.</rdfs:comment>
        <rdfs:isDefinedBy rdf:resource="http://www.ease-crc.org/ont/SOMA-OBJ.owl"/>
    </owl:Class>
    


    <!-- http://www.ease-crc.org/ont/SOMA.owl#CleanlinessRegion -->


    <owl:Class rdf:about="http://www.ease-crc.org/ont/SOMA.owl#CleanlinessRegion">
        <rdfs:subClassOf rdf:resource="http://www.ontologydesignpatterns.org/ont/dul/DUL.owl#Region"/>
        <rdfs:comment>Encodes the cleanliness of an object.</rdfs:comment>
        <rdfs:isDefinedBy rdf:resource="http://www.ease-crc.org/ont/SOMA-OBJ.owl"/>
        <rdfs:label xml:lang="en">Cleanliness region</rdfs:label>
    </owl:Class>
    


    <!-- http://www.ease-crc.org/ont/SOMA.owl#Client-Server_Specification -->


    <owl:Class rdf:about="http://www.ease-crc.org/ont/SOMA.owl#Client-Server_Specification">
        <rdfs:subClassOf rdf:resource="http://www.ease-crc.org/ont/SOMA.owl#InterfaceSpecification"/>
        <rdfs:subClassOf>
            <owl:Class>
                <owl:intersectionOf rdf:parseType="Collection">
                    <owl:Restriction>
                        <owl:onProperty rdf:resource="http://www.ontologydesignpatterns.org/ont/dul/DUL.owl#definesRole"/>
                        <owl:someValuesFrom rdf:resource="http://www.ease-crc.org/ont/SOMA.owl#ClientRole"/>
                    </owl:Restriction>
                    <owl:Restriction>
                        <owl:onProperty rdf:resource="http://www.ontologydesignpatterns.org/ont/dul/DUL.owl#definesRole"/>
                        <owl:someValuesFrom rdf:resource="http://www.ease-crc.org/ont/SOMA.owl#ServerRole"/>
                    </owl:Restriction>
                </owl:intersectionOf>
            </owl:Class>
        </rdfs:subClassOf>
        <rdfs:isDefinedBy rdf:resource="http://www.ease-crc.org/ont/SOMA-IO.owl"/>
        <rdfs:label xml:lang="en">An API Secification that describes the well known Client-Server pattern:

The Client-server model is a distributed application structure that partitions tasks or workloads between the providers of a resource or service, called servers, and service requesters, called clients Often clients and servers communicate over a computer network on separate hardware, but both client and server may reside in the same system. A server host runs one or more server programs, which share their resources with clients. A client usually does not share any of its resources, but it requests content or service from a server. Clients, therefore, initiate communication sessions with servers, which await incoming requests. Examples of computer applications that use the client-server model are email, network printing, and the World Wide Web.

Source: https://en.wikipedia.org/wiki/Client%E2%80%93server_model</rdfs:label>
        <rdfs:label xml:lang="en">Client-Server Specification</rdfs:label>
    </owl:Class>
    


    <!-- http://www.ease-crc.org/ont/SOMA.owl#ClientRole -->


    <owl:Class rdf:about="http://www.ease-crc.org/ont/SOMA.owl#ClientRole">
        <rdfs:subClassOf rdf:resource="http://www.ease-crc.org/ont/SOMA.owl#InterfaceComponentRole"/>
        <rdfs:subClassOf>
            <owl:Restriction>
                <owl:onProperty rdf:resource="http://www.ontologydesignpatterns.org/ont/dul/DUL.owl#isDefinedIn"/>
                <owl:someValuesFrom rdf:resource="http://www.ease-crc.org/ont/SOMA.owl#Client-Server_Specification"/>
            </owl:Restriction>
        </rdfs:subClassOf>
        <rdfs:comment xml:lang="en">The Client-server model is a distributed application structure that partitions tasks or workloads between the providers of a resource or service, called servers, and service requesters, called clients Often clients and servers communicate over a computer network on separate hardware, but both client and server may reside in the same system. A server host runs one or more server programs, which share their resources with clients. A client usually does not share any of its resources, but it requests content or service from a server. Clients, therefore, initiate communication sessions with servers, which await incoming requests. Examples of computer applications that use the client-server model are email, network printing, and the World Wide Web.

Source: https://en.wikipedia.org/wiki/Client%E2%80%93server_model</rdfs:comment>
        <rdfs:isDefinedBy rdf:resource="http://www.ease-crc.org/ont/SOMA-IO.owl"/>
        <rdfs:label xml:lang="en">Client role</rdfs:label>
    </owl:Class>
    


    <!-- http://www.ease-crc.org/ont/SOMA.owl#Closing -->


    <owl:Class rdf:about="http://www.ease-crc.org/ont/SOMA.owl#Closing">
        <rdfs:subClassOf rdf:resource="http://www.ease-crc.org/ont/SOMA.owl#Actuating"/>
        <owl:disjointWith rdf:resource="http://www.ease-crc.org/ont/SOMA.owl#Delivering"/>
        <owl:disjointWith rdf:resource="http://www.ease-crc.org/ont/SOMA.owl#Fetching"/>
        <owl:disjointWith rdf:resource="http://www.ease-crc.org/ont/SOMA.owl#Lifting"/>
        <owl:disjointWith rdf:resource="http://www.ease-crc.org/ont/SOMA.owl#Opening"/>
        <owl:disjointWith rdf:resource="http://www.ease-crc.org/ont/SOMA.owl#Pulling"/>
        <owl:disjointWith rdf:resource="http://www.ease-crc.org/ont/SOMA.owl#Pushing"/>
        <owl:disjointWith rdf:resource="http://www.ease-crc.org/ont/SOMA.owl#Squeezing"/>
        <rdfs:comment>A task in which an Agent manipulates a container so as to block access to its interior.</rdfs:comment>
        <rdfs:isDefinedBy rdf:resource="http://www.ease-crc.org/ont/SOMA-ACT.owl"/>
    </owl:Class>
    


    <!-- http://www.ease-crc.org/ont/SOMA.owl#Collision -->


    <owl:Class rdf:about="http://www.ease-crc.org/ont/SOMA.owl#Collision">
        <rdfs:subClassOf rdf:resource="http://www.ease-crc.org/ont/SOMA.owl#ProcessType"/>
        <rdfs:comment>A contact event of objects bumping into each other such that their movement is affected.</rdfs:comment>
        <rdfs:isDefinedBy rdf:resource="http://www.ease-crc.org/ont/SOMA-PROC.owl"/>
    </owl:Class>
    


    <!-- http://www.ease-crc.org/ont/SOMA.owl#Color -->


    <owl:Class rdf:about="http://www.ease-crc.org/ont/SOMA.owl#Color">
        <rdfs:subClassOf rdf:resource="http://www.ease-crc.org/ont/SOMA.owl#Extrinsic"/>
        <rdfs:subClassOf>
            <owl:Restriction>
                <owl:onProperty rdf:resource="http://www.ontologydesignpatterns.org/ont/dul/DUL.owl#hasRegion"/>
                <owl:someValuesFrom rdf:resource="http://www.ease-crc.org/ont/SOMA.owl#ColorRegion"/>
            </owl:Restriction>
        </rdfs:subClassOf>
        <rdfs:subClassOf>
            <owl:Restriction>
                <owl:onProperty rdf:resource="http://www.ontologydesignpatterns.org/ont/dul/DUL.owl#hasRegion"/>
                <owl:allValuesFrom rdf:resource="http://www.ease-crc.org/ont/SOMA.owl#ColorRegion"/>
            </owl:Restriction>
        </rdfs:subClassOf>
        <rdfs:comment>The color of an object. Color regions encode the color value in some space such as RGB or HSV, and may further be used to classify the color as red, dark, etc. The color of an object may have different facets, e.g. a red and blue color.</rdfs:comment>
        <rdfs:isDefinedBy rdf:resource="http://www.ease-crc.org/ont/SOMA-OBJ.owl"/>
        <rdfs:label>Color</rdfs:label>
    </owl:Class>
    


    <!-- http://www.ease-crc.org/ont/SOMA.owl#ColorRegion -->


    <owl:Class rdf:about="http://www.ease-crc.org/ont/SOMA.owl#ColorRegion">
        <rdfs:subClassOf rdf:resource="http://www.ontologydesignpatterns.org/ont/dul/DUL.owl#Region"/>
        <rdfs:subClassOf>
            <owl:Restriction>
                <owl:onProperty rdf:resource="http://www.ontologydesignpatterns.org/ont/dul/DUL.owl#isRegionFor"/>
                <owl:allValuesFrom rdf:resource="http://www.ease-crc.org/ont/SOMA.owl#Color"/>
            </owl:Restriction>
        </rdfs:subClassOf>
        <rdfs:comment>Encodes the color of an object.</rdfs:comment>
        <rdfs:isDefinedBy rdf:resource="http://www.ease-crc.org/ont/SOMA-OBJ.owl"/>
        <rdfs:label>Color region</rdfs:label>
    </owl:Class>
    


    <!-- http://www.ease-crc.org/ont/SOMA.owl#CommandingTask -->


    <owl:Class rdf:about="http://www.ease-crc.org/ont/SOMA.owl#CommandingTask">
        <rdfs:subClassOf rdf:resource="http://www.ease-crc.org/ont/SOMA.owl#IllocutionaryTask"/>
        <rdfs:subClassOf>
            <owl:Restriction>
                <owl:onProperty rdf:resource="http://www.ontologydesignpatterns.org/ont/dul/DUL.owl#classifies"/>
                <owl:allValuesFrom>
                    <owl:Restriction>
                        <owl:onProperty rdf:resource="http://www.ontologydesignpatterns.org/ont/dul/DUL.owl#hasParticipant"/>
                        <owl:someValuesFrom rdf:resource="http://www.ease-crc.org/ont/SOMA.owl#ImperativeClause"/>
                    </owl:Restriction>
                </owl:allValuesFrom>
            </owl:Restriction>
        </rdfs:subClassOf>
        <rdfs:comment xml:lang="en">An Illocutionary act where the Sender emits some Message with the intent to cause the Receiver to perform some action.</rdfs:comment>
        <rdfs:isDefinedBy rdf:resource="http://www.ease-crc.org/ont/SOMA-ACT.owl"/>
        <rdfs:label xml:lang="en">Commanding task</rdfs:label>
    </owl:Class>
    


    <!-- http://www.ease-crc.org/ont/SOMA.owl#CommitedObject -->


    <owl:Class rdf:about="http://www.ease-crc.org/ont/SOMA.owl#CommitedObject">
        <rdfs:subClassOf rdf:resource="http://www.ease-crc.org/ont/SOMA.owl#ConnectedObject"/>
        <rdfs:comment>An object committed to a bigger whole. After being committed, the object does not exist anymore in its old form.</rdfs:comment>
        <rdfs:isDefinedBy rdf:resource="http://www.ease-crc.org/ont/SOMA-OBJ.owl"/>
        <rdfs:label xml:lang="en">Commited object</rdfs:label>
    </owl:Class>
    


    <!-- http://www.ease-crc.org/ont/SOMA.owl#CommunicationAction -->


    <owl:Class rdf:about="http://www.ease-crc.org/ont/SOMA.owl#CommunicationAction">
        <rdfs:subClassOf rdf:resource="http://www.ontologydesignpatterns.org/ont/dul/DUL.owl#Action"/>
        <rdfs:subClassOf>
            <owl:Restriction>
                <owl:onProperty rdf:resource="http://www.ontologydesignpatterns.org/ont/dul/DUL.owl#hasParticipant"/>
                <owl:someValuesFrom rdf:resource="http://www.ease-crc.org/ont/SOMA.owl#LinguisticObject"/>
            </owl:Restriction>
        </rdfs:subClassOf>
        <rdfs:comment xml:lang="en">An action in which an Agent uses some actuator for communication purposes.</rdfs:comment>
        <rdfs:isDefinedBy rdf:resource="http://www.ease-crc.org/ont/SOMA-ACT.owl"/>
        <rdfs:label xml:lang="en">Locutionary action</rdfs:label>
    </owl:Class>
    


    <!-- http://www.ease-crc.org/ont/SOMA.owl#CommunicationReport -->


    <owl:Class rdf:about="http://www.ease-crc.org/ont/SOMA.owl#CommunicationReport">
        <rdfs:subClassOf rdf:resource="http://www.ease-crc.org/ont/SOMA.owl#CommunicationTask"/>
        <rdfs:comment>A task in which an Agent endeavors to describe truthfully some state of affairs.</rdfs:comment>
        <rdfs:isDefinedBy rdf:resource="http://www.ease-crc.org/ont/SOMA-ACT.owl"/>
        <rdfs:label xml:lang="en">Communication report</rdfs:label>
    </owl:Class>
    


    <!-- http://www.ease-crc.org/ont/SOMA.owl#CommunicationTask -->


    <owl:Class rdf:about="http://www.ease-crc.org/ont/SOMA.owl#CommunicationTask">
        <rdfs:subClassOf rdf:resource="http://www.ontologydesignpatterns.org/ont/dul/DUL.owl#Task"/>
        <rdfs:subClassOf>
            <owl:Class>
                <owl:intersectionOf rdf:parseType="Collection">
                    <owl:Restriction>
                        <owl:onProperty rdf:resource="http://www.ontologydesignpatterns.org/ont/dul/DUL.owl#isTaskOf"/>
                        <owl:someValuesFrom rdf:resource="http://www.ease-crc.org/ont/SOMA.owl#Channel"/>
                    </owl:Restriction>
                    <owl:Restriction>
                        <owl:onProperty rdf:resource="http://www.ontologydesignpatterns.org/ont/dul/DUL.owl#isTaskOf"/>
                        <owl:someValuesFrom rdf:resource="http://www.ease-crc.org/ont/SOMA.owl#Message"/>
                    </owl:Restriction>
                    <owl:Restriction>
                        <owl:onProperty rdf:resource="http://www.ontologydesignpatterns.org/ont/dul/DUL.owl#isTaskOf"/>
                        <owl:someValuesFrom rdf:resource="http://www.ease-crc.org/ont/SOMA.owl#Receiver"/>
                    </owl:Restriction>
                    <owl:Restriction>
                        <owl:onProperty rdf:resource="http://www.ontologydesignpatterns.org/ont/dul/DUL.owl#isTaskOf"/>
                        <owl:someValuesFrom rdf:resource="http://www.ease-crc.org/ont/SOMA.owl#Sender"/>
                    </owl:Restriction>
                </owl:intersectionOf>
            </owl:Class>
        </rdfs:subClassOf>
        <rdfs:subClassOf>
            <owl:Restriction>
                <owl:onProperty rdf:resource="http://www.ontologydesignpatterns.org/ont/dul/DUL.owl#classifies"/>
                <owl:allValuesFrom>
                    <owl:Restriction>
                        <owl:onProperty rdf:resource="http://www.ontologydesignpatterns.org/ont/dul/DUL.owl#hasParticipant"/>
                        <owl:allValuesFrom>
                            <owl:Class>
                                <owl:unionOf rdf:parseType="Collection">
                                    <rdf:Description rdf:about="http://www.ontologydesignpatterns.org/ont/dul/DUL.owl#Agent"/>
                                    <rdf:Description rdf:about="http://www.ontologydesignpatterns.org/ont/dul/DUL.owl#SocialObject"/>
                                </owl:unionOf>
                            </owl:Class>
                        </owl:allValuesFrom>
                    </owl:Restriction>
                </owl:allValuesFrom>
            </owl:Restriction>
        </rdfs:subClassOf>
        <rdfs:comment>A Task in which two or more Agents exchange information. A CommunicationTask classifies only Events that have only Agents and Social objects as participants.

Of course, the means of exchange is Physical, however this concept is to classify events for which we are not interested in the physical substrate, but rather who communicated and what the information content was.</rdfs:comment>
        <rdfs:isDefinedBy rdf:resource="http://www.ease-crc.org/ont/SOMA-ACT.owl"/>
        <rdfs:label xml:lang="en">Communication task</rdfs:label>
    </owl:Class>
    


    <!-- http://www.ease-crc.org/ont/SOMA.owl#CommunicationTopic -->


    <owl:Class rdf:about="http://www.ease-crc.org/ont/SOMA.owl#CommunicationTopic">
        <rdfs:subClassOf rdf:resource="http://www.ease-crc.org/ont/SOMA.owl#ResourceRole"/>
        <rdfs:subClassOf>
            <owl:Restriction>
                <owl:onProperty rdf:resource="http://www.ontologydesignpatterns.org/ont/dul/DUL.owl#classifies"/>
                <owl:allValuesFrom>
                    <owl:Class>
                        <owl:intersectionOf rdf:parseType="Collection">
                            <rdf:Description rdf:about="http://www.ontologydesignpatterns.org/ont/dul/DUL.owl#SocialObject"/>
                            <owl:Restriction>
                                <owl:onProperty rdf:resource="http://www.ontologydesignpatterns.org/ont/dul/DUL.owl#isParticipantIn"/>
                                <owl:someValuesFrom>
                                    <owl:Restriction>
                                        <owl:onProperty rdf:resource="http://www.ontologydesignpatterns.org/ont/dul/DUL.owl#isClassifiedBy"/>
                                        <owl:someValuesFrom rdf:resource="http://www.ease-crc.org/ont/SOMA.owl#CommunicationTask"/>
                                    </owl:Restriction>
                                </owl:someValuesFrom>
                            </owl:Restriction>
                        </owl:intersectionOf>
                    </owl:Class>
                </owl:allValuesFrom>
            </owl:Restriction>
        </rdfs:subClassOf>
        <rdfs:comment>A role that appears in communication tasks, and indicates what the communication is about.

CommunicationTopic can only classify a Social object that participates in an Action that is classified as (the execution of) a CommunicationTask.

Note that classifies here is used in the plays-role sense. This isn&apos;t to say that the social object, ie the information exchanged in the communication, is an instance of the topic. Rather, the topic role refers to what the information is about.

For example, if the topic of a communication is flowers, this does not mean the words themselves are flowers, merely that, in some sense, they are about flowers.</rdfs:comment>
        <rdfs:isDefinedBy rdf:resource="http://www.ease-crc.org/ont/SOMA-ACT.owl"/>
        <rdfs:label xml:lang="en">Communication topic</rdfs:label>
    </owl:Class>
    


    <!-- http://www.ease-crc.org/ont/SOMA.owl#Compartment -->


    <owl:Class rdf:about="http://www.ease-crc.org/ont/SOMA.owl#Compartment">
        <rdfs:subClassOf rdf:resource="http://www.ease-crc.org/ont/SOMA.owl#DesignedComponent"/>
        <rdfs:isDefinedBy rdf:resource="http://www.ease-crc.org/ont/SOMA-HOME.owl"/>
    </owl:Class>
    


    <!-- http://www.ease-crc.org/ont/SOMA.owl#Composing -->


    <owl:Class rdf:about="http://www.ease-crc.org/ont/SOMA.owl#Composing">
        <rdfs:subClassOf rdf:resource="http://www.ease-crc.org/ont/SOMA.owl#Variability"/>
        <rdfs:subClassOf>
            <owl:Restriction>
                <owl:onProperty rdf:resource="http://www.ease-crc.org/ont/SOMA.owl#affordsTrigger"/>
                <owl:allValuesFrom rdf:resource="http://www.ease-crc.org/ont/SOMA.owl#ConnectedObject"/>
            </owl:Restriction>
        </rdfs:subClassOf>
        <rdfs:comment>The disposition of an object (the tool) to change the compositional structure of others.</rdfs:comment>
        <rdfs:isDefinedBy rdf:resource="http://www.ease-crc.org/ont/SOMA-OBJ.owl"/>
    </owl:Class>
    


    <!-- http://www.ease-crc.org/ont/SOMA.owl#Computer_Language -->


    <owl:Class rdf:about="http://www.ease-crc.org/ont/SOMA.owl#Computer_Language">
        <rdfs:subClassOf rdf:resource="http://www.ease-crc.org/ont/SOMA.owl#FormalLanguage"/>
        <rdfs:comment xml:lang="en">A computer language is a formal language used in communication with a computer.

From Wikipedia: https://en.wikipedia.org/wiki/Computer_language</rdfs:comment>
        <rdfs:isDefinedBy rdf:resource="http://www.ease-crc.org/ont/SOMA-IO.owl"/>
        <rdfs:label xml:lang="en">Computer Language</rdfs:label>
    </owl:Class>
    


    <!-- http://www.ease-crc.org/ont/SOMA.owl#Computer_Program -->


    <owl:Class rdf:about="http://www.ease-crc.org/ont/SOMA.owl#Computer_Program">
        <owl:equivalentClass>
            <owl:Class>
                <owl:intersectionOf rdf:parseType="Collection">
                    <rdf:Description rdf:about="http://www.ease-crc.org/ont/SOMA.owl#Structured_Text"/>
                    <owl:Restriction>
                        <owl:onProperty rdf:resource="http://www.ease-crc.org/ont/SOMA.owl#isGivenMeaningBy"/>
                        <owl:someValuesFrom rdf:resource="http://www.ease-crc.org/ont/SOMA.owl#Programming_Language"/>
                    </owl:Restriction>
                </owl:intersectionOf>
            </owl:Class>
        </owl:equivalentClass>
        <owl:equivalentClass>
            <owl:Class>
                <owl:intersectionOf rdf:parseType="Collection">
                    <rdf:Description rdf:about="http://www.ease-crc.org/ont/SOMA.owl#Structured_Text"/>
                    <owl:Restriction>
                        <owl:onProperty rdf:resource="http://www.ontologydesignpatterns.org/ont/dul/DUL.owl#expresses"/>
                        <owl:someValuesFrom rdf:resource="http://www.ease-crc.org/ont/SOMA.owl#Algorithm"/>
                    </owl:Restriction>
                </owl:intersectionOf>
            </owl:Class>
        </owl:equivalentClass>
        <rdfs:comment xml:lang="en">The Program itself (the specific set of instruction in a Programming Language), not the file that it is contained in nor the implemented algorithm!</rdfs:comment>
        <rdfs:isDefinedBy rdf:resource="http://www.ease-crc.org/ont/SOMA-IO.owl"/>
        <rdfs:label xml:lang="en">Computer program</rdfs:label>
    </owl:Class>
    


    <!-- http://www.ease-crc.org/ont/SOMA.owl#ConditionalSuccedence -->


    <owl:Class rdf:about="http://www.ease-crc.org/ont/SOMA.owl#ConditionalSuccedence">
        <rdfs:subClassOf rdf:resource="http://www.ease-crc.org/ont/SOMA.owl#Succedence"/>
        <rdfs:subClassOf>
            <owl:Restriction>
                <owl:onProperty rdf:resource="http://www.ease-crc.org/ont/SOMA.owl#hasBinding"/>
                <owl:allValuesFrom rdf:resource="http://www.ease-crc.org/ont/SOMA.owl#CounterfactualBinding"/>
            </owl:Restriction>
        </rdfs:subClassOf>
        <rdfs:comment>A relation that holds between two OGPTasks that belong to the same OGPWorkflow, and which means that, if a condition is met, the successor task invocation is to be executed after the predecessor task invocation completes.

The condition is a conjunction of CounterfactualBindings. These bindings may be RoleRoleBindings (meaning, test whether the fillers for these Roles/Parameters are the same) or RoleFillerBindings (meaning, test whether the filler of the Role unifies with the candidate Entity).

An empty conjunction of CounterfactualBindings is assumed to be True.</rdfs:comment>
        <rdfs:comment>Note: in RobotWorkflows, Tasks typically may have several possible successors, to be selected based on condition-testing.</rdfs:comment>
        <rdfs:isDefinedBy rdf:resource="http://www.ease-crc.org/ont/SOMA-WF.owl"/>
        <rdfs:label xml:lang="en">Conditional succedence</rdfs:label>
    </owl:Class>
    


    <!-- http://www.ease-crc.org/ont/SOMA.owl#Configuration -->


    <owl:Class rdf:about="http://www.ease-crc.org/ont/SOMA.owl#Configuration">
        <rdfs:subClassOf rdf:resource="http://www.ontologydesignpatterns.org/ont/dul/DUL.owl#Description"/>
        <rdfs:subClassOf>
            <owl:Restriction>
                <owl:onProperty rdf:resource="http://www.ontologydesignpatterns.org/ont/dul/DUL.owl#describes"/>
                <owl:someValuesFrom rdf:resource="http://www.ease-crc.org/ont/SOMA.owl#StateType"/>
            </owl:Restriction>
        </rdfs:subClassOf>
        <rdfs:comment>A description of a State. This includes e.g. what acceptable regions for participant objects of the State might look like.
A configuration of the world is construed to be stable on its own. Outside disturbances may cause state transitions, and the settling into some other, self-stable configuration.

Several other Description subclasses may function as Configurations. For example, a Goal is a description of a desired State. A Norm describes a State that should be maintained. A Diagnosis describes a State that causes certain symptoms etc.

Note a couple of issues here. First one relates to what &quot;configuration&quot; means; in particular, this doesn&apos;t mean a configuration that is unchanging according to any viewpoint. The analogy here is the &quot;macrostate&quot; from thermodynamics: a macrostate with two gases mixed does not mean all gas particles are motionless, but rather that the locations and movements of gas particles are such that any particle is likely to have as many neighbors of one type as the other.

The second issue relates to what is &quot;outside&quot;. The state is a configuration of some, but not necessarily all, Entities in the world. Entities not in this configuration are outside of it.</rdfs:comment>
        <rdfs:isDefinedBy rdf:resource="http://www.ease-crc.org/ont/SOMA-STATE.owl"/>
    </owl:Class>
    


    <!-- http://www.ease-crc.org/ont/SOMA.owl#ConnectedObject -->


    <owl:Class rdf:about="http://www.ease-crc.org/ont/SOMA.owl#ConnectedObject">
        <rdfs:subClassOf rdf:resource="http://www.ease-crc.org/ont/SOMA.owl#Patient"/>
        <rdfs:comment>An object that is combined with another object.</rdfs:comment>
        <rdfs:isDefinedBy rdf:resource="http://www.ease-crc.org/ont/SOMA-OBJ.owl"/>
        <rdfs:isDefinedBy rdf:resource="http://www.ease-crc.org/ont/SOMA-STATE.owl"/>
        <rdfs:label xml:lang="en">Connected object</rdfs:label>
    </owl:Class>
    


    <!-- http://www.ease-crc.org/ont/SOMA.owl#Connectivity -->


    <owl:Class rdf:about="http://www.ease-crc.org/ont/SOMA.owl#Connectivity">
        <rdfs:subClassOf rdf:resource="http://www.ease-crc.org/ont/SOMA.owl#Disposition"/>
        <rdfs:subClassOf>
            <owl:Restriction>
                <owl:onProperty rdf:resource="http://www.ease-crc.org/ont/SOMA.owl#affordsBearer"/>
                <owl:allValuesFrom rdf:resource="http://www.ease-crc.org/ont/SOMA.owl#ConnectedObject"/>
            </owl:Restriction>
        </rdfs:subClassOf>
        <rdfs:subClassOf>
            <owl:Restriction>
                <owl:onProperty rdf:resource="http://www.ease-crc.org/ont/SOMA.owl#affordsTrigger"/>
                <owl:allValuesFrom rdf:resource="http://www.ease-crc.org/ont/SOMA.owl#ConnectedObject"/>
            </owl:Restriction>
        </rdfs:subClassOf>
        <rdfs:comment>The disposition of an object (the connected object) to establish a connection with others.</rdfs:comment>
        <rdfs:isDefinedBy rdf:resource="http://www.ease-crc.org/ont/SOMA-OBJ.owl"/>
    </owl:Class>
    


    <!-- http://www.ease-crc.org/ont/SOMA.owl#Constructing -->


    <owl:Class rdf:about="http://www.ease-crc.org/ont/SOMA.owl#Constructing">
        <rdfs:subClassOf rdf:resource="http://www.ease-crc.org/ont/SOMA.owl#PhysicalTask"/>
        <owl:disjointWith rdf:resource="http://www.ease-crc.org/ont/SOMA.owl#ModifyingPhysicalObject"/>
        <rdfs:comment>A task in which an Agent creates a new object.</rdfs:comment>
        <rdfs:isDefinedBy rdf:resource="http://www.ease-crc.org/ont/SOMA-ACT.owl"/>
    </owl:Class>
    


    <!-- http://www.ease-crc.org/ont/SOMA.owl#ContactState -->


    <owl:Class rdf:about="http://www.ease-crc.org/ont/SOMA.owl#ContactState">
        <rdfs:subClassOf rdf:resource="http://www.ease-crc.org/ont/SOMA.owl#StateType"/>
        <rdfs:subClassOf>
            <owl:Restriction>
                <owl:onProperty rdf:resource="http://www.ontologydesignpatterns.org/ont/dul/DUL.owl#classifies"/>
                <owl:allValuesFrom>
                    <owl:Restriction>
                        <owl:onProperty rdf:resource="http://www.ontologydesignpatterns.org/ont/dul/DUL.owl#hasParticipant"/>
                        <owl:minQualifiedCardinality rdf:datatype="http://www.w3.org/2001/XMLSchema#nonNegativeInteger">2</owl:minQualifiedCardinality>
                        <owl:onClass rdf:resource="http://www.ontologydesignpatterns.org/ont/dul/DUL.owl#PhysicalObject"/>
                    </owl:Restriction>
                </owl:allValuesFrom>
            </owl:Restriction>
        </rdfs:subClassOf>
        <rdfs:comment>Classifies States in which some objects are in contact.</rdfs:comment>
        <rdfs:isDefinedBy rdf:resource="http://www.ease-crc.org/ont/SOMA-STATE.owl"/>
        <rdfs:label xml:lang="en">Contact state</rdfs:label>
    </owl:Class>
    


    <!-- http://www.ease-crc.org/ont/SOMA.owl#Container -->


    <owl:Class rdf:about="http://www.ease-crc.org/ont/SOMA.owl#Container">
        <rdfs:subClassOf rdf:resource="http://www.ease-crc.org/ont/SOMA.owl#Restrictor"/>
        <rdfs:comment>A role classifying an object used to contain others.</rdfs:comment>
        <rdfs:isDefinedBy rdf:resource="http://www.ease-crc.org/ont/SOMA-OBJ.owl"/>
        <rdfs:isDefinedBy rdf:resource="http://www.ease-crc.org/ont/SOMA-STATE.owl"/>
    </owl:Class>
    


    <!-- http://www.ease-crc.org/ont/SOMA.owl#Containment -->


    <owl:Class rdf:about="http://www.ease-crc.org/ont/SOMA.owl#Containment">
        <rdfs:subClassOf rdf:resource="http://www.ease-crc.org/ont/SOMA.owl#Disposition"/>
        <rdfs:subClassOf>
            <owl:Restriction>
                <owl:onProperty rdf:resource="http://www.ease-crc.org/ont/SOMA.owl#affordsBearer"/>
                <owl:allValuesFrom rdf:resource="http://www.ease-crc.org/ont/SOMA.owl#Container"/>
            </owl:Restriction>
        </rdfs:subClassOf>
        <rdfs:subClassOf>
            <owl:Restriction>
                <owl:onProperty rdf:resource="http://www.ease-crc.org/ont/SOMA.owl#affordsTrigger"/>
                <owl:allValuesFrom rdf:resource="http://www.ease-crc.org/ont/SOMA.owl#IncludedObject"/>
            </owl:Restriction>
        </rdfs:subClassOf>
        <rdfs:subClassOf>
            <owl:Restriction>
                <owl:onProperty rdf:resource="http://www.ease-crc.org/ont/SOMA.owl#isDispositionOf"/>
                <owl:allValuesFrom>
                    <owl:Restriction>
                        <owl:onProperty rdf:resource="http://www.ontologydesignpatterns.org/ont/dul/DUL.owl#hasQuality"/>
                        <owl:someValuesFrom rdf:resource="http://www.ease-crc.org/ont/SOMA.owl#Capacity"/>
                    </owl:Restriction>
                </owl:allValuesFrom>
            </owl:Restriction>
        </rdfs:subClassOf>
        <rdfs:comment>Classifies States in which an object is placed inside another.</rdfs:comment>
        <rdfs:comment>The disposition of an object (the container) to contain others.</rdfs:comment>
        <rdfs:isDefinedBy rdf:resource="http://www.ease-crc.org/ont/SOMA-HOME.owl"/>
        <rdfs:isDefinedBy rdf:resource="http://www.ease-crc.org/ont/SOMA-OBJ.owl"/>
        <rdfs:isDefinedBy rdf:resource="http://www.ease-crc.org/ont/SOMA-STATE.owl"/>
    </owl:Class>
    


    <!-- http://www.ease-crc.org/ont/SOMA.owl#ContainmentTheory -->


    <owl:Class rdf:about="http://www.ease-crc.org/ont/SOMA.owl#ContainmentTheory">
        <rdfs:subClassOf rdf:resource="http://www.ease-crc.org/ont/SOMA.owl#ControlTheory"/>
        <rdfs:comment>A schematic theory that describes a functional relation which ensures that the location of some entity, the locatum, is constrained to be within some region which is the interior of some other entity, the relatum.

This is also known as FunctionalControlInternal in GUM-4-space (Bateman et al. 2010).

Let xL, xR be objects filling the locatum, relatum roles of this schema. Then one can infer that xL isInsideOf xR.</rdfs:comment>
        <rdfs:isDefinedBy rdf:resource="http://www.ease-crc.org/ont/SOMA-SAY.owl"/>
        <rdfs:label xml:lang="en">Containment theory</rdfs:label>
    </owl:Class>
    


    <!-- http://www.ease-crc.org/ont/SOMA.owl#ControlTheory -->


    <owl:Class rdf:about="http://www.ease-crc.org/ont/SOMA.owl#ControlTheory">
        <rdfs:subClassOf rdf:resource="http://www.ease-crc.org/ont/SOMA.owl#FunctionalSpatialSchemaTheory"/>
        <rdfs:comment>A description of functional-spatial configurations where one object controls another object&apos;s position in space, e.g. if a pot moves, then the popcorn contained therein moves, as well. Note that the objects do not need to be in direct contact.

Adopted from GUM-4-space (Bateman et al. 2010).</rdfs:comment>
        <rdfs:isDefinedBy rdf:resource="http://www.ease-crc.org/ont/SOMA-SAY.owl"/>
        <rdfs:label xml:lang="en">Control theory</rdfs:label>
    </owl:Class>
    


    <!-- http://www.ease-crc.org/ont/SOMA.owl#CounterfactualBinding -->


    <owl:Class rdf:about="http://www.ease-crc.org/ont/SOMA.owl#CounterfactualBinding">
        <rdfs:subClassOf rdf:resource="http://www.ease-crc.org/ont/SOMA.owl#Binding"/>
        <owl:disjointWith rdf:resource="http://www.ease-crc.org/ont/SOMA.owl#FactualBinding"/>
        <rdfs:comment>CounterfactualBindings are used to express conditions:

-- that two roles share a filler (RoleRoleBindings);
-- that the filler of a role is a particular entity (RoleFillerBindings). This is typically the case when the filler of the role may be one of a few constants, as is the case with the execution status of a robot task.

TODO: for the robot workflows we are likely to need at the start, testing equality of fillers is enough. In the future, we may want to replace that with unifiability of fillers.</rdfs:comment>
        <rdfs:isDefinedBy rdf:resource="http://www.ease-crc.org/ont/SOMA-WF.owl"/>
        <rdfs:label xml:lang="en">Counterfactual binding</rdfs:label>
    </owl:Class>
    


    <!-- http://www.ease-crc.org/ont/SOMA.owl#Countertop -->


    <owl:Class rdf:about="http://www.ease-crc.org/ont/SOMA.owl#Countertop">
        <rdfs:subClassOf rdf:resource="http://www.ease-crc.org/ont/SOMA.owl#DesignedComponent"/>
        <rdfs:comment>A flat surface for working on.</rdfs:comment>
        <rdfs:isDefinedBy rdf:resource="http://www.ease-crc.org/ont/SOMA-HOME.owl"/>
    </owl:Class>
    


    <!-- http://www.ease-crc.org/ont/SOMA.owl#Cover -->


    <owl:Class rdf:about="http://www.ease-crc.org/ont/SOMA.owl#Cover">
        <rdfs:subClassOf rdf:resource="http://www.ease-crc.org/ont/SOMA.owl#Barrier"/>
        <rdfs:comment>An object used to cover up others, such as a lid used as a cover for a pot.</rdfs:comment>
        <rdfs:isDefinedBy rdf:resource="http://www.ease-crc.org/ont/SOMA-OBJ.owl"/>
    </owl:Class>
    


    <!-- http://www.ease-crc.org/ont/SOMA.owl#Coverage -->


    <owl:Class rdf:about="http://www.ease-crc.org/ont/SOMA.owl#Coverage">
        <rdfs:subClassOf rdf:resource="http://www.ease-crc.org/ont/SOMA.owl#Blockage"/>
        <rdfs:subClassOf>
            <owl:Restriction>
                <owl:onProperty rdf:resource="http://www.ease-crc.org/ont/SOMA.owl#affordsBearer"/>
                <owl:allValuesFrom rdf:resource="http://www.ease-crc.org/ont/SOMA.owl#Cover"/>
            </owl:Restriction>
        </rdfs:subClassOf>
        <rdfs:subClassOf>
            <owl:Restriction>
                <owl:onProperty rdf:resource="http://www.ease-crc.org/ont/SOMA.owl#affordsTrigger"/>
                <owl:allValuesFrom rdf:resource="http://www.ease-crc.org/ont/SOMA.owl#CoveredObject"/>
            </owl:Restriction>
        </rdfs:subClassOf>
        <rdfs:comment>The disposition of an object (the cover) to hide or to protect objects by covering them. An example is a door that covers items in a container to e.g. prevent dust getting inside of the container.</rdfs:comment>
        <rdfs:isDefinedBy rdf:resource="http://www.ease-crc.org/ont/SOMA-OBJ.owl"/>
    </owl:Class>
    


    <!-- http://www.ease-crc.org/ont/SOMA.owl#CoverageTheory -->


    <owl:Class rdf:about="http://www.ease-crc.org/ont/SOMA.owl#CoverageTheory">
        <rdfs:subClassOf rdf:resource="http://www.ease-crc.org/ont/SOMA.owl#FunctionalSpatialSchemaTheory"/>
        <rdfs:comment>A schematic theory of a functional relation between two objects such that one of them, the locatum, blocks access to the interior of the relatum.

Let xL, xR be objects filling the locatum, relatum roles of this schema. Then one can infer that xL coversObject xR.</rdfs:comment>
        <rdfs:isDefinedBy rdf:resource="http://www.ease-crc.org/ont/SOMA-SAY.owl"/>
    </owl:Class>
    


    <!-- http://www.ease-crc.org/ont/SOMA.owl#CoveredObject -->


    <owl:Class rdf:about="http://www.ease-crc.org/ont/SOMA.owl#CoveredObject">
        <rdfs:subClassOf rdf:resource="http://www.ease-crc.org/ont/SOMA.owl#BlockedObject"/>
        <rdfs:comment>An object that is covered.</rdfs:comment>
        <rdfs:isDefinedBy rdf:resource="http://www.ease-crc.org/ont/SOMA-OBJ.owl"/>
        <rdfs:label xml:lang="en">Covered object</rdfs:label>
    </owl:Class>
    


    <!-- http://www.ease-crc.org/ont/SOMA.owl#CoveringTheory -->


    <owl:Class rdf:about="http://www.ease-crc.org/ont/SOMA.owl#CoveringTheory">
        <rdfs:subClassOf rdf:resource="http://www.ease-crc.org/ont/SOMA.owl#ExecutableSchematicTheory"/>
        <rdfs:subClassOf>
            <owl:Restriction>
                <owl:onProperty rdf:resource="http://www.ontologydesignpatterns.org/ont/dul/DUL.owl#defines"/>
                <owl:someValuesFrom rdf:resource="http://www.ease-crc.org/ont/SOMA.owl#Instrument"/>
            </owl:Restriction>
        </rdfs:subClassOf>
        <rdfs:subClassOf>
            <owl:Restriction>
                <owl:onProperty rdf:resource="http://www.ontologydesignpatterns.org/ont/dul/DUL.owl#defines"/>
                <owl:qualifiedCardinality rdf:datatype="http://www.w3.org/2001/XMLSchema#nonNegativeInteger">1</owl:qualifiedCardinality>
                <owl:onClass rdf:resource="http://www.ease-crc.org/ont/SOMA.owl#Patient"/>
            </owl:Restriction>
        </rdfs:subClassOf>
        <rdfs:comment>A schematic theory of how an agent can use an instrument to prevent access to the interior of a patient.</rdfs:comment>
        <rdfs:isDefinedBy rdf:resource="http://www.ease-crc.org/ont/SOMA-SAY.owl"/>
        <rdfs:label xml:lang="en">Covering theory</rdfs:label>
    </owl:Class>
    


    <!-- http://www.ease-crc.org/ont/SOMA.owl#CrackingTheory -->


    <owl:Class rdf:about="http://www.ease-crc.org/ont/SOMA.owl#CrackingTheory">
        <rdfs:subClassOf rdf:resource="http://www.ease-crc.org/ont/SOMA.owl#ExecutableSchematicTheory"/>
        <rdfs:subClassOf>
            <owl:Restriction>
                <owl:onProperty rdf:resource="http://www.ontologydesignpatterns.org/ont/dul/DUL.owl#defines"/>
                <owl:someValuesFrom rdf:resource="http://www.ease-crc.org/ont/SOMA.owl#Instrument"/>
            </owl:Restriction>
        </rdfs:subClassOf>
        <rdfs:subClassOf>
            <owl:Restriction>
                <owl:onProperty rdf:resource="http://www.ontologydesignpatterns.org/ont/dul/DUL.owl#defines"/>
                <owl:someValuesFrom rdf:resource="http://www.ease-crc.org/ont/SOMA.owl#Patient"/>
            </owl:Restriction>
        </rdfs:subClassOf>
        <rdfs:comment>A schematic theory of how an agent can inflict damage to the surface of an object.</rdfs:comment>
        <rdfs:isDefinedBy rdf:resource="http://www.ease-crc.org/ont/SOMA-SAY.owl"/>
        <rdfs:label xml:lang="en">Cracking theory</rdfs:label>
    </owl:Class>
    


    <!-- http://www.ease-crc.org/ont/SOMA.owl#CreatedObject -->


    <owl:Class rdf:about="http://www.ease-crc.org/ont/SOMA.owl#CreatedObject">
        <rdfs:subClassOf rdf:resource="http://www.ease-crc.org/ont/SOMA.owl#Patient"/>
        <rdfs:comment>An object that is created.</rdfs:comment>
        <rdfs:isDefinedBy rdf:resource="http://www.ease-crc.org/ont/SOMA-OBJ.owl"/>
        <rdfs:isDefinedBy rdf:resource="http://www.ease-crc.org/ont/SOMA-PROC.owl"/>
        <rdfs:label xml:lang="en">Created object</rdfs:label>
    </owl:Class>
    


    <!-- http://www.ease-crc.org/ont/SOMA.owl#Creation -->


    <owl:Class rdf:about="http://www.ease-crc.org/ont/SOMA.owl#Creation">
        <rdfs:subClassOf rdf:resource="http://www.ease-crc.org/ont/SOMA.owl#ProcessType"/>
        <rdfs:subClassOf>
            <owl:Restriction>
                <owl:onProperty rdf:resource="http://www.ease-crc.org/ont/SOMA.owl#isProcessTypeOf"/>
                <owl:someValuesFrom rdf:resource="http://www.ease-crc.org/ont/SOMA.owl#CreatedObject"/>
            </owl:Restriction>
        </rdfs:subClassOf>
        <rdfs:comment>A process by which an Entity is created in the physical world.

Note, most of the physical Entities we will be considering here are in fact arrangements of many other, smaller physical Entities. Therefore another way to look at this is, a &apos;Physical creation&apos; is the process by which a set of physical Entities is arranged in a certain way, and the arrangement is then itself considered a physical Entity.</rdfs:comment>
        <rdfs:isDefinedBy rdf:resource="http://www.ease-crc.org/ont/SOMA-PROC.owl"/>
        <rdfs:label>Creation</rdfs:label>
    </owl:Class>
    


    <!-- http://www.ease-crc.org/ont/SOMA.owl#Crockery -->


    <owl:Class rdf:about="http://www.ease-crc.org/ont/SOMA.owl#Crockery">
        <rdfs:subClassOf rdf:resource="http://www.ease-crc.org/ont/SOMA.owl#DesignedContainer"/>
        <rdfs:subClassOf rdf:resource="http://www.ease-crc.org/ont/SOMA.owl#Tableware"/>
        <rdfs:subClassOf>
            <owl:Restriction>
                <owl:onProperty rdf:resource="http://www.ease-crc.org/ont/SOMA.owl#hasDisposition"/>
                <owl:qualifiedCardinality rdf:datatype="http://www.w3.org/2001/XMLSchema#nonNegativeInteger">1</owl:qualifiedCardinality>
                <owl:onClass rdf:resource="http://www.ease-crc.org/ont/SOMA.owl#Insertion"/>
            </owl:Restriction>
        </rdfs:subClassOf>
        <rdfs:subClassOf>
            <owl:Restriction>
                <owl:onProperty rdf:resource="http://www.ease-crc.org/ont/SOMA.owl#hasDisposition"/>
                <owl:qualifiedCardinality rdf:datatype="http://www.w3.org/2001/XMLSchema#nonNegativeInteger">1</owl:qualifiedCardinality>
                <owl:onClass>
                    <owl:Class>
                        <owl:intersectionOf rdf:parseType="Collection">
                            <rdf:Description rdf:about="http://www.ease-crc.org/ont/SOMA.owl#Insertion"/>
                            <owl:Restriction>
                                <owl:onProperty rdf:resource="http://www.ease-crc.org/ont/SOMA.owl#affordsTrigger"/>
                                <owl:allValuesFrom>
                                    <owl:Restriction>
                                        <owl:onProperty rdf:resource="http://www.ontologydesignpatterns.org/ont/dul/DUL.owl#classifies"/>
                                        <owl:allValuesFrom rdf:resource="http://www.ontologydesignpatterns.org/ont/dul/DUL.owl#Substance"/>
                                    </owl:Restriction>
                                </owl:allValuesFrom>
                            </owl:Restriction>
                        </owl:intersectionOf>
                    </owl:Class>
                </owl:onClass>
            </owl:Restriction>
        </rdfs:subClassOf>
        <rdfs:comment>An object designed to contain food to store, cook, eat, or serve it.</rdfs:comment>
        <rdfs:isDefinedBy rdf:resource="http://www.ease-crc.org/ont/SOMA-HOME.owl"/>
    </owl:Class>
    


    <!-- http://www.ease-crc.org/ont/SOMA.owl#Cupboard -->


    <owl:Class rdf:about="http://www.ease-crc.org/ont/SOMA.owl#Cupboard">
        <rdfs:subClassOf rdf:resource="http://www.ease-crc.org/ont/SOMA.owl#DesignedContainer"/>
        <rdfs:subClassOf rdf:resource="http://www.ease-crc.org/ont/SOMA.owl#DesignedFurniture"/>
        <rdfs:subClassOf>
            <owl:Restriction>
                <owl:onProperty rdf:resource="http://www.ease-crc.org/ont/SOMA.owl#hasPhysicalComponent"/>
                <owl:someValuesFrom rdf:resource="http://www.ease-crc.org/ont/SOMA.owl#Rack"/>
            </owl:Restriction>
        </rdfs:subClassOf>
        <rdfs:comment>A piece of furniture for storing things.</rdfs:comment>
        <rdfs:isDefinedBy rdf:resource="http://www.ease-crc.org/ont/SOMA-HOME.owl"/>
    </owl:Class>
    


    <!-- http://www.ease-crc.org/ont/SOMA.owl#Cutlery -->


    <owl:Class rdf:about="http://www.ease-crc.org/ont/SOMA.owl#Cutlery">
        <rdfs:subClassOf rdf:resource="http://www.ease-crc.org/ont/SOMA.owl#Tableware"/>
        <rdfs:isDefinedBy rdf:resource="http://www.ease-crc.org/ont/SOMA-HOME.owl"/>
    </owl:Class>
    


    <!-- http://www.ease-crc.org/ont/SOMA.owl#Cutting -->


    <owl:Class rdf:about="http://www.ease-crc.org/ont/SOMA.owl#Cutting">
        <rdfs:subClassOf rdf:resource="http://www.ease-crc.org/ont/SOMA.owl#ModifyingPhysicalObject"/>
        <rdfs:comment>The goal of this task is to separate one or more pieces from some target object by means of cutting into its constituent material. Unlike a disassembly, a cut is usually not easily reversible.</rdfs:comment>
        <rdfs:isDefinedBy rdf:resource="http://www.ease-crc.org/ont/SOMA-ACT.owl"/>
    </owl:Class>
    


    <!-- http://www.ease-crc.org/ont/SOMA.owl#CuttingTool -->


    <owl:Class rdf:about="http://www.ease-crc.org/ont/SOMA.owl#CuttingTool">
        <rdfs:subClassOf rdf:resource="http://www.ease-crc.org/ont/SOMA.owl#DesignedTool"/>
        <rdfs:subClassOf>
            <owl:Restriction>
                <owl:onProperty rdf:resource="http://www.ease-crc.org/ont/SOMA.owl#hasDisposition"/>
                <owl:someValuesFrom rdf:resource="http://www.ease-crc.org/ont/SOMA.owl#Shaping"/>
            </owl:Restriction>
        </rdfs:subClassOf>
        <rdfs:isDefinedBy rdf:resource="http://www.ease-crc.org/ont/SOMA-HOME.owl"/>
    </owl:Class>
    


    <!-- http://www.ease-crc.org/ont/SOMA.owl#CylinderShape -->


    <owl:Class rdf:about="http://www.ease-crc.org/ont/SOMA.owl#CylinderShape">
        <rdfs:subClassOf rdf:resource="http://www.ease-crc.org/ont/SOMA.owl#ShapeRegion"/>
        <rdfs:subClassOf>
            <owl:Restriction>
                <owl:onProperty rdf:resource="http://www.ease-crc.org/ont/SOMA.owl#hasRadius"/>
                <owl:someValuesFrom rdf:resource="http://www.w3.org/2001/XMLSchema#float"/>
            </owl:Restriction>
        </rdfs:subClassOf>
        <rdfs:subClassOf>
            <owl:Restriction>
                <owl:onProperty rdf:resource="http://www.ease-crc.org/ont/SOMA.owl#hasLength"/>
                <owl:qualifiedCardinality rdf:datatype="http://www.w3.org/2001/XMLSchema#nonNegativeInteger">1</owl:qualifiedCardinality>
                <owl:onDataRange rdf:resource="http://www.w3.org/2001/XMLSchema#float"/>
            </owl:Restriction>
        </rdfs:subClassOf>
        <rdfs:comment>A solid geometrical figure with straight parallel sides and a circular or oval cross section.</rdfs:comment>
        <rdfs:isDefinedBy rdf:resource="http://www.ease-crc.org/ont/SOMA-OBJ.owl"/>
        <rdfs:label>Cylinder shape</rdfs:label>
    </owl:Class>
    


    <!-- http://www.ease-crc.org/ont/SOMA.owl#Database -->


    <owl:Class rdf:about="http://www.ease-crc.org/ont/SOMA.owl#Database">
        <rdfs:subClassOf rdf:resource="http://www.ease-crc.org/ont/SOMA.owl#SoftwareRole"/>
        <rdfs:comment xml:lang="en">A Database is a Software that organizes a collection of data stored and and allows for access, usually via some query engine.

Source: https://en.wikipedia.org/wiki/Database</rdfs:comment>
        <rdfs:isDefinedBy rdf:resource="http://www.ease-crc.org/ont/SOMA-IO.owl"/>
    </owl:Class>
    


    <!-- http://www.ease-crc.org/ont/SOMA.owl#DeclarativeClause -->


    <owl:Class rdf:about="http://www.ease-crc.org/ont/SOMA.owl#DeclarativeClause">
        <rdfs:subClassOf rdf:resource="http://www.ease-crc.org/ont/SOMA.owl#ClausalObject"/>
        <rdfs:comment>A clause which makes an assertion or declaration.</rdfs:comment>
        <rdfs:isDefinedBy rdf:resource="http://www.ease-crc.org/ont/SOMA-SAY.owl"/>
        <rdfs:label>Declarative clause</rdfs:label>
    </owl:Class>
    


    <!-- http://www.ease-crc.org/ont/SOMA.owl#DeductiveReasoning -->


    <owl:Class rdf:about="http://www.ease-crc.org/ont/SOMA.owl#DeductiveReasoning">
        <rdfs:subClassOf rdf:resource="http://www.ease-crc.org/ont/SOMA.owl#Reasoning"/>
        <rdfs:comment>A task in which the Agent, using general logical principles that it considers logically valid, applied to premises that it considers logically true, arrives at conclusions that it considers logically certain.

Deduction is often explained as starting from the &quot;general&quot; (some property X is known about all members of a set S), applying it to the &quot;specific&quot; (some Entity Y is known to belong to set S), to arrive at a specialization of the general property (X applies to Y).</rdfs:comment>
        <rdfs:isDefinedBy rdf:resource="http://www.ease-crc.org/ont/SOMA-ACT.owl"/>
        <rdfs:label xml:lang="en">Deductive reasoning</rdfs:label>
    </owl:Class>
    


    <!-- http://www.ease-crc.org/ont/SOMA.owl#Deformation -->


    <owl:Class rdf:about="http://www.ease-crc.org/ont/SOMA.owl#Deformation">
        <rdfs:subClassOf rdf:resource="http://www.ease-crc.org/ont/SOMA.owl#Alteration"/>
        <rdfs:subClassOf>
            <owl:Restriction>
                <owl:onProperty rdf:resource="http://www.ease-crc.org/ont/SOMA.owl#isProcessTypeOf"/>
                <owl:qualifiedCardinality rdf:datatype="http://www.w3.org/2001/XMLSchema#nonNegativeInteger">1</owl:qualifiedCardinality>
                <owl:onClass rdf:resource="http://www.ease-crc.org/ont/SOMA.owl#ShapedObject"/>
            </owl:Restriction>
        </rdfs:subClassOf>
        <owl:disjointWith rdf:resource="http://www.ease-crc.org/ont/SOMA.owl#FluidFlow"/>
        <rdfs:comment>A process by which a physical Entity changes its shape under the influence of some factors outside of the Entity.

Note, changes of shape may be self-caused; for example, a gas will naturally disperse. This however would be a different type of process (Dispersion).

A soft slab of clay deforming under its own weight on Earth would still count as deformation: it is the gravity of the Earth (so, a factor outside the slab of clay) which makes the slab change shape.</rdfs:comment>
        <rdfs:isDefinedBy rdf:resource="http://www.ease-crc.org/ont/SOMA-PROC.owl"/>
    </owl:Class>
    


    <!-- http://www.ease-crc.org/ont/SOMA.owl#Delivering -->


    <owl:Class rdf:about="http://www.ease-crc.org/ont/SOMA.owl#Delivering">
        <rdfs:subClassOf rdf:resource="http://www.ease-crc.org/ont/SOMA.owl#Actuating"/>
        <owl:disjointWith rdf:resource="http://www.ease-crc.org/ont/SOMA.owl#Fetching"/>
        <owl:disjointWith rdf:resource="http://www.ease-crc.org/ont/SOMA.owl#Lifting"/>
        <owl:disjointWith rdf:resource="http://www.ease-crc.org/ont/SOMA.owl#Opening"/>
        <owl:disjointWith rdf:resource="http://www.ease-crc.org/ont/SOMA.owl#Pulling"/>
        <owl:disjointWith rdf:resource="http://www.ease-crc.org/ont/SOMA.owl#Pushing"/>
        <owl:disjointWith rdf:resource="http://www.ease-crc.org/ont/SOMA.owl#Squeezing"/>
        <rdfs:comment>A task in which an Agent brings an item that the Agent already carries to a specified target.</rdfs:comment>
        <rdfs:isDefinedBy rdf:resource="http://www.ease-crc.org/ont/SOMA-ACT.owl"/>
    </owl:Class>
    


    <!-- http://www.ease-crc.org/ont/SOMA.owl#DependentPlace -->


    <owl:Class rdf:about="http://www.ease-crc.org/ont/SOMA.owl#DependentPlace">
        <rdfs:subClassOf rdf:resource="http://www.ease-crc.org/ont/SOMA.owl#Feature"/>
        <rdfs:comment>A feature that is not part of its host, like a hole in a piece of cheese.</rdfs:comment>
        <rdfs:isDefinedBy rdf:resource="http://www.ease-crc.org/ont/SOMA-OBJ.owl"/>
        <rdfs:label xml:lang="en">Dependent place</rdfs:label>
    </owl:Class>
    


    <!-- http://www.ease-crc.org/ont/SOMA.owl#Deposit -->


    <owl:Class rdf:about="http://www.ease-crc.org/ont/SOMA.owl#Deposit">
        <rdfs:subClassOf rdf:resource="http://www.ease-crc.org/ont/SOMA.owl#Instrument"/>
        <rdfs:comment>A role classifying an object ontop which others are put to e.g. store them, or to place them in a meaningful way for future activities.</rdfs:comment>
        <rdfs:isDefinedBy rdf:resource="http://www.ease-crc.org/ont/SOMA-OBJ.owl"/>
    </owl:Class>
    


    <!-- http://www.ease-crc.org/ont/SOMA.owl#DepositedObject -->


    <owl:Class rdf:about="http://www.ease-crc.org/ont/SOMA.owl#DepositedObject">
        <rdfs:subClassOf rdf:resource="http://www.ease-crc.org/ont/SOMA.owl#Patient"/>
        <rdfs:comment>An object placed ontop of another one.</rdfs:comment>
        <rdfs:isDefinedBy rdf:resource="http://www.ease-crc.org/ont/SOMA-OBJ.owl"/>
        <rdfs:label xml:lang="en">Deposited object</rdfs:label>
    </owl:Class>
    


    <!-- http://www.ease-crc.org/ont/SOMA.owl#Deposition -->


    <owl:Class rdf:about="http://www.ease-crc.org/ont/SOMA.owl#Deposition">
        <rdfs:subClassOf rdf:resource="http://www.ease-crc.org/ont/SOMA.owl#Disposition"/>
        <rdfs:subClassOf>
            <owl:Restriction>
                <owl:onProperty rdf:resource="http://www.ease-crc.org/ont/SOMA.owl#affordsBearer"/>
                <owl:allValuesFrom rdf:resource="http://www.ease-crc.org/ont/SOMA.owl#Deposit"/>
            </owl:Restriction>
        </rdfs:subClassOf>
        <rdfs:subClassOf>
            <owl:Restriction>
                <owl:onProperty rdf:resource="http://www.ease-crc.org/ont/SOMA.owl#affordsTrigger"/>
                <owl:allValuesFrom rdf:resource="http://www.ease-crc.org/ont/SOMA.owl#DepositedObject"/>
            </owl:Restriction>
        </rdfs:subClassOf>
        <rdfs:comment>The disposition to support objects.</rdfs:comment>
        <rdfs:isDefinedBy rdf:resource="http://www.ease-crc.org/ont/SOMA-OBJ.owl"/>
    </owl:Class>
    


    <!-- http://www.ease-crc.org/ont/SOMA.owl#DesignedComponent -->


    <owl:Class rdf:about="http://www.ease-crc.org/ont/SOMA.owl#DesignedComponent">
        <rdfs:subClassOf rdf:resource="http://www.ease-crc.org/ont/SOMA.owl#FunctionalPart"/>
        <rdfs:subClassOf rdf:resource="http://www.ontologydesignpatterns.org/ont/dul/DUL.owl#DesignedArtifact"/>
        <rdfs:subClassOf>
            <owl:Restriction>
                <owl:onProperty rdf:resource="http://www.ease-crc.org/ont/SOMA.owl#hasDisposition"/>
                <owl:someValuesFrom rdf:resource="http://www.ease-crc.org/ont/SOMA.owl#Connectivity"/>
            </owl:Restriction>
        </rdfs:subClassOf>
        <rdfs:comment>An object designed to be part or element of a larger whole.</rdfs:comment>
        <rdfs:isDefinedBy rdf:resource="http://www.ease-crc.org/ont/SOMA-HOME.owl"/>
        <rdfs:isDefinedBy rdf:resource="http://www.ease-crc.org/ont/SOMA-OBJ.owl"/>
        <rdfs:label>Designed component</rdfs:label>
    </owl:Class>
    


    <!-- http://www.ease-crc.org/ont/SOMA.owl#DesignedContainer -->


    <owl:Class rdf:about="http://www.ease-crc.org/ont/SOMA.owl#DesignedContainer">
        <rdfs:subClassOf rdf:resource="http://www.ontologydesignpatterns.org/ont/dul/DUL.owl#DesignedArtifact"/>
        <rdfs:subClassOf>
            <owl:Restriction>
                <owl:onProperty rdf:resource="http://www.ease-crc.org/ont/SOMA.owl#hasDisposition"/>
                <owl:someValuesFrom rdf:resource="http://www.ease-crc.org/ont/SOMA.owl#Containment"/>
            </owl:Restriction>
        </rdfs:subClassOf>
        <rdfs:comment>An item designed to be able to hold some other items, preventing their free movement and/or protecting them from outside influence. Containers may be used for storage, or to obtain control over items that are otherwise hard to manipulate directly (e.g. liquids).</rdfs:comment>
        <rdfs:isDefinedBy rdf:resource="http://www.ease-crc.org/ont/SOMA-HOME.owl"/>
        <rdfs:isDefinedBy rdf:resource="http://www.ease-crc.org/ont/SOMA-OBJ.owl"/>
        <rdfs:label>Designed container</rdfs:label>
    </owl:Class>
    


    <!-- http://www.ease-crc.org/ont/SOMA.owl#DesignedFurniture -->


    <owl:Class rdf:about="http://www.ease-crc.org/ont/SOMA.owl#DesignedFurniture">
        <rdfs:subClassOf rdf:resource="http://www.ontologydesignpatterns.org/ont/dul/DUL.owl#DesignedArtifact"/>
        <rdfs:comment>An object used to make a room or building suitable for living or working.</rdfs:comment>
        <rdfs:isDefinedBy rdf:resource="http://www.ease-crc.org/ont/SOMA-HOME.owl"/>
        <rdfs:isDefinedBy rdf:resource="http://www.ease-crc.org/ont/SOMA-OBJ.owl"/>
        <rdfs:label>Designed furniture</rdfs:label>
    </owl:Class>
    


    <!-- http://www.ease-crc.org/ont/SOMA.owl#DesignedHandle -->


    <owl:Class rdf:about="http://www.ease-crc.org/ont/SOMA.owl#DesignedHandle">
        <rdfs:subClassOf rdf:resource="http://www.ease-crc.org/ont/SOMA.owl#DesignedComponent"/>
        <rdfs:subClassOf>
            <owl:Restriction>
                <owl:onProperty rdf:resource="http://www.ease-crc.org/ont/SOMA.owl#hasDisposition"/>
                <owl:someValuesFrom rdf:resource="http://www.ease-crc.org/ont/SOMA.owl#Graspability"/>
            </owl:Restriction>
        </rdfs:subClassOf>
        <rdfs:comment>An item designed to fit well within a grasping hand, often attached to another item to enhance its manipulability.</rdfs:comment>
        <rdfs:isDefinedBy rdf:resource="http://www.ease-crc.org/ont/SOMA-HOME.owl"/>
        <rdfs:label>Designed handle</rdfs:label>
    </owl:Class>
    


    <!-- http://www.ease-crc.org/ont/SOMA.owl#DesignedSpade -->


    <owl:Class rdf:about="http://www.ease-crc.org/ont/SOMA.owl#DesignedSpade">
        <rdfs:subClassOf rdf:resource="http://www.ease-crc.org/ont/SOMA.owl#DesignedComponent"/>
        <rdfs:comment>A sharp-edged metal blade used for digging or cutting.</rdfs:comment>
        <rdfs:isDefinedBy rdf:resource="http://www.ease-crc.org/ont/SOMA-HOME.owl"/>
        <rdfs:label>Designed spade</rdfs:label>
    </owl:Class>
    


    <!-- http://www.ease-crc.org/ont/SOMA.owl#DesignedTool -->


    <owl:Class rdf:about="http://www.ease-crc.org/ont/SOMA.owl#DesignedTool">
        <rdfs:subClassOf rdf:resource="http://www.ontologydesignpatterns.org/ont/dul/DUL.owl#DesignedArtifact"/>
        <rdfs:comment>An item designed to enable some action, in which it will play an instrumental role.</rdfs:comment>
        <rdfs:isDefinedBy rdf:resource="http://www.ease-crc.org/ont/SOMA-HOME.owl"/>
        <rdfs:isDefinedBy rdf:resource="http://www.ease-crc.org/ont/SOMA-IO.owl"/>
        <rdfs:isDefinedBy rdf:resource="http://www.ease-crc.org/ont/SOMA-OBJ.owl"/>
        <rdfs:label>Designed tool</rdfs:label>
    </owl:Class>
    


    <!-- http://www.ease-crc.org/ont/SOMA.owl#Destination -->


    <owl:Class rdf:about="http://www.ease-crc.org/ont/SOMA.owl#Destination">
        <rdfs:subClassOf rdf:resource="http://www.ease-crc.org/ont/SOMA.owl#Location"/>
        <rdfs:comment>A role classifying the location where an event or object is directed towards.</rdfs:comment>
        <rdfs:isDefinedBy rdf:resource="http://www.ease-crc.org/ont/SOMA-OBJ.owl"/>
    </owl:Class>
    


    <!-- http://www.ease-crc.org/ont/SOMA.owl#DestroyedObject -->


    <owl:Class rdf:about="http://www.ease-crc.org/ont/SOMA.owl#DestroyedObject">
        <rdfs:subClassOf rdf:resource="http://www.ease-crc.org/ont/SOMA.owl#Patient"/>
        <rdfs:comment>An object that is detroyed.</rdfs:comment>
        <rdfs:isDefinedBy rdf:resource="http://www.ease-crc.org/ont/SOMA-OBJ.owl"/>
        <rdfs:isDefinedBy rdf:resource="http://www.ease-crc.org/ont/SOMA-PROC.owl"/>
        <rdfs:label xml:lang="en">Destroyed object</rdfs:label>
    </owl:Class>
    


    <!-- http://www.ease-crc.org/ont/SOMA.owl#Destruction -->


    <owl:Class rdf:about="http://www.ease-crc.org/ont/SOMA.owl#Destruction">
        <rdfs:subClassOf rdf:resource="http://www.ease-crc.org/ont/SOMA.owl#ProcessType"/>
        <rdfs:subClassOf>
            <owl:Restriction>
                <owl:onProperty rdf:resource="http://www.ease-crc.org/ont/SOMA.owl#isProcessTypeOf"/>
                <owl:someValuesFrom rdf:resource="http://www.ease-crc.org/ont/SOMA.owl#DestroyedObject"/>
            </owl:Restriction>
        </rdfs:subClassOf>
        <rdfs:comment>A process by which a physical Entity is destroyed.

Note, most of the physical Entities we are concerned with are actually arrangements of many smaller physical Entities, so another way to look at this is that a &apos;Physical destruction&apos; is a process by which an arrangement of physical Entities, which was previously itself considered a physical Entity, is changed to such an extent that it is no longer recognized as continuing to exist.</rdfs:comment>
        <rdfs:isDefinedBy rdf:resource="http://www.ease-crc.org/ont/SOMA-PROC.owl"/>
        <rdfs:label>Destruction</rdfs:label>
    </owl:Class>
    


    <!-- http://www.ease-crc.org/ont/SOMA.owl#DetectedObject -->


    <owl:Class rdf:about="http://www.ease-crc.org/ont/SOMA.owl#DetectedObject">
        <rdfs:subClassOf rdf:resource="http://www.ease-crc.org/ont/SOMA.owl#Patient"/>
        <rdfs:comment>An object that is detected.</rdfs:comment>
        <rdfs:isDefinedBy rdf:resource="http://www.ease-crc.org/ont/SOMA-OBJ.owl"/>
        <rdfs:label xml:lang="en">Detected object</rdfs:label>
    </owl:Class>
    


    <!-- http://www.ease-crc.org/ont/SOMA.owl#DeviceState -->


    <owl:Class rdf:about="http://www.ease-crc.org/ont/SOMA.owl#DeviceState">
        <rdfs:subClassOf rdf:resource="http://www.ease-crc.org/ont/SOMA.owl#Intrinsic"/>
        <rdfs:comment>A quality belonging to a device which indicates its overall functional state.</rdfs:comment>
        <rdfs:isDefinedBy rdf:resource="http://www.ease-crc.org/ont/SOMA-OBJ.owl"/>
    </owl:Class>
    


    <!-- http://www.ease-crc.org/ont/SOMA.owl#DeviceStateRange -->


    <owl:Class rdf:about="http://www.ease-crc.org/ont/SOMA.owl#DeviceStateRange">
        <owl:equivalentClass>
            <owl:Class>
                <owl:unionOf rdf:parseType="Collection">
                    <rdf:Description rdf:about="http://www.ease-crc.org/ont/SOMA.owl#DeviceTurnedOff"/>
                    <rdf:Description rdf:about="http://www.ease-crc.org/ont/SOMA.owl#DeviceTurnedOn"/>
                </owl:unionOf>
            </owl:Class>
        </owl:equivalentClass>
        <rdfs:subClassOf rdf:resource="http://www.ontologydesignpatterns.org/ont/dul/DUL.owl#Region"/>
        <rdfs:comment>This class defines the values that a device state can take.</rdfs:comment>
        <rdfs:isDefinedBy rdf:resource="http://www.ease-crc.org/ont/SOMA-OBJ.owl"/>
        <rdfs:label xml:lang="en">Device state range</rdfs:label>
    </owl:Class>
    


    <!-- http://www.ease-crc.org/ont/SOMA.owl#DeviceTurnedOff -->


    <owl:Class rdf:about="http://www.ease-crc.org/ont/SOMA.owl#DeviceTurnedOff">
        <rdfs:subClassOf rdf:resource="http://www.ease-crc.org/ont/SOMA.owl#DeviceStateRange"/>
        <rdfs:comment>A value indicating a device is not in operation.</rdfs:comment>
        <rdfs:isDefinedBy rdf:resource="http://www.ease-crc.org/ont/SOMA-OBJ.owl"/>
        <rdfs:label xml:lang="en">Device turned off</rdfs:label>
    </owl:Class>
    


    <!-- http://www.ease-crc.org/ont/SOMA.owl#DeviceTurnedOn -->


    <owl:Class rdf:about="http://www.ease-crc.org/ont/SOMA.owl#DeviceTurnedOn">
        <rdfs:subClassOf rdf:resource="http://www.ease-crc.org/ont/SOMA.owl#DeviceStateRange"/>
        <rdfs:comment>A value indicating a device is in operation.</rdfs:comment>
        <rdfs:isDefinedBy rdf:resource="http://www.ease-crc.org/ont/SOMA-OBJ.owl"/>
        <rdfs:label xml:lang="en">Device turned on</rdfs:label>
    </owl:Class>
    


    <!-- http://www.ease-crc.org/ont/SOMA.owl#Dicing -->


    <owl:Class rdf:about="http://www.ease-crc.org/ont/SOMA.owl#Dicing">
        <rdfs:subClassOf rdf:resource="http://www.ease-crc.org/ont/SOMA.owl#Cutting"/>
        <rdfs:comment>A particular kind of cutting where the goal is to produce small pieces out of some object or material. Unlike slices, the pieces to be obtained do not have one or two dimensions being more prominent than others. &quot;Dice&quot;, the pieces dicing results in, are approximately cubic.</rdfs:comment>
        <rdfs:isDefinedBy rdf:resource="http://www.ease-crc.org/ont/SOMA-ACT.owl"/>
    </owl:Class>
    


    <!-- http://www.ease-crc.org/ont/SOMA.owl#Digital_File -->


    <owl:Class rdf:about="http://www.ease-crc.org/ont/SOMA.owl#Digital_File">
        <rdfs:subClassOf rdf:resource="http://www.ontologydesignpatterns.org/ont/dul/DUL.owl#InformationRealization"/>
        <rdfs:subClassOf rdf:nodeID="genid241"/>
        <rdfs:subClassOf rdf:nodeID="genid243"/>
        <rdfs:comment xml:lang="en">Any file that exists as a digital resource (but not its content), e.g., a text file actually laying on some hard drive, but not the contained text.</rdfs:comment>
        <rdfs:isDefinedBy rdf:resource="http://www.ease-crc.org/ont/SOMA-IO.owl"/>
        <rdfs:label xml:lang="en">Computer File</rdfs:label>
        <rdfs:label xml:lang="en">Digital File</rdfs:label>
    </owl:Class>
    <owl:Restriction rdf:nodeID="genid241">
        <owl:onProperty rdf:resource="http://www.ontologydesignpatterns.org/ont/dul/DUL.owl#realizes"/>
        <owl:someValuesFrom rdf:resource="http://www.ease-crc.org/ont/SOMA.owl#Structured_Text"/>
    </owl:Restriction>
    <owl:Restriction rdf:nodeID="genid243">
        <owl:onProperty rdf:resource="http://www.ease-crc.org/ont/SOMA.owl#hasNameString"/>
        <owl:someValuesFrom rdf:resource="http://www.w3.org/2001/XMLSchema#string"/>
    </owl:Restriction>
    <owl:Axiom>
        <owl:annotatedSource rdf:resource="http://www.ease-crc.org/ont/SOMA.owl#Digital_File"/>
        <owl:annotatedProperty rdf:resource="http://www.w3.org/2000/01/rdf-schema#subClassOf"/>
        <owl:annotatedTarget rdf:nodeID="genid241"/>
        <rdfs:comment xml:lang="en">The file content.</rdfs:comment>
    </owl:Axiom>
    <owl:Axiom>
        <owl:annotatedSource rdf:resource="http://www.ease-crc.org/ont/SOMA.owl#Digital_File"/>
        <owl:annotatedProperty rdf:resource="http://www.w3.org/2000/01/rdf-schema#subClassOf"/>
        <owl:annotatedTarget rdf:nodeID="genid243"/>
        <rdfs:comment xml:lang="en">The path of the file on a computer system.</rdfs:comment>
    </owl:Axiom>
    


    <!-- http://www.ease-crc.org/ont/SOMA.owl#DirectedMotion -->


    <owl:Class rdf:about="http://www.ease-crc.org/ont/SOMA.owl#DirectedMotion">
        <rdfs:subClassOf rdf:resource="http://www.ease-crc.org/ont/SOMA.owl#Motion"/>
        <owl:disjointWith rdf:resource="http://www.ease-crc.org/ont/SOMA.owl#UndirectedMotion"/>
        <rdfs:comment>A Motion that is considered to be toward a location or along a path. It is not important that the final location or path be the intention of some Agent, but it is considered that the important feature of this Motion is that it has a path and/or destination.</rdfs:comment>
        <rdfs:isDefinedBy rdf:resource="http://www.ease-crc.org/ont/SOMA-PROC.owl"/>
        <rdfs:label>Directed motion</rdfs:label>
    </owl:Class>
    


    <!-- http://www.ease-crc.org/ont/SOMA.owl#Dirty -->


    <owl:Class rdf:about="http://www.ease-crc.org/ont/SOMA.owl#Dirty">
        <rdfs:subClassOf rdf:resource="http://www.ease-crc.org/ont/SOMA.owl#CleanlinessRegion"/>
        <rdfs:comment>A cleanliness region with values considered as dirty.</rdfs:comment>
        <rdfs:isDefinedBy rdf:resource="http://www.ease-crc.org/ont/SOMA-OBJ.owl"/>
    </owl:Class>
    


    <!-- http://www.ease-crc.org/ont/SOMA.owl#Dish -->


    <owl:Class rdf:about="http://www.ease-crc.org/ont/SOMA.owl#Dish">
        <rdfs:subClassOf rdf:resource="http://www.ontologydesignpatterns.org/ont/dul/DUL.owl#DesignedArtifact"/>
        <rdfs:isDefinedBy rdf:resource="http://www.ease-crc.org/ont/SOMA-HOME.owl"/>
    </owl:Class>
    


    <!-- http://www.ease-crc.org/ont/SOMA.owl#Dishwasher -->


    <owl:Class rdf:about="http://www.ease-crc.org/ont/SOMA.owl#Dishwasher">
        <rdfs:subClassOf rdf:resource="http://www.ease-crc.org/ont/SOMA.owl#Appliance"/>
        <rdfs:subClassOf rdf:resource="http://www.ease-crc.org/ont/SOMA.owl#DesignedContainer"/>
        <rdfs:comment>An appliance for washing dishes and cutlery automatically.</rdfs:comment>
        <rdfs:isDefinedBy rdf:resource="http://www.ease-crc.org/ont/SOMA-HOME.owl"/>
    </owl:Class>
    


    <!-- http://www.ease-crc.org/ont/SOMA.owl#DishwasherTab -->


    <owl:Class rdf:about="http://www.ease-crc.org/ont/SOMA.owl#DishwasherTab">
        <rdfs:subClassOf rdf:resource="http://www.ontologydesignpatterns.org/ont/dul/DUL.owl#DesignedSubstance"/>
        <rdfs:comment>A solid detergent inserted into dishwashers.</rdfs:comment>
        <rdfs:isDefinedBy rdf:resource="http://www.ease-crc.org/ont/SOMA-HOME.owl"/>
    </owl:Class>
    


    <!-- http://www.ease-crc.org/ont/SOMA.owl#Disposition -->


    <owl:Class rdf:about="http://www.ease-crc.org/ont/SOMA.owl#Disposition">
        <rdfs:subClassOf rdf:resource="http://www.ease-crc.org/ont/SOMA.owl#Extrinsic"/>
        <rdfs:subClassOf>
            <owl:Restriction>
                <owl:onProperty rdf:resource="http://www.ontologydesignpatterns.org/ont/dul/DUL.owl#isDescribedBy"/>
                <owl:qualifiedCardinality rdf:datatype="http://www.w3.org/2001/XMLSchema#nonNegativeInteger">1</owl:qualifiedCardinality>
                <owl:onClass rdf:resource="http://www.ease-crc.org/ont/SOMA.owl#Affordance"/>
            </owl:Restriction>
        </rdfs:subClassOf>
        <rdfs:subClassOf>
            <owl:Restriction>
                <owl:onProperty rdf:resource="http://www.ontologydesignpatterns.org/ont/dul/DUL.owl#isDescribedBy"/>
                <owl:qualifiedCardinality rdf:datatype="http://www.w3.org/2001/XMLSchema#nonNegativeInteger">1</owl:qualifiedCardinality>
                <owl:onClass>
                    <owl:Class>
                        <owl:intersectionOf rdf:parseType="Collection">
                            <rdf:Description rdf:about="http://www.ease-crc.org/ont/SOMA.owl#Affordance"/>
                            <owl:Restriction>
                                <owl:onProperty rdf:resource="http://www.ease-crc.org/ont/SOMA.owl#definesBearer"/>
                                <owl:qualifiedCardinality rdf:datatype="http://www.w3.org/2001/XMLSchema#nonNegativeInteger">1</owl:qualifiedCardinality>
                                <owl:onClass rdf:resource="http://www.ontologydesignpatterns.org/ont/dul/DUL.owl#Role"/>
                            </owl:Restriction>
                            <owl:Restriction>
                                <owl:onProperty rdf:resource="http://www.ease-crc.org/ont/SOMA.owl#definesTrigger"/>
                                <owl:qualifiedCardinality rdf:datatype="http://www.w3.org/2001/XMLSchema#nonNegativeInteger">1</owl:qualifiedCardinality>
                                <owl:onClass rdf:resource="http://www.ontologydesignpatterns.org/ont/dul/DUL.owl#Role"/>
                            </owl:Restriction>
                            <owl:Restriction>
                                <owl:onProperty rdf:resource="http://www.ontologydesignpatterns.org/ont/dul/DUL.owl#definesTask"/>
                                <owl:qualifiedCardinality rdf:datatype="http://www.w3.org/2001/XMLSchema#nonNegativeInteger">1</owl:qualifiedCardinality>
                                <owl:onClass rdf:resource="http://www.ontologydesignpatterns.org/ont/dul/DUL.owl#Task"/>
                            </owl:Restriction>
                        </owl:intersectionOf>
                    </owl:Class>
                </owl:onClass>
            </owl:Restriction>
        </rdfs:subClassOf>
        <rdfs:comment>The tendency of an object (the bearer) to be used to perform certain tasks with others (the triggers).</rdfs:comment>
        <rdfs:comment>extrinsic</rdfs:comment>
        <rdfs:isDefinedBy rdf:resource="http://www.ease-crc.org/ont/SOMA-OBJ.owl"/>
    </owl:Class>
    


    <!-- http://www.ease-crc.org/ont/SOMA.owl#Distancing -->


    <owl:Class rdf:about="http://www.ease-crc.org/ont/SOMA.owl#Distancing">
        <rdfs:subClassOf rdf:resource="http://www.ease-crc.org/ont/SOMA.owl#Navigating"/>
        <rdfs:comment>A task in which an Agent increases its distance from some location.</rdfs:comment>
        <rdfs:isDefinedBy rdf:resource="http://www.ease-crc.org/ont/SOMA-ACT.owl"/>
    </owl:Class>
    


    <!-- http://www.ease-crc.org/ont/SOMA.owl#Door -->


    <owl:Class rdf:about="http://www.ease-crc.org/ont/SOMA.owl#Door">
        <rdfs:subClassOf rdf:resource="http://www.ease-crc.org/ont/SOMA.owl#DesignedComponent"/>
        <rdfs:comment>A hinged, sliding, or revolving barrier at the entrance to a building, room, or vehicle, or in the frame of a cupboard.</rdfs:comment>
        <rdfs:isDefinedBy rdf:resource="http://www.ease-crc.org/ont/SOMA-HOME.owl"/>
    </owl:Class>
    


    <!-- http://www.ease-crc.org/ont/SOMA.owl#Drawer -->


    <owl:Class rdf:about="http://www.ease-crc.org/ont/SOMA.owl#Drawer">
        <rdfs:subClassOf rdf:resource="http://www.ease-crc.org/ont/SOMA.owl#DesignedComponent"/>
        <rdfs:subClassOf rdf:resource="http://www.ease-crc.org/ont/SOMA.owl#DesignedContainer"/>
        <rdfs:comment>A storage compartment without a lid, made to slide horizontally in and out of a piece of furniture.</rdfs:comment>
        <rdfs:isDefinedBy rdf:resource="http://www.ease-crc.org/ont/SOMA-HOME.owl"/>
    </owl:Class>
    


    <!-- http://www.ease-crc.org/ont/SOMA.owl#Dreaming -->


    <owl:Class rdf:about="http://www.ease-crc.org/ont/SOMA.owl#Dreaming">
        <rdfs:subClassOf rdf:resource="http://www.ease-crc.org/ont/SOMA.owl#MentalTask"/>
        <rdfs:comment>Any form of re-processing episodic memories for long-term memory by natural or aritifical agents.</rdfs:comment>
        <rdfs:isDefinedBy rdf:resource="http://www.ease-crc.org/ont/SOMA-ACT.owl"/>
    </owl:Class>
    


    <!-- http://www.ease-crc.org/ont/SOMA.owl#Driving -->


    <owl:Class rdf:about="http://www.ease-crc.org/ont/SOMA.owl#Driving">
        <rdfs:subClassOf rdf:resource="http://www.ease-crc.org/ont/SOMA.owl#Locomotion"/>
        <owl:disjointWith rdf:resource="http://www.ease-crc.org/ont/SOMA.owl#Flying"/>
        <owl:disjointWith rdf:resource="http://www.ease-crc.org/ont/SOMA.owl#Swimming"/>
        <owl:disjointWith rdf:resource="http://www.ease-crc.org/ont/SOMA.owl#Walking"/>
        <rdfs:comment>A process type classifying a motion of a body that exists because this body is attached to and controls some other moving body, usually a vehicle.</rdfs:comment>
        <rdfs:isDefinedBy rdf:resource="http://www.ease-crc.org/ont/SOMA-PROC.owl"/>
    </owl:Class>
    


    <!-- http://www.ease-crc.org/ont/SOMA.owl#Dropping -->


    <owl:Class rdf:about="http://www.ease-crc.org/ont/SOMA.owl#Dropping">
        <rdfs:subClassOf rdf:resource="http://www.ease-crc.org/ont/SOMA.owl#Actuating"/>
        <owl:disjointWith rdf:resource="http://www.ease-crc.org/ont/SOMA.owl#Placing"/>
        <rdfs:comment>The dropped object falls mainly under the influence of gravity. However, an agent may also drop something during navigation. The difference to &apos;Throwing&apos; is that there is no &apos;Limb motion&apos; which is a constitiuent of the action.

&apos;Dropping&apos; is intentional. Dropping by accident may not has a phase to release the grasp. It could be that the grasp was not strong enough and the objects &quot;slips&quot; away.</rdfs:comment>
        <rdfs:isDefinedBy rdf:resource="http://www.ease-crc.org/ont/SOMA-ACT.owl"/>
    </owl:Class>
    


    <!-- http://www.ease-crc.org/ont/SOMA.owl#ESTSchemaTheory -->


    <owl:Class rdf:about="http://www.ease-crc.org/ont/SOMA.owl#ESTSchemaTheory">
        <rdfs:subClassOf rdf:resource="http://www.ease-crc.org/ont/SOMA.owl#ImageSchemaTheory"/>
        <rdfs:subClassOf>
            <owl:Restriction>
                <owl:onProperty rdf:resource="http://www.ontologydesignpatterns.org/ont/dul/DUL.owl#defines"/>
                <owl:someValuesFrom rdf:resource="http://www.ease-crc.org/ont/SOMA.owl#ExistingObjectRole"/>
            </owl:Restriction>
        </rdfs:subClassOf>
        <rdfs:subClassOf>
            <owl:Restriction>
                <owl:onProperty rdf:resource="http://www.ontologydesignpatterns.org/ont/dul/DUL.owl#defines"/>
                <owl:cardinality rdf:datatype="http://www.w3.org/2001/XMLSchema#nonNegativeInteger">1</owl:cardinality>
            </owl:Restriction>
        </rdfs:subClassOf>
        <rdfs:comment>A schematic theory that describes the existence of an entity.

Developmental psychology posits that &quot;object permanence&quot; (the assumption that physical objects keep existing even when the agent doesn&apos;t perceive them, which consequently informs reasoning about where an object should be, even when perception of it is lost) is a cognitive ability that is not, at least in the very young human child, immediately manifest. Rather, it seems learned via interaction, and usually is among an infant&apos;s cognitive repertoire by age 2.

In SOMA, we represent this ability of a cognitive agent as an ability to generate and maintain ESTSchemaTheories. Each instance of such a theory refers to one particular physical object, the one that the instance of the ESTSchemaTheory asserts to exist.

Because each instance of an ESTSchemaTheory refers to a single object, ESTSchemaTheories are not associated to any relation between OWL individuals.</rdfs:comment>
        <rdfs:isDefinedBy rdf:resource="http://www.ease-crc.org/ont/SOMA-SAY.owl"/>
        <rdfs:label xml:lang="en">EST schema theory</rdfs:label>
    </owl:Class>
    


    <!-- http://www.ease-crc.org/ont/SOMA.owl#Effort -->


    <owl:Class rdf:about="http://www.ease-crc.org/ont/SOMA.owl#Effort">
        <rdfs:subClassOf rdf:resource="http://www.ontologydesignpatterns.org/ont/dul/DUL.owl#Parameter"/>
        <rdfs:comment>A parameter describing the amount of force to be exerted by some actuator.</rdfs:comment>
        <rdfs:isDefinedBy rdf:resource="http://www.ease-crc.org/ont/SOMA-OBJ.owl"/>
    </owl:Class>
    


    <!-- http://www.ease-crc.org/ont/SOMA.owl#EnclosedObject -->


    <owl:Class rdf:about="http://www.ease-crc.org/ont/SOMA.owl#EnclosedObject">
        <rdfs:subClassOf rdf:resource="http://www.ease-crc.org/ont/SOMA.owl#IncludedObject"/>
        <rdfs:comment>An object included within the spatial boundaries of another object.</rdfs:comment>
        <rdfs:isDefinedBy rdf:resource="http://www.ease-crc.org/ont/SOMA-OBJ.owl"/>
        <rdfs:label xml:lang="en">Enclosed object</rdfs:label>
    </owl:Class>
    


    <!-- http://www.ease-crc.org/ont/SOMA.owl#Enclosing -->


    <owl:Class rdf:about="http://www.ease-crc.org/ont/SOMA.owl#Enclosing">
        <rdfs:subClassOf rdf:resource="http://www.ease-crc.org/ont/SOMA.owl#Containment"/>
        <rdfs:subClassOf>
            <owl:Restriction>
                <owl:onProperty rdf:resource="http://www.ease-crc.org/ont/SOMA.owl#affordsTrigger"/>
                <owl:allValuesFrom rdf:resource="http://www.ease-crc.org/ont/SOMA.owl#EnclosedObject"/>
            </owl:Restriction>
        </rdfs:subClassOf>
        <rdfs:comment>The disposition of an object (the container) to contain other objects by enclosing them to prevent their free movement.</rdfs:comment>
        <rdfs:isDefinedBy rdf:resource="http://www.ease-crc.org/ont/SOMA-OBJ.owl"/>
    </owl:Class>
    


    <!-- http://www.ease-crc.org/ont/SOMA.owl#EndEffectorPositioning -->


    <owl:Class rdf:about="http://www.ease-crc.org/ont/SOMA.owl#EndEffectorPositioning">
        <rdfs:subClassOf rdf:resource="http://www.ease-crc.org/ont/SOMA.owl#Manipulating"/>
        <rdfs:comment>A task in which an Agent places its end effectors at particular poses.</rdfs:comment>
        <rdfs:isDefinedBy rdf:resource="http://www.ease-crc.org/ont/SOMA-ACT.owl"/>
        <rdfs:label xml:lang="en">End effector positioning</rdfs:label>
    </owl:Class>
    


    <!-- http://www.ease-crc.org/ont/SOMA.owl#EventAdjacentRole -->


    <owl:Class rdf:about="http://www.ease-crc.org/ont/SOMA.owl#EventAdjacentRole">
        <rdfs:subClassOf rdf:resource="http://www.ontologydesignpatterns.org/ont/dul/DUL.owl#Role"/>
        <rdfs:comment>A role classifying a participant in an event.

In linguistics, this is also known as a thematic role.</rdfs:comment>
        <rdfs:isDefinedBy rdf:resource="http://www.ease-crc.org/ont/SOMA-OBJ.owl"/>
        <rdfs:label xml:lang="en">Event adjacent role</rdfs:label>
        <rdfs:label xml:lang="en">Thematic role</rdfs:label>
    </owl:Class>
    


    <!-- http://www.ease-crc.org/ont/SOMA.owl#ExecutableFile -->


    <owl:Class rdf:about="http://www.ease-crc.org/ont/SOMA.owl#ExecutableFile">
        <owl:equivalentClass>
            <owl:Class>
                <owl:intersectionOf rdf:parseType="Collection">
                    <rdf:Description rdf:about="http://www.ease-crc.org/ont/SOMA.owl#Digital_File"/>
                    <owl:Restriction>
                        <owl:onProperty rdf:resource="http://www.ontologydesignpatterns.org/ont/dul/DUL.owl#realizes"/>
                        <owl:someValuesFrom rdf:resource="http://www.ease-crc.org/ont/SOMA.owl#Executable_Code"/>
                    </owl:Restriction>
                </owl:intersectionOf>
            </owl:Class>
        </owl:equivalentClass>
        <rdfs:comment xml:lang="en">An Executable File, sometimes simply referred to as an executable or binary, causes a computer &quot;to perform indicated tasks according to encoded instructions&quot;, as opposed to a data file that must be interpreted (parsed) by a program to be meaningful.

The exact interpretation depends upon the use. &quot;Instructions&quot; is traditionally taken to mean machine code instructions for a physical CPU. In some contexts, a file containing scripting instructions (such as bytecode) may also be considered executable.</rdfs:comment>
        <rdfs:isDefinedBy rdf:resource="http://www.ease-crc.org/ont/SOMA-IO.owl"/>
        <rdfs:label xml:lang="en">Executable File</rdfs:label>
    </owl:Class>
    


    <!-- http://www.ease-crc.org/ont/SOMA.owl#ExecutableFormat -->


    <owl:Class rdf:about="http://www.ease-crc.org/ont/SOMA.owl#ExecutableFormat">
        <rdfs:subClassOf rdf:resource="http://www.ease-crc.org/ont/SOMA.owl#File_format"/>
        <rdfs:subClassOf>
            <owl:Restriction>
                <owl:onProperty rdf:resource="http://www.ease-crc.org/ont/SOMA.owl#givesMeaningTo"/>
                <owl:allValuesFrom rdf:resource="http://www.ease-crc.org/ont/SOMA.owl#Executable_Code"/>
            </owl:Restriction>
        </rdfs:subClassOf>
        <rdfs:comment xml:lang="en">An Executable Format is a File Format that allows computers to directly execute the content. Examples are MZ (DOS) or COFF.</rdfs:comment>
        <rdfs:isDefinedBy rdf:resource="http://www.ease-crc.org/ont/SOMA-IO.owl"/>
        <rdfs:label xml:lang="en">Executable Format</rdfs:label>
    </owl:Class>
    


    <!-- http://www.ease-crc.org/ont/SOMA.owl#ExecutableSchematicTheory -->


    <owl:Class rdf:about="http://www.ease-crc.org/ont/SOMA.owl#ExecutableSchematicTheory">
        <rdfs:subClassOf rdf:resource="http://www.ease-crc.org/ont/SOMA.owl#SchematicTheory"/>
        <rdfs:subClassOf>
            <owl:Restriction>
                <owl:onProperty rdf:resource="http://www.ontologydesignpatterns.org/ont/dul/DUL.owl#defines"/>
                <owl:someValuesFrom rdf:resource="http://www.ease-crc.org/ont/SOMA.owl#AgentRole"/>
            </owl:Restriction>
        </rdfs:subClassOf>
        <rdfs:comment>Also known as &quot;executing schemas&quot; or &quot;x-schemas&quot;, these were defined by Bergen and Chang in their work &quot;Embodied Construction Grammar in Simulation-Based Language Understanding&quot; as:

&quot;Executing schemas, or x-schemas, are dynamic representations motivated in part by motor and perceptual systems (Bailey 1997; Narayanan 1997), on the assumption that the same underlying representations used for executing and perceiving an action are brought to bear in understanding language about that action. The x-schema formalism is an extension of Petri nets (Murata 1989) that can model sequential, concurrent, and
asynchronous events&quot;

SOMA does not restrict the formalism of ExecutableSchematicTheories; i.e. they don&apos;t have to be Petri Nets.

They maintain their role however as representations able to drive a simulation, at some level of abstraction, of an embodied action. This level of abstraction may be still fairly underspecified as in the case of the original x-schemas and as such not a plan that an agent could run in an actual physical environment without further information.</rdfs:comment>
        <rdfs:isDefinedBy rdf:resource="http://www.ease-crc.org/ont/SOMA-SAY.owl"/>
        <rdfs:label xml:lang="en">Executable schematic theory</rdfs:label>
    </owl:Class>
    


    <!-- http://www.ease-crc.org/ont/SOMA.owl#ExecutableSoftware -->


    <owl:Class rdf:about="http://www.ease-crc.org/ont/SOMA.owl#ExecutableSoftware">
        <owl:equivalentClass>
            <owl:Class>
                <owl:intersectionOf rdf:parseType="Collection">
                    <rdf:Description rdf:about="http://www.ease-crc.org/ont/SOMA.owl#Software"/>
                    <owl:Restriction>
                        <owl:onProperty rdf:resource="http://www.ontologydesignpatterns.org/ont/dul/DUL.owl#hasMember"/>
                        <owl:someValuesFrom rdf:resource="http://www.ease-crc.org/ont/SOMA.owl#ExecutableFile"/>
                    </owl:Restriction>
                </owl:intersectionOf>
            </owl:Class>
        </owl:equivalentClass>
        <rdfs:comment xml:lang="en">Executable Software is Software that can directly be executed, in comparison to a Software Library, which might only contain functionality via interfaces, but offers no execution entry point.</rdfs:comment>
        <rdfs:isDefinedBy rdf:resource="http://www.ease-crc.org/ont/SOMA-IO.owl"/>
        <rdfs:label xml:lang="en">Executable Software</rdfs:label>
    </owl:Class>
    


    <!-- http://www.ease-crc.org/ont/SOMA.owl#Executable_Code -->


    <owl:Class rdf:about="http://www.ease-crc.org/ont/SOMA.owl#Executable_Code">
        <owl:equivalentClass>
            <owl:Class>
                <owl:intersectionOf rdf:parseType="Collection">
                    <rdf:Description rdf:about="http://www.ease-crc.org/ont/SOMA.owl#Computer_Program"/>
                    <owl:Restriction>
                        <owl:onProperty rdf:resource="http://www.ease-crc.org/ont/SOMA.owl#isGivenMeaningBy"/>
                        <owl:someValuesFrom rdf:resource="http://www.ease-crc.org/ont/SOMA.owl#ExecutableFormat"/>
                    </owl:Restriction>
                </owl:intersectionOf>
            </owl:Class>
        </owl:equivalentClass>
        <rdfs:subClassOf rdf:resource="http://www.ease-crc.org/ont/SOMA.owl#Computer_Program"/>
        <rdfs:comment xml:lang="en">Executable Code is Code that when compiled / interpreted, has some clear entrance point and can be executed. Note the difference to an Executable File, which is the file that contains such (compiled) code.</rdfs:comment>
        <rdfs:isDefinedBy rdf:resource="http://www.ease-crc.org/ont/SOMA-IO.owl"/>
        <rdfs:label xml:lang="en">Executable Code</rdfs:label>
    </owl:Class>
    


    <!-- http://www.ease-crc.org/ont/SOMA.owl#ExecutionStateRegion -->


    <owl:Class rdf:about="http://www.ease-crc.org/ont/SOMA.owl#ExecutionStateRegion">
        <owl:equivalentClass>
            <owl:Class>
                <owl:oneOf rdf:parseType="Collection">
                    <rdf:Description rdf:about="http://www.ease-crc.org/ont/SOMA.owl#ExecutionState_Active"/>
                    <rdf:Description rdf:about="http://www.ease-crc.org/ont/SOMA.owl#ExecutionState_Cancelled"/>
                    <rdf:Description rdf:about="http://www.ease-crc.org/ont/SOMA.owl#ExecutionState_Failed"/>
                    <rdf:Description rdf:about="http://www.ease-crc.org/ont/SOMA.owl#ExecutionState_Paused"/>
                    <rdf:Description rdf:about="http://www.ease-crc.org/ont/SOMA.owl#ExecutionState_Pending"/>
                    <rdf:Description rdf:about="http://www.ease-crc.org/ont/SOMA.owl#ExecutionState_Succeeded"/>
                </owl:oneOf>
            </owl:Class>
        </owl:equivalentClass>
        <rdfs:subClassOf rdf:resource="http://www.ontologydesignpatterns.org/ont/dul/DUL.owl#Region"/>
        <rdfs:comment>A region containing labels that describe different states in the evolution/completion of a task execution.</rdfs:comment>
        <rdfs:isDefinedBy rdf:resource="http://www.ease-crc.org/ont/SOMA-ACT.owl"/>
        <rdfs:label>Execution state region</rdfs:label>
    </owl:Class>
    


    <!-- http://www.ease-crc.org/ont/SOMA.owl#ExistingObjectRole -->


    <owl:Class rdf:about="http://www.ease-crc.org/ont/SOMA.owl#ExistingObjectRole">
        <rdfs:subClassOf rdf:resource="http://www.ease-crc.org/ont/SOMA.owl#RelationAdjacentRole"/>
        <rdfs:subClassOf>
            <owl:Restriction>
                <owl:onProperty rdf:resource="http://www.ontologydesignpatterns.org/ont/dul/DUL.owl#classifies"/>
                <owl:allValuesFrom rdf:resource="http://www.ontologydesignpatterns.org/ont/dul/DUL.owl#PhysicalObject"/>
            </owl:Restriction>
        </rdfs:subClassOf>
        <rdfs:comment>A role that requires of its filler simply to exist, unlike other roles that may demand e.g. agentive or instrumental participation in some executable schema or plan (AgentRole and Instrument respectively).

The intention behind such a simple role is to have a way to represent, in a schematic formalism used to describe some scene, that an object is present. In particular, the schema used to convey this information is the ESTSchemaTheory, which has ExistingObjectRole as its sole defined role.</rdfs:comment>
        <rdfs:isDefinedBy rdf:resource="http://www.ease-crc.org/ont/SOMA-OBJ.owl"/>
        <rdfs:label xml:lang="en">Existing object role</rdfs:label>
    </owl:Class>
    


    <!-- http://www.ease-crc.org/ont/SOMA.owl#ExperiencerRole -->


    <owl:Class rdf:about="http://www.ease-crc.org/ont/SOMA.owl#ExperiencerRole">
        <rdfs:subClassOf rdf:resource="http://www.ease-crc.org/ont/SOMA.owl#AgentRole"/>
        <rdfs:comment>A role used in frame semantics to classify agents performing perception actions, or being the subjects affected by some biological process.</rdfs:comment>
        <rdfs:isDefinedBy rdf:resource="http://www.ease-crc.org/ont/SOMA-OBJ.owl"/>
        <rdfs:label xml:lang="en">Experiencer role</rdfs:label>
    </owl:Class>
    


    <!-- http://www.ease-crc.org/ont/SOMA.owl#ExtractedObject -->


    <owl:Class rdf:about="http://www.ease-crc.org/ont/SOMA.owl#ExtractedObject">
        <rdfs:subClassOf rdf:resource="http://www.ease-crc.org/ont/SOMA.owl#Patient"/>
        <rdfs:comment>An object that is removed from a container or system.</rdfs:comment>
        <rdfs:isDefinedBy rdf:resource="http://www.ease-crc.org/ont/SOMA-OBJ.owl"/>
        <rdfs:label xml:lang="en">Extracted object</rdfs:label>
    </owl:Class>
    


    <!-- http://www.ease-crc.org/ont/SOMA.owl#Extrinsic -->


    <owl:Class rdf:about="http://www.ease-crc.org/ont/SOMA.owl#Extrinsic">
        <rdfs:subClassOf rdf:resource="http://www.ease-crc.org/ont/SOMA.owl#PhysicalQuality"/>
        <owl:disjointWith rdf:resource="http://www.ease-crc.org/ont/SOMA.owl#Intrinsic"/>
        <rdfs:comment>A physical quality that depends on relationships to other objects, such as the color of an object which depends on light conditions in the environment.</rdfs:comment>
        <rdfs:isDefinedBy rdf:resource="http://www.ease-crc.org/ont/SOMA-OBJ.owl"/>
    </owl:Class>
    


    <!-- http://www.ease-crc.org/ont/SOMA.owl#FactualBinding -->


    <owl:Class rdf:about="http://www.ease-crc.org/ont/SOMA.owl#FactualBinding">
        <rdfs:subClassOf rdf:resource="http://www.ease-crc.org/ont/SOMA.owl#Binding"/>
        <rdfs:comment>FactualBindings are used in a workflow to assert that:

-- task- or workflow-defined roles share fillers (RoleRoleBindings). Example, the instrument of a cutting task may be the actee of a grasping task;
-- task- or workflow-defined roles are filled by a particular entity (RoleFillerBindings). This is typically the case when roles, and especially parameters, can be assigned to constants. Example, the waiting time to cook soft eggs is 3 minutes.</rdfs:comment>
        <rdfs:isDefinedBy rdf:resource="http://www.ease-crc.org/ont/SOMA-WF.owl"/>
        <rdfs:label xml:lang="en">Factial binding</rdfs:label>
    </owl:Class>
    


    <!-- http://www.ease-crc.org/ont/SOMA.owl#FaultySoftware -->


    <owl:Class rdf:about="http://www.ease-crc.org/ont/SOMA.owl#FaultySoftware">
        <rdfs:subClassOf rdf:resource="http://www.ease-crc.org/ont/SOMA.owl#SoftwareDiagnosis"/>
        <rdfs:comment>A description of a situation where some software has a bug.</rdfs:comment>
        <rdfs:isDefinedBy rdf:resource="http://www.ease-crc.org/ont/SOMA-IO.owl"/>
        <rdfs:label xml:lang="en">Faulty software</rdfs:label>
    </owl:Class>
    


    <!-- http://www.ease-crc.org/ont/SOMA.owl#Feature -->


    <owl:Class rdf:about="http://www.ease-crc.org/ont/SOMA.owl#Feature">
        <rdfs:subClassOf rdf:resource="http://www.ontologydesignpatterns.org/ont/dul/DUL.owl#Object"/>
        <rdfs:subClassOf>
            <owl:Restriction>
                <owl:onProperty rdf:resource="http://www.ontologydesignpatterns.org/ont/dul/DUL.owl#hasPart"/>
                <owl:allValuesFrom rdf:resource="http://www.ease-crc.org/ont/SOMA.owl#Feature"/>
            </owl:Restriction>
        </rdfs:subClassOf>
        <rdfs:subClassOf>
            <owl:Restriction>
                <owl:onProperty rdf:resource="http://www.ease-crc.org/ont/SOMA.owl#isFeatureOf"/>
                <owl:qualifiedCardinality rdf:datatype="http://www.w3.org/2001/XMLSchema#nonNegativeInteger">1</owl:qualifiedCardinality>
                <owl:onClass rdf:resource="http://www.ontologydesignpatterns.org/ont/dul/DUL.owl#PhysicalObject"/>
            </owl:Restriction>
        </rdfs:subClassOf>
        <owl:disjointWith rdf:resource="http://www.ontologydesignpatterns.org/ont/dul/DUL.owl#Agent"/>
        <owl:disjointWith rdf:resource="http://www.ontologydesignpatterns.org/ont/dul/DUL.owl#PhysicalObject"/>
        <owl:disjointWith rdf:resource="http://www.ontologydesignpatterns.org/ont/dul/DUL.owl#SocialObject"/>
        <rdfs:comment>Features are &apos;parasitic&apos; entities that only exist insofar their host exists. Typical examples are holes, bumps, boundaries, or spots of color.</rdfs:comment>
        <rdfs:isDefinedBy rdf:resource="http://www.ease-crc.org/ont/SOMA-OBJ.owl"/>
    </owl:Class>
    


    <!-- http://www.ease-crc.org/ont/SOMA.owl#Fetching -->


    <owl:Class rdf:about="http://www.ease-crc.org/ont/SOMA.owl#Fetching">
        <rdfs:subClassOf rdf:resource="http://www.ease-crc.org/ont/SOMA.owl#PhysicalAcquiring"/>
        <owl:disjointWith rdf:resource="http://www.ease-crc.org/ont/SOMA.owl#Lifting"/>
        <owl:disjointWith rdf:resource="http://www.ease-crc.org/ont/SOMA.owl#Opening"/>
        <owl:disjointWith rdf:resource="http://www.ease-crc.org/ont/SOMA.owl#Pulling"/>
        <owl:disjointWith rdf:resource="http://www.ease-crc.org/ont/SOMA.owl#Pushing"/>
        <owl:disjointWith rdf:resource="http://www.ease-crc.org/ont/SOMA.owl#Squeezing"/>
        <rdfs:comment>A task in which an Agent retrieves an object from a particular location, which puts the object under the Agent&apos;s control, who can now e.g. transport the object somewhere else; this task may include repositioning the Agent to better reach the object. Note that while in normal linguistic use fetch can mean transport, we use it here to refer only to (a part of) the first stage of transport.</rdfs:comment>
        <rdfs:isDefinedBy rdf:resource="http://www.ease-crc.org/ont/SOMA-ACT.owl"/>
    </owl:Class>
    


    <!-- http://www.ease-crc.org/ont/SOMA.owl#FileConfiguration -->


    <owl:Class rdf:about="http://www.ease-crc.org/ont/SOMA.owl#FileConfiguration">
        <owl:equivalentClass>
            <owl:Class>
                <owl:intersectionOf rdf:parseType="Collection">
                    <rdf:Description rdf:about="http://www.ontologydesignpatterns.org/ont/dul/DUL.owl#Configuration"/>
                    <owl:Restriction>
                        <owl:onProperty rdf:resource="http://www.ontologydesignpatterns.org/ont/dul/DUL.owl#hasMember"/>
                        <owl:allValuesFrom rdf:resource="http://www.ease-crc.org/ont/SOMA.owl#Digital_File"/>
                    </owl:Restriction>
                </owl:intersectionOf>
            </owl:Class>
        </owl:equivalentClass>
        <rdfs:comment xml:lang="en">A configuration whose members are all files. Used to model, e.g., concrete collections of zip- and jar-files (and so on).</rdfs:comment>
        <rdfs:isDefinedBy rdf:resource="http://www.ease-crc.org/ont/SOMA-IO.owl"/>
        <rdfs:label xml:lang="en">File Configuration</rdfs:label>
    </owl:Class>
    


    <!-- http://www.ease-crc.org/ont/SOMA.owl#File_format -->


    <owl:Class rdf:about="http://www.ease-crc.org/ont/SOMA.owl#File_format">
        <rdfs:subClassOf rdf:resource="http://www.ease-crc.org/ont/SOMA.owl#Computer_Language"/>
        <rdfs:comment xml:lang="en">A File Format is a standard way that information is encoded for storage in a computer file. It specifies how bits are used to encode information in a digital storage medium.

From Wikipedia: https://en.wikipedia.org/wiki/File_format</rdfs:comment>
        <rdfs:isDefinedBy rdf:resource="http://www.ease-crc.org/ont/SOMA-IO.owl"/>
        <rdfs:label xml:lang="en">File Format</rdfs:label>
    </owl:Class>
    


    <!-- http://www.ease-crc.org/ont/SOMA.owl#Finger -->


    <owl:Class rdf:about="http://www.ease-crc.org/ont/SOMA.owl#Finger">
        <rdfs:subClassOf rdf:resource="http://www.ease-crc.org/ont/SOMA.owl#Limb"/>
        <rdfs:subClassOf>
            <owl:Restriction>
                <owl:onProperty rdf:resource="http://www.ontologydesignpatterns.org/ont/dul/DUL.owl#isPartOf"/>
                <owl:someValuesFrom rdf:resource="http://www.ease-crc.org/ont/SOMA.owl#Hand"/>
            </owl:Restriction>
        </rdfs:subClassOf>
        <rdfs:comment>A limb used for grasping objects.</rdfs:comment>
        <rdfs:isDefinedBy rdf:resource="http://www.ease-crc.org/ont/SOMA-OBJ.owl"/>
    </owl:Class>
    


    <!-- http://www.ease-crc.org/ont/SOMA.owl#Floor -->


    <owl:Class rdf:about="http://www.ease-crc.org/ont/SOMA.owl#Floor">
        <rdfs:subClassOf rdf:resource="http://www.ease-crc.org/ont/SOMA.owl#RoomSurface"/>
        <owl:disjointWith rdf:resource="http://www.ease-crc.org/ont/SOMA.owl#Wall"/>
        <rdfs:comment>The lower interior surface of a room.</rdfs:comment>
        <rdfs:isDefinedBy rdf:resource="http://www.ease-crc.org/ont/SOMA-HOME.owl"/>
    </owl:Class>
    


    <!-- http://www.ease-crc.org/ont/SOMA.owl#Fluid -->


    <owl:Class rdf:about="http://www.ease-crc.org/ont/SOMA.owl#Fluid">
        <rdfs:isDefinedBy rdf:resource="http://www.ease-crc.org/ont/SOMA-PROC.owl"/>
    </owl:Class>
    


    <!-- http://www.ease-crc.org/ont/SOMA.owl#FluidFlow -->


    <owl:Class rdf:about="http://www.ease-crc.org/ont/SOMA.owl#FluidFlow">
        <rdfs:subClassOf rdf:resource="http://www.ease-crc.org/ont/SOMA.owl#Motion"/>
        <rdfs:subClassOf>
            <owl:Restriction>
                <owl:onProperty rdf:resource="http://www.ease-crc.org/ont/SOMA.owl#isProcessTypeOf"/>
                <owl:someValuesFrom rdf:resource="http://www.ease-crc.org/ont/SOMA.owl#MovedObject"/>
            </owl:Restriction>
        </rdfs:subClassOf>
        <rdfs:comment>A process by which a fluid moves or is moved from a location to another, but such that it maintains its constitution. A fluid is an Entity made of many smaller Entities, loosely bound to each other.

An issue to highlight here is the maintenance of constitution. Fluids-- gases in particular-- are prone to disperse. Such a process is not flow however, because the loose bounds between the constituents become even looser, to the point of the original Entity becoming entirely discombobulated. </rdfs:comment>
        <rdfs:isDefinedBy rdf:resource="http://www.ease-crc.org/ont/SOMA-PROC.owl"/>
        <rdfs:label>Fluid flow</rdfs:label>
    </owl:Class>
    


    <!-- http://www.ease-crc.org/ont/SOMA.owl#Flying -->


    <owl:Class rdf:about="http://www.ease-crc.org/ont/SOMA.owl#Flying">
        <rdfs:subClassOf rdf:resource="http://www.ease-crc.org/ont/SOMA.owl#Locomotion"/>
        <owl:disjointWith rdf:resource="http://www.ease-crc.org/ont/SOMA.owl#Swimming"/>
        <owl:disjointWith rdf:resource="http://www.ease-crc.org/ont/SOMA.owl#Walking"/>
        <rdfs:comment>A process type classifying a motion of a body that, through its own power, keeps itself aloft.</rdfs:comment>
        <rdfs:isDefinedBy rdf:resource="http://www.ease-crc.org/ont/SOMA-PROC.owl"/>
    </owl:Class>
    


    <!-- http://www.ease-crc.org/ont/SOMA.owl#ForceInteraction -->


    <owl:Class rdf:about="http://www.ease-crc.org/ont/SOMA.owl#ForceInteraction">
        <owl:equivalentClass>
            <owl:Class>
                <owl:unionOf rdf:parseType="Collection">
                    <rdf:Description rdf:about="http://www.ease-crc.org/ont/SOMA.owl#AlterativeInteraction"/>
                    <rdf:Description rdf:about="http://www.ease-crc.org/ont/SOMA.owl#PreservativeInteraction"/>
                </owl:unionOf>
            </owl:Class>
        </owl:equivalentClass>
        <rdfs:subClassOf rdf:resource="http://www.ease-crc.org/ont/SOMA.owl#ProcessType"/>
        <rdfs:subClassOf>
            <owl:Restriction>
                <owl:onProperty rdf:resource="http://www.ease-crc.org/ont/SOMA.owl#isProcessTypeOf"/>
                <owl:someValuesFrom rdf:resource="http://www.ease-crc.org/ont/SOMA.owl#Agonist"/>
            </owl:Restriction>
        </rdfs:subClassOf>
        <rdfs:subClassOf>
            <owl:Restriction>
                <owl:onProperty rdf:resource="http://www.ease-crc.org/ont/SOMA.owl#isProcessTypeOf"/>
                <owl:someValuesFrom rdf:resource="http://www.ease-crc.org/ont/SOMA.owl#Antagonist"/>
            </owl:Restriction>
        </rdfs:subClassOf>
        <rdfs:comment>Classifies events in which two entities interact with each other with a reference to force. One of the entities, the agonist, has a tendency to either set the other entity (the antagonist) into motion, or to keep it still under the influence of some other force. The tendency only manifests in case the agonist is the &quot;stronger entity&quot;.</rdfs:comment>
        <rdfs:isDefinedBy rdf:resource="http://www.ease-crc.org/ont/SOMA-PROC.owl"/>
        <rdfs:label>Force interaction</rdfs:label>
        <rdfs:seeAlso>Talmy, Leonard (1981) ‘Force Dynamics’. Language and Mental Imagery. May 1981, University of California, Berkeley.</rdfs:seeAlso>
    </owl:Class>
    


    <!-- http://www.ease-crc.org/ont/SOMA.owl#Fork -->


    <owl:Class rdf:about="http://www.ease-crc.org/ont/SOMA.owl#Fork">
        <rdfs:subClassOf rdf:resource="http://www.ease-crc.org/ont/SOMA.owl#Cutlery"/>
        <rdfs:subClassOf>
            <owl:Restriction>
                <owl:onProperty rdf:resource="http://www.ease-crc.org/ont/SOMA.owl#hasPhysicalComponent"/>
                <owl:someValuesFrom rdf:resource="http://www.ease-crc.org/ont/SOMA.owl#DesignedHandle"/>
            </owl:Restriction>
        </rdfs:subClassOf>
        <rdfs:comment>Cutlery with two or more prongs used for lifting food to the mouth or holding it when cutting.</rdfs:comment>
        <rdfs:isDefinedBy rdf:resource="http://www.ease-crc.org/ont/SOMA-HOME.owl"/>
    </owl:Class>
    


    <!-- http://www.ease-crc.org/ont/SOMA.owl#FormalLanguage -->


    <owl:Class rdf:about="http://www.ease-crc.org/ont/SOMA.owl#FormalLanguage">
        <rdfs:subClassOf rdf:resource="http://www.ease-crc.org/ont/SOMA.owl#Language"/>
        <rdfs:subClassOf>
            <owl:Restriction>
                <owl:onProperty rdf:resource="http://www.ease-crc.org/ont/SOMA.owl#givesMeaningTo"/>
                <owl:allValuesFrom rdf:resource="http://www.ease-crc.org/ont/SOMA.owl#Structured_Text"/>
            </owl:Restriction>
        </rdfs:subClassOf>
        <rdfs:comment xml:lang="en">A Formal Language consists of words whose letters are taken from an alphabet and are well-formed according to a specific set of rules.

From Wikipedia: https://en.wikipedia.org/wiki/Formal_language</rdfs:comment>
        <rdfs:isDefinedBy rdf:resource="http://www.ease-crc.org/ont/SOMA-IO.owl"/>
        <rdfs:label xml:lang="en">Formal Language</rdfs:label>
    </owl:Class>
    


    <!-- http://www.ease-crc.org/ont/SOMA.owl#FreezerCompartment -->


    <owl:Class rdf:about="http://www.ease-crc.org/ont/SOMA.owl#FreezerCompartment">
        <rdfs:subClassOf rdf:resource="http://www.ease-crc.org/ont/SOMA.owl#Compartment"/>
        <rdfs:comment>A freezer compartment used to regulate the temperature of contained objects to a value below zero degree Celsius.</rdfs:comment>
        <rdfs:isDefinedBy rdf:resource="http://www.ease-crc.org/ont/SOMA-HOME.owl"/>
    </owl:Class>
    


    <!-- http://www.ease-crc.org/ont/SOMA.owl#FrictionAttribute -->


    <owl:Class rdf:about="http://www.ease-crc.org/ont/SOMA.owl#FrictionAttribute">
        <rdfs:subClassOf rdf:resource="http://www.ontologydesignpatterns.org/ont/dul/DUL.owl#PhysicalAttribute"/>
        <rdfs:subClassOf>
            <owl:Restriction>
                <owl:onProperty rdf:resource="http://www.ease-crc.org/ont/SOMA.owl#hasFrictionValue"/>
                <owl:qualifiedCardinality rdf:datatype="http://www.w3.org/2001/XMLSchema#nonNegativeInteger">1</owl:qualifiedCardinality>
                <owl:onDataRange rdf:resource="http://www.w3.org/2001/XMLSchema#double"/>
            </owl:Restriction>
        </rdfs:subClassOf>
        <rdfs:comment>The resistance that one surface or object encounters when moving over another.</rdfs:comment>
        <rdfs:isDefinedBy rdf:resource="http://www.ease-crc.org/ont/SOMA-OBJ.owl"/>
        <rdfs:label>Friction attribute</rdfs:label>
    </owl:Class>
    


    <!-- http://www.ease-crc.org/ont/SOMA.owl#FunctionalControl -->


    <owl:Class rdf:about="http://www.ease-crc.org/ont/SOMA.owl#FunctionalControl">
        <rdfs:subClassOf rdf:resource="http://www.ease-crc.org/ont/SOMA.owl#StateType"/>
        <rdfs:subClassOf>
            <owl:Restriction>
                <owl:onProperty rdf:resource="http://www.ease-crc.org/ont/SOMA.owl#isStateTypeOf"/>
                <owl:someValuesFrom rdf:resource="http://www.ease-crc.org/ont/SOMA.owl#Item"/>
            </owl:Restriction>
        </rdfs:subClassOf>
        <rdfs:subClassOf>
            <owl:Restriction>
                <owl:onProperty rdf:resource="http://www.ease-crc.org/ont/SOMA.owl#isStateTypeOf"/>
                <owl:someValuesFrom rdf:resource="http://www.ease-crc.org/ont/SOMA.owl#Restrictor"/>
            </owl:Restriction>
        </rdfs:subClassOf>
        <rdfs:comment>Classifies States in which an object restricts the movement of another, at least partially. Usually neither object is construed to be an agent.

Note that this State focuses on how the interaction of, usually non-agentive, objects restricts their motion. This is in contrast to Blockage/Accessibility states where the placement of some objects influences the access to some of them by a third, usually agentive party.</rdfs:comment>
        <rdfs:isDefinedBy rdf:resource="http://www.ease-crc.org/ont/SOMA-STATE.owl"/>
        <rdfs:label xml:lang="en">Functional state</rdfs:label>
    </owl:Class>
    


    <!-- http://www.ease-crc.org/ont/SOMA.owl#FunctionalDesign -->


    <owl:Class rdf:about="http://www.ease-crc.org/ont/SOMA.owl#FunctionalDesign">
        <rdfs:subClassOf rdf:resource="http://www.ontologydesignpatterns.org/ont/dul/DUL.owl#Design"/>
        <rdfs:comment>The design of an object from functionality point of view. A functional design is useful to develop complex modular objects with components that have a specific purpose, and can function with minimum side effect on other components of that object. </rdfs:comment>
        <rdfs:isDefinedBy rdf:resource="http://www.ease-crc.org/ont/SOMA-OBJ.owl"/>
        <rdfs:label>Functional Design</rdfs:label>
    </owl:Class>
    


    <!-- http://www.ease-crc.org/ont/SOMA.owl#FunctionalPart -->


    <owl:Class rdf:about="http://www.ease-crc.org/ont/SOMA.owl#FunctionalPart">
        <rdfs:subClassOf rdf:resource="http://www.ontologydesignpatterns.org/ont/dul/DUL.owl#PhysicalBody"/>
        <rdfs:subClassOf>
            <owl:Restriction>
                <owl:onProperty rdf:resource="http://www.ontologydesignpatterns.org/ont/dul/DUL.owl#isComponentOf"/>
                <owl:allValuesFrom>
                    <owl:Class>
                        <owl:unionOf rdf:parseType="Collection">
                            <rdf:Description rdf:about="http://www.ontologydesignpatterns.org/ont/dul/DUL.owl#Agent"/>
                            <rdf:Description rdf:about="http://www.ontologydesignpatterns.org/ont/dul/DUL.owl#DesignedArtifact"/>
                        </owl:unionOf>
                    </owl:Class>
                </owl:allValuesFrom>
            </owl:Restriction>
        </rdfs:subClassOf>
        <rdfs:comment>Parts of an agent or an artifact are considered as functional parts.</rdfs:comment>
        <rdfs:isDefinedBy rdf:resource="http://www.ease-crc.org/ont/SOMA-OBJ.owl"/>
        <rdfs:label>Functional part</rdfs:label>
    </owl:Class>
    


    <!-- http://www.ease-crc.org/ont/SOMA.owl#FunctionalSpatialSchemaTheory -->


    <owl:Class rdf:about="http://www.ease-crc.org/ont/SOMA.owl#FunctionalSpatialSchemaTheory">
        <rdfs:subClassOf rdf:resource="http://www.ease-crc.org/ont/SOMA.owl#ImageSchemaTheory"/>
        <rdfs:subClassOf>
            <owl:Restriction>
                <owl:onProperty rdf:resource="http://www.ontologydesignpatterns.org/ont/dul/DUL.owl#defines"/>
                <owl:someValuesFrom rdf:resource="http://www.ease-crc.org/ont/SOMA.owl#LocatumRole"/>
            </owl:Restriction>
        </rdfs:subClassOf>
        <rdfs:subClassOf>
            <owl:Restriction>
                <owl:onProperty rdf:resource="http://www.ontologydesignpatterns.org/ont/dul/DUL.owl#defines"/>
                <owl:someValuesFrom rdf:resource="http://www.ease-crc.org/ont/SOMA.owl#RelatumRole"/>
            </owl:Restriction>
        </rdfs:subClassOf>
        <rdfs:comment>The superclass for theories describing functional spatial relations.

Adopted from GUM-4-space (Bateman et al. 2010).</rdfs:comment>
        <rdfs:isDefinedBy rdf:resource="http://www.ease-crc.org/ont/SOMA-SAY.owl"/>
        <rdfs:label xml:lang="en">Functional spatial schema theory</rdfs:label>
    </owl:Class>
    


    <!-- http://www.ease-crc.org/ont/SOMA.owl#GetTaskParameter -->


    <owl:Class rdf:about="http://www.ease-crc.org/ont/SOMA.owl#GetTaskParameter">
        <rdfs:subClassOf rdf:resource="http://www.ease-crc.org/ont/SOMA.owl#MentalTask"/>
        <rdfs:comment>A task in which an Agent computes some parameter relevant for another task.</rdfs:comment>
        <rdfs:isDefinedBy rdf:resource="http://www.ease-crc.org/ont/SOMA-ACT.owl"/>
        <rdfs:label xml:lang="en">Get task parameter</rdfs:label>
    </owl:Class>
    


    <!-- http://www.ease-crc.org/ont/SOMA.owl#GoalRole -->


    <owl:Class rdf:about="http://www.ease-crc.org/ont/SOMA.owl#GoalRole">
        <rdfs:subClassOf rdf:resource="http://www.ease-crc.org/ont/SOMA.owl#EventAdjacentRole"/>
        <rdfs:comment>A role classifying objects that constitute the goal of an action.</rdfs:comment>
        <rdfs:isDefinedBy rdf:resource="http://www.ease-crc.org/ont/SOMA-OBJ.owl"/>
        <rdfs:label xml:lang="en">Goal role</rdfs:label>
    </owl:Class>
    


    <!-- http://www.ease-crc.org/ont/SOMA.owl#GraphDatabase -->


    <owl:Class rdf:about="http://www.ease-crc.org/ont/SOMA.owl#GraphDatabase">
        <rdfs:subClassOf rdf:resource="http://www.ease-crc.org/ont/SOMA.owl#Database"/>
        <rdfs:comment xml:lang="en">A Graph Database is a Database that uses graph structures for semantic queries with nodes, edges, and properties to represent and store data.</rdfs:comment>
        <rdfs:isDefinedBy rdf:resource="http://www.ease-crc.org/ont/SOMA-IO.owl"/>
        <rdfs:label xml:lang="en">Graph database</rdfs:label>
    </owl:Class>
    


    <!-- http://www.ease-crc.org/ont/SOMA.owl#GraphQueryLanguage -->


    <owl:Class rdf:about="http://www.ease-crc.org/ont/SOMA.owl#GraphQueryLanguage">
        <rdfs:subClassOf rdf:resource="http://www.ease-crc.org/ont/SOMA.owl#QueryLanguage"/>
        <rdfs:comment xml:lang="en">A Query Language that is designed for communication with some Graph Database.</rdfs:comment>
        <rdfs:isDefinedBy rdf:resource="http://www.ease-crc.org/ont/SOMA-IO.owl"/>
        <rdfs:label xml:lang="en">Graph query language</rdfs:label>
    </owl:Class>
    


    <!-- http://www.ease-crc.org/ont/SOMA.owl#GraspTransfer -->


    <owl:Class rdf:about="http://www.ease-crc.org/ont/SOMA.owl#GraspTransfer">
        <rdfs:subClassOf rdf:resource="http://www.ease-crc.org/ont/SOMA.owl#Grasping"/>
        <rdfs:comment>A task in which an Agent switches which of its end effectors holds an object.</rdfs:comment>
        <rdfs:isDefinedBy rdf:resource="http://www.ease-crc.org/ont/SOMA-ACT.owl"/>
        <rdfs:label xml:lang="en">Grasp transfer</rdfs:label>
    </owl:Class>
    


    <!-- http://www.ease-crc.org/ont/SOMA.owl#Graspability -->


    <owl:Class rdf:about="http://www.ease-crc.org/ont/SOMA.owl#Graspability">
        <rdfs:subClassOf rdf:resource="http://www.ease-crc.org/ont/SOMA.owl#Disposition"/>
        <rdfs:comment>The disposition of an object (e.g. the handle) to afford grasping the object.</rdfs:comment>
        <rdfs:isDefinedBy rdf:resource="http://www.ease-crc.org/ont/SOMA-HOME.owl"/>
        <rdfs:isDefinedBy rdf:resource="http://www.ease-crc.org/ont/SOMA-OBJ.owl"/>
    </owl:Class>
    


    <!-- http://www.ease-crc.org/ont/SOMA.owl#Grasping -->


    <owl:Class rdf:about="http://www.ease-crc.org/ont/SOMA.owl#Grasping">
        <rdfs:subClassOf rdf:resource="http://www.ease-crc.org/ont/SOMA.owl#Manipulating"/>
        <owl:disjointWith rdf:resource="http://www.ease-crc.org/ont/SOMA.owl#Releasing"/>
        <rdfs:comment>A task in which an Agent uses its end effectors to grasp an object, thus gaining kinematic control over it.</rdfs:comment>
        <rdfs:isDefinedBy rdf:resource="http://www.ease-crc.org/ont/SOMA-ACT.owl"/>
    </owl:Class>
    


    <!-- http://www.ease-crc.org/ont/SOMA.owl#GraspingMotion -->


    <owl:Class rdf:about="http://www.ease-crc.org/ont/SOMA.owl#GraspingMotion">
        <owl:equivalentClass>
            <owl:Class>
                <owl:unionOf rdf:parseType="Collection">
                    <rdf:Description rdf:about="http://www.ease-crc.org/ont/SOMA.owl#IntermediateGrasp"/>
                    <rdf:Description rdf:about="http://www.ease-crc.org/ont/SOMA.owl#PowerGrasp"/>
                    <rdf:Description rdf:about="http://www.ease-crc.org/ont/SOMA.owl#PrecisionGrasp"/>
                </owl:unionOf>
            </owl:Class>
        </owl:equivalentClass>
        <rdfs:subClassOf rdf:resource="http://www.ease-crc.org/ont/SOMA.owl#PrehensileMotion"/>
        <owl:disjointWith rdf:resource="http://www.ease-crc.org/ont/SOMA.owl#ReleasingMotion"/>
        <rdfs:comment>A process type classifying a motion by which some end effector acquires kinematic control over some other object.</rdfs:comment>
        <rdfs:isDefinedBy rdf:resource="http://www.ease-crc.org/ont/SOMA-PROC.owl"/>
        <rdfs:label>Grasping motion</rdfs:label>
    </owl:Class>
    


    <!-- http://www.ease-crc.org/ont/SOMA.owl#GreenColor -->


    <owl:Class rdf:about="http://www.ease-crc.org/ont/SOMA.owl#GreenColor">
        <rdfs:subClassOf rdf:resource="http://www.ease-crc.org/ont/SOMA.owl#ColorRegion"/>
        <rdfs:comment>A color region with dominant green color.</rdfs:comment>
        <rdfs:isDefinedBy rdf:resource="http://www.ease-crc.org/ont/SOMA-OBJ.owl"/>
        <rdfs:label>Green color</rdfs:label>
    </owl:Class>
    


    <!-- http://www.ease-crc.org/ont/SOMA.owl#Gripper -->


    <owl:Class rdf:about="http://www.ease-crc.org/ont/SOMA.owl#Gripper">
        <rdfs:subClassOf rdf:resource="http://www.ease-crc.org/ont/SOMA.owl#PrehensileEffector"/>
        <rdfs:comment>A mechanical device that grasps and holds things.</rdfs:comment>
        <rdfs:isDefinedBy rdf:resource="http://www.ease-crc.org/ont/SOMA-OBJ.owl"/>
    </owl:Class>
    


    <!-- http://www.ease-crc.org/ont/SOMA.owl#Hand -->


    <owl:Class rdf:about="http://www.ease-crc.org/ont/SOMA.owl#Hand">
        <rdfs:subClassOf rdf:resource="http://www.ease-crc.org/ont/SOMA.owl#PrehensileEffector"/>
        <rdfs:comment>A prehensile effector including palm, fingers, and thumb.</rdfs:comment>
        <rdfs:isDefinedBy rdf:resource="http://www.ease-crc.org/ont/SOMA-OBJ.owl"/>
    </owl:Class>
    


    <!-- http://www.ease-crc.org/ont/SOMA.owl#HasQualityRegion -->


    <owl:Class rdf:about="http://www.ease-crc.org/ont/SOMA.owl#HasQualityRegion">
        <rdfs:subClassOf rdf:resource="http://www.ontologydesignpatterns.org/ont/dul/DUL.owl#Relation"/>
        <rdfs:subClassOf>
            <owl:Restriction>
                <owl:onProperty rdf:resource="http://www.ontologydesignpatterns.org/ont/dul/DUL.owl#hasQuality"/>
                <owl:qualifiedCardinality rdf:datatype="http://www.w3.org/2001/XMLSchema#nonNegativeInteger">1</owl:qualifiedCardinality>
                <owl:onClass rdf:resource="http://www.ontologydesignpatterns.org/ont/dul/DUL.owl#Quality"/>
            </owl:Restriction>
        </rdfs:subClassOf>
        <rdfs:subClassOf>
            <owl:Restriction>
                <owl:onProperty rdf:resource="http://www.ontologydesignpatterns.org/ont/dul/DUL.owl#hasRegion"/>
                <owl:qualifiedCardinality rdf:datatype="http://www.w3.org/2001/XMLSchema#nonNegativeInteger">1</owl:qualifiedCardinality>
                <owl:onClass rdf:resource="http://www.ontologydesignpatterns.org/ont/dul/DUL.owl#Region"/>
            </owl:Restriction>
        </rdfs:subClassOf>
        <rdfs:comment>The relation between an individual quality and a region.</rdfs:comment>
        <rdfs:comment>todo(DB): added for NEEMs (quale change), but not sure yet about it...</rdfs:comment>
        <rdfs:isDefinedBy rdf:resource="http://www.ease-crc.org/ont/SOMA-OBJ.owl"/>
        <rdfs:label xml:lang="en">Has quality region</rdfs:label>
    </owl:Class>
    


    <!-- http://www.ease-crc.org/ont/SOMA.owl#Head -->


    <owl:Class rdf:about="http://www.ease-crc.org/ont/SOMA.owl#Head">
        <rdfs:subClassOf rdf:resource="http://www.ease-crc.org/ont/SOMA.owl#FunctionalPart"/>
        <rdfs:comment>A functional part of the body responsible for carrying high bandwidth sensors, i.e., camera.</rdfs:comment>
        <rdfs:isDefinedBy rdf:resource="http://www.ease-crc.org/ont/SOMA-OBJ.owl"/>
    </owl:Class>
    


    <!-- http://www.ease-crc.org/ont/SOMA.owl#HeadMovement -->


    <owl:Class rdf:about="http://www.ease-crc.org/ont/SOMA.owl#HeadMovement">
        <rdfs:subClassOf rdf:resource="http://www.ease-crc.org/ont/SOMA.owl#BodyMovement"/>
        <rdfs:comment>The Agent moves a part of their body carrying high-bandwidth sensors such as cameras. The movement of other body parts is not significant.</rdfs:comment>
        <rdfs:comment>todo: (Mihai:) This seems too specific, given the &quot;Directed&quot;/&quot;Undirected motion&quot; categories.</rdfs:comment>
        <rdfs:isDefinedBy rdf:resource="http://www.ease-crc.org/ont/SOMA-PROC.owl"/>
    </owl:Class>
    


    <!-- http://www.ease-crc.org/ont/SOMA.owl#HeadTurning -->


    <owl:Class rdf:about="http://www.ease-crc.org/ont/SOMA.owl#HeadTurning">
        <rdfs:subClassOf rdf:resource="http://www.ease-crc.org/ont/SOMA.owl#HeadMovement"/>
        <rdfs:comment>A process type classifying a motion of an Agent&apos;s head such that the direction this head faces changes relative to the facing direction of the Agent&apos;s body as a whole.</rdfs:comment>
        <rdfs:isDefinedBy rdf:resource="http://www.ease-crc.org/ont/SOMA-PROC.owl"/>
    </owl:Class>
    


    <!-- http://www.ease-crc.org/ont/SOMA.owl#Holding -->


    <owl:Class rdf:about="http://www.ease-crc.org/ont/SOMA.owl#Holding">
        <rdfs:subClassOf rdf:resource="http://www.ease-crc.org/ont/SOMA.owl#Manipulating"/>
        <rdfs:comment>A task by which an Agent keeps an object over which it has kinematic control, typically via grasping, at some specified pose.</rdfs:comment>
        <rdfs:isDefinedBy rdf:resource="http://www.ease-crc.org/ont/SOMA-ACT.owl"/>
    </owl:Class>
    


    <!-- http://www.ease-crc.org/ont/SOMA.owl#HostRole -->


    <owl:Class rdf:about="http://www.ease-crc.org/ont/SOMA.owl#HostRole">
        <rdfs:subClassOf rdf:resource="http://www.ease-crc.org/ont/SOMA.owl#InterfaceComponentRole"/>
        <rdfs:subClassOf>
            <owl:Restriction>
                <owl:onProperty rdf:resource="http://www.ontologydesignpatterns.org/ont/dul/DUL.owl#isDefinedIn"/>
                <owl:someValuesFrom rdf:resource="http://www.ease-crc.org/ont/SOMA.owl#PluginSpecification"/>
            </owl:Restriction>
        </rdfs:subClassOf>
        <rdfs:comment xml:lang="en">In the Plug-in-Host pattern, a Host application provides services which the Plug-in can use, including a way for Plug-ins to register themselves with the Host application and a protocol for the exchange of data withPplug-ins. Plug-ins depend on the services provided by the host application and do not usually work by themselves. Conversely, the host application operates independently of the plug-ins, making it possible for end-users to add and update plug-ins dynamically without needing to make changes to the host application.

Source: https://en.wikipedia.org/wiki/Plug-in_(computing)</rdfs:comment>
        <rdfs:isDefinedBy rdf:resource="http://www.ease-crc.org/ont/SOMA-IO.owl"/>
        <rdfs:label xml:lang="en">Host role</rdfs:label>
    </owl:Class>
    


    <!-- http://www.ease-crc.org/ont/SOMA.owl#Hotplate -->


    <owl:Class rdf:about="http://www.ease-crc.org/ont/SOMA.owl#Hotplate">
        <rdfs:subClassOf rdf:resource="http://www.ease-crc.org/ont/SOMA.owl#DesignedComponent"/>
        <rdfs:comment>A flat heated surface used for cooking food or keeping it hot.</rdfs:comment>
        <rdfs:isDefinedBy rdf:resource="http://www.ease-crc.org/ont/SOMA-HOME.owl"/>
    </owl:Class>
    


    <!-- http://www.ease-crc.org/ont/SOMA.owl#Human-readable_Programming_Language -->


    <owl:Class rdf:about="http://www.ease-crc.org/ont/SOMA.owl#Human-readable_Programming_Language">
        <rdfs:subClassOf rdf:resource="http://www.ease-crc.org/ont/SOMA.owl#Programming_Language"/>
        <rdfs:subClassOf>
            <owl:Restriction>
                <owl:onProperty rdf:resource="http://www.ease-crc.org/ont/SOMA.owl#givesMeaningTo"/>
                <owl:allValuesFrom rdf:resource="http://www.ease-crc.org/ont/SOMA.owl#Source_Code"/>
            </owl:Restriction>
        </rdfs:subClassOf>
        <rdfs:comment xml:lang="en">A Programming language like Java, Python etc. but not binary machine code.</rdfs:comment>
        <rdfs:isDefinedBy rdf:resource="http://www.ease-crc.org/ont/SOMA-IO.owl"/>
        <rdfs:label xml:lang="en">Human-readable Programming Language</rdfs:label>
    </owl:Class>
    


    <!-- http://www.ease-crc.org/ont/SOMA.owl#IllocutionaryTask -->


    <owl:Class rdf:about="http://www.ease-crc.org/ont/SOMA.owl#IllocutionaryTask">
        <rdfs:subClassOf>
            <owl:Class>
                <owl:intersectionOf rdf:parseType="Collection">
                    <rdf:Description rdf:about="http://www.ease-crc.org/ont/SOMA.owl#CommunicationTask"/>
                    <owl:Restriction>
                        <owl:onProperty rdf:resource="http://www.ontologydesignpatterns.org/ont/dul/DUL.owl#classifies"/>
                        <owl:allValuesFrom>
                            <owl:Restriction>
                                <owl:onProperty rdf:resource="http://www.ontologydesignpatterns.org/ont/dul/DUL.owl#hasParticipant"/>
                                <owl:allValuesFrom>
                                    <owl:Class>
                                        <owl:unionOf rdf:parseType="Collection">
                                            <rdf:Description rdf:about="http://www.ontologydesignpatterns.org/ont/dul/DUL.owl#Agent"/>
                                            <rdf:Description rdf:about="http://www.ontologydesignpatterns.org/ont/dul/DUL.owl#SocialObject"/>
                                        </owl:unionOf>
                                    </owl:Class>
                                </owl:allValuesFrom>
                            </owl:Restriction>
                        </owl:allValuesFrom>
                    </owl:Restriction>
                </owl:intersectionOf>
            </owl:Class>
        </rdfs:subClassOf>
        <rdfs:comment xml:lang="en">A task which is executed by a Locution action: A Locution is what was said and meant, Illocution is what was done.

When somebody says &quot;Is there any salt?&quot; at the dinner table, the illocutionary act is a request: &quot;please give me some salt&quot; even though the locutionary act (the literal sentence) was to ask a question about the presence of salt.

Source: https://en.wikipedia.org/wiki/Illocutionary_act</rdfs:comment>
        <rdfs:isDefinedBy rdf:resource="http://www.ease-crc.org/ont/SOMA-ACT.owl"/>
        <rdfs:label xml:lang="en">Illocutionary act</rdfs:label>
    </owl:Class>
    


    <!-- http://www.ease-crc.org/ont/SOMA.owl#ImageSchemaTheory -->


    <owl:Class rdf:about="http://www.ease-crc.org/ont/SOMA.owl#ImageSchemaTheory">
        <rdfs:subClassOf rdf:resource="http://www.ease-crc.org/ont/SOMA.owl#SchematicTheory"/>
        <rdfs:comment>A theory that describes an image-schematic relationship between some entities.

Image schemas are considered as fundamental, pre-conceptual, building blocks of cognition. They were introduced to characterize how human beings are believed to organize and make sense of experience.

For SOMA, whereas the focus of executable schematic theories is to describe how an agent might act, image schematic theories focus on descriptions of how objects behave in the absence of, or after, an active intervention from an agent.</rdfs:comment>
        <rdfs:isDefinedBy rdf:resource="http://www.ease-crc.org/ont/SOMA-SAY.owl"/>
        <rdfs:label xml:lang="en">Image schema theory</rdfs:label>
    </owl:Class>
    


    <!-- http://www.ease-crc.org/ont/SOMA.owl#Imagining -->


    <owl:Class rdf:about="http://www.ease-crc.org/ont/SOMA.owl#Imagining">
        <rdfs:subClassOf rdf:resource="http://www.ease-crc.org/ont/SOMA.owl#MentalTask"/>
        <rdfs:comment>A Mental task in which the Agent constructs a mental representation of a possible world. An Agent performing an Imagining activity does not aim to construct a representation that aspires to be faithful to some past, present, or future state of affairs of the actual world it is embodied in.</rdfs:comment>
        <rdfs:isDefinedBy rdf:resource="http://www.ease-crc.org/ont/SOMA-ACT.owl"/>
    </owl:Class>
    


    <!-- http://www.ease-crc.org/ont/SOMA.owl#Impediment -->


    <owl:Class rdf:about="http://www.ease-crc.org/ont/SOMA.owl#Impediment">
        <rdfs:subClassOf rdf:resource="http://www.ease-crc.org/ont/SOMA.owl#Blockage"/>
        <rdfs:subClassOf>
            <owl:Restriction>
                <owl:onProperty rdf:resource="http://www.ease-crc.org/ont/SOMA.owl#affordsBearer"/>
                <owl:allValuesFrom rdf:resource="http://www.ease-crc.org/ont/SOMA.owl#Obstacle"/>
            </owl:Restriction>
        </rdfs:subClassOf>
        <rdfs:subClassOf>
            <owl:Restriction>
                <owl:onProperty rdf:resource="http://www.ease-crc.org/ont/SOMA.owl#affordsTrigger"/>
                <owl:allValuesFrom rdf:resource="http://www.ease-crc.org/ont/SOMA.owl#RestrictedObject"/>
            </owl:Restriction>
        </rdfs:subClassOf>
        <rdfs:comment>The disposition of an object (the obstacle) to prohibit certain ways of entering or leaving a space or group. An example is a doorstopper constraining a door, prohibiting it to enter the area behind it.</rdfs:comment>
        <rdfs:isDefinedBy rdf:resource="http://www.ease-crc.org/ont/SOMA-OBJ.owl"/>
    </owl:Class>
    


    <!-- http://www.ease-crc.org/ont/SOMA.owl#ImperativeClause -->


    <owl:Class rdf:about="http://www.ease-crc.org/ont/SOMA.owl#ImperativeClause">
        <rdfs:subClassOf rdf:resource="http://www.ease-crc.org/ont/SOMA.owl#ClausalObject"/>
        <rdfs:subClassOf>
            <owl:Restriction>
                <owl:onProperty rdf:resource="http://www.ontologydesignpatterns.org/ont/dul/DUL.owl#expresses"/>
                <owl:someValuesFrom rdf:resource="http://www.ease-crc.org/ont/SOMA.owl#StateTransition"/>
            </owl:Restriction>
        </rdfs:subClassOf>
        <rdfs:subClassOf>
            <owl:Restriction>
                <owl:onProperty rdf:resource="http://www.ontologydesignpatterns.org/ont/dul/DUL.owl#expresses"/>
                <owl:allValuesFrom rdf:resource="http://www.ease-crc.org/ont/SOMA.owl#StateTransition"/>
            </owl:Restriction>
        </rdfs:subClassOf>
        <rdfs:comment>A clause which commands some agent to perform a task or bring about a state of affairs.</rdfs:comment>
        <rdfs:isDefinedBy rdf:resource="http://www.ease-crc.org/ont/SOMA-SAY.owl"/>
        <rdfs:label>Imperative clause</rdfs:label>
    </owl:Class>
    


    <!-- http://www.ease-crc.org/ont/SOMA.owl#IncludedObject -->


    <owl:Class rdf:about="http://www.ease-crc.org/ont/SOMA.owl#IncludedObject">
        <rdfs:subClassOf rdf:resource="http://www.ease-crc.org/ont/SOMA.owl#Patient"/>
        <rdfs:comment>An object that is contained in something. This is meant very general and includes, e.g., elements contained in a set, or things that are spatially contained within the boundaries of some object.</rdfs:comment>
        <rdfs:isDefinedBy rdf:resource="http://www.ease-crc.org/ont/SOMA-OBJ.owl"/>
        <rdfs:label xml:lang="en">Included object</rdfs:label>
    </owl:Class>
    


    <!-- http://www.ease-crc.org/ont/SOMA.owl#IncompatibleSoftware -->


    <owl:Class rdf:about="http://www.ease-crc.org/ont/SOMA.owl#IncompatibleSoftware">
        <rdfs:subClassOf rdf:resource="http://www.ease-crc.org/ont/SOMA.owl#SoftwareDiagnosis"/>
        <rdfs:comment>A description of a situation where two software systems are incompatible with each other.</rdfs:comment>
        <rdfs:isDefinedBy rdf:resource="http://www.ease-crc.org/ont/SOMA-IO.owl"/>
        <rdfs:label xml:lang="en">Incompatible software</rdfs:label>
    </owl:Class>
    


    <!-- http://www.ease-crc.org/ont/SOMA.owl#InductiveReasoning -->


    <owl:Class rdf:about="http://www.ease-crc.org/ont/SOMA.owl#InductiveReasoning">
        <rdfs:subClassOf rdf:resource="http://www.ease-crc.org/ont/SOMA.owl#Reasoning"/>
        <rdfs:comment>A task in which the Agent endeavors to accumulate confidence in some general statement about the world, by gathering instances in which this general statement appears to apply. Note that perfect confidence can never be guaranteed by induction.

Induction is often described as a move from many &quot;specifics&quot; (swan A is white, swan B is white, swan C is white, ...) to the &quot;general&quot; (all swans are white).</rdfs:comment>
        <rdfs:isDefinedBy rdf:resource="http://www.ease-crc.org/ont/SOMA-ACT.owl"/>
        <rdfs:label xml:lang="en">Inductive resoning</rdfs:label>
    </owl:Class>
    


    <!-- http://www.ease-crc.org/ont/SOMA.owl#InsertedObject -->


    <owl:Class rdf:about="http://www.ease-crc.org/ont/SOMA.owl#InsertedObject">
        <rdfs:subClassOf rdf:resource="http://www.ease-crc.org/ont/SOMA.owl#EnclosedObject"/>
        <rdfs:comment>An object inserted into another object.</rdfs:comment>
        <rdfs:isDefinedBy rdf:resource="http://www.ease-crc.org/ont/SOMA-OBJ.owl"/>
        <rdfs:label xml:lang="en">Inserted object</rdfs:label>
    </owl:Class>
    


    <!-- http://www.ease-crc.org/ont/SOMA.owl#Insertion -->


    <owl:Class rdf:about="http://www.ease-crc.org/ont/SOMA.owl#Insertion">
        <rdfs:subClassOf rdf:resource="http://www.ease-crc.org/ont/SOMA.owl#Enclosing"/>
        <rdfs:subClassOf>
            <owl:Restriction>
                <owl:onProperty rdf:resource="http://www.ease-crc.org/ont/SOMA.owl#affordsTrigger"/>
                <owl:allValuesFrom rdf:resource="http://www.ease-crc.org/ont/SOMA.owl#InsertedObject"/>
            </owl:Restriction>
        </rdfs:subClassOf>
        <rdfs:comment>The disposition of an object (the container) to contain other objects that can be inserted into the container through a portal.</rdfs:comment>
        <rdfs:isDefinedBy rdf:resource="http://www.ease-crc.org/ont/SOMA-HOME.owl"/>
        <rdfs:isDefinedBy rdf:resource="http://www.ease-crc.org/ont/SOMA-OBJ.owl"/>
    </owl:Class>
    


    <!-- http://www.ease-crc.org/ont/SOMA.owl#Instrument -->


    <owl:Class rdf:about="http://www.ease-crc.org/ont/SOMA.owl#Instrument">
        <rdfs:subClassOf rdf:resource="http://www.ease-crc.org/ont/SOMA.owl#ResourceRole"/>
        <rdfs:comment>An object used to carry out the event.</rdfs:comment>
        <rdfs:isDefinedBy rdf:resource="http://www.ease-crc.org/ont/SOMA-OBJ.owl"/>
        <rdfs:isDefinedBy rdf:resource="http://www.ease-crc.org/ont/SOMA-SAY.owl"/>
    </owl:Class>
    


    <!-- http://www.ease-crc.org/ont/SOMA.owl#InterfaceComponentRole -->


    <owl:Class rdf:about="http://www.ease-crc.org/ont/SOMA.owl#InterfaceComponentRole">
        <owl:equivalentClass>
            <owl:Class>
                <owl:intersectionOf rdf:parseType="Collection">
                    <rdf:Description rdf:about="http://www.ease-crc.org/ont/SOMA.owl#SoftwareRole"/>
                    <owl:Restriction>
                        <owl:onProperty rdf:resource="http://www.ontologydesignpatterns.org/ont/dul/DUL.owl#isDefinedIn"/>
                        <owl:allValuesFrom rdf:resource="http://www.ease-crc.org/ont/SOMA.owl#InterfaceSpecification"/>
                    </owl:Restriction>
                </owl:intersectionOf>
            </owl:Class>
        </owl:equivalentClass>
        <rdfs:subClassOf rdf:resource="http://www.ease-crc.org/ont/SOMA.owl#SoftwareRole"/>
        <rdfs:isDefinedBy rdf:resource="http://www.ease-crc.org/ont/SOMA-IO.owl"/>
        <rdfs:label xml:lang="en">Interface component role</rdfs:label>
    </owl:Class>
    


    <!-- http://www.ease-crc.org/ont/SOMA.owl#InterfaceSpecification -->


    <owl:Class rdf:about="http://www.ease-crc.org/ont/SOMA.owl#InterfaceSpecification">
        <rdfs:subClassOf rdf:resource="http://www.ontologydesignpatterns.org/ont/dul/DUL.owl#Design"/>
        <rdfs:comment xml:lang="en">The Specification of an Interface between software, computer hardware, peripheral devices, humans and combinations of these.

Source: https://en.wikipedia.org/wiki/Interface_(computing)</rdfs:comment>
        <rdfs:isDefinedBy rdf:resource="http://www.ease-crc.org/ont/SOMA-IO.owl"/>
        <rdfs:label xml:lang="en">Interface Specification</rdfs:label>
    </owl:Class>
    


    <!-- http://www.ease-crc.org/ont/SOMA.owl#IntermediateGrasp -->


    <owl:Class rdf:about="http://www.ease-crc.org/ont/SOMA.owl#IntermediateGrasp">
        <rdfs:subClassOf rdf:resource="http://www.ease-crc.org/ont/SOMA.owl#GraspingMotion"/>
        <owl:disjointWith rdf:resource="http://www.ease-crc.org/ont/SOMA.owl#PowerGrasp"/>
        <owl:disjointWith rdf:resource="http://www.ease-crc.org/ont/SOMA.owl#PrecisionGrasp"/>
        <rdfs:comment>A kind of grasp that acquires kinematic control over the gripped object, but without attempting to achieve either strong holding force nor precision of subsequent movement of the gripped object.</rdfs:comment>
        <rdfs:isDefinedBy rdf:resource="http://www.ease-crc.org/ont/SOMA-PROC.owl"/>
        <rdfs:label>Intermediate grasp</rdfs:label>
    </owl:Class>
    


    <!-- http://www.ease-crc.org/ont/SOMA.owl#InterrogativeClause -->


    <owl:Class rdf:about="http://www.ease-crc.org/ont/SOMA.owl#InterrogativeClause">
        <rdfs:subClassOf rdf:resource="http://www.ease-crc.org/ont/SOMA.owl#ClausalObject"/>
        <rdfs:comment>A clause which makes a request, typically information, of some agent.

Note that in a semantic sense such clauses always request information, but in a pragmatic sense they can be used to convey commands or requests for action, such as e.g. &quot;can you close the door?&quot; The question is not just a request for information about ability, but a request to perform a task.</rdfs:comment>
        <rdfs:isDefinedBy rdf:resource="http://www.ease-crc.org/ont/SOMA-SAY.owl"/>
        <rdfs:label>Interrogative clause</rdfs:label>
    </owl:Class>
    


    <!-- http://www.ease-crc.org/ont/SOMA.owl#Intrinsic -->


    <owl:Class rdf:about="http://www.ease-crc.org/ont/SOMA.owl#Intrinsic">
        <rdfs:subClassOf rdf:resource="http://www.ease-crc.org/ont/SOMA.owl#PhysicalQuality"/>
        <rdfs:comment>A physical quality that is independent of context.</rdfs:comment>
        <rdfs:comment>intrinsic</rdfs:comment>
        <rdfs:isDefinedBy rdf:resource="http://www.ease-crc.org/ont/SOMA-OBJ.owl"/>
    </owl:Class>
    


    <!-- http://www.ease-crc.org/ont/SOMA.owl#Item -->


    <owl:Class rdf:about="http://www.ease-crc.org/ont/SOMA.owl#Item">
        <rdfs:subClassOf rdf:resource="http://www.ease-crc.org/ont/SOMA.owl#Patient"/>
        <rdfs:comment>A role played by a non-agentive object operated on by an action.</rdfs:comment>
        <rdfs:isDefinedBy rdf:resource="http://www.ease-crc.org/ont/SOMA-OBJ.owl"/>
        <rdfs:isDefinedBy rdf:resource="http://www.ease-crc.org/ont/SOMA-STATE.owl"/>
    </owl:Class>
    


    <!-- http://www.ease-crc.org/ont/SOMA.owl#KineticFrictionAttribute -->


    <owl:Class rdf:about="http://www.ease-crc.org/ont/SOMA.owl#KineticFrictionAttribute">
        <rdfs:subClassOf rdf:resource="http://www.ease-crc.org/ont/SOMA.owl#FrictionAttribute"/>
        <rdfs:comment>Friction that occurs when two touching objects are moving relative to each other.</rdfs:comment>
        <rdfs:isDefinedBy rdf:resource="http://www.ease-crc.org/ont/SOMA-OBJ.owl"/>
        <rdfs:label>Kinetic friction attribute</rdfs:label>
    </owl:Class>
    


    <!-- http://www.ease-crc.org/ont/SOMA.owl#KinoDynamicData -->


    <owl:Class rdf:about="http://www.ease-crc.org/ont/SOMA.owl#KinoDynamicData">
        <rdfs:subClassOf rdf:resource="http://www.ontologydesignpatterns.org/ont/dul/DUL.owl#InformationObject"/>
        <rdfs:subClassOf>
            <owl:Restriction>
                <owl:onProperty rdf:resource="http://www.ontologydesignpatterns.org/ont/dul/DUL.owl#isAbout"/>
                <owl:allValuesFrom rdf:resource="http://www.ontologydesignpatterns.org/ont/dul/DUL.owl#PhysicalObject"/>
            </owl:Restriction>
        </rdfs:subClassOf>
        <rdfs:comment>An InformationObject containing data about how a physical object is put together such that its parts may move relative to each other, and what the physical characteristics of those parts are.</rdfs:comment>
        <rdfs:isDefinedBy rdf:resource="http://www.ease-crc.org/ont/SOMA-NEEM.owl"/>
        <rdfs:label xml:lang="en">Kino-dynamic data</rdfs:label>
    </owl:Class>
    


    <!-- http://www.ease-crc.org/ont/SOMA.owl#Knife -->


    <owl:Class rdf:about="http://www.ease-crc.org/ont/SOMA.owl#Knife">
        <rdfs:subClassOf rdf:resource="http://www.ease-crc.org/ont/SOMA.owl#CuttingTool"/>
        <rdfs:subClassOf>
            <owl:Restriction>
                <owl:onProperty rdf:resource="http://www.ease-crc.org/ont/SOMA.owl#hasPhysicalComponent"/>
                <owl:someValuesFrom rdf:resource="http://www.ease-crc.org/ont/SOMA.owl#Blade"/>
            </owl:Restriction>
        </rdfs:subClassOf>
        <rdfs:subClassOf>
            <owl:Restriction>
                <owl:onProperty rdf:resource="http://www.ease-crc.org/ont/SOMA.owl#hasPhysicalComponent"/>
                <owl:someValuesFrom rdf:resource="http://www.ease-crc.org/ont/SOMA.owl#DesignedHandle"/>
            </owl:Restriction>
        </rdfs:subClassOf>
        <rdfs:comment>An instrument composed of a blade fixed into a handle, used for cutting or as a weapon.</rdfs:comment>
        <rdfs:isDefinedBy rdf:resource="http://www.ease-crc.org/ont/SOMA-HOME.owl"/>
    </owl:Class>
    


    <!-- http://www.ease-crc.org/ont/SOMA.owl#KnowledgeRepresentationLanguage -->


    <owl:Class rdf:about="http://www.ease-crc.org/ont/SOMA.owl#KnowledgeRepresentationLanguage">
        <rdfs:subClassOf rdf:resource="http://www.ease-crc.org/ont/SOMA.owl#Computer_Language"/>
        <rdfs:comment xml:lang="en">A Knowledge Representation Language is a Language with fixed semantics and syntax to describe some knowledge. Examples are JSON and the different OWL Profiles.</rdfs:comment>
        <rdfs:isDefinedBy rdf:resource="http://www.ease-crc.org/ont/SOMA-IO.owl"/>
        <rdfs:label xml:lang="en">Knowledge Representation Language</rdfs:label>
    </owl:Class>
    


    <!-- http://www.ease-crc.org/ont/SOMA.owl#Language -->


    <owl:Class rdf:about="http://www.ease-crc.org/ont/SOMA.owl#Language">
        <rdfs:subClassOf rdf:resource="http://www.ease-crc.org/ont/SOMA.owl#System"/>
        <rdfs:subClassOf>
            <owl:Restriction>
                <owl:onProperty rdf:resource="http://www.ease-crc.org/ont/SOMA.owl#givesMeaningTo"/>
                <owl:allValuesFrom rdf:resource="http://www.ease-crc.org/ont/SOMA.owl#Text"/>
            </owl:Restriction>
        </rdfs:subClassOf>
        <rdfs:comment xml:lang="en">A Language is a structured System for communication.

From Wikipedia: https://en.wikipedia.org/wiki/Language</rdfs:comment>
        <rdfs:isDefinedBy rdf:resource="http://www.ease-crc.org/ont/SOMA-IO.owl"/>
        <rdfs:label xml:lang="en">Language</rdfs:label>
    </owl:Class>
    


    <!-- http://www.ease-crc.org/ont/SOMA.owl#Leaning -->


    <owl:Class rdf:about="http://www.ease-crc.org/ont/SOMA.owl#Leaning">
        <rdfs:subClassOf rdf:resource="http://www.ease-crc.org/ont/SOMA.owl#PosturalMoving"/>
        <rdfs:comment>An Agent pitches its body in some direction.</rdfs:comment>
        <rdfs:isDefinedBy rdf:resource="http://www.ease-crc.org/ont/SOMA-PROC.owl"/>
    </owl:Class>
    


    <!-- http://www.ease-crc.org/ont/SOMA.owl#Leg -->


    <owl:Class rdf:about="http://www.ease-crc.org/ont/SOMA.owl#Leg">
        <rdfs:subClassOf rdf:resource="http://www.ease-crc.org/ont/SOMA.owl#Limb"/>
        <rdfs:comment>A limb on which an agent walks or stands.</rdfs:comment>
        <rdfs:isDefinedBy rdf:resource="http://www.ease-crc.org/ont/SOMA-OBJ.owl"/>
    </owl:Class>
    


    <!-- http://www.ease-crc.org/ont/SOMA.owl#Lid -->


    <owl:Class rdf:about="http://www.ease-crc.org/ont/SOMA.owl#Lid">
        <rdfs:subClassOf rdf:resource="http://www.ease-crc.org/ont/SOMA.owl#DesignedComponent"/>
        <rdfs:comment>A removable or hinged cover for the top of a container.</rdfs:comment>
        <rdfs:isDefinedBy rdf:resource="http://www.ease-crc.org/ont/SOMA-HOME.owl"/>
    </owl:Class>
    


    <!-- http://www.ease-crc.org/ont/SOMA.owl#Lifting -->


    <owl:Class rdf:about="http://www.ease-crc.org/ont/SOMA.owl#Lifting">
        <rdfs:subClassOf rdf:resource="http://www.ease-crc.org/ont/SOMA.owl#Actuating"/>
        <owl:disjointWith rdf:resource="http://www.ease-crc.org/ont/SOMA.owl#Opening"/>
        <owl:disjointWith rdf:resource="http://www.ease-crc.org/ont/SOMA.owl#Pulling"/>
        <owl:disjointWith rdf:resource="http://www.ease-crc.org/ont/SOMA.owl#Pushing"/>
        <owl:disjointWith rdf:resource="http://www.ease-crc.org/ont/SOMA.owl#Squeezing"/>
        <rdfs:comment>todo: how to distinguish from e.g. &apos;pushing from the table&apos;</rdfs:comment>
        <rdfs:isDefinedBy rdf:resource="http://www.ease-crc.org/ont/SOMA-ACT.owl"/>
    </owl:Class>
    


    <!-- http://www.ease-crc.org/ont/SOMA.owl#Limb -->


    <owl:Class rdf:about="http://www.ease-crc.org/ont/SOMA.owl#Limb">
        <owl:equivalentClass>
            <owl:Class>
                <owl:unionOf rdf:parseType="Collection">
                    <rdf:Description rdf:about="http://www.ease-crc.org/ont/SOMA.owl#Arm"/>
                    <rdf:Description rdf:about="http://www.ease-crc.org/ont/SOMA.owl#Leg"/>
                </owl:unionOf>
            </owl:Class>
        </owl:equivalentClass>
        <rdfs:subClassOf rdf:resource="http://www.ease-crc.org/ont/SOMA.owl#PhysicalEffector"/>
        <rdfs:comment>An arm or leg of an embodied agent.</rdfs:comment>
        <rdfs:isDefinedBy rdf:resource="http://www.ease-crc.org/ont/SOMA-OBJ.owl"/>
        <rdfs:isDefinedBy rdf:resource="http://www.ease-crc.org/ont/SOMA-PROC.owl"/>
    </owl:Class>
    


    <!-- http://www.ease-crc.org/ont/SOMA.owl#LimbMotion -->


    <owl:Class rdf:about="http://www.ease-crc.org/ont/SOMA.owl#LimbMotion">
        <rdfs:subClassOf rdf:resource="http://www.ease-crc.org/ont/SOMA.owl#DirectedMotion"/>
        <rdfs:subClassOf>
            <owl:Restriction>
                <owl:onProperty rdf:resource="http://www.ease-crc.org/ont/SOMA.owl#isProcessTypeOf"/>
                <owl:someValuesFrom>
                    <owl:Class>
                        <owl:intersectionOf rdf:parseType="Collection">
                            <rdf:Description rdf:about="http://www.ease-crc.org/ont/SOMA.owl#MovedObject"/>
                            <owl:Restriction>
                                <owl:onProperty rdf:resource="http://www.ontologydesignpatterns.org/ont/dul/DUL.owl#classifies"/>
                                <owl:allValuesFrom rdf:resource="http://www.ease-crc.org/ont/SOMA.owl#Limb"/>
                            </owl:Restriction>
                        </owl:intersectionOf>
                    </owl:Class>
                </owl:someValuesFrom>
            </owl:Restriction>
        </rdfs:subClassOf>
        <owl:disjointWith rdf:resource="http://www.ease-crc.org/ont/SOMA.owl#Locomotion"/>
        <owl:disjointWith rdf:resource="http://www.ease-crc.org/ont/SOMA.owl#PrehensileMotion"/>
        <rdfs:comment>An Agent moves its limbs in some way.</rdfs:comment>
        <rdfs:isDefinedBy rdf:resource="http://www.ease-crc.org/ont/SOMA-PROC.owl"/>
        <rdfs:label>Limb motion</rdfs:label>
    </owl:Class>
    


    <!-- http://www.ease-crc.org/ont/SOMA.owl#LinguisticObject -->


    <owl:Class rdf:about="http://www.ease-crc.org/ont/SOMA.owl#LinguisticObject">
        <rdfs:subClassOf rdf:resource="http://www.ontologydesignpatterns.org/ont/dul/DUL.owl#InformationObject"/>
        <rdfs:isDefinedBy rdf:resource="http://www.ease-crc.org/ont/SOMA-ACT.owl"/>
        <rdfs:isDefinedBy rdf:resource="http://www.ease-crc.org/ont/SOMA-SAY.owl"/>
        <rdfs:isDefinedBy rdf:resource="http://www.ontologydesignpatterns.org/ont/dul/IOLite.owl"/>
        <rdfs:label xml:lang="en">Linguistic object</rdfs:label>
    </owl:Class>
    


    <!-- http://www.ease-crc.org/ont/SOMA.owl#Linkage -->


    <owl:Class rdf:about="http://www.ease-crc.org/ont/SOMA.owl#Linkage">
        <rdfs:subClassOf rdf:resource="http://www.ease-crc.org/ont/SOMA.owl#Connectivity"/>
        <rdfs:subClassOf>
            <owl:Restriction>
                <owl:onProperty rdf:resource="http://www.ease-crc.org/ont/SOMA.owl#affordsBearer"/>
                <owl:allValuesFrom rdf:resource="http://www.ease-crc.org/ont/SOMA.owl#LinkedObject"/>
            </owl:Restriction>
        </rdfs:subClassOf>
        <rdfs:subClassOf>
            <owl:Restriction>
                <owl:onProperty rdf:resource="http://www.ease-crc.org/ont/SOMA.owl#affordsTrigger"/>
                <owl:allValuesFrom rdf:resource="http://www.ease-crc.org/ont/SOMA.owl#LinkedObject"/>
            </owl:Restriction>
        </rdfs:subClassOf>
        <rdfs:comment>The disposition of an object (the linked object) to establish a connection with others by being linked together.</rdfs:comment>
        <rdfs:isDefinedBy rdf:resource="http://www.ease-crc.org/ont/SOMA-HOME.owl"/>
        <rdfs:isDefinedBy rdf:resource="http://www.ease-crc.org/ont/SOMA-OBJ.owl"/>
    </owl:Class>
    


    <!-- http://www.ease-crc.org/ont/SOMA.owl#LinkageState -->


    <owl:Class rdf:about="http://www.ease-crc.org/ont/SOMA.owl#LinkageState">
        <rdfs:subClassOf rdf:resource="http://www.ease-crc.org/ont/SOMA.owl#StateType"/>
        <rdfs:subClassOf>
            <owl:Restriction>
                <owl:onProperty rdf:resource="http://www.ease-crc.org/ont/SOMA.owl#isStateTypeOf"/>
                <owl:someValuesFrom rdf:resource="http://www.ease-crc.org/ont/SOMA.owl#LinkedObject"/>
            </owl:Restriction>
        </rdfs:subClassOf>
        <rdfs:comment>Classifies States in which two objects are in a rigid connection, such that the movement of one determines the movement of the other.</rdfs:comment>
        <rdfs:isDefinedBy rdf:resource="http://www.ease-crc.org/ont/SOMA-STATE.owl"/>
        <rdfs:label xml:lang="en">Linkage state</rdfs:label>
    </owl:Class>
    


    <!-- http://www.ease-crc.org/ont/SOMA.owl#LinkedObject -->


    <owl:Class rdf:about="http://www.ease-crc.org/ont/SOMA.owl#LinkedObject">
        <rdfs:subClassOf rdf:resource="http://www.ease-crc.org/ont/SOMA.owl#ConnectedObject"/>
        <rdfs:comment>An object that is linked to some other object.</rdfs:comment>
        <rdfs:isDefinedBy rdf:resource="http://www.ease-crc.org/ont/SOMA-OBJ.owl"/>
        <rdfs:isDefinedBy rdf:resource="http://www.ease-crc.org/ont/SOMA-STATE.owl"/>
        <rdfs:label xml:lang="en">Linked object</rdfs:label>
    </owl:Class>
    


    <!-- http://www.ease-crc.org/ont/SOMA.owl#Localization -->


    <owl:Class rdf:about="http://www.ease-crc.org/ont/SOMA.owl#Localization">
        <rdfs:subClassOf rdf:resource="http://www.ease-crc.org/ont/SOMA.owl#Extrinsic"/>
        <rdfs:subClassOf>
            <owl:Restriction>
                <owl:onProperty rdf:resource="http://www.ontologydesignpatterns.org/ont/dul/DUL.owl#hasRegion"/>
                <owl:someValuesFrom rdf:resource="http://www.ontologydesignpatterns.org/ont/dul/DUL.owl#SpaceRegion"/>
            </owl:Restriction>
        </rdfs:subClassOf>
        <rdfs:subClassOf>
            <owl:Restriction>
                <owl:onProperty rdf:resource="http://www.ontologydesignpatterns.org/ont/dul/DUL.owl#hasRegion"/>
                <owl:allValuesFrom rdf:resource="http://www.ontologydesignpatterns.org/ont/dul/DUL.owl#SpaceRegion"/>
            </owl:Restriction>
        </rdfs:subClassOf>
        <rdfs:comment>The localization of an object. The region of this quality encodes values to localize the object in a dimensional space, e.g. Euclidean positions that localize the object in Euclidean space.</rdfs:comment>
        <rdfs:isDefinedBy rdf:resource="http://www.ease-crc.org/ont/SOMA-OBJ.owl"/>
    </owl:Class>
    


    <!-- http://www.ease-crc.org/ont/SOMA.owl#Location -->


    <owl:Class rdf:about="http://www.ease-crc.org/ont/SOMA.owl#Location">
        <rdfs:subClassOf rdf:resource="http://www.ease-crc.org/ont/SOMA.owl#SpatioTemporalRole"/>
        <rdfs:comment>A role classifying a location of interest, often specified as a spatial relation between several objects, themselves usually classified by spatial relation roles.</rdfs:comment>
        <rdfs:isDefinedBy rdf:resource="http://www.ease-crc.org/ont/SOMA-OBJ.owl"/>
    </owl:Class>
    


    <!-- http://www.ease-crc.org/ont/SOMA.owl#LocatumRole -->


    <owl:Class rdf:about="http://www.ease-crc.org/ont/SOMA.owl#LocatumRole">
        <rdfs:subClassOf rdf:resource="http://www.ease-crc.org/ont/SOMA.owl#SpatialRelationRole"/>
        <rdfs:subClassOf>
            <owl:Restriction>
                <owl:onProperty rdf:resource="http://www.ontologydesignpatterns.org/ont/dul/DUL.owl#classifies"/>
                <owl:allValuesFrom rdf:resource="http://www.ontologydesignpatterns.org/ont/dul/DUL.owl#PhysicalObject"/>
            </owl:Restriction>
        </rdfs:subClassOf>
        <rdfs:comment>Denotes the object with primary focal prominence in a spatial or spatio-temporal schema. Terminological variants that appear in the literature on cognitive linguistics include Figure (Talmy 1983) and Trajector (Langacker 1986).</rdfs:comment>
        <rdfs:isDefinedBy rdf:resource="http://www.ease-crc.org/ont/SOMA-OBJ.owl"/>
        <rdfs:label xml:lang="en">Locatum role</rdfs:label>
    </owl:Class>
    


    <!-- http://www.ease-crc.org/ont/SOMA.owl#Locomotion -->


    <owl:Class rdf:about="http://www.ease-crc.org/ont/SOMA.owl#Locomotion">
        <rdfs:subClassOf rdf:resource="http://www.ease-crc.org/ont/SOMA.owl#BodyMovement"/>
        <rdfs:subClassOf rdf:resource="http://www.ease-crc.org/ont/SOMA.owl#DirectedMotion"/>
        <owl:disjointWith rdf:resource="http://www.ease-crc.org/ont/SOMA.owl#PrehensileMotion"/>
        <rdfs:comment>Conceptually related to Navigation, but distinguishable from it because of the profile, ie. the focus of the task.

Navigation is about reaching some goal.

Locomotion is concerned more with the actual motion.</rdfs:comment>
        <rdfs:comment>The Agent repositions their body in the environment.</rdfs:comment>
        <rdfs:isDefinedBy rdf:resource="http://www.ease-crc.org/ont/SOMA-PROC.owl"/>
    </owl:Class>
    


    <!-- http://www.ease-crc.org/ont/SOMA.owl#LocutionaryAction -->


    <owl:Class rdf:about="http://www.ease-crc.org/ont/SOMA.owl#LocutionaryAction">
        <owl:equivalentClass>
            <owl:Class>
                <owl:intersectionOf rdf:parseType="Collection">
                    <rdf:Description rdf:about="http://www.ease-crc.org/ont/SOMA.owl#CommunicationAction"/>
                    <owl:Restriction>
                        <owl:onProperty rdf:resource="http://www.ontologydesignpatterns.org/ont/dul/DUL.owl#hasParticipant"/>
                        <owl:someValuesFrom rdf:resource="http://www.ontologydesignpatterns.org/ont/dul/DUL.owl#Agent"/>
                    </owl:Restriction>
                </owl:intersectionOf>
            </owl:Class>
        </owl:equivalentClass>
        <rdfs:comment xml:lang="en">A Locutionary Act is the performance of an utterance (source: https://en.wikipedia.org/wiki/Locutionary_act).

We additionally require a Locutionary Act to be performed by an Agent, not an Actor - this is what sets it apart from a Communication Action.</rdfs:comment>
        <rdfs:isDefinedBy rdf:resource="http://www.ease-crc.org/ont/SOMA-SAY.owl"/>
        <rdfs:label xml:lang="en">Locutionary action</rdfs:label>
    </owl:Class>
    


    <!-- http://www.ease-crc.org/ont/SOMA.owl#LookingAt -->


    <owl:Class rdf:about="http://www.ease-crc.org/ont/SOMA.owl#LookingAt">
        <rdfs:subClassOf rdf:resource="http://www.ease-crc.org/ont/SOMA.owl#PhysicalTask"/>
        <rdfs:comment>better: Gazing</rdfs:comment>
        <rdfs:isDefinedBy rdf:resource="http://www.ease-crc.org/ont/SOMA-ACT.owl"/>
    </owl:Class>
    


    <!-- http://www.ease-crc.org/ont/SOMA.owl#LookingFor -->


    <owl:Class rdf:about="http://www.ease-crc.org/ont/SOMA.owl#LookingFor">
        <rdfs:subClassOf rdf:resource="http://www.ease-crc.org/ont/SOMA.owl#Perceiving"/>
        <rdfs:comment>A task by which an Agent uses its perception apparatus to check for the presence of an object in some specified area.</rdfs:comment>
        <rdfs:isDefinedBy rdf:resource="http://www.ease-crc.org/ont/SOMA-ACT.owl"/>
        <rdfs:label xml:lang="en">Looking for</rdfs:label>
    </owl:Class>
    


    <!-- http://www.ease-crc.org/ont/SOMA.owl#Lowering -->


    <owl:Class rdf:about="http://www.ease-crc.org/ont/SOMA.owl#Lowering">
        <rdfs:subClassOf rdf:resource="http://www.ease-crc.org/ont/SOMA.owl#Actuating"/>
        <rdfs:comment>A task in which an Agent reduces the elevation at which they hold an item.</rdfs:comment>
        <rdfs:isDefinedBy rdf:resource="http://www.ease-crc.org/ont/SOMA-ACT.owl"/>
    </owl:Class>
    


    <!-- http://www.ease-crc.org/ont/SOMA.owl#Manipulating -->


    <owl:Class rdf:about="http://www.ease-crc.org/ont/SOMA.owl#Manipulating">
        <rdfs:subClassOf rdf:resource="http://www.ease-crc.org/ont/SOMA.owl#PhysicalTask"/>
        <rdfs:subClassOf>
            <owl:Restriction>
                <owl:onProperty rdf:resource="http://www.ontologydesignpatterns.org/ont/dul/DUL.owl#classifies"/>
                <owl:allValuesFrom rdf:resource="http://www.ease-crc.org/ont/SOMA.owl#PhysicalAction"/>
            </owl:Restriction>
        </rdfs:subClassOf>
        <rdfs:comment>Tasks where the goal is to move the prehensile effectors, ie. hands, of an agent so as to achieve some spatial or functional relation with some manipulated object. 

Spatial relations refer to positioning the hands in certain ways relative to the manipulated object, for example nearing or distancing them, or aligning them with some relevant axis.

Functional relations here refer to interactions between the hands and manipulated object which constrain the possible behavior of the object. Examples of functional relations in manipulation are support and kinematic control.

Note that manipulation tasks are usually performed with the intention of moving an object in some way, so there is a large conceptual overlap between Manipulating and Actuating.

However these concepts are nonetheless distinguished in what they &quot;profile&quot;, ie. what they focus on as particularly important.

Actuating profiles the movement of the object itself.

Manipulating profiles the movement of the hands and the functional relations, such as kinematic control, they establish with the manipulated object.

Note: we employ Manipulating here in its literal, original sense, of using hands for some purpose, and not in the metaphorical sense of exerting psychological pressure on someone.</rdfs:comment>
        <rdfs:isDefinedBy rdf:resource="http://www.ease-crc.org/ont/SOMA-ACT.owl"/>
    </owl:Class>
    


    <!-- http://www.ease-crc.org/ont/SOMA.owl#Markup_Language -->


    <owl:Class rdf:about="http://www.ease-crc.org/ont/SOMA.owl#Markup_Language">
        <rdfs:subClassOf rdf:resource="http://www.ease-crc.org/ont/SOMA.owl#Computer_Language"/>
        <rdfs:comment xml:lang="en">Markup refers to data included in an electronic document which is distinct from the document&apos;s content in that it is typically not included in representations of the document for end users, for example on paper or a computer screen, or in an audio stream. Markup is often used to control the display of the document or to enrich its content to facilitate automated processing. A markup language is a set of rules governing what markup information may be included in a document and how it is combined with the content of the document in a way to facilitate use by humans and computer programs.

From Wikipedia: https://en.wikipedia.org/wiki/Markup_language</rdfs:comment>
        <rdfs:isDefinedBy rdf:resource="http://www.ease-crc.org/ont/SOMA-IO.owl"/>
        <rdfs:label xml:lang="en">Markup Language</rdfs:label>
    </owl:Class>
    


    <!-- http://www.ease-crc.org/ont/SOMA.owl#MassAttribute -->


    <owl:Class rdf:about="http://www.ease-crc.org/ont/SOMA.owl#MassAttribute">
        <rdfs:subClassOf rdf:resource="http://www.ontologydesignpatterns.org/ont/dul/DUL.owl#PhysicalAttribute"/>
        <rdfs:subClassOf>
            <owl:Restriction>
                <owl:onProperty rdf:resource="http://www.ease-crc.org/ont/SOMA.owl#hasMassValue"/>
                <owl:qualifiedCardinality rdf:datatype="http://www.w3.org/2001/XMLSchema#nonNegativeInteger">1</owl:qualifiedCardinality>
                <owl:onDataRange rdf:resource="http://www.w3.org/2001/XMLSchema#double"/>
            </owl:Restriction>
        </rdfs:subClassOf>
        <rdfs:comment>The quantity of matter which a body contains, as measured by its acceleration under given force or by the force exerted on it by a gravitational field.</rdfs:comment>
        <rdfs:isDefinedBy rdf:resource="http://www.ease-crc.org/ont/SOMA-OBJ.owl"/>
        <rdfs:label>Mass attribute</rdfs:label>
    </owl:Class>
    


    <!-- http://www.ease-crc.org/ont/SOMA.owl#Material -->


    <owl:Class rdf:about="http://www.ease-crc.org/ont/SOMA.owl#Material">
        <rdfs:subClassOf rdf:resource="http://www.ease-crc.org/ont/SOMA.owl#Intrinsic"/>
        <rdfs:comment>The matter from which a thing is made.</rdfs:comment>
        <rdfs:isDefinedBy rdf:resource="http://www.ease-crc.org/ont/SOMA-OBJ.owl"/>
    </owl:Class>
    


    <!-- http://www.ease-crc.org/ont/SOMA.owl#MentalAction -->


    <owl:Class rdf:about="http://www.ease-crc.org/ont/SOMA.owl#MentalAction">
        <rdfs:subClassOf rdf:resource="http://www.ontologydesignpatterns.org/ont/dul/DUL.owl#Action"/>
        <rdfs:subClassOf>
            <owl:Restriction>
                <owl:onProperty rdf:resource="http://www.ontologydesignpatterns.org/ont/dul/DUL.owl#hasParticipant"/>
                <owl:allValuesFrom>
                    <owl:Class>
                        <owl:unionOf rdf:parseType="Collection">
                            <rdf:Description rdf:about="http://www.ontologydesignpatterns.org/ont/dul/DUL.owl#Agent"/>
                            <rdf:Description rdf:about="http://www.ontologydesignpatterns.org/ont/dul/DUL.owl#SocialObject"/>
                        </owl:unionOf>
                    </owl:Class>
                </owl:allValuesFrom>
            </owl:Restriction>
        </rdfs:subClassOf>
        <rdfs:comment>An Event construed as the Agent participant affecting Entities that are representations of actual or potential Entities or Events in the physical world in which the Agent is embodied. These representations are maintained by the Agent participant in the &apos;Mental action&apos; event.

One could argue Mental actions are all Physical actions, because anything the Agent may use to maintain such representations will be physical things, However, we make this distinction because for Mental actions it is less important to consider the physical support of the representation and how it changes, and more important to track how the information content of the representation changes.</rdfs:comment>
        <rdfs:isDefinedBy rdf:resource="http://www.ease-crc.org/ont/SOMA-ACT.owl"/>
        <rdfs:label>Mental action</rdfs:label>
    </owl:Class>
    


    <!-- http://www.ease-crc.org/ont/SOMA.owl#MentalTask -->


    <owl:Class rdf:about="http://www.ease-crc.org/ont/SOMA.owl#MentalTask">
        <rdfs:subClassOf rdf:resource="http://www.ontologydesignpatterns.org/ont/dul/DUL.owl#Task"/>
        <rdfs:subClassOf>
            <owl:Restriction>
                <owl:onProperty rdf:resource="http://www.ontologydesignpatterns.org/ont/dul/DUL.owl#classifies"/>
                <owl:allValuesFrom rdf:resource="http://www.ease-crc.org/ont/SOMA.owl#MentalAction"/>
            </owl:Restriction>
        </rdfs:subClassOf>
        <rdfs:comment>A Task classifying some MentalAction, that is, an Action through which an Agent manipulates representations stored in its own cognition.</rdfs:comment>
        <rdfs:isDefinedBy rdf:resource="http://www.ease-crc.org/ont/SOMA-ACT.owl"/>
        <rdfs:label xml:lang="en">Mental task</rdfs:label>
    </owl:Class>
    


    <!-- http://www.ease-crc.org/ont/SOMA.owl#MeshShape -->


    <owl:Class rdf:about="http://www.ease-crc.org/ont/SOMA.owl#MeshShape">
        <rdfs:subClassOf rdf:resource="http://www.ease-crc.org/ont/SOMA.owl#ShapeRegion"/>
        <rdfs:subClassOf>
            <owl:Restriction>
                <owl:onProperty rdf:resource="http://www.ease-crc.org/ont/SOMA.owl#hasFilePath"/>
                <owl:qualifiedCardinality rdf:datatype="http://www.w3.org/2001/XMLSchema#nonNegativeInteger">1</owl:qualifiedCardinality>
                <owl:onDataRange rdf:resource="http://www.w3.org/2001/XMLSchema#string"/>
            </owl:Restriction>
        </rdfs:subClassOf>
        <rdfs:subClassOf>
            <owl:Restriction>
                <owl:onProperty rdf:resource="http://www.ease-crc.org/ont/SOMA-OBJ.owl#hasShapeScale"/>
                <owl:maxQualifiedCardinality rdf:datatype="http://www.w3.org/2001/XMLSchema#nonNegativeInteger">1</owl:maxQualifiedCardinality>
                <owl:onDataRange rdf:resource="http://www.ease-crc.org/ont/SOMA.owl#array_double"/>
            </owl:Restriction>
        </rdfs:subClassOf>
        <rdfs:comment>A solid geometrical figure described in a mesh file.</rdfs:comment>
        <rdfs:isDefinedBy rdf:resource="http://www.ease-crc.org/ont/SOMA-OBJ.owl"/>
        <rdfs:label>Mesh shape</rdfs:label>
    </owl:Class>
    


    <!-- http://www.ease-crc.org/ont/SOMA.owl#MeshShapeData -->


    <owl:Class rdf:about="http://www.ease-crc.org/ont/SOMA.owl#MeshShapeData">
        <rdfs:subClassOf rdf:resource="http://www.ontologydesignpatterns.org/ont/dul/DUL.owl#InformationObject"/>
        <rdfs:subClassOf>
            <owl:Restriction>
                <owl:onProperty rdf:resource="http://www.ontologydesignpatterns.org/ont/dul/DUL.owl#isAbout"/>
                <owl:allValuesFrom rdf:resource="http://www.ontologydesignpatterns.org/ont/dul/DUL.owl#PhysicalObject"/>
            </owl:Restriction>
        </rdfs:subClassOf>
        <rdfs:comment>An InformationObject containing data about the geometry of a physical object.</rdfs:comment>
        <rdfs:isDefinedBy rdf:resource="http://www.ease-crc.org/ont/SOMA-NEEM.owl"/>
        <rdfs:label xml:lang="en">Mesh-shape data</rdfs:label>
    </owl:Class>
    


    <!-- http://www.ease-crc.org/ont/SOMA.owl#Message -->


    <owl:Class rdf:about="http://www.ease-crc.org/ont/SOMA.owl#Message">
        <rdfs:subClassOf rdf:resource="http://www.ease-crc.org/ont/SOMA.owl#Item"/>
        <rdfs:subClassOf>
            <owl:Restriction>
                <owl:onProperty rdf:resource="http://www.ontologydesignpatterns.org/ont/dul/DUL.owl#hasTask"/>
                <owl:someValuesFrom rdf:resource="http://www.ease-crc.org/ont/SOMA.owl#CommunicationTask"/>
            </owl:Restriction>
        </rdfs:subClassOf>
        <rdfs:subClassOf>
            <owl:Restriction>
                <owl:onProperty rdf:resource="http://www.ontologydesignpatterns.org/ont/dul/DUL.owl#classifies"/>
                <owl:allValuesFrom rdf:resource="http://www.ontologydesignpatterns.org/ont/dul/DUL.owl#InformationRealization"/>
            </owl:Restriction>
        </rdfs:subClassOf>
        <rdfs:comment xml:lang="en">A message is a discrete unit of communication intended by the source for consumption by some recipient or group of recipients (Source: https://en.wikipedia.org/wiki/Message).

Note that the Role Message classifies the Information Realization, not the content.</rdfs:comment>
        <rdfs:isDefinedBy rdf:resource="http://www.ease-crc.org/ont/SOMA-ACT.owl"/>
        <rdfs:label xml:lang="en">Message</rdfs:label>
    </owl:Class>
    


    <!-- http://www.ease-crc.org/ont/SOMA.owl#MetaCognitionEvaluationTopic -->


    <owl:Class rdf:about="http://www.ease-crc.org/ont/SOMA.owl#MetaCognitionEvaluationTopic">
        <rdfs:subClassOf rdf:resource="http://www.ease-crc.org/ont/SOMA.owl#MetaCognitionTopic"/>
        <rdfs:comment>A topic used while an Agent describes its own cognitive processes and acions to evaluate them according to some metric.</rdfs:comment>
        <rdfs:isDefinedBy rdf:resource="http://www.ease-crc.org/ont/SOMA-ACT.owl"/>
    </owl:Class>
    


    <!-- http://www.ease-crc.org/ont/SOMA.owl#MetaCognitionMemoryTopic -->


    <owl:Class rdf:about="http://www.ease-crc.org/ont/SOMA.owl#MetaCognitionMemoryTopic">
        <rdfs:subClassOf rdf:resource="http://www.ease-crc.org/ont/SOMA.owl#MetaCognitionTopic"/>
        <rdfs:comment>A topic used while an Agent describes its own cognitive processes and actions, and which covers descriptions of what memories are involved in them.</rdfs:comment>
        <rdfs:isDefinedBy rdf:resource="http://www.ease-crc.org/ont/SOMA-ACT.owl"/>
    </owl:Class>
    


    <!-- http://www.ease-crc.org/ont/SOMA.owl#MetaCognitionPlanningTopic -->


    <owl:Class rdf:about="http://www.ease-crc.org/ont/SOMA.owl#MetaCognitionPlanningTopic">
        <rdfs:subClassOf rdf:resource="http://www.ease-crc.org/ont/SOMA.owl#MetaCognitionTopic"/>
        <rdfs:comment>A topic used while an Agent describes the planning it does for its own cognitive processes and actions.</rdfs:comment>
        <rdfs:isDefinedBy rdf:resource="http://www.ease-crc.org/ont/SOMA-ACT.owl"/>
    </owl:Class>
    


    <!-- http://www.ease-crc.org/ont/SOMA.owl#MetaCognitionTopic -->


    <owl:Class rdf:about="http://www.ease-crc.org/ont/SOMA.owl#MetaCognitionTopic">
        <rdfs:subClassOf rdf:resource="http://www.ease-crc.org/ont/SOMA.owl#ThinkAloudTopic"/>
        <rdfs:comment>A topic for a description that an Agent might make of its own cognitive processes and actions.</rdfs:comment>
        <rdfs:isDefinedBy rdf:resource="http://www.ease-crc.org/ont/SOMA-ACT.owl"/>
    </owl:Class>
    


    <!-- http://www.ease-crc.org/ont/SOMA.owl#Mixing -->


    <owl:Class rdf:about="http://www.ease-crc.org/ont/SOMA.owl#Mixing">
        <rdfs:subClassOf rdf:resource="http://www.ease-crc.org/ont/SOMA.owl#Constructing"/>
        <rdfs:comment>A task by which an Agent combines several entities, such that the combination is difficult or in practice impossible to reverse.</rdfs:comment>
        <rdfs:isDefinedBy rdf:resource="http://www.ease-crc.org/ont/SOMA-ACT.owl"/>
    </owl:Class>
    


    <!-- http://www.ease-crc.org/ont/SOMA.owl#MixingTheory -->


    <owl:Class rdf:about="http://www.ease-crc.org/ont/SOMA.owl#MixingTheory">
        <rdfs:subClassOf rdf:resource="http://www.ease-crc.org/ont/SOMA.owl#ExecutableSchematicTheory"/>
        <rdfs:subClassOf>
            <owl:Restriction>
                <owl:onProperty rdf:resource="http://www.ontologydesignpatterns.org/ont/dul/DUL.owl#defines"/>
                <owl:someValuesFrom rdf:resource="http://www.ease-crc.org/ont/SOMA.owl#Instrument"/>
            </owl:Restriction>
        </rdfs:subClassOf>
        <rdfs:subClassOf>
            <owl:Restriction>
                <owl:onProperty rdf:resource="http://www.ontologydesignpatterns.org/ont/dul/DUL.owl#defines"/>
                <owl:someValuesFrom rdf:resource="http://www.ease-crc.org/ont/SOMA.owl#Patient"/>
            </owl:Restriction>
        </rdfs:subClassOf>
        <rdfs:comment>A schematic theory about how an agent can mix a fluid or particulate object.</rdfs:comment>
        <rdfs:isDefinedBy rdf:resource="http://www.ease-crc.org/ont/SOMA-SAY.owl"/>
        <rdfs:label xml:lang="en">Mixing theory</rdfs:label>
    </owl:Class>
    


    <!-- http://www.ease-crc.org/ont/SOMA.owl#ModifyingPhysicalObject -->


    <owl:Class rdf:about="http://www.ease-crc.org/ont/SOMA.owl#ModifyingPhysicalObject">
        <rdfs:subClassOf rdf:resource="http://www.ease-crc.org/ont/SOMA.owl#PhysicalTask"/>
        <rdfs:comment>Superconcept for tasks that involve affecting some state that an object is in (e.g. where it is located), without creating or destroying the object.</rdfs:comment>
        <rdfs:isDefinedBy rdf:resource="http://www.ease-crc.org/ont/SOMA-ACT.owl"/>
        <rdfs:label xml:lang="en">Modifying physical object</rdfs:label>
    </owl:Class>
    


    <!-- http://www.ease-crc.org/ont/SOMA.owl#MonitoringJointState -->


    <owl:Class rdf:about="http://www.ease-crc.org/ont/SOMA.owl#MonitoringJointState">
        <rdfs:subClassOf rdf:resource="http://www.ease-crc.org/ont/SOMA.owl#Proprioceiving"/>
        <rdfs:comment>A task in which the Agent keeps track of the physical state of its joints, e.g. their positions, velocities, efforts.</rdfs:comment>
        <rdfs:isDefinedBy rdf:resource="http://www.ease-crc.org/ont/SOMA-ACT.owl"/>
        <rdfs:label xml:lang="en">Monitoring joint state</rdfs:label>
    </owl:Class>
    


    <!-- http://www.ease-crc.org/ont/SOMA.owl#Motion -->


    <owl:Class rdf:about="http://www.ease-crc.org/ont/SOMA.owl#Motion">
        <rdfs:subClassOf rdf:resource="http://www.ease-crc.org/ont/SOMA.owl#ProcessType"/>
        <rdfs:comment>An EventType that classifies motion Processes.</rdfs:comment>
        <rdfs:comment>Motion type</rdfs:comment>
        <rdfs:isDefinedBy rdf:resource="http://www.ease-crc.org/ont/SOMA-PROC.owl"/>
    </owl:Class>
    


    <!-- http://www.ease-crc.org/ont/SOMA.owl#MovedObject -->


    <owl:Class rdf:about="http://www.ease-crc.org/ont/SOMA.owl#MovedObject">
        <rdfs:subClassOf rdf:resource="http://www.ease-crc.org/ont/SOMA.owl#AlteredObject"/>
        <rdfs:subClassOf>
            <owl:Restriction>
                <owl:onProperty rdf:resource="http://www.ease-crc.org/ont/SOMA.owl#isTriggerDefinedIn"/>
                <owl:someValuesFrom>
                    <owl:Restriction>
                        <owl:onProperty rdf:resource="http://www.ease-crc.org/ont/SOMA.owl#describesQuality"/>
                        <owl:allValuesFrom rdf:resource="http://www.ease-crc.org/ont/SOMA.owl#Localization"/>
                    </owl:Restriction>
                </owl:someValuesFrom>
            </owl:Restriction>
        </rdfs:subClassOf>
        <rdfs:subClassOf>
            <owl:Restriction>
                <owl:onProperty rdf:resource="http://www.ontologydesignpatterns.org/ont/dul/DUL.owl#classifies"/>
                <owl:allValuesFrom>
                    <owl:Restriction>
                        <owl:onProperty rdf:resource="http://www.ontologydesignpatterns.org/ont/dul/DUL.owl#hasQuality"/>
                        <owl:someValuesFrom rdf:resource="http://www.ease-crc.org/ont/SOMA.owl#Localization"/>
                    </owl:Restriction>
                </owl:allValuesFrom>
            </owl:Restriction>
        </rdfs:subClassOf>
        <rdfs:comment>An object undergoing location change.</rdfs:comment>
        <rdfs:isDefinedBy rdf:resource="http://www.ease-crc.org/ont/SOMA-OBJ.owl"/>
        <rdfs:isDefinedBy rdf:resource="http://www.ease-crc.org/ont/SOMA-PROC.owl"/>
        <rdfs:label xml:lang="en">Moved object</rdfs:label>
    </owl:Class>
    


    <!-- http://www.ease-crc.org/ont/SOMA.owl#MovingAway -->


    <owl:Class rdf:about="http://www.ease-crc.org/ont/SOMA.owl#MovingAway">
        <rdfs:subClassOf rdf:resource="http://www.ease-crc.org/ont/SOMA.owl#Locomotion"/>
        <rdfs:comment>A process type classifying a motion by which some Agent puts distance between itself and another object or location.</rdfs:comment>
        <rdfs:isDefinedBy rdf:resource="http://www.ease-crc.org/ont/SOMA-PROC.owl"/>
    </owl:Class>
    


    <!-- http://www.ease-crc.org/ont/SOMA.owl#MovingTo -->


    <owl:Class rdf:about="http://www.ease-crc.org/ont/SOMA.owl#MovingTo">
        <rdfs:subClassOf rdf:resource="http://www.ease-crc.org/ont/SOMA.owl#Navigating"/>
        <rdfs:comment>A task in which an Agent moves towards a location.</rdfs:comment>
        <rdfs:isDefinedBy rdf:resource="http://www.ease-crc.org/ont/SOMA-ACT.owl"/>
    </owl:Class>
    


    <!-- http://www.ease-crc.org/ont/SOMA.owl#Natural_Language -->


    <owl:Class rdf:about="http://www.ease-crc.org/ont/SOMA.owl#Natural_Language">
        <rdfs:subClassOf rdf:resource="http://www.ease-crc.org/ont/SOMA.owl#Language"/>
        <rdfs:subClassOf>
            <owl:Restriction>
                <owl:onProperty rdf:resource="http://www.ease-crc.org/ont/SOMA.owl#givesMeaningTo"/>
                <owl:allValuesFrom rdf:resource="http://www.ease-crc.org/ont/SOMA.owl#Natural_Language_Text"/>
            </owl:Restriction>
        </rdfs:subClassOf>
        <rdfs:comment xml:lang="en">A Natural Language is any language that has evolved naturally in humans through use and repetition without conscious planning or premeditation.

From Wikipedia: https://en.wikipedia.org/wiki/Natural_language</rdfs:comment>
        <rdfs:isDefinedBy rdf:resource="http://www.ease-crc.org/ont/SOMA-IO.owl"/>
        <rdfs:label xml:lang="en">Natural Language</rdfs:label>
    </owl:Class>
    


    <!-- http://www.ease-crc.org/ont/SOMA.owl#Natural_Language_Text -->


    <owl:Class rdf:about="http://www.ease-crc.org/ont/SOMA.owl#Natural_Language_Text">
        <owl:equivalentClass>
            <owl:Class>
                <owl:intersectionOf rdf:parseType="Collection">
                    <rdf:Description rdf:about="http://www.ease-crc.org/ont/SOMA.owl#Text"/>
                    <owl:Restriction>
                        <owl:onProperty rdf:resource="http://www.ease-crc.org/ont/SOMA.owl#isGivenMeaningBy"/>
                        <owl:someValuesFrom rdf:resource="http://www.ease-crc.org/ont/SOMA.owl#Natural_Language"/>
                    </owl:Restriction>
                </owl:intersectionOf>
            </owl:Class>
        </owl:equivalentClass>
        <rdfs:comment xml:lang="en">A Text in a Natural Language.</rdfs:comment>
        <rdfs:isDefinedBy rdf:resource="http://www.ease-crc.org/ont/SOMA-IO.owl"/>
        <rdfs:label xml:lang="en">Natural language text</rdfs:label>
    </owl:Class>
    


    <!-- http://www.ease-crc.org/ont/SOMA.owl#Navigating -->


    <owl:Class rdf:about="http://www.ease-crc.org/ont/SOMA.owl#Navigating">
        <rdfs:subClassOf rdf:resource="http://www.ease-crc.org/ont/SOMA.owl#PhysicalTask"/>
        <rdfs:comment>A task in which an Agent moves through space so as to arrive at some location, follow some path, or increase its distance from some location or other entity. Often, navigation involves finding paths around obstacles and forbidden areas.</rdfs:comment>
        <rdfs:isDefinedBy rdf:resource="http://www.ease-crc.org/ont/SOMA-ACT.owl"/>
    </owl:Class>
    


    <!-- http://www.ease-crc.org/ont/SOMA.owl#Obstacle -->


    <owl:Class rdf:about="http://www.ease-crc.org/ont/SOMA.owl#Obstacle">
        <rdfs:subClassOf rdf:resource="http://www.ease-crc.org/ont/SOMA.owl#Barrier"/>
        <rdfs:comment>An object used to restrict access to a protected space or group.</rdfs:comment>
        <rdfs:isDefinedBy rdf:resource="http://www.ease-crc.org/ont/SOMA-OBJ.owl"/>
    </owl:Class>
    


    <!-- http://www.ease-crc.org/ont/SOMA.owl#Ontology -->


    <owl:Class rdf:about="http://www.ease-crc.org/ont/SOMA.owl#Ontology">
        <owl:equivalentClass>
            <owl:Class>
                <owl:intersectionOf rdf:parseType="Collection">
                    <rdf:Description rdf:about="http://www.ease-crc.org/ont/SOMA.owl#Structured_Text"/>
                    <owl:Restriction>
                        <owl:onProperty rdf:resource="http://www.ease-crc.org/ont/SOMA.owl#isGivenMeaningBy"/>
                        <owl:someValuesFrom rdf:resource="http://www.ease-crc.org/ont/SOMA.owl#Ontology_Language"/>
                    </owl:Restriction>
                </owl:intersectionOf>
            </owl:Class>
        </owl:equivalentClass>
        <rdfs:subClassOf rdf:resource="http://www.ease-crc.org/ont/SOMA.owl#Structured_Text"/>
        <rdfs:comment xml:lang="en">An ontology encompasses a representation, formal naming, and definition of the categories, properties, and relations between the concepts, data, and entities that substantiate one, many, or all domains of discourse. More simply, an ontology is a way of showing the properties of a subject area and how they are related, by defining a set of concepts and categories that represent the subject.

From Wikipedia: https://en.wikipedia.org/wiki/Ontology_(information_science)</rdfs:comment>
        <rdfs:isDefinedBy rdf:resource="http://www.ease-crc.org/ont/SOMA-IO.owl"/>
    </owl:Class>
    


    <!-- http://www.ease-crc.org/ont/SOMA.owl#Ontology_Language -->


    <owl:Class rdf:about="http://www.ease-crc.org/ont/SOMA.owl#Ontology_Language">
        <rdfs:subClassOf rdf:resource="http://www.ease-crc.org/ont/SOMA.owl#KnowledgeRepresentationLanguage"/>
        <rdfs:subClassOf>
            <owl:Restriction>
                <owl:onProperty rdf:resource="http://www.ease-crc.org/ont/SOMA.owl#givesMeaningTo"/>
                <owl:allValuesFrom rdf:resource="http://www.ease-crc.org/ont/SOMA.owl#Ontology"/>
            </owl:Restriction>
        </rdfs:subClassOf>
        <rdfs:comment xml:lang="en">An Ontology Language is a Knowledge Representation Language to describe knowledge about properties of a subject area and how they are related, by defining a set of concepts and categories that represent the subject using logic. Examples are the different OWL Profiles.

Source: https://en.wikipedia.org/wiki/Ontology_(information_science)</rdfs:comment>
        <rdfs:isDefinedBy rdf:resource="http://www.ease-crc.org/ont/SOMA-IO.owl"/>
        <rdfs:label xml:lang="en">Ontology Language</rdfs:label>
    </owl:Class>
    


    <!-- http://www.ease-crc.org/ont/SOMA.owl#Opening -->


    <owl:Class rdf:about="http://www.ease-crc.org/ont/SOMA.owl#Opening">
        <rdfs:subClassOf rdf:resource="http://www.ease-crc.org/ont/SOMA.owl#Actuating"/>
        <owl:disjointWith rdf:resource="http://www.ease-crc.org/ont/SOMA.owl#Pulling"/>
        <owl:disjointWith rdf:resource="http://www.ease-crc.org/ont/SOMA.owl#Pushing"/>
        <owl:disjointWith rdf:resource="http://www.ease-crc.org/ont/SOMA.owl#Squeezing"/>
        <rdfs:comment>A task in which an Agent manipulates a container so as to expose its interior.</rdfs:comment>
        <rdfs:isDefinedBy rdf:resource="http://www.ease-crc.org/ont/SOMA-ACT.owl"/>
    </owl:Class>
    


    <!-- http://www.ease-crc.org/ont/SOMA.owl#Orienting -->


    <owl:Class rdf:about="http://www.ease-crc.org/ont/SOMA.owl#Orienting">
        <rdfs:subClassOf rdf:resource="http://www.ease-crc.org/ont/SOMA.owl#Positioning"/>
        <rdfs:comment>A task in which an Agent adjusts the orientation of an object.</rdfs:comment>
        <rdfs:isDefinedBy rdf:resource="http://www.ease-crc.org/ont/SOMA-ACT.owl"/>
    </owl:Class>
    


    <!-- http://www.ease-crc.org/ont/SOMA.owl#Origin -->


    <owl:Class rdf:about="http://www.ease-crc.org/ont/SOMA.owl#Origin">
        <rdfs:subClassOf rdf:resource="http://www.ease-crc.org/ont/SOMA.owl#Location"/>
        <rdfs:comment>A role classifying the location where an event or object originated.</rdfs:comment>
        <rdfs:isDefinedBy rdf:resource="http://www.ease-crc.org/ont/SOMA-OBJ.owl"/>
    </owl:Class>
    


    <!-- http://www.ease-crc.org/ont/SOMA.owl#Pack -->


    <owl:Class rdf:about="http://www.ease-crc.org/ont/SOMA.owl#Pack">
        <rdfs:subClassOf rdf:resource="http://www.ease-crc.org/ont/SOMA.owl#DesignedContainer"/>
        <rdfs:comment>A small cardboard or paper container.</rdfs:comment>
        <rdfs:isDefinedBy rdf:resource="http://www.ease-crc.org/ont/SOMA-HOME.owl"/>
    </owl:Class>
    


    <!-- http://www.ease-crc.org/ont/SOMA.owl#Pan -->


    <owl:Class rdf:about="http://www.ease-crc.org/ont/SOMA.owl#Pan">
        <rdfs:subClassOf rdf:resource="http://www.ease-crc.org/ont/SOMA.owl#Crockery"/>
        <rdfs:comment>A container used for cooking food.</rdfs:comment>
        <rdfs:isDefinedBy rdf:resource="http://www.ease-crc.org/ont/SOMA-HOME.owl"/>
    </owl:Class>
    


    <!-- http://www.ease-crc.org/ont/SOMA.owl#Pancake -->


    <owl:Class rdf:about="http://www.ease-crc.org/ont/SOMA.owl#Pancake">
        <rdfs:subClassOf rdf:resource="http://www.ease-crc.org/ont/SOMA.owl#BakedGood"/>
        <rdfs:isDefinedBy rdf:resource="http://www.ease-crc.org/ont/SOMA-HOME.owl"/>
    </owl:Class>
    


    <!-- http://www.ease-crc.org/ont/SOMA.owl#PancakeMix -->


    <owl:Class rdf:about="http://www.ease-crc.org/ont/SOMA.owl#PancakeMix">
        <rdfs:subClassOf rdf:resource="http://www.ontologydesignpatterns.org/ont/dul/DUL.owl#DesignedSubstance"/>
        <rdfs:isDefinedBy rdf:resource="http://www.ease-crc.org/ont/SOMA-HOME.owl"/>
    </owl:Class>
    


    <!-- http://www.ease-crc.org/ont/SOMA.owl#ParkingArms -->


    <owl:Class rdf:about="http://www.ease-crc.org/ont/SOMA.owl#ParkingArms">
        <rdfs:subClassOf rdf:resource="http://www.ease-crc.org/ont/SOMA.owl#AssumingArmPose"/>
        <rdfs:comment>A task by which an Agent arranges its arms in such a way so as to minimize opportunities for collision while moving through the environment.</rdfs:comment>
        <rdfs:isDefinedBy rdf:resource="http://www.ease-crc.org/ont/SOMA-ACT.owl"/>
        <rdfs:label xml:lang="en">Parking arms</rdfs:label>
    </owl:Class>
    


    <!-- http://www.ease-crc.org/ont/SOMA.owl#PathRole -->


    <owl:Class rdf:about="http://www.ease-crc.org/ont/SOMA.owl#PathRole">
        <rdfs:subClassOf rdf:resource="http://www.ease-crc.org/ont/SOMA.owl#SpatioTemporalRole"/>
        <rdfs:comment>A role that classifies the path of a motion.</rdfs:comment>
        <rdfs:isDefinedBy rdf:resource="http://www.ease-crc.org/ont/SOMA-OBJ.owl"/>
        <rdfs:label xml:lang="en">Path role</rdfs:label>
    </owl:Class>
    


    <!-- http://www.ease-crc.org/ont/SOMA.owl#Patient -->


    <owl:Class rdf:about="http://www.ease-crc.org/ont/SOMA.owl#Patient">
        <rdfs:subClassOf rdf:resource="http://www.ease-crc.org/ont/SOMA.owl#EventAdjacentRole"/>
        <rdfs:comment>A role classifying an object that undergoes/is the primary object affected by the event.</rdfs:comment>
        <rdfs:isDefinedBy rdf:resource="http://www.ease-crc.org/ont/SOMA-OBJ.owl"/>
        <rdfs:isDefinedBy rdf:resource="http://www.ease-crc.org/ont/SOMA-PROC.owl"/>
        <rdfs:isDefinedBy rdf:resource="http://www.ease-crc.org/ont/SOMA-SAY.owl"/>
    </owl:Class>
    


    <!-- http://www.ease-crc.org/ont/SOMA.owl#Perceiving -->


    <owl:Class rdf:about="http://www.ease-crc.org/ont/SOMA.owl#Perceiving">
        <rdfs:subClassOf rdf:resource="http://www.ease-crc.org/ont/SOMA.owl#PhysicalTask"/>
        <rdfs:comment>A task in which the Agent gathers and interprets sensor information about its surroundings.</rdfs:comment>
        <rdfs:isDefinedBy rdf:resource="http://www.ease-crc.org/ont/SOMA-ACT.owl"/>
    </owl:Class>
    


    <!-- http://www.ease-crc.org/ont/SOMA.owl#PhaseTransition -->


    <owl:Class rdf:about="http://www.ease-crc.org/ont/SOMA.owl#PhaseTransition">
        <rdfs:subClassOf rdf:resource="http://www.ease-crc.org/ont/SOMA.owl#Alteration"/>
        <rdfs:comment>An EventType that classifies processes by which matter changes from some distinguishable phase to another. We will use this to refer to the classical phase transitions between Solid, Liquid, Gaseous, Plasma etc. phases.</rdfs:comment>
        <rdfs:isDefinedBy rdf:resource="http://www.ease-crc.org/ont/SOMA-PROC.owl"/>
        <rdfs:label>Phase transition</rdfs:label>
        <rdfs:seeAlso>The phase transition concept has also been more or less metaphorically applied in other contexts. An example from physics is the &quot;jamming transition&quot;, and sometimes &quot;phase transitions&quot; are spoken of when describing problem spaces such as 3SAT.

In all these cases, the metaphor points to the existence of several regions of qualitatively different behavior (unimpeded passage of solid grains vs deadlock in a corridor; problem instances where the answer NO is trivial to prove vs. problem instances where the answer YES is trivial to prove), separated fairly sharply when some quantity reaches a threshold.</rdfs:seeAlso>
    </owl:Class>
    


    <!-- http://www.ease-crc.org/ont/SOMA.owl#Phrase -->


    <owl:Class rdf:about="http://www.ease-crc.org/ont/SOMA.owl#Phrase">
        <rdfs:subClassOf rdf:resource="http://www.ease-crc.org/ont/SOMA.owl#LinguisticObject"/>
        <rdfs:isDefinedBy rdf:resource="http://www.ease-crc.org/ont/SOMA-SAY.owl"/>
        <rdfs:isDefinedBy rdf:resource="http://www.ontologydesignpatterns.org/ont/dul/IOLite.owl"/>
    </owl:Class>
    


    <!-- http://www.ease-crc.org/ont/SOMA.owl#PhysicalAccessibility -->


    <owl:Class rdf:about="http://www.ease-crc.org/ont/SOMA.owl#PhysicalAccessibility">
        <rdfs:subClassOf rdf:resource="http://www.ease-crc.org/ont/SOMA.owl#StateType"/>
        <rdfs:subClassOf>
            <owl:Restriction>
                <owl:onProperty rdf:resource="http://www.ease-crc.org/ont/SOMA.owl#isStateTypeOf"/>
                <owl:someValuesFrom rdf:resource="http://www.ease-crc.org/ont/SOMA.owl#Item"/>
            </owl:Restriction>
        </rdfs:subClassOf>
        <rdfs:subClassOf>
            <owl:Restriction>
                <owl:onProperty rdf:resource="http://www.ease-crc.org/ont/SOMA.owl#isStateTypeOf"/>
                <owl:someValuesFrom rdf:resource="http://www.ease-crc.org/ont/SOMA.owl#Restrictor"/>
            </owl:Restriction>
        </rdfs:subClassOf>
        <rdfs:comment>Classifies States in which an item is placed in a container or protected by a protector, but the placement of the item and container is such that a, usually agentive, accessor may nevertheless reach the item in order to perform a task.</rdfs:comment>
        <rdfs:isDefinedBy rdf:resource="http://www.ease-crc.org/ont/SOMA-STATE.owl"/>
        <rdfs:label xml:lang="en">Physical accessibility</rdfs:label>
    </owl:Class>
    


    <!-- http://www.ease-crc.org/ont/SOMA.owl#PhysicalAcquiring -->


    <owl:Class rdf:about="http://www.ease-crc.org/ont/SOMA.owl#PhysicalAcquiring">
        <rdfs:subClassOf rdf:resource="http://www.ease-crc.org/ont/SOMA.owl#ModifyingPhysicalObject"/>
        <rdfs:comment>The goal of this task is to make some object usable for other tasks, by possibly changing its physical state. Usually, it overlaps some task that describes the manner in which an object is obtained.

The prototypical example of PhysicalAcquiring is picking up an object.

Note that buying an object is NOT PhysicalAcquiring. Buying, or ownership transfer in general, also involves an adjustment in social structures describing ownership.</rdfs:comment>
        <rdfs:isDefinedBy rdf:resource="http://www.ease-crc.org/ont/SOMA-ACT.owl"/>
        <rdfs:label xml:lang="en">Physical acquiring</rdfs:label>
    </owl:Class>
    


    <!-- http://www.ease-crc.org/ont/SOMA.owl#PhysicalAction -->


    <owl:Class rdf:about="http://www.ease-crc.org/ont/SOMA.owl#PhysicalAction">
        <rdfs:subClassOf rdf:resource="http://www.ontologydesignpatterns.org/ont/dul/DUL.owl#Action"/>
        <rdfs:comment>An action performed by an agent by using its body in some way to interact with the physical world, e.g., through manipulation of objects, or by changing the posture.</rdfs:comment>
        <rdfs:isDefinedBy rdf:resource="http://www.ease-crc.org/ont/SOMA-ACT.owl"/>
        <rdfs:label>Physical action</rdfs:label>
    </owl:Class>
    


    <!-- http://www.ease-crc.org/ont/SOMA.owl#PhysicalBlockage -->


    <owl:Class rdf:about="http://www.ease-crc.org/ont/SOMA.owl#PhysicalBlockage">
        <rdfs:subClassOf rdf:resource="http://www.ease-crc.org/ont/SOMA.owl#StateType"/>
        <rdfs:subClassOf>
            <owl:Restriction>
                <owl:onProperty rdf:resource="http://www.ease-crc.org/ont/SOMA.owl#isStateTypeOf"/>
                <owl:someValuesFrom rdf:resource="http://www.ease-crc.org/ont/SOMA.owl#Item"/>
            </owl:Restriction>
        </rdfs:subClassOf>
        <rdfs:subClassOf>
            <owl:Restriction>
                <owl:onProperty rdf:resource="http://www.ease-crc.org/ont/SOMA.owl#isStateTypeOf"/>
                <owl:someValuesFrom rdf:resource="http://www.ease-crc.org/ont/SOMA.owl#Restrictor"/>
            </owl:Restriction>
        </rdfs:subClassOf>
        <rdfs:comment>Classifies States in which an object, in general called restrictor, blocks access to an item. A usually agentive accessor, whose access is blocked, may be specified.</rdfs:comment>
        <rdfs:isDefinedBy rdf:resource="http://www.ease-crc.org/ont/SOMA-STATE.owl"/>
        <rdfs:label xml:lang="en">Physical blockage</rdfs:label>
    </owl:Class>
    


    <!-- http://www.ease-crc.org/ont/SOMA.owl#PhysicalEffector -->


    <owl:Class rdf:about="http://www.ease-crc.org/ont/SOMA.owl#PhysicalEffector">
        <rdfs:subClassOf rdf:resource="http://www.ease-crc.org/ont/SOMA.owl#FunctionalPart"/>
        <rdfs:subClassOf>
            <owl:Restriction>
                <owl:onProperty>
                    <rdf:Description>
                        <owl:inverseOf rdf:resource="http://www.ontologydesignpatterns.org/ont/dul/DUL.owl#hasPart"/>
                    </rdf:Description>
                </owl:onProperty>
                <owl:someValuesFrom rdf:resource="http://www.ontologydesignpatterns.org/ont/dul/DUL.owl#PhysicalAgent"/>
            </owl:Restriction>
        </rdfs:subClassOf>
        <rdfs:comment>A functional part belonging to an Agent and which allows that Agent to act upon its surroundings.</rdfs:comment>
        <rdfs:isDefinedBy rdf:resource="http://www.ease-crc.org/ont/SOMA-OBJ.owl"/>
        <rdfs:isDefinedBy rdf:resource="http://www.ease-crc.org/ont/SOMA-PROC.owl"/>
        <rdfs:label>Physical effector</rdfs:label>
    </owl:Class>
    


    <!-- http://www.ease-crc.org/ont/SOMA.owl#PhysicalExistence -->


    <owl:Class rdf:about="http://www.ease-crc.org/ont/SOMA.owl#PhysicalExistence">
        <rdfs:subClassOf rdf:resource="http://www.ease-crc.org/ont/SOMA.owl#PhysicalState"/>
        <rdfs:comment>A State in which an Entity is said to exist in the physical world.</rdfs:comment>
        <rdfs:isDefinedBy rdf:resource="http://www.ease-crc.org/ont/SOMA-STATE.owl"/>
        <rdfs:label xml:lang="en">Physical Existince</rdfs:label>
    </owl:Class>
    


    <!-- http://www.ease-crc.org/ont/SOMA.owl#PhysicalQuality -->


    <owl:Class rdf:about="http://www.ease-crc.org/ont/SOMA.owl#PhysicalQuality">
        <rdfs:subClassOf rdf:resource="http://www.ontologydesignpatterns.org/ont/dul/DUL.owl#Quality"/>
        <rdfs:subClassOf>
            <owl:Restriction>
                <owl:onProperty rdf:resource="http://www.ontologydesignpatterns.org/ont/dul/DUL.owl#isQualityOf"/>
                <owl:qualifiedCardinality rdf:datatype="http://www.w3.org/2001/XMLSchema#nonNegativeInteger">1</owl:qualifiedCardinality>
                <owl:onClass rdf:resource="http://www.ontologydesignpatterns.org/ont/dul/DUL.owl#PhysicalObject"/>
            </owl:Restriction>
        </rdfs:subClassOf>
        <rdfs:comment>Any aspect of an entity that is dependent on its physical manifestation.</rdfs:comment>
        <rdfs:isDefinedBy rdf:resource="http://www.ease-crc.org/ont/SOMA-OBJ.owl"/>
        <rdfs:label>Physical quality</rdfs:label>
    </owl:Class>
    


    <!-- http://www.ease-crc.org/ont/SOMA.owl#PhysicalState -->


    <owl:Class rdf:about="http://www.ease-crc.org/ont/SOMA.owl#PhysicalState">
        <rdfs:subClassOf rdf:resource="http://www.ease-crc.org/ont/SOMA.owl#State"/>
        <rdfs:subClassOf>
            <owl:Restriction>
                <owl:onProperty rdf:resource="http://www.ontologydesignpatterns.org/ont/dul/DUL.owl#hasParticipant"/>
                <owl:someValuesFrom rdf:resource="http://www.ontologydesignpatterns.org/ont/dul/DUL.owl#PhysicalObject"/>
            </owl:Restriction>
        </rdfs:subClassOf>
        <rdfs:comment>A State describing how Entities in the physical world relate to each other.</rdfs:comment>
        <rdfs:isDefinedBy rdf:resource="http://www.ease-crc.org/ont/SOMA-STATE.owl"/>
        <rdfs:label>Physical state</rdfs:label>
    </owl:Class>
    


    <!-- http://www.ease-crc.org/ont/SOMA.owl#PhysicalTask -->


    <owl:Class rdf:about="http://www.ease-crc.org/ont/SOMA.owl#PhysicalTask">
        <rdfs:subClassOf rdf:resource="http://www.ontologydesignpatterns.org/ont/dul/DUL.owl#Task"/>
        <rdfs:subClassOf>
            <owl:Restriction>
                <owl:onProperty rdf:resource="http://www.ontologydesignpatterns.org/ont/dul/DUL.owl#classifies"/>
                <owl:allValuesFrom>
                    <owl:Class>
                        <owl:intersectionOf rdf:parseType="Collection">
                            <rdf:Description rdf:about="http://www.ontologydesignpatterns.org/ont/dul/DUL.owl#Action"/>
                            <owl:Class>
                                <owl:unionOf rdf:parseType="Collection">
                                    <owl:Restriction>
                                        <owl:onProperty rdf:resource="http://www.ontologydesignpatterns.org/ont/dul/DUL.owl#hasParticipant"/>
                                        <owl:someValuesFrom rdf:resource="http://www.ontologydesignpatterns.org/ont/dul/DUL.owl#PhysicalAgent"/>
                                    </owl:Restriction>
                                    <owl:Restriction>
                                        <owl:onProperty rdf:resource="http://www.ontologydesignpatterns.org/ont/dul/DUL.owl#hasParticipant"/>
                                        <owl:someValuesFrom rdf:resource="http://www.ontologydesignpatterns.org/ont/dul/DUL.owl#PhysicalObject"/>
                                    </owl:Restriction>
                                </owl:unionOf>
                            </owl:Class>
                        </owl:intersectionOf>
                    </owl:Class>
                </owl:allValuesFrom>
            </owl:Restriction>
        </rdfs:subClassOf>
        <rdfs:comment>A task in which a PhysicalAgent affects some physical object.</rdfs:comment>
        <rdfs:isDefinedBy rdf:resource="http://www.ease-crc.org/ont/SOMA-ACT.owl"/>
        <rdfs:label xml:lang="en">Physical task</rdfs:label>
    </owl:Class>
    


    <!-- http://www.ease-crc.org/ont/SOMA.owl#PhysicsProcess -->


    <owl:Class rdf:about="http://www.ease-crc.org/ont/SOMA.owl#PhysicsProcess">
        <rdfs:subClassOf rdf:resource="http://www.ontologydesignpatterns.org/ont/dul/DUL.owl#Process"/>
        <rdfs:subClassOf>
            <owl:Restriction>
                <owl:onProperty rdf:resource="http://www.ontologydesignpatterns.org/ont/dul/DUL.owl#hasParticipant"/>
                <owl:someValuesFrom rdf:resource="http://www.ontologydesignpatterns.org/ont/dul/DUL.owl#PhysicalObject"/>
            </owl:Restriction>
        </rdfs:subClassOf>
        <rdfs:comment>A process involving physical objects and phenomena which does not change the chemical constituency of the affected objects.</rdfs:comment>
        <rdfs:isDefinedBy rdf:resource="http://www.ease-crc.org/ont/SOMA-PROC.owl"/>
        <rdfs:label>Physical process</rdfs:label>
    </owl:Class>
    


    <!-- http://www.ease-crc.org/ont/SOMA.owl#PickingUp -->


    <owl:Class rdf:about="http://www.ease-crc.org/ont/SOMA.owl#PickingUp">
        <rdfs:subClassOf rdf:resource="http://www.ease-crc.org/ont/SOMA.owl#Manipulating"/>
        <rdfs:comment>A task in which the Agent uses one or more of its grippers to grasp a usually stationary object.</rdfs:comment>
        <rdfs:isDefinedBy rdf:resource="http://www.ease-crc.org/ont/SOMA-ACT.owl"/>
    </owl:Class>
    


    <!-- http://www.ease-crc.org/ont/SOMA.owl#Placing -->


    <owl:Class rdf:about="http://www.ease-crc.org/ont/SOMA.owl#Placing">
        <rdfs:subClassOf rdf:resource="http://www.ease-crc.org/ont/SOMA.owl#PhysicalTask"/>
        <rdfs:comment>Distinguished from Positioning in that this task is more about placing an object at a functionally specified location (e.g., place the cup on the table) as opposed to positioning an object at a location defined by coordinates or a region of coordinates (position the cup at xyz).</rdfs:comment>
        <rdfs:isDefinedBy rdf:resource="http://www.ease-crc.org/ont/SOMA-ACT.owl"/>
    </owl:Class>
    


    <!-- http://www.ease-crc.org/ont/SOMA.owl#PlacingTheory -->


    <owl:Class rdf:about="http://www.ease-crc.org/ont/SOMA.owl#PlacingTheory">
        <rdfs:subClassOf rdf:resource="http://www.ease-crc.org/ont/SOMA.owl#ExecutableSchematicTheory"/>
        <rdfs:subClassOf>
            <owl:Restriction>
                <owl:onProperty rdf:resource="http://www.ontologydesignpatterns.org/ont/dul/DUL.owl#defines"/>
                <owl:someValuesFrom rdf:resource="http://www.ease-crc.org/ont/SOMA.owl#Destination"/>
            </owl:Restriction>
        </rdfs:subClassOf>
        <rdfs:subClassOf>
            <owl:Restriction>
                <owl:onProperty rdf:resource="http://www.ontologydesignpatterns.org/ont/dul/DUL.owl#defines"/>
                <owl:someValuesFrom rdf:resource="http://www.ease-crc.org/ont/SOMA.owl#Patient"/>
            </owl:Restriction>
        </rdfs:subClassOf>
        <rdfs:comment>A schematic theory of how an agent can place a patient at a particular goal location.</rdfs:comment>
        <rdfs:isDefinedBy rdf:resource="http://www.ease-crc.org/ont/SOMA-SAY.owl"/>
        <rdfs:label xml:lang="en">Placing theory</rdfs:label>
    </owl:Class>
    


    <!-- http://www.ease-crc.org/ont/SOMA.owl#Planning -->


    <owl:Class rdf:about="http://www.ease-crc.org/ont/SOMA.owl#Planning">
        <rdfs:subClassOf rdf:resource="http://www.ease-crc.org/ont/SOMA.owl#Prospecting"/>
        <rdfs:subClassOf>
            <owl:Restriction>
                <owl:onProperty rdf:resource="http://www.ontologydesignpatterns.org/ont/dul/DUL.owl#isTaskOf"/>
                <owl:someValuesFrom>
                    <owl:Restriction>
                        <owl:onProperty rdf:resource="http://www.ontologydesignpatterns.org/ont/dul/DUL.owl#classifies"/>
                        <owl:someValuesFrom rdf:resource="http://www.ontologydesignpatterns.org/ont/dul/DUL.owl#Plan"/>
                    </owl:Restriction>
                </owl:someValuesFrom>
            </owl:Restriction>
        </rdfs:subClassOf>
        <rdfs:comment>A Mental task in which the Agent endeavours to create a sequence of actions for itself which, if followed, will bring about a particular state of affairs in the world. This particular state of affairs is known to the agent and is often called the goal state of the planning action. Planning commits itself to feasibility: the Agent attempts to find a sequence of actions that it believes it will actually be able to perform.</rdfs:comment>
        <rdfs:isDefinedBy rdf:resource="http://www.ease-crc.org/ont/SOMA-ACT.owl"/>
    </owl:Class>
    


    <!-- http://www.ease-crc.org/ont/SOMA.owl#Plate -->


    <owl:Class rdf:about="http://www.ease-crc.org/ont/SOMA.owl#Plate">
        <rdfs:subClassOf rdf:resource="http://www.ease-crc.org/ont/SOMA.owl#Crockery"/>
        <rdfs:comment>A flat and usually circular object from which food is eaten or served.</rdfs:comment>
        <rdfs:isDefinedBy rdf:resource="http://www.ease-crc.org/ont/SOMA-HOME.owl"/>
    </owl:Class>
    


    <!-- http://www.ease-crc.org/ont/SOMA.owl#PluginRole -->


    <owl:Class rdf:about="http://www.ease-crc.org/ont/SOMA.owl#PluginRole">
        <rdfs:subClassOf rdf:resource="http://www.ease-crc.org/ont/SOMA.owl#InterfaceComponentRole"/>
        <rdfs:subClassOf>
            <owl:Restriction>
                <owl:onProperty rdf:resource="http://www.ontologydesignpatterns.org/ont/dul/DUL.owl#isDefinedIn"/>
                <owl:someValuesFrom rdf:resource="http://www.ease-crc.org/ont/SOMA.owl#PluginSpecification"/>
            </owl:Restriction>
        </rdfs:subClassOf>
        <rdfs:comment xml:lang="en">In the Plug-in-Host pattern, a Host application provides services which the Plug-in can use, including a way for Plug-ins to register themselves with the Host application and a protocol for the exchange of data withPplug-ins. Plug-ins depend on the services provided by the host application and do not usually work by themselves. Conversely, the host application operates independently of the plug-ins, making it possible for end-users to add and update plug-ins dynamically without needing to make changes to the host application.

Source: https://en.wikipedia.org/wiki/Plug-in_(computing)</rdfs:comment>
        <rdfs:isDefinedBy rdf:resource="http://www.ease-crc.org/ont/SOMA-IO.owl"/>
        <rdfs:label xml:lang="en">Plugin role</rdfs:label>
    </owl:Class>
    


    <!-- http://www.ease-crc.org/ont/SOMA.owl#PluginSpecification -->


    <owl:Class rdf:about="http://www.ease-crc.org/ont/SOMA.owl#PluginSpecification">
        <rdfs:subClassOf rdf:resource="http://www.ease-crc.org/ont/SOMA.owl#API_Specification"/>
        <rdfs:subClassOf>
            <owl:Class>
                <owl:intersectionOf rdf:parseType="Collection">
                    <owl:Restriction>
                        <owl:onProperty rdf:resource="http://www.ontologydesignpatterns.org/ont/dul/DUL.owl#definesRole"/>
                        <owl:someValuesFrom rdf:resource="http://www.ease-crc.org/ont/SOMA.owl#HostRole"/>
                    </owl:Restriction>
                    <owl:Restriction>
                        <owl:onProperty rdf:resource="http://www.ontologydesignpatterns.org/ont/dul/DUL.owl#definesRole"/>
                        <owl:someValuesFrom rdf:resource="http://www.ease-crc.org/ont/SOMA.owl#PluginRole"/>
                    </owl:Restriction>
                </owl:intersectionOf>
            </owl:Class>
        </rdfs:subClassOf>
        <rdfs:comment xml:lang="en">The Specification of a Plugin interface defines how a Host and a Plug-in function together and exchange information.</rdfs:comment>
        <rdfs:isDefinedBy rdf:resource="http://www.ease-crc.org/ont/SOMA-IO.owl"/>
        <rdfs:label xml:lang="en">Plugin Specification</rdfs:label>
    </owl:Class>
    


    <!-- http://www.ease-crc.org/ont/SOMA.owl#Positioning -->


    <owl:Class rdf:about="http://www.ease-crc.org/ont/SOMA.owl#Positioning">
        <rdfs:subClassOf rdf:resource="http://www.ease-crc.org/ont/SOMA.owl#Actuating"/>
        <rdfs:comment>A task in which an Agent places an object at a particular position.</rdfs:comment>
        <rdfs:isDefinedBy rdf:resource="http://www.ease-crc.org/ont/SOMA-ACT.owl"/>
    </owl:Class>
    


    <!-- http://www.ease-crc.org/ont/SOMA.owl#PosturalMoving -->


    <owl:Class rdf:about="http://www.ease-crc.org/ont/SOMA.owl#PosturalMoving">
        <rdfs:subClassOf rdf:resource="http://www.ease-crc.org/ont/SOMA.owl#BodyMovement"/>
        <rdfs:comment>The Agent changes or takes an overall configuration of its body but is otherwise not significantly affecting other objects nor moving a significant amount from its original location.

Posture changes may take place as part of other actions, for example turning when walking.</rdfs:comment>
        <rdfs:isDefinedBy rdf:resource="http://www.ease-crc.org/ont/SOMA-PROC.owl"/>
    </owl:Class>
    


    <!-- http://www.ease-crc.org/ont/SOMA.owl#Pot -->


    <owl:Class rdf:about="http://www.ease-crc.org/ont/SOMA.owl#Pot">
        <rdfs:subClassOf rdf:resource="http://www.ease-crc.org/ont/SOMA.owl#Crockery"/>
        <rdfs:comment>A container used for cooking food.</rdfs:comment>
        <rdfs:isDefinedBy rdf:resource="http://www.ease-crc.org/ont/SOMA-HOME.owl"/>
    </owl:Class>
    


    <!-- http://www.ease-crc.org/ont/SOMA.owl#PowerGrasp -->


    <owl:Class rdf:about="http://www.ease-crc.org/ont/SOMA.owl#PowerGrasp">
        <rdfs:subClassOf rdf:resource="http://www.ease-crc.org/ont/SOMA.owl#GraspingMotion"/>
        <owl:disjointWith rdf:resource="http://www.ease-crc.org/ont/SOMA.owl#PrecisionGrasp"/>
        <rdfs:comment>An Agent grasps an object, and focuses on obtaining a strong grasping force upon it, resulting in a grasp able to resist significant outside disturbances. This is useful when using tools with which to later exert force on other things, e.g. when hammering nails.</rdfs:comment>
        <rdfs:isDefinedBy rdf:resource="http://www.ease-crc.org/ont/SOMA-PROC.owl"/>
        <rdfs:label>Power grasp</rdfs:label>
    </owl:Class>
    


    <!-- http://www.ease-crc.org/ont/SOMA.owl#PrecisionGrasp -->


    <owl:Class rdf:about="http://www.ease-crc.org/ont/SOMA.owl#PrecisionGrasp">
        <rdfs:subClassOf rdf:resource="http://www.ease-crc.org/ont/SOMA.owl#GraspingMotion"/>
        <rdfs:comment>An Agent grasps an object, and focuses on obtaining precise kinematic control over it. This is useful for then following precise movements, e.g. when writing.</rdfs:comment>
        <rdfs:isDefinedBy rdf:resource="http://www.ease-crc.org/ont/SOMA-PROC.owl"/>
        <rdfs:label>Precision grasp</rdfs:label>
    </owl:Class>
    


    <!-- http://www.ease-crc.org/ont/SOMA.owl#Prediction -->


    <owl:Class rdf:about="http://www.ease-crc.org/ont/SOMA.owl#Prediction">
        <rdfs:subClassOf rdf:resource="http://www.ease-crc.org/ont/SOMA.owl#Prospecting"/>
        <rdfs:comment>A Mental task in which the Agent endeavours to construct a representation of a future state of the world. Prediction commits itself to some degree of accuracy: the Agent believes that eventually something similar to the predicted state will come to pass.</rdfs:comment>
        <rdfs:isDefinedBy rdf:resource="http://www.ease-crc.org/ont/SOMA-ACT.owl"/>
    </owl:Class>
    


    <!-- http://www.ease-crc.org/ont/SOMA.owl#PrehensileEffector -->


    <owl:Class rdf:about="http://www.ease-crc.org/ont/SOMA.owl#PrehensileEffector">
        <rdfs:subClassOf rdf:resource="http://www.ease-crc.org/ont/SOMA.owl#PhysicalEffector"/>
        <rdfs:comment>An effector used to grasp objects, such as a hand of a human, or the long prehensile tail of a monkey.</rdfs:comment>
        <rdfs:isDefinedBy rdf:resource="http://www.ease-crc.org/ont/SOMA-OBJ.owl"/>
        <rdfs:isDefinedBy rdf:resource="http://www.ease-crc.org/ont/SOMA-PROC.owl"/>
        <rdfs:label>Prehensile effector</rdfs:label>
    </owl:Class>
    


    <!-- http://www.ease-crc.org/ont/SOMA.owl#PrehensileMotion -->


    <owl:Class rdf:about="http://www.ease-crc.org/ont/SOMA.owl#PrehensileMotion">
        <owl:equivalentClass>
            <owl:Class>
                <owl:unionOf rdf:parseType="Collection">
                    <rdf:Description rdf:about="http://www.ease-crc.org/ont/SOMA.owl#GraspingMotion"/>
                    <rdf:Description rdf:about="http://www.ease-crc.org/ont/SOMA.owl#ReleasingMotion"/>
                </owl:unionOf>
            </owl:Class>
        </owl:equivalentClass>
        <rdfs:subClassOf rdf:resource="http://www.ease-crc.org/ont/SOMA.owl#DirectedMotion"/>
        <rdfs:subClassOf>
            <owl:Restriction>
                <owl:onProperty rdf:resource="http://www.ease-crc.org/ont/SOMA.owl#isProcessTypeOf"/>
                <owl:someValuesFrom>
                    <owl:Class>
                        <owl:intersectionOf rdf:parseType="Collection">
                            <rdf:Description rdf:about="http://www.ease-crc.org/ont/SOMA.owl#MovedObject"/>
                            <owl:Restriction>
                                <owl:onProperty rdf:resource="http://www.ontologydesignpatterns.org/ont/dul/DUL.owl#classifies"/>
                                <owl:allValuesFrom rdf:resource="http://www.ease-crc.org/ont/SOMA.owl#PrehensileEffector"/>
                            </owl:Restriction>
                        </owl:intersectionOf>
                    </owl:Class>
                </owl:someValuesFrom>
            </owl:Restriction>
        </rdfs:subClassOf>
        <rdfs:comment>A motion of a prehensile effector.</rdfs:comment>
        <rdfs:isDefinedBy rdf:resource="http://www.ease-crc.org/ont/SOMA-PROC.owl"/>
        <rdfs:label>Prehensile motion</rdfs:label>
    </owl:Class>
    


    <!-- http://www.ease-crc.org/ont/SOMA.owl#PreservativeInteraction -->


    <owl:Class rdf:about="http://www.ease-crc.org/ont/SOMA.owl#PreservativeInteraction">
        <rdfs:subClassOf rdf:resource="http://www.ease-crc.org/ont/SOMA.owl#ForceInteraction"/>
        <rdfs:comment>A force interaction where the agonist has a tendency to keep another object still. An example is &apos;holding a door closed&apos; where some object interacts with the door to neutralize forces that could set the door into motion.</rdfs:comment>
        <rdfs:isDefinedBy rdf:resource="http://www.ease-crc.org/ont/SOMA-PROC.owl"/>
        <rdfs:label>Preservative interaction</rdfs:label>
    </owl:Class>
    


    <!-- http://www.ease-crc.org/ont/SOMA.owl#ProcessFlow -->


    <owl:Class rdf:about="http://www.ease-crc.org/ont/SOMA.owl#ProcessFlow">
        <rdfs:subClassOf rdf:resource="http://www.ontologydesignpatterns.org/ont/dul/DUL.owl#Description"/>
        <rdfs:subClassOf>
            <owl:Restriction>
                <owl:onProperty rdf:resource="http://www.ease-crc.org/ont/SOMA.owl#definesProcess"/>
                <owl:someValuesFrom rdf:resource="http://www.ease-crc.org/ont/SOMA.owl#ProcessType"/>
            </owl:Restriction>
        </rdfs:subClassOf>
        <rdfs:comment>A description that structures a Process.</rdfs:comment>
        <rdfs:isDefinedBy rdf:resource="http://www.ease-crc.org/ont/SOMA-PROC.owl"/>
        <rdfs:label>Process flow</rdfs:label>
    </owl:Class>
    


    <!-- http://www.ease-crc.org/ont/SOMA.owl#ProcessType -->


    <owl:Class rdf:about="http://www.ease-crc.org/ont/SOMA.owl#ProcessType">
        <rdfs:subClassOf rdf:resource="http://www.ontologydesignpatterns.org/ont/dul/DUL.owl#EventType"/>
        <rdfs:subClassOf>
            <owl:Restriction>
                <owl:onProperty rdf:resource="http://www.ontologydesignpatterns.org/ont/dul/DUL.owl#classifies"/>
                <owl:allValuesFrom rdf:resource="http://www.ontologydesignpatterns.org/ont/dul/DUL.owl#Process"/>
            </owl:Restriction>
        </rdfs:subClassOf>
        <rdfs:subClassOf>
            <owl:Restriction>
                <owl:onProperty rdf:resource="http://www.ontologydesignpatterns.org/ont/dul/DUL.owl#hasPart"/>
                <owl:allValuesFrom rdf:resource="http://www.ease-crc.org/ont/SOMA.owl#ProcessType"/>
            </owl:Restriction>
        </rdfs:subClassOf>
        <rdfs:subClassOf>
            <owl:Restriction>
                <owl:onProperty rdf:resource="http://www.ontologydesignpatterns.org/ont/dul/DUL.owl#isDefinedIn"/>
                <owl:allValuesFrom rdf:resource="http://www.ontologydesignpatterns.org/ont/dul/DUL.owl#Description"/>
            </owl:Restriction>
        </rdfs:subClassOf>
        <rdfs:comment>An EventType that classifies Processes.</rdfs:comment>
        <rdfs:isDefinedBy rdf:resource="http://www.ease-crc.org/ont/SOMA-PROC.owl"/>
        <rdfs:label>Process type</rdfs:label>
    </owl:Class>
    


    <!-- http://www.ease-crc.org/ont/SOMA.owl#Programming_Language -->


    <owl:Class rdf:about="http://www.ease-crc.org/ont/SOMA.owl#Programming_Language">
        <rdfs:subClassOf rdf:resource="http://www.ease-crc.org/ont/SOMA.owl#Computer_Language"/>
        <rdfs:subClassOf>
            <owl:Restriction>
                <owl:onProperty rdf:resource="http://www.ease-crc.org/ont/SOMA.owl#givesMeaningTo"/>
                <owl:allValuesFrom rdf:resource="http://www.ease-crc.org/ont/SOMA.owl#Computer_Program"/>
            </owl:Restriction>
        </rdfs:subClassOf>
        <rdfs:comment xml:lang="en">Any Programming Language, including both human-readable like Java and non-human-readable languages like binary machine code.</rdfs:comment>
        <rdfs:isDefinedBy rdf:resource="http://www.ease-crc.org/ont/SOMA-IO.owl"/>
        <rdfs:label xml:lang="en">Programming language</rdfs:label>
    </owl:Class>
    


    <!-- http://www.ease-crc.org/ont/SOMA.owl#Progression -->


    <owl:Class rdf:about="http://www.ease-crc.org/ont/SOMA.owl#Progression">
        <owl:equivalentClass>
            <owl:Restriction>
                <owl:onProperty rdf:resource="http://www.ontologydesignpatterns.org/ont/dul/DUL.owl#satisfies"/>
                <owl:someValuesFrom rdf:resource="http://www.ease-crc.org/ont/SOMA.owl#ProcessFlow"/>
            </owl:Restriction>
        </owl:equivalentClass>
        <rdfs:subClassOf rdf:resource="http://www.ontologydesignpatterns.org/ont/dul/DUL.owl#Situation"/>
        <rdfs:comment>A situation that sattisies a description of how a process evolves over time.</rdfs:comment>
        <rdfs:isDefinedBy rdf:resource="http://www.ease-crc.org/ont/SOMA-PROC.owl"/>
    </owl:Class>
    


    <!-- http://www.ease-crc.org/ont/SOMA.owl#Proprioceiving -->


    <owl:Class rdf:about="http://www.ease-crc.org/ont/SOMA.owl#Proprioceiving">
        <rdfs:subClassOf rdf:resource="http://www.ease-crc.org/ont/SOMA.owl#PhysicalTask"/>
        <rdfs:comment>A task in which the Agent gathers and interprets sensor information about itself.</rdfs:comment>
        <rdfs:isDefinedBy rdf:resource="http://www.ease-crc.org/ont/SOMA-ACT.owl"/>
    </owl:Class>
    


    <!-- http://www.ease-crc.org/ont/SOMA.owl#Prospecting -->


    <owl:Class rdf:about="http://www.ease-crc.org/ont/SOMA.owl#Prospecting">
        <rdfs:subClassOf rdf:resource="http://www.ease-crc.org/ont/SOMA.owl#MentalTask"/>
        <rdfs:comment>A Mental task in which an Agent endeavours to construct a representation of a future state of affairs of the world it is embodied in.</rdfs:comment>
        <rdfs:isDefinedBy rdf:resource="http://www.ease-crc.org/ont/SOMA-ACT.owl"/>
    </owl:Class>
    


    <!-- http://www.ease-crc.org/ont/SOMA.owl#Protector -->


    <owl:Class rdf:about="http://www.ease-crc.org/ont/SOMA.owl#Protector">
        <rdfs:subClassOf rdf:resource="http://www.ease-crc.org/ont/SOMA.owl#Restrictor"/>
        <rdfs:comment>A role classifying an object that protects another by preventing other entities from coming in contact with the protected object.</rdfs:comment>
        <rdfs:isDefinedBy rdf:resource="http://www.ease-crc.org/ont/SOMA-OBJ.owl"/>
    </owl:Class>
    


    <!-- http://www.ease-crc.org/ont/SOMA.owl#ProximalTheory -->


    <owl:Class rdf:about="http://www.ease-crc.org/ont/SOMA.owl#ProximalTheory">
        <rdfs:subClassOf rdf:resource="http://www.ease-crc.org/ont/SOMA.owl#ImageSchemaTheory"/>
        <rdfs:subClassOf>
            <owl:Restriction>
                <owl:onProperty rdf:resource="http://www.ontologydesignpatterns.org/ont/dul/DUL.owl#defines"/>
                <owl:someValuesFrom rdf:resource="http://www.ease-crc.org/ont/SOMA.owl#LocatumRole"/>
            </owl:Restriction>
        </rdfs:subClassOf>
        <rdfs:subClassOf>
            <owl:Restriction>
                <owl:onProperty rdf:resource="http://www.ontologydesignpatterns.org/ont/dul/DUL.owl#defines"/>
                <owl:someValuesFrom rdf:resource="http://www.ease-crc.org/ont/SOMA.owl#RelatumRole"/>
            </owl:Restriction>
        </rdfs:subClassOf>
        <rdfs:comment>An image schematic theory that describes a qualitative spatial relation indicating relative proximity, as expressed by the prepositions &apos;near&apos;, &apos;close to&apos;, &apos;next to&apos;, etc.

It may seem that proximity is a very simple notion, requiring no sophisticated theoretical underpinnings. However, proximity is an extremely object- and purpose-dependent relation. A store next door is in a closeness relation to a person, and so is the Sun in the sky, despite the physical distances being different by several orders of magnitude.

As such, a theory, i.e. a description of what a particular kind of closeness means and in which contexts it applies, is necessary.

Adopted from GUM-4-space (Bateman et al. 2010).

Let xL, xR be objects filling the locatum, relatum roles of this schema. Then one can infer that xL &apos;near to&apos; xR.</rdfs:comment>
        <rdfs:isDefinedBy rdf:resource="http://www.ease-crc.org/ont/SOMA-SAY.owl"/>
        <rdfs:label xml:lang="en">Proximal theory</rdfs:label>
    </owl:Class>
    


    <!-- http://www.ease-crc.org/ont/SOMA.owl#Pulling -->


    <owl:Class rdf:about="http://www.ease-crc.org/ont/SOMA.owl#Pulling">
        <rdfs:subClassOf rdf:resource="http://www.ease-crc.org/ont/SOMA.owl#Actuating"/>
        <owl:disjointWith rdf:resource="http://www.ease-crc.org/ont/SOMA.owl#Pushing"/>
        <owl:disjointWith rdf:resource="http://www.ease-crc.org/ont/SOMA.owl#Squeezing"/>
        <rdfs:comment>A task in which an Agent moves an object in a direction loosely from the object&apos;s center of mass towards the contact point between agent and object.</rdfs:comment>
        <rdfs:isDefinedBy rdf:resource="http://www.ease-crc.org/ont/SOMA-ACT.owl"/>
    </owl:Class>
    


    <!-- http://www.ease-crc.org/ont/SOMA.owl#Purification -->


    <owl:Class rdf:about="http://www.ease-crc.org/ont/SOMA.owl#Purification">
        <rdfs:subClassOf rdf:resource="http://www.ease-crc.org/ont/SOMA.owl#Variability"/>
        <rdfs:subClassOf>
            <owl:Restriction>
                <owl:onProperty rdf:resource="http://www.ease-crc.org/ont/SOMA.owl#affordsSetpoint"/>
                <owl:allValuesFrom>
                    <owl:Restriction>
                        <owl:onProperty rdf:resource="http://www.ontologydesignpatterns.org/ont/dul/DUL.owl#classifies"/>
                        <owl:allValuesFrom>
                            <owl:Class>
                                <owl:intersectionOf rdf:parseType="Collection">
                                    <rdf:Description rdf:about="http://www.ease-crc.org/ont/SOMA.owl#Clean"/>
                                    <owl:Restriction>
                                        <owl:onProperty rdf:resource="http://www.ontologydesignpatterns.org/ont/dul/DUL.owl#isRegionFor"/>
                                        <owl:allValuesFrom rdf:resource="http://www.ease-crc.org/ont/SOMA.owl#Cleanliness"/>
                                    </owl:Restriction>
                                </owl:intersectionOf>
                            </owl:Class>
                        </owl:allValuesFrom>
                    </owl:Restriction>
                </owl:allValuesFrom>
            </owl:Restriction>
        </rdfs:subClassOf>
        <rdfs:subClassOf>
            <owl:Restriction>
                <owl:onProperty rdf:resource="http://www.ease-crc.org/ont/SOMA.owl#affordsTrigger"/>
                <owl:allValuesFrom>
                    <owl:Restriction>
                        <owl:onProperty rdf:resource="http://www.ontologydesignpatterns.org/ont/dul/DUL.owl#classifies"/>
                        <owl:allValuesFrom rdf:resource="http://www.ontologydesignpatterns.org/ont/dul/DUL.owl#PhysicalObject"/>
                    </owl:Restriction>
                </owl:allValuesFrom>
            </owl:Restriction>
        </rdfs:subClassOf>
        <rdfs:comment>The disposition of an object (the tool) to change the cleanliness of others.</rdfs:comment>
        <rdfs:isDefinedBy rdf:resource="http://www.ease-crc.org/ont/SOMA-OBJ.owl"/>
    </owl:Class>
    


    <!-- http://www.ease-crc.org/ont/SOMA.owl#Pushing -->


    <owl:Class rdf:about="http://www.ease-crc.org/ont/SOMA.owl#Pushing">
        <rdfs:subClassOf rdf:resource="http://www.ease-crc.org/ont/SOMA.owl#Actuating"/>
        <owl:disjointWith rdf:resource="http://www.ease-crc.org/ont/SOMA.owl#Squeezing"/>
        <rdfs:comment>A task in which an Agent moves an object in a direction loosely from the the contact point between agent and object towards object&apos;s center of mass. todo: define subclass &apos;PushingOver&apos;? Would we expect two distinct contacts with the same surface then?</rdfs:comment>
        <rdfs:isDefinedBy rdf:resource="http://www.ease-crc.org/ont/SOMA-ACT.owl"/>
    </owl:Class>
    


    <!-- http://www.ease-crc.org/ont/SOMA.owl#PushingAway -->


    <owl:Class rdf:about="http://www.ease-crc.org/ont/SOMA.owl#PushingAway">
        <rdfs:subClassOf rdf:resource="http://www.ease-crc.org/ont/SOMA.owl#Pushing"/>
        <owl:disjointWith rdf:resource="http://www.ease-crc.org/ont/SOMA.owl#PushingDown"/>
        <rdfs:comment>A task in which an Agent pushes an object in front of themselves.</rdfs:comment>
        <rdfs:isDefinedBy rdf:resource="http://www.ease-crc.org/ont/SOMA-ACT.owl"/>
        <rdfs:label xml:lang="en">Pushing away</rdfs:label>
    </owl:Class>
    


    <!-- http://www.ease-crc.org/ont/SOMA.owl#PushingDown -->


    <owl:Class rdf:about="http://www.ease-crc.org/ont/SOMA.owl#PushingDown">
        <rdfs:subClassOf rdf:resource="http://www.ease-crc.org/ont/SOMA.owl#Pushing"/>
        <rdfs:comment>A task in which an Agent pushes an object downwards.</rdfs:comment>
        <rdfs:isDefinedBy rdf:resource="http://www.ease-crc.org/ont/SOMA-ACT.owl"/>
        <rdfs:label xml:lang="en">Pushing down</rdfs:label>
    </owl:Class>
    


    <!-- http://www.ease-crc.org/ont/SOMA.owl#PuttingDown -->


    <owl:Class rdf:about="http://www.ease-crc.org/ont/SOMA.owl#PuttingDown">
        <rdfs:subClassOf rdf:resource="http://www.ease-crc.org/ont/SOMA.owl#Manipulating"/>
        <rdfs:comment>A task in which an Agent puts down an object they have kinematic control over, e.g. a grasped object.</rdfs:comment>
        <rdfs:isDefinedBy rdf:resource="http://www.ease-crc.org/ont/SOMA-ACT.owl"/>
    </owl:Class>
    


    <!-- http://www.ease-crc.org/ont/SOMA.owl#QualityTransition -->


    <owl:Class rdf:about="http://www.ease-crc.org/ont/SOMA.owl#QualityTransition">
        <rdfs:subClassOf rdf:resource="http://www.ontologydesignpatterns.org/ont/dul/DUL.owl#Transition"/>
        <rdfs:comment>todo(DB): added for NEEMs (quale change), but not sure yet about it...</rdfs:comment>
        <rdfs:isDefinedBy rdf:resource="http://www.ease-crc.org/ont/SOMA-OBJ.owl"/>
        <rdfs:label xml:lang="en">Quality transition</rdfs:label>
    </owl:Class>
    


    <!-- http://www.ease-crc.org/ont/SOMA.owl#Query -->


    <owl:Class rdf:about="http://www.ease-crc.org/ont/SOMA.owl#Query">
        <rdfs:subClassOf rdf:resource="http://www.ease-crc.org/ont/SOMA.owl#Message"/>
        <rdfs:comment xml:lang="en">A role played by some Information Realization that carries meaning, where this meaning is a query of some sort.</rdfs:comment>
        <rdfs:isDefinedBy rdf:resource="http://www.ease-crc.org/ont/SOMA-ACT.owl"/>
        <rdfs:label xml:lang="en">Query</rdfs:label>
    </owl:Class>
    


    <!-- http://www.ease-crc.org/ont/SOMA.owl#QueryEngine -->


    <owl:Class rdf:about="http://www.ease-crc.org/ont/SOMA.owl#QueryEngine">
        <rdfs:subClassOf rdf:resource="http://www.ease-crc.org/ont/SOMA.owl#SoftwareRole"/>
        <rdfs:comment xml:lang="en">A Query Engine is a Software that can answer some queries.</rdfs:comment>
        <rdfs:isDefinedBy rdf:resource="http://www.ease-crc.org/ont/SOMA-IO.owl"/>
        <rdfs:label xml:lang="en">Query engine</rdfs:label>
    </owl:Class>
    


    <!-- http://www.ease-crc.org/ont/SOMA.owl#QueryLanguage -->


    <owl:Class rdf:about="http://www.ease-crc.org/ont/SOMA.owl#QueryLanguage">
        <rdfs:subClassOf rdf:resource="http://www.ease-crc.org/ont/SOMA.owl#Computer_Language"/>
        <rdfs:comment xml:lang="en">Query languages, are Computer languages used to make queries in databases and information systems (Source: https://en.wikipedia.org/wiki/Query_language).

Note that despite their name, Query languages typically come with syntax and semantic to not only ask for information, but also provide them, e.g., via SQL Update. In that sense, the term &quot;query&quot; from above refers to any formal object of information exchange with a database.</rdfs:comment>
        <rdfs:isDefinedBy rdf:resource="http://www.ease-crc.org/ont/SOMA-IO.owl"/>
        <rdfs:label xml:lang="en">Query language</rdfs:label>
    </owl:Class>
    


    <!-- http://www.ease-crc.org/ont/SOMA.owl#QueryingTask -->


    <owl:Class rdf:about="http://www.ease-crc.org/ont/SOMA.owl#QueryingTask">
        <rdfs:subClassOf rdf:resource="http://www.ease-crc.org/ont/SOMA.owl#IllocutionaryTask"/>
        <rdfs:subClassOf>
            <owl:Restriction>
                <owl:onProperty rdf:resource="http://www.ontologydesignpatterns.org/ont/dul/DUL.owl#isTaskOf"/>
                <owl:someValuesFrom rdf:resource="http://www.ease-crc.org/ont/SOMA.owl#Query"/>
            </owl:Restriction>
        </rdfs:subClassOf>
        <rdfs:subClassOf>
            <owl:Restriction>
                <owl:onProperty rdf:resource="http://www.ontologydesignpatterns.org/ont/dul/DUL.owl#classifies"/>
                <owl:allValuesFrom>
                    <owl:Restriction>
                        <owl:onProperty rdf:resource="http://www.ontologydesignpatterns.org/ont/dul/DUL.owl#hasParticipant"/>
                        <owl:someValuesFrom rdf:resource="http://www.ease-crc.org/ont/SOMA.owl#InterrogativeClause"/>
                    </owl:Restriction>
                </owl:allValuesFrom>
            </owl:Restriction>
        </rdfs:subClassOf>
        <rdfs:comment>An Illocutionary act where the Sender of the Message does so to trigger the Receiver to return some information that is specified within the content of the Message.</rdfs:comment>
        <rdfs:isDefinedBy rdf:resource="http://www.ease-crc.org/ont/SOMA-ACT.owl"/>
        <rdfs:label xml:lang="en">Querying task</rdfs:label>
    </owl:Class>
    


    <!-- http://www.ease-crc.org/ont/SOMA.owl#Rack -->


    <owl:Class rdf:about="http://www.ease-crc.org/ont/SOMA.owl#Rack">
        <rdfs:subClassOf rdf:resource="http://www.ease-crc.org/ont/SOMA.owl#DesignedComponent"/>
        <rdfs:comment>A frame for holding or storing things.</rdfs:comment>
        <rdfs:isDefinedBy rdf:resource="http://www.ease-crc.org/ont/SOMA-HOME.owl"/>
    </owl:Class>
    


    <!-- http://www.ease-crc.org/ont/SOMA.owl#Reaching -->


    <owl:Class rdf:about="http://www.ease-crc.org/ont/SOMA.owl#Reaching">
        <rdfs:subClassOf rdf:resource="http://www.ease-crc.org/ont/SOMA.owl#EndEffectorPositioning"/>
        <owl:disjointWith rdf:resource="http://www.ease-crc.org/ont/SOMA.owl#Retracting"/>
        <rdfs:comment>A task in which an Agent moves one or more of its arms towards a location or object.</rdfs:comment>
        <rdfs:isDefinedBy rdf:resource="http://www.ease-crc.org/ont/SOMA-ACT.owl"/>
    </owl:Class>
    


    <!-- http://www.ease-crc.org/ont/SOMA.owl#Reasoner -->


    <owl:Class rdf:about="http://www.ease-crc.org/ont/SOMA.owl#Reasoner">
        <rdfs:subClassOf rdf:resource="http://www.ease-crc.org/ont/SOMA.owl#SoftwareRole"/>
        <rdfs:comment xml:lang="en">A Reasoner is some Software that can infer new, implicit knowlegde from explicitly stated knowledge.

This definition is broad and we consider any System fitting the above description as reasoners. For example, the following can be seen as Reasoners:
* A simulation, where the explicit knowledge corresponds to the initial situation, and the implicit knowlegde corresponds to the situation that is derived from that by simulating some unfolding processes.
* A machine learning algorithm, e.g., an image classifier: The explicit knowledge is the visual content of a picture (even down to the pixel), the implicit knowledge is the derived classification.
* A logic based rule engine, where initial facts are the explicit knowledge, and derived facts are the implicit knowledge.</rdfs:comment>
        <rdfs:isDefinedBy rdf:resource="http://www.ease-crc.org/ont/SOMA-IO.owl"/>
    </owl:Class>
    


    <!-- http://www.ease-crc.org/ont/SOMA.owl#Reasoning -->


    <owl:Class rdf:about="http://www.ease-crc.org/ont/SOMA.owl#Reasoning">
        <rdfs:subClassOf rdf:resource="http://www.ease-crc.org/ont/SOMA.owl#MentalTask"/>
        <rdfs:comment>A Mental task in which an Agent endeavours to obtain new knowledge from knowledge it already possesses.</rdfs:comment>
        <rdfs:comment>todo: a taxonomy of reasoning is not trivial. Classical theory distinguishes Deductive, Inductive, and with a stretch Abductive reasoning. However, modern practice distinguishes other categories that overlap with these, e.g. Probabilistic and Non-monotonic.

Both Abductive and Inductive inference may, and often do, use Probabilistic methods. Probabilistic inference is, by its nature, most opposed to Deductive inference which, classically, requires logical certainty.

Any of the Abductive/Deductive/Inductive triad can be further affected by the Monotone/Non-monotone distinction. There are preferences (Inductive and Abductive reasoning is probably most often non-monotonic; most of Deductive reasoning is probably done in monotonic formalisms), but it is certainly the case that, e.g., non-monotone Deduction is possible.

Note, this classification has nothing to do with reasoning domain (e.g. SpatialReasoning, TemporalReasoning, ...) and merely with techniques/logical-mathematical underpinnings.</rdfs:comment>
        <rdfs:isDefinedBy rdf:resource="http://www.ease-crc.org/ont/SOMA-ACT.owl"/>
    </owl:Class>
    


    <!-- http://www.ease-crc.org/ont/SOMA.owl#Receiver -->


    <owl:Class rdf:about="http://www.ease-crc.org/ont/SOMA.owl#Receiver">
        <rdfs:subClassOf rdf:resource="http://www.ease-crc.org/ont/SOMA.owl#AgentRole"/>
        <rdfs:subClassOf>
            <owl:Restriction>
                <owl:onProperty rdf:resource="http://www.ontologydesignpatterns.org/ont/dul/DUL.owl#hasTask"/>
                <owl:someValuesFrom rdf:resource="http://www.ease-crc.org/ont/SOMA.owl#CommunicationTask"/>
            </owl:Restriction>
        </rdfs:subClassOf>
        <rdfs:comment xml:lang="en">The role played by an Agent in a Communication Task that perceives and interpretes some incoming Message.</rdfs:comment>
        <rdfs:isDefinedBy rdf:resource="http://www.ease-crc.org/ont/SOMA-ACT.owl"/>
        <rdfs:label xml:lang="en">Receiver</rdfs:label>
    </owl:Class>
    


    <!-- http://www.ease-crc.org/ont/SOMA.owl#RecipientRole -->


    <owl:Class rdf:about="http://www.ease-crc.org/ont/SOMA.owl#RecipientRole">
        <rdfs:subClassOf rdf:resource="http://www.ease-crc.org/ont/SOMA.owl#BeneficiaryRole"/>
        <rdfs:comment>A role which classifies an agent who receives an object modified or created by an action.</rdfs:comment>
        <rdfs:isDefinedBy rdf:resource="http://www.ease-crc.org/ont/SOMA-OBJ.owl"/>
        <rdfs:label xml:lang="en">Recipent role</rdfs:label>
    </owl:Class>
    


    <!-- http://www.ease-crc.org/ont/SOMA.owl#RedColor -->


    <owl:Class rdf:about="http://www.ease-crc.org/ont/SOMA.owl#RedColor">
        <rdfs:subClassOf rdf:resource="http://www.ease-crc.org/ont/SOMA.owl#ColorRegion"/>
        <rdfs:comment>A color region with dominant red color.</rdfs:comment>
        <rdfs:isDefinedBy rdf:resource="http://www.ease-crc.org/ont/SOMA-OBJ.owl"/>
        <rdfs:label>Red color</rdfs:label>
    </owl:Class>
    


    <!-- http://www.ease-crc.org/ont/SOMA.owl#Refrigerator -->


    <owl:Class rdf:about="http://www.ease-crc.org/ont/SOMA.owl#Refrigerator">
        <rdfs:subClassOf rdf:resource="http://www.ease-crc.org/ont/SOMA.owl#Appliance"/>
        <rdfs:subClassOf rdf:resource="http://www.ease-crc.org/ont/SOMA.owl#DesignedContainer"/>
        <rdfs:subClassOf>
            <owl:Restriction>
                <owl:onProperty rdf:resource="http://www.ease-crc.org/ont/SOMA.owl#hasPhysicalComponent"/>
                <owl:someValuesFrom rdf:resource="http://www.ease-crc.org/ont/SOMA.owl#Door"/>
            </owl:Restriction>
        </rdfs:subClassOf>
        <rdfs:comment>An appliance which is artificially kept cool and used to store food and drink.</rdfs:comment>
        <rdfs:isDefinedBy rdf:resource="http://www.ease-crc.org/ont/SOMA-HOME.owl"/>
    </owl:Class>
    


    <!-- http://www.ease-crc.org/ont/SOMA.owl#RelationAdjacentRole -->


    <owl:Class rdf:about="http://www.ease-crc.org/ont/SOMA.owl#RelationAdjacentRole">
        <rdfs:subClassOf rdf:resource="http://www.ontologydesignpatterns.org/ont/dul/DUL.owl#Role"/>
        <rdfs:comment>A role classifying an object participating in some relation, e.g. a participant in a spatial relation or a linguistic fragment in a rhetorical relation to another.</rdfs:comment>
        <rdfs:isDefinedBy rdf:resource="http://www.ease-crc.org/ont/SOMA-OBJ.owl"/>
        <rdfs:label xml:lang="en">Relation adjacent role</rdfs:label>
    </owl:Class>
    


    <!-- http://www.ease-crc.org/ont/SOMA.owl#RelationalDatabase -->


    <owl:Class rdf:about="http://www.ease-crc.org/ont/SOMA.owl#RelationalDatabase">
        <rdfs:subClassOf rdf:resource="http://www.ease-crc.org/ont/SOMA.owl#Database"/>
        <rdfs:comment xml:lang="en">A Relational Database is a Database based on the relational model of data, which organizes data into one or more tables (or &quot;relations&quot;) of columns and rows, with a unique key identifying each row.

Source: https://en.wikipedia.org/wiki/Relational_database</rdfs:comment>
        <rdfs:isDefinedBy rdf:resource="http://www.ease-crc.org/ont/SOMA-IO.owl"/>
        <rdfs:label xml:lang="en">Relational database</rdfs:label>
    </owl:Class>
    


    <!-- http://www.ease-crc.org/ont/SOMA.owl#RelationalQueryLanguage -->


    <owl:Class rdf:about="http://www.ease-crc.org/ont/SOMA.owl#RelationalQueryLanguage">
        <rdfs:subClassOf rdf:resource="http://www.ease-crc.org/ont/SOMA.owl#QueryLanguage"/>
        <rdfs:comment xml:lang="en">A Query Language that is designed for communication with some Relational Database.</rdfs:comment>
        <rdfs:isDefinedBy rdf:resource="http://www.ease-crc.org/ont/SOMA-IO.owl"/>
        <rdfs:label xml:lang="en">Relational query language</rdfs:label>
    </owl:Class>
    


    <!-- http://www.ease-crc.org/ont/SOMA.owl#RelatumRole -->


    <owl:Class rdf:about="http://www.ease-crc.org/ont/SOMA.owl#RelatumRole">
        <rdfs:subClassOf rdf:resource="http://www.ease-crc.org/ont/SOMA.owl#SpatialRelationRole"/>
        <rdfs:subClassOf>
            <owl:Restriction>
                <owl:onProperty rdf:resource="http://www.ontologydesignpatterns.org/ont/dul/DUL.owl#classifies"/>
                <owl:allValuesFrom rdf:resource="http://www.ontologydesignpatterns.org/ont/dul/DUL.owl#PhysicalObject"/>
            </owl:Restriction>
        </rdfs:subClassOf>
        <rdfs:comment>Denotes the reference object in a spatial or spatio-temporal schema, i.e. the object with secondary focal prominence. Terminological variants: Ground (Talmy 1983), Landmark (Langacker 1986).</rdfs:comment>
        <rdfs:isDefinedBy rdf:resource="http://www.ease-crc.org/ont/SOMA-OBJ.owl"/>
        <rdfs:label xml:lang="en">Relatum role</rdfs:label>
    </owl:Class>
    


    <!-- http://www.ease-crc.org/ont/SOMA.owl#Releasing -->


    <owl:Class rdf:about="http://www.ease-crc.org/ont/SOMA.owl#Releasing">
        <rdfs:subClassOf rdf:resource="http://www.ease-crc.org/ont/SOMA.owl#Manipulating"/>
        <rdfs:comment>A task in which an agent relinquishes its kinematic control over an object, typically by releasing it from its grasp.</rdfs:comment>
        <rdfs:isDefinedBy rdf:resource="http://www.ease-crc.org/ont/SOMA-ACT.owl"/>
    </owl:Class>
    


    <!-- http://www.ease-crc.org/ont/SOMA.owl#ReleasingMotion -->


    <owl:Class rdf:about="http://www.ease-crc.org/ont/SOMA.owl#ReleasingMotion">
        <rdfs:subClassOf rdf:resource="http://www.ease-crc.org/ont/SOMA.owl#PrehensileMotion"/>
        <rdfs:comment>A motion by which a prehensile effector relinquishes kinematic control over an object.</rdfs:comment>
        <rdfs:isDefinedBy rdf:resource="http://www.ease-crc.org/ont/SOMA-PROC.owl"/>
        <rdfs:label>Releasing motion</rdfs:label>
    </owl:Class>
    


    <!-- http://www.ease-crc.org/ont/SOMA.owl#RelevantPart -->


    <owl:Class rdf:about="http://www.ease-crc.org/ont/SOMA.owl#RelevantPart">
        <rdfs:subClassOf rdf:resource="http://www.ease-crc.org/ont/SOMA.owl#Feature"/>
        <rdfs:comment>Features that are relevant parts of their host, like a bump or an edge.</rdfs:comment>
        <rdfs:isDefinedBy rdf:resource="http://www.ease-crc.org/ont/SOMA-OBJ.owl"/>
        <rdfs:label xml:lang="en">Relevant part</rdfs:label>
    </owl:Class>
    


    <!-- http://www.ease-crc.org/ont/SOMA.owl#Remembering -->


    <owl:Class rdf:about="http://www.ease-crc.org/ont/SOMA.owl#Remembering">
        <rdfs:subClassOf rdf:resource="http://www.ease-crc.org/ont/SOMA.owl#Retrospecting"/>
        <rdfs:comment>A Mental task in which the Agent endeavours to recall a record of a previous state of affairs in the world. The Agent must have witnessed this state of affairs in order to record it. Remembering commits itself to accuracy: the Agent attempts to reconstruct as accurate a record as it can. Note, this does not mean the Agent will communicate the recollection accurately.</rdfs:comment>
        <rdfs:isDefinedBy rdf:resource="http://www.ease-crc.org/ont/SOMA-ACT.owl"/>
    </owl:Class>
    


    <!-- http://www.ease-crc.org/ont/SOMA.owl#ResourceRole -->


    <owl:Class rdf:about="http://www.ease-crc.org/ont/SOMA.owl#ResourceRole">
        <rdfs:subClassOf rdf:resource="http://www.ease-crc.org/ont/SOMA.owl#EventAdjacentRole"/>
        <rdfs:comment>A role classifying objects that are useful or even necessary to sustain the unfolding of an event.

Resources are usually not agentive; a different set of roles classifies the agentive participants in actions. Likewise, typically resources do not play causative or goal roles for the event.

Resources are often consumed by their participation in an event, but this need not always be the case. An instrument and capital are examples of resources that are reusable.</rdfs:comment>
        <rdfs:isDefinedBy rdf:resource="http://www.ease-crc.org/ont/SOMA-OBJ.owl"/>
        <rdfs:label xml:lang="en">Resource role</rdfs:label>
    </owl:Class>
    


    <!-- http://www.ease-crc.org/ont/SOMA.owl#RestrictedObject -->


    <owl:Class rdf:about="http://www.ease-crc.org/ont/SOMA.owl#RestrictedObject">
        <rdfs:subClassOf rdf:resource="http://www.ease-crc.org/ont/SOMA.owl#BlockedObject"/>
        <rdfs:comment>An object with restrictions to access something.</rdfs:comment>
        <rdfs:isDefinedBy rdf:resource="http://www.ease-crc.org/ont/SOMA-OBJ.owl"/>
        <rdfs:label xml:lang="en">Restricted object</rdfs:label>
    </owl:Class>
    


    <!-- http://www.ease-crc.org/ont/SOMA.owl#Restrictor -->


    <owl:Class rdf:about="http://www.ease-crc.org/ont/SOMA.owl#Restrictor">
        <rdfs:subClassOf rdf:resource="http://www.ease-crc.org/ont/SOMA.owl#Instrument"/>
        <rdfs:comment>A role classifying an object used to deny access to some other entity.</rdfs:comment>
        <rdfs:isDefinedBy rdf:resource="http://www.ease-crc.org/ont/SOMA-OBJ.owl"/>
        <rdfs:isDefinedBy rdf:resource="http://www.ease-crc.org/ont/SOMA-STATE.owl"/>
    </owl:Class>
    


    <!-- http://www.ease-crc.org/ont/SOMA.owl#ResultRole -->


    <owl:Class rdf:about="http://www.ease-crc.org/ont/SOMA.owl#ResultRole">
        <rdfs:subClassOf rdf:resource="http://www.ease-crc.org/ont/SOMA.owl#GoalRole"/>
        <rdfs:comment>A role classifying the object that is the outcome of a creation or modification action or process.</rdfs:comment>
        <rdfs:isDefinedBy rdf:resource="http://www.ease-crc.org/ont/SOMA-OBJ.owl"/>
        <rdfs:label xml:lang="en">Result role</rdfs:label>
    </owl:Class>
    


    <!-- http://www.ease-crc.org/ont/SOMA.owl#Retracting -->


    <owl:Class rdf:about="http://www.ease-crc.org/ont/SOMA.owl#Retracting">
        <rdfs:subClassOf rdf:resource="http://www.ease-crc.org/ont/SOMA.owl#EndEffectorPositioning"/>
        <rdfs:comment>A task in which an Agent moves its arms away from a location.</rdfs:comment>
        <rdfs:isDefinedBy rdf:resource="http://www.ease-crc.org/ont/SOMA-ACT.owl"/>
    </owl:Class>
    


    <!-- http://www.ease-crc.org/ont/SOMA.owl#Retrospecting -->


    <owl:Class rdf:about="http://www.ease-crc.org/ont/SOMA.owl#Retrospecting">
        <rdfs:subClassOf rdf:resource="http://www.ease-crc.org/ont/SOMA.owl#MentalTask"/>
        <rdfs:comment>A Mental task in which an Agent endeavors to construct a representation of a past state of affairs of the world it is embodied in.</rdfs:comment>
        <rdfs:comment>Done by analogy with Prospecting. Currently mono-subcategory, but perhaps we might find more.

As an example, a kind of Abductive reasoning would fit here: reconstruction, in which the agent attempts to create a representation of a past state of affairs which the agent has not actually observed, based on traces and clues surviving to the present.</rdfs:comment>
        <rdfs:isDefinedBy rdf:resource="http://www.ease-crc.org/ont/SOMA-ACT.owl"/>
    </owl:Class>
    


    <!-- http://www.ease-crc.org/ont/SOMA.owl#RoleFillerBinding -->


    <owl:Class rdf:about="http://www.ease-crc.org/ont/SOMA.owl#RoleFillerBinding">
        <rdfs:subClassOf rdf:resource="http://www.ease-crc.org/ont/SOMA.owl#Binding"/>
        <owl:disjointWith rdf:resource="http://www.ease-crc.org/ont/SOMA.owl#RoleRoleBinding"/>
        <rdfs:comment>A binding that connects a role to a particular filler.</rdfs:comment>
        <rdfs:isDefinedBy rdf:resource="http://www.ease-crc.org/ont/SOMA-WF.owl"/>
        <rdfs:label xml:lang="en">Role filler binding</rdfs:label>
    </owl:Class>
    


    <!-- http://www.ease-crc.org/ont/SOMA.owl#RoleRoleBinding -->


    <owl:Class rdf:about="http://www.ease-crc.org/ont/SOMA.owl#RoleRoleBinding">
        <rdfs:subClassOf rdf:resource="http://www.ease-crc.org/ont/SOMA.owl#Binding"/>
        <rdfs:subClassOf>
            <owl:Restriction>
                <owl:onProperty rdf:resource="http://www.ease-crc.org/ont/SOMA.owl#hasBindingFiller"/>
                <owl:allValuesFrom>
                    <owl:Class>
                        <owl:unionOf rdf:parseType="Collection">
                            <rdf:Description rdf:about="http://www.ontologydesignpatterns.org/ont/dul/DUL.owl#Parameter"/>
                            <rdf:Description rdf:about="http://www.ontologydesignpatterns.org/ont/dul/DUL.owl#Role"/>
                        </owl:unionOf>
                    </owl:Class>
                </owl:allValuesFrom>
            </owl:Restriction>
        </rdfs:subClassOf>
        <rdfs:comment>A binding that asserts that two roles have the same filler.</rdfs:comment>
        <rdfs:isDefinedBy rdf:resource="http://www.ease-crc.org/ont/SOMA-WF.owl"/>
        <rdfs:label xml:lang="en">Role role binding</rdfs:label>
    </owl:Class>
    


    <!-- http://www.ease-crc.org/ont/SOMA.owl#Room -->


    <owl:Class rdf:about="http://www.ease-crc.org/ont/SOMA.owl#Room">
        <rdfs:subClassOf rdf:resource="http://www.ontologydesignpatterns.org/ont/dul/DUL.owl#PhysicalPlace"/>
        <rdfs:comment>Space that can be occupied or where something can be done.</rdfs:comment>
        <rdfs:isDefinedBy rdf:resource="http://www.ease-crc.org/ont/SOMA-HOME.owl"/>
        <rdfs:isDefinedBy rdf:resource="http://www.ease-crc.org/ont/SOMA-OBJ.owl"/>
    </owl:Class>
    


    <!-- http://www.ease-crc.org/ont/SOMA.owl#RoomSurface -->


    <owl:Class rdf:about="http://www.ease-crc.org/ont/SOMA.owl#RoomSurface">
        <rdfs:subClassOf rdf:resource="http://www.ease-crc.org/ont/SOMA.owl#Surface"/>
        <rdfs:comment>The surface of a room.</rdfs:comment>
        <rdfs:isDefinedBy rdf:resource="http://www.ease-crc.org/ont/SOMA-HOME.owl"/>
        <rdfs:isDefinedBy rdf:resource="http://www.ease-crc.org/ont/SOMA-OBJ.owl"/>
        <rdfs:label xml:lang="en">Room surface</rdfs:label>
    </owl:Class>
    


    <!-- http://www.ease-crc.org/ont/SOMA.owl#Rubbing -->


    <owl:Class rdf:about="http://www.ease-crc.org/ont/SOMA.owl#Rubbing">
        <rdfs:subClassOf rdf:resource="http://www.ease-crc.org/ont/SOMA.owl#DirectedMotion"/>
        <rdfs:comment>The motion of an object sliding along the surface of another, for example, to clean the surface.</rdfs:comment>
        <rdfs:isDefinedBy rdf:resource="http://www.ease-crc.org/ont/SOMA-PROC.owl"/>
    </owl:Class>
    


    <!-- http://www.ease-crc.org/ont/SOMA.owl#Scene -->


    <owl:Class rdf:about="http://www.ease-crc.org/ont/SOMA.owl#Scene">
        <rdfs:subClassOf rdf:resource="http://www.ontologydesignpatterns.org/ont/dul/DUL.owl#Situation"/>
        <rdfs:subClassOf>
            <owl:Restriction>
                <owl:onProperty rdf:resource="http://www.ontologydesignpatterns.org/ont/dul/DUL.owl#includesEvent"/>
                <owl:someValuesFrom rdf:resource="http://www.ease-crc.org/ont/SOMA.owl#State"/>
            </owl:Restriction>
        </rdfs:subClassOf>
        <rdfs:subClassOf>
            <owl:Restriction>
                <owl:onProperty rdf:resource="http://www.ontologydesignpatterns.org/ont/dul/DUL.owl#satisfies"/>
                <owl:someValuesFrom rdf:resource="http://www.ease-crc.org/ont/SOMA.owl#ImageSchemaTheory"/>
            </owl:Restriction>
        </rdfs:subClassOf>
        <rdfs:comment>Scenes are Situations which interpret a State in terms of its conformance to some qualitative, image schematic description. I.e., the scene is described in terms of qualitative functional and spatial relations existing between participating objects.</rdfs:comment>
        <rdfs:isDefinedBy rdf:resource="http://www.ease-crc.org/ont/SOMA-SAY.owl"/>
    </owl:Class>
    


    <!-- http://www.ease-crc.org/ont/SOMA.owl#SchematicTheory -->


    <owl:Class rdf:about="http://www.ease-crc.org/ont/SOMA.owl#SchematicTheory">
        <rdfs:subClassOf rdf:resource="http://www.ontologydesignpatterns.org/ont/dul/DUL.owl#Theory"/>
        <rdfs:comment>A theory used to describe, analyze, and reason with the meaning of a linguistic message.

Note that such theories are useful both when analyzing an actual linguistic production, and when creating a linguistic production to describe some observed experience.</rdfs:comment>
        <rdfs:isDefinedBy rdf:resource="http://www.ease-crc.org/ont/SOMA-SAY.owl"/>
        <rdfs:label xml:lang="en">Schematic theory</rdfs:label>
    </owl:Class>
    


    <!-- http://www.ease-crc.org/ont/SOMA.owl#SelectedObject -->


    <owl:Class rdf:about="http://www.ease-crc.org/ont/SOMA.owl#SelectedObject">
        <rdfs:subClassOf rdf:resource="http://www.ontologydesignpatterns.org/ont/dul/DUL.owl#Role"/>
        <rdfs:comment>An object chosen as the result of some selection task.</rdfs:comment>
        <rdfs:isDefinedBy rdf:resource="http://www.ease-crc.org/ont/SOMA-OBJ.owl"/>
        <rdfs:label xml:lang="en">Selected object</rdfs:label>
    </owl:Class>
    


    <!-- http://www.ease-crc.org/ont/SOMA.owl#SelectingItem -->


    <owl:Class rdf:about="http://www.ease-crc.org/ont/SOMA.owl#SelectingItem">
        <rdfs:subClassOf rdf:resource="http://www.ease-crc.org/ont/SOMA.owl#GetTaskParameter"/>
        <rdfs:subClassOf>
            <owl:Restriction>
                <owl:onProperty rdf:resource="http://www.ease-crc.org/ont/SOMA.owl#isTaskOfOutputRole"/>
                <owl:someValuesFrom>
                    <owl:Class>
                        <owl:intersectionOf rdf:parseType="Collection">
                            <rdf:Description rdf:about="http://www.ease-crc.org/ont/SOMA.owl#SelectedObject"/>
                            <owl:Restriction>
                                <owl:onProperty rdf:resource="http://www.ontologydesignpatterns.org/ont/dul/DUL.owl#classifies"/>
                                <owl:allValuesFrom rdf:resource="http://www.ontologydesignpatterns.org/ont/dul/DUL.owl#PhysicalObject"/>
                            </owl:Restriction>
                        </owl:intersectionOf>
                    </owl:Class>
                </owl:someValuesFrom>
            </owl:Restriction>
        </rdfs:subClassOf>
        <rdfs:comment>A task in which an Agent selects some object to use for a subsequent task.</rdfs:comment>
        <rdfs:isDefinedBy rdf:resource="http://www.ease-crc.org/ont/SOMA-ACT.owl"/>
        <rdfs:label xml:lang="en">Selecting item</rdfs:label>
    </owl:Class>
    


    <!-- http://www.ease-crc.org/ont/SOMA.owl#Sender -->


    <owl:Class rdf:about="http://www.ease-crc.org/ont/SOMA.owl#Sender">
        <rdfs:subClassOf rdf:resource="http://www.ease-crc.org/ont/SOMA.owl#AgentRole"/>
        <rdfs:subClassOf>
            <owl:Restriction>
                <owl:onProperty rdf:resource="http://www.ontologydesignpatterns.org/ont/dul/DUL.owl#hasTask"/>
                <owl:someValuesFrom rdf:resource="http://www.ease-crc.org/ont/SOMA.owl#CommunicationTask"/>
            </owl:Restriction>
        </rdfs:subClassOf>
        <rdfs:comment xml:lang="en">The Role played by an Agent in a Communication Task that emits some Information Realization with the purpose of percipience by some Receiver.</rdfs:comment>
        <rdfs:isDefinedBy rdf:resource="http://www.ease-crc.org/ont/SOMA-ACT.owl"/>
        <rdfs:label xml:lang="en">Sender</rdfs:label>
    </owl:Class>
    


    <!-- http://www.ease-crc.org/ont/SOMA.owl#ServerRole -->


    <owl:Class rdf:about="http://www.ease-crc.org/ont/SOMA.owl#ServerRole">
        <rdfs:subClassOf rdf:resource="http://www.ease-crc.org/ont/SOMA.owl#InterfaceComponentRole"/>
        <rdfs:subClassOf>
            <owl:Restriction>
                <owl:onProperty rdf:resource="http://www.ontologydesignpatterns.org/ont/dul/DUL.owl#isDefinedIn"/>
                <owl:someValuesFrom rdf:resource="http://www.ease-crc.org/ont/SOMA.owl#Client-Server_Specification"/>
            </owl:Restriction>
        </rdfs:subClassOf>
        <rdfs:comment xml:lang="en">The Client-server model is a distributed application structure that partitions tasks or workloads between the providers of a resource or service, called servers, and service requesters, called clients Often clients and servers communicate over a computer network on separate hardware, but both client and server may reside in the same system. A server host runs one or more server programs, which share their resources with clients. A client usually does not share any of its resources, but it requests content or service from a server. Clients, therefore, initiate communication sessions with servers, which await incoming requests. Examples of computer applications that use the client-server model are email, network printing, and the World Wide Web.

Source: https://en.wikipedia.org/wiki/Client%E2%80%93server_model</rdfs:comment>
        <rdfs:isDefinedBy rdf:resource="http://www.ease-crc.org/ont/SOMA-IO.owl"/>
        <rdfs:label xml:lang="en">Server role</rdfs:label>
    </owl:Class>
    


    <!-- http://www.ease-crc.org/ont/SOMA.owl#Setpoint -->


    <owl:Class rdf:about="http://www.ease-crc.org/ont/SOMA.owl#Setpoint">
        <rdfs:subClassOf rdf:resource="http://www.ontologydesignpatterns.org/ont/dul/DUL.owl#Parameter"/>
        <rdfs:comment>Classifies some dedicated goal region.</rdfs:comment>
        <rdfs:isDefinedBy rdf:resource="http://www.ease-crc.org/ont/SOMA-OBJ.owl"/>
    </owl:Class>
    


    <!-- http://www.ease-crc.org/ont/SOMA.owl#SettingGripper -->


    <owl:Class rdf:about="http://www.ease-crc.org/ont/SOMA.owl#SettingGripper">
        <rdfs:subClassOf rdf:resource="http://www.ease-crc.org/ont/SOMA.owl#AssumingPose"/>
        <rdfs:comment>A task by which an Agent arranges one/some/all of its grippers in some configuration.</rdfs:comment>
        <rdfs:isDefinedBy rdf:resource="http://www.ease-crc.org/ont/SOMA-ACT.owl"/>
        <rdfs:label xml:lang="en">Setting gripper</rdfs:label>
    </owl:Class>
    


    <!-- http://www.ease-crc.org/ont/SOMA.owl#Shape -->


    <owl:Class rdf:about="http://www.ease-crc.org/ont/SOMA.owl#Shape">
        <rdfs:subClassOf rdf:resource="http://www.ease-crc.org/ont/SOMA.owl#Intrinsic"/>
        <rdfs:subClassOf>
            <owl:Restriction>
                <owl:onProperty rdf:resource="http://www.ontologydesignpatterns.org/ont/dul/DUL.owl#hasRegion"/>
                <owl:someValuesFrom rdf:resource="http://www.ease-crc.org/ont/SOMA.owl#ShapeRegion"/>
            </owl:Restriction>
        </rdfs:subClassOf>
        <rdfs:subClassOf>
            <owl:Restriction>
                <owl:onProperty rdf:resource="http://www.ontologydesignpatterns.org/ont/dul/DUL.owl#hasRegion"/>
                <owl:allValuesFrom rdf:resource="http://www.ease-crc.org/ont/SOMA.owl#ShapeRegion"/>
            </owl:Restriction>
        </rdfs:subClassOf>
        <rdfs:comment>The external form, contours, or outline of an object.</rdfs:comment>
        <rdfs:isDefinedBy rdf:resource="http://www.ease-crc.org/ont/SOMA-OBJ.owl"/>
    </owl:Class>
    


    <!-- http://www.ease-crc.org/ont/SOMA.owl#ShapeRegion -->


    <owl:Class rdf:about="http://www.ease-crc.org/ont/SOMA.owl#ShapeRegion">
        <rdfs:subClassOf rdf:resource="http://www.ontologydesignpatterns.org/ont/dul/DUL.owl#Region"/>
        <rdfs:subClassOf>
            <owl:Restriction>
                <owl:onProperty rdf:resource="http://www.ease-crc.org/ont/SOMA.owl#hasSpaceRegion"/>
                <owl:maxQualifiedCardinality rdf:datatype="http://www.w3.org/2001/XMLSchema#nonNegativeInteger">1</owl:maxQualifiedCardinality>
                <owl:onClass rdf:resource="http://www.ease-crc.org/ont/SOMA.owl#6DPose"/>
            </owl:Restriction>
        </rdfs:subClassOf>
        <rdfs:comment>Encodes the shape of an object.

Note that sometimes the shape as actually used for some purpose may be displaced. This is the case, e.g., for robot links which use a mesh file to describe their shape, but the reference pose of the link uses the mesh translated/rotated in the link&apos;s local coordinate frame.</rdfs:comment>
        <rdfs:isDefinedBy rdf:resource="http://www.ease-crc.org/ont/SOMA-OBJ.owl"/>
        <rdfs:label>Shape region</rdfs:label>
    </owl:Class>
    


    <!-- http://www.ease-crc.org/ont/SOMA.owl#ShapedObject -->


    <owl:Class rdf:about="http://www.ease-crc.org/ont/SOMA.owl#ShapedObject">
        <rdfs:subClassOf rdf:resource="http://www.ease-crc.org/ont/SOMA.owl#AlteredObject"/>
        <rdfs:subClassOf>
            <owl:Restriction>
                <owl:onProperty rdf:resource="http://www.ease-crc.org/ont/SOMA.owl#isTriggerDefinedIn"/>
                <owl:someValuesFrom>
                    <owl:Restriction>
                        <owl:onProperty rdf:resource="http://www.ease-crc.org/ont/SOMA.owl#describesQuality"/>
                        <owl:allValuesFrom rdf:resource="http://www.ease-crc.org/ont/SOMA.owl#Shape"/>
                    </owl:Restriction>
                </owl:someValuesFrom>
            </owl:Restriction>
        </rdfs:subClassOf>
        <rdfs:subClassOf>
            <owl:Restriction>
                <owl:onProperty rdf:resource="http://www.ontologydesignpatterns.org/ont/dul/DUL.owl#classifies"/>
                <owl:allValuesFrom>
                    <owl:Restriction>
                        <owl:onProperty rdf:resource="http://www.ontologydesignpatterns.org/ont/dul/DUL.owl#hasQuality"/>
                        <owl:someValuesFrom rdf:resource="http://www.ease-crc.org/ont/SOMA.owl#Shape"/>
                    </owl:Restriction>
                </owl:allValuesFrom>
            </owl:Restriction>
        </rdfs:subClassOf>
        <rdfs:comment>An object undergoing shape change.</rdfs:comment>
        <rdfs:isDefinedBy rdf:resource="http://www.ease-crc.org/ont/SOMA-OBJ.owl"/>
        <rdfs:isDefinedBy rdf:resource="http://www.ease-crc.org/ont/SOMA-PROC.owl"/>
        <rdfs:label xml:lang="en">Shaped object</rdfs:label>
    </owl:Class>
    


    <!-- http://www.ease-crc.org/ont/SOMA.owl#Shaping -->


    <owl:Class rdf:about="http://www.ease-crc.org/ont/SOMA.owl#Shaping">
        <rdfs:subClassOf rdf:resource="http://www.ease-crc.org/ont/SOMA.owl#Variability"/>
        <rdfs:subClassOf>
            <owl:Restriction>
                <owl:onProperty rdf:resource="http://www.ease-crc.org/ont/SOMA.owl#affordsSetpoint"/>
                <owl:allValuesFrom>
                    <owl:Restriction>
                        <owl:onProperty rdf:resource="http://www.ontologydesignpatterns.org/ont/dul/DUL.owl#classifies"/>
                        <owl:allValuesFrom rdf:resource="http://www.ease-crc.org/ont/SOMA.owl#Shape"/>
                    </owl:Restriction>
                </owl:allValuesFrom>
            </owl:Restriction>
        </rdfs:subClassOf>
        <rdfs:subClassOf>
            <owl:Restriction>
                <owl:onProperty rdf:resource="http://www.ease-crc.org/ont/SOMA.owl#affordsTrigger"/>
                <owl:allValuesFrom rdf:resource="http://www.ease-crc.org/ont/SOMA.owl#ShapedObject"/>
            </owl:Restriction>
        </rdfs:subClassOf>
        <rdfs:comment>The disposition of an object (the tool) to change the shape of others.</rdfs:comment>
        <rdfs:isDefinedBy rdf:resource="http://www.ease-crc.org/ont/SOMA-HOME.owl"/>
        <rdfs:isDefinedBy rdf:resource="http://www.ease-crc.org/ont/SOMA-OBJ.owl"/>
    </owl:Class>
    


    <!-- http://www.ease-crc.org/ont/SOMA.owl#Sharpness -->


    <owl:Class rdf:about="http://www.ease-crc.org/ont/SOMA.owl#Sharpness">
        <rdfs:subClassOf rdf:resource="http://www.ease-crc.org/ont/SOMA.owl#Intrinsic"/>
        <rdfs:comment>The quality of having a thin edge or point that can cut something or make a hole into something. It is worth to note here that the social aspect of sharpness such as the quality of being clear, intelligent etc is not considered as sharpness according to this definition.</rdfs:comment>
        <rdfs:isDefinedBy rdf:resource="http://www.ease-crc.org/ont/SOMA-OBJ.owl"/>
    </owl:Class>
    


    <!-- http://www.ease-crc.org/ont/SOMA.owl#Shifting -->


    <owl:Class rdf:about="http://www.ease-crc.org/ont/SOMA.owl#Shifting">
        <rdfs:subClassOf rdf:resource="http://www.ease-crc.org/ont/SOMA.owl#Variability"/>
        <rdfs:subClassOf>
            <owl:Restriction>
                <owl:onProperty rdf:resource="http://www.ease-crc.org/ont/SOMA.owl#affordsSetpoint"/>
                <owl:allValuesFrom>
                    <owl:Restriction>
                        <owl:onProperty rdf:resource="http://www.ontologydesignpatterns.org/ont/dul/DUL.owl#classifies"/>
                        <owl:allValuesFrom rdf:resource="http://www.ease-crc.org/ont/SOMA.owl#Localization"/>
                    </owl:Restriction>
                </owl:allValuesFrom>
            </owl:Restriction>
        </rdfs:subClassOf>
        <rdfs:subClassOf>
            <owl:Restriction>
                <owl:onProperty rdf:resource="http://www.ease-crc.org/ont/SOMA.owl#affordsTrigger"/>
                <owl:allValuesFrom rdf:resource="http://www.ease-crc.org/ont/SOMA.owl#MovedObject"/>
            </owl:Restriction>
        </rdfs:subClassOf>
        <rdfs:comment>The disposition of an object (the tool) to change the localization of others.</rdfs:comment>
        <rdfs:isDefinedBy rdf:resource="http://www.ease-crc.org/ont/SOMA-OBJ.owl"/>
    </owl:Class>
    


    <!-- http://www.ease-crc.org/ont/SOMA.owl#Simulating -->


    <owl:Class rdf:about="http://www.ease-crc.org/ont/SOMA.owl#Simulating">
        <rdfs:subClassOf rdf:resource="http://www.ease-crc.org/ont/SOMA.owl#Prospecting"/>
        <rdfs:comment>A Mental task in which the Agent endeavours to create representations of a sequence of states of affairs in the world. Simulation commits itself to some degree of transition accuracy: supposing the actual state of the world was the initial state of the simulation, the world state and simulation state should evolve to some degree similarly.

Simulation does not commit itself to state accuracy: the initial state of the simulation is not constrained to be faithful to the actual state of the world in which the Agent is embodied. Counterfactual simulation (&quot;what would happen if--?&quot;) is possible.</rdfs:comment>
        <rdfs:isDefinedBy rdf:resource="http://www.ease-crc.org/ont/SOMA-ACT.owl"/>
    </owl:Class>
    


    <!-- http://www.ease-crc.org/ont/SOMA.owl#Simulation_Reasoner -->


    <owl:Class rdf:about="http://www.ease-crc.org/ont/SOMA.owl#Simulation_Reasoner">
        <rdfs:subClassOf rdf:resource="http://www.ease-crc.org/ont/SOMA.owl#Reasoner"/>
        <rdfs:isDefinedBy rdf:resource="http://www.ease-crc.org/ont/SOMA-IO.owl"/>
        <rdfs:label xml:lang="en">A Simulation-based Reasoner is a simulation that is used as a reasoner, where the explicit knowledge corresponds to the initial situation, and the implicit knowlegde corresponds to the situation that is derived from that by simulating some unfolding processes.</rdfs:label>
        <rdfs:label xml:lang="en">Simulation-based reasoner</rdfs:label>
    </owl:Class>
    


    <!-- http://www.ease-crc.org/ont/SOMA.owl#SituationTransition -->


    <owl:Class rdf:about="http://www.ease-crc.org/ont/SOMA.owl#SituationTransition">
        <rdfs:subClassOf rdf:resource="http://www.ontologydesignpatterns.org/ont/dul/DUL.owl#Transition"/>
        <rdfs:comment>A transition between two situations, usually brought about by the Action of some Agent.</rdfs:comment>
        <rdfs:isDefinedBy rdf:resource="http://www.ease-crc.org/ont/SOMA-ACT.owl"/>
        <rdfs:label xml:lang="en">Situation transition</rdfs:label>
    </owl:Class>
    


    <!-- http://www.ease-crc.org/ont/SOMA.owl#Size -->


    <owl:Class rdf:about="http://www.ease-crc.org/ont/SOMA.owl#Size">
        <rdfs:subClassOf rdf:resource="http://www.ease-crc.org/ont/SOMA.owl#Intrinsic"/>
        <rdfs:comment>The magnitude or dimension of a thing which can be measured as length, width, height, diameter, perimeter, area, volume.</rdfs:comment>
        <rdfs:isDefinedBy rdf:resource="http://www.ease-crc.org/ont/SOMA-OBJ.owl"/>
    </owl:Class>
    


    <!-- http://www.ease-crc.org/ont/SOMA.owl#Slicing -->


    <owl:Class rdf:about="http://www.ease-crc.org/ont/SOMA.owl#Slicing">
        <rdfs:subClassOf rdf:resource="http://www.ease-crc.org/ont/SOMA.owl#Cutting"/>
        <rdfs:comment>A particular kind of cutting where the goal is to produce slices from some solid object.</rdfs:comment>
        <rdfs:isDefinedBy rdf:resource="http://www.ease-crc.org/ont/SOMA-ACT.owl"/>
    </owl:Class>
    


    <!-- http://www.ease-crc.org/ont/SOMA.owl#SocialQuality -->


    <owl:Class rdf:about="http://www.ease-crc.org/ont/SOMA.owl#SocialQuality">
        <rdfs:subClassOf rdf:resource="http://www.ontologydesignpatterns.org/ont/dul/DUL.owl#Quality"/>
        <rdfs:comment>Any aspect of an entity that specifies social characteristics.</rdfs:comment>
        <rdfs:isDefinedBy rdf:resource="http://www.ease-crc.org/ont/SOMA-OBJ.owl"/>
        <rdfs:label>Social quality</rdfs:label>
    </owl:Class>
    


    <!-- http://www.ease-crc.org/ont/SOMA.owl#SocialState -->


    <owl:Class rdf:about="http://www.ease-crc.org/ont/SOMA.owl#SocialState">
        <rdfs:subClassOf rdf:resource="http://www.ease-crc.org/ont/SOMA.owl#State"/>
        <rdfs:subClassOf>
            <owl:Restriction>
                <owl:onProperty rdf:resource="http://www.ontologydesignpatterns.org/ont/dul/DUL.owl#hasParticipant"/>
                <owl:someValuesFrom rdf:resource="http://www.ontologydesignpatterns.org/ont/dul/DUL.owl#Agent"/>
            </owl:Restriction>
        </rdfs:subClassOf>
        <rdfs:comment>A State which describes how Agents relate to each other.

One can argue that any Social state is a Physical state, since anything the Agents may use to construct a social relationship is made of physical things. The difference is that the physical support of the social relationships is not important here, what matters instead is the nature and content of the social relations, regardless of how they are physically realized.</rdfs:comment>
        <rdfs:comment>Note here a distinction: the Agents involved must be able to communicate. This is because while it is often assumed that an Agent has or aspires to have similar cognitive capacities to a human, This need not be the case; in particular, not all Agents need to maintain theories of mind about each other and therefore not all Agents need to communicate with each other. It is hard to see what sort of meaning Social concepts might have to such Agents, since Social concepts are all about shared constructions.

Note also that the DUL SocialAgent class is not an appropriate restriction however. SocialAgent is one that exists by agreement of PhysicalAgents. For example, a corporation or a nation are SocialAgents. An Agent with the capability to engage socially is not necessarily a DUL SocialAgent.</rdfs:comment>
        <rdfs:isDefinedBy rdf:resource="http://www.ease-crc.org/ont/SOMA-STATE.owl"/>
        <rdfs:label>Social state</rdfs:label>
    </owl:Class>
    


    <!-- http://www.ease-crc.org/ont/SOMA.owl#Software -->


    <owl:Class rdf:about="http://www.ease-crc.org/ont/SOMA.owl#Software">
        <rdfs:subClassOf rdf:resource="http://www.ontologydesignpatterns.org/ont/dul/DUL.owl#Design"/>
        <rdfs:isDefinedBy rdf:resource="http://www.ease-crc.org/ont/SOMA-IO.owl"/>
        <rdfs:label xml:lang="en">Software</rdfs:label>
        <rdfs:label xml:lang="en">We see Software as the Design of a DesignedTool: the running instance of said Software. Software as a design also follows the Function-Behaviour-Structure model:

The Function is the purpose or problem solving embodied by the Software Instance, e.g., sorting a list.

The Behaviour are the algoirthms used by the Software Instance, e.g., Bubble Sort.

The Structure is the organization of files, classes, objects and method calls of the program code.</rdfs:label>
    </owl:Class>
    


    <!-- http://www.ease-crc.org/ont/SOMA.owl#SoftwareInstance -->


    <owl:Class rdf:about="http://www.ease-crc.org/ont/SOMA.owl#SoftwareInstance">
        <rdfs:subClassOf>
            <owl:Class>
                <owl:intersectionOf rdf:parseType="Collection">
                    <rdf:Description rdf:about="http://www.ease-crc.org/ont/SOMA.owl#DesignedTool"/>
                    <owl:Restriction>
                        <owl:onProperty rdf:resource="http://www.ease-crc.org/ont/SOMA.owl#isDesignedBy"/>
                        <owl:someValuesFrom rdf:resource="http://www.ease-crc.org/ont/SOMA.owl#Software"/>
                    </owl:Restriction>
                </owl:intersectionOf>
            </owl:Class>
        </rdfs:subClassOf>
        <rdfs:subClassOf>
            <owl:Class>
                <owl:intersectionOf rdf:parseType="Collection">
                    <rdf:Description rdf:about="http://www.ontologydesignpatterns.org/ont/dul/DUL.owl#SocialAgent"/>
                    <owl:Restriction>
                        <owl:onProperty rdf:resource="http://www.ontologydesignpatterns.org/ont/dul/DUL.owl#actsFor"/>
                        <owl:someValuesFrom rdf:resource="http://www.ontologydesignpatterns.org/ont/dul/DUL.owl#Agent"/>
                    </owl:Restriction>
                </owl:intersectionOf>
            </owl:Class>
        </rdfs:subClassOf>
        <rdfs:comment xml:lang="en">A Software instance is an entity to represent the agent that emerges from and while executing software: Some object, that can perform actions and communicate via some interfaces.
In this view, we see the of an Agent required intentionality its intentionality as bestowed upon the Software instance from the agents who started the program or gave an input (e.g., via a mouse click) to achieve some goal.

Another apporach might be to not model this entity at all and only see Execution of Software as a Process (see, e.g., https://en.wikipedia.org/wiki/Execution_(computing)). However, this would complicate modeling communication between running Software processes.</rdfs:comment>
        <rdfs:isDefinedBy rdf:resource="http://www.ease-crc.org/ont/SOMA-IO.owl"/>
        <rdfs:label xml:lang="en">Software instance</rdfs:label>
    </owl:Class>
    


    <!-- http://www.ease-crc.org/ont/SOMA.owl#SoftwareLibrary -->


    <owl:Class rdf:about="http://www.ease-crc.org/ont/SOMA.owl#SoftwareLibrary">
        <rdfs:subClassOf rdf:resource="http://www.ease-crc.org/ont/SOMA.owl#Software"/>
        <rdfs:isDefinedBy rdf:resource="http://www.ease-crc.org/ont/SOMA-IO.owl"/>
        <rdfs:label xml:lang="en">Software Library</rdfs:label>
    </owl:Class>
    


    <!-- http://www.ease-crc.org/ont/SOMA.owl#SoftwareRole -->


    <owl:Class rdf:about="http://www.ease-crc.org/ont/SOMA.owl#SoftwareRole">
        <rdfs:subClassOf rdf:resource="http://www.ontologydesignpatterns.org/ont/dul/DUL.owl#Role"/>
        <rdfs:subClassOf>
            <owl:Restriction>
                <owl:onProperty rdf:resource="http://www.ontologydesignpatterns.org/ont/dul/DUL.owl#classifies"/>
                <owl:allValuesFrom rdf:resource="http://www.ease-crc.org/ont/SOMA.owl#Software"/>
            </owl:Restriction>
        </rdfs:subClassOf>
        <rdfs:comment xml:lang="en">A Software Role is a Role applying to only Software and encoding the purpose of the Software: Its Role within Interface Patterns (e.g. Client vs. Server), its functionality (e.g. Database vs. Comnputer Game), and so on.</rdfs:comment>
        <rdfs:isDefinedBy rdf:resource="http://www.ease-crc.org/ont/SOMA-IO.owl"/>
        <rdfs:label xml:lang="en">Software role</rdfs:label>
    </owl:Class>
    


    <!-- http://www.ease-crc.org/ont/SOMA.owl#Software_Configuration -->


    <owl:Class rdf:about="http://www.ease-crc.org/ont/SOMA.owl#Software_Configuration">
        <rdfs:subClassOf rdf:resource="http://www.ontologydesignpatterns.org/ont/dul/DUL.owl#Configuration"/>
        <rdfs:isDefinedBy rdf:resource="http://www.ease-crc.org/ont/SOMA-IO.owl"/>
        <rdfs:label xml:lang="en">Software Configuration</rdfs:label>
        <rdfs:label xml:lang="en">The part-whole relationship of Software and its components. Every Software has (at least 1) such configuration that exactly describes all Resources that make up the software (i.e., that are needed for the Software to function).
We support seperate views:
1. The Software Configuration describes all the necessary files, in which it should also be a File Configuration
2. It describes a Software Suit, e.g., &apos;Open Office&apos; consists of Writer, Calc, Impress etc. Note that thus. Software can consist of other Software - this pattern may also be useful when describing Software Components, e.g., that some Software relies on a Database Software.
3. It describes not the files, but their content (the program code), which can also be seen as the part-whole relationship if one abstracts away from the files.</rdfs:label>
    </owl:Class>
    


    <!-- http://www.ease-crc.org/ont/SOMA.owl#SourceMaterialRole -->


    <owl:Class rdf:about="http://www.ease-crc.org/ont/SOMA.owl#SourceMaterialRole">
        <rdfs:subClassOf rdf:resource="http://www.ease-crc.org/ont/SOMA.owl#ResourceRole"/>
        <rdfs:comment>A role classifying a substance or object that enters a process of transformation intended to create some other object.</rdfs:comment>
        <rdfs:isDefinedBy rdf:resource="http://www.ease-crc.org/ont/SOMA-OBJ.owl"/>
        <rdfs:label xml:lang="en">Source material role</rdfs:label>
    </owl:Class>
    


    <!-- http://www.ease-crc.org/ont/SOMA.owl#SourcePathGoalTheory -->


    <owl:Class rdf:about="http://www.ease-crc.org/ont/SOMA.owl#SourcePathGoalTheory">
        <rdfs:subClassOf rdf:resource="http://www.ease-crc.org/ont/SOMA.owl#ImageSchemaTheory"/>
        <rdfs:subClassOf>
            <owl:Restriction>
                <owl:onProperty rdf:resource="http://www.ontologydesignpatterns.org/ont/dul/DUL.owl#defines"/>
                <owl:someValuesFrom rdf:resource="http://www.ease-crc.org/ont/SOMA.owl#Destination"/>
            </owl:Restriction>
        </rdfs:subClassOf>
        <rdfs:subClassOf>
            <owl:Restriction>
                <owl:onProperty rdf:resource="http://www.ontologydesignpatterns.org/ont/dul/DUL.owl#defines"/>
                <owl:someValuesFrom rdf:resource="http://www.ease-crc.org/ont/SOMA.owl#Origin"/>
            </owl:Restriction>
        </rdfs:subClassOf>
        <rdfs:subClassOf>
            <owl:Restriction>
                <owl:onProperty rdf:resource="http://www.ontologydesignpatterns.org/ont/dul/DUL.owl#defines"/>
                <owl:someValuesFrom rdf:resource="http://www.ease-crc.org/ont/SOMA.owl#PathRole"/>
            </owl:Restriction>
        </rdfs:subClassOf>
        <rdfs:comment>A very general image-schema of the Path family, this schema describes movement along a path from a source towards a goal.

Note: in cognitive linguistics literature, the roles of this schema are Source, Path, Goal. However, to avoid overloading some other terminology in SOMA, we renamed Source to Origin and Goal to Destination.

As yet, this schema is not associated to any object property.</rdfs:comment>
        <rdfs:isDefinedBy rdf:resource="http://www.ease-crc.org/ont/SOMA-SAY.owl"/>
        <rdfs:label xml:lang="en">Source-path-goal theory</rdfs:label>
    </owl:Class>
    


    <!-- http://www.ease-crc.org/ont/SOMA.owl#Source_Code -->


    <owl:Class rdf:about="http://www.ease-crc.org/ont/SOMA.owl#Source_Code">
        <owl:equivalentClass>
            <owl:Class>
                <owl:intersectionOf rdf:parseType="Collection">
                    <rdf:Description rdf:about="http://www.ease-crc.org/ont/SOMA.owl#Computer_Program"/>
                    <owl:Restriction>
                        <owl:onProperty rdf:resource="http://www.ease-crc.org/ont/SOMA.owl#isGivenMeaningBy"/>
                        <owl:someValuesFrom rdf:resource="http://www.ease-crc.org/ont/SOMA.owl#Human-readable_Programming_Language"/>
                    </owl:Restriction>
                </owl:intersectionOf>
            </owl:Class>
        </owl:equivalentClass>
        <rdfs:subClassOf rdf:resource="http://www.ease-crc.org/ont/SOMA.owl#Computer_Program"/>
        <rdfs:comment xml:lang="en">The Source Code itself (the specific set of instruction in a human-readable Programming Language), not the file that it is contained in nor the implemented algorithm!</rdfs:comment>
        <rdfs:isDefinedBy rdf:resource="http://www.ease-crc.org/ont/SOMA-IO.owl"/>
        <rdfs:label xml:lang="en">Source code</rdfs:label>
    </owl:Class>
    


    <!-- http://www.ease-crc.org/ont/SOMA.owl#SpatialRelationRole -->


    <owl:Class rdf:about="http://www.ease-crc.org/ont/SOMA.owl#SpatialRelationRole">
        <rdfs:subClassOf rdf:resource="http://www.ease-crc.org/ont/SOMA.owl#RelationAdjacentRole"/>
        <rdfs:comment>Roles classifying entities participating in some spatial relation.</rdfs:comment>
        <rdfs:isDefinedBy rdf:resource="http://www.ease-crc.org/ont/SOMA-OBJ.owl"/>
        <rdfs:label xml:lang="en">Spatial relation role</rdfs:label>
    </owl:Class>
    


    <!-- http://www.ease-crc.org/ont/SOMA.owl#SpatioTemporalRole -->


    <owl:Class rdf:about="http://www.ease-crc.org/ont/SOMA.owl#SpatioTemporalRole">
        <rdfs:subClassOf rdf:resource="http://www.ease-crc.org/ont/SOMA.owl#EventAdjacentRole"/>
        <rdfs:comment>Roles that classify entities which locate an event or object in space and time.</rdfs:comment>
        <rdfs:isDefinedBy rdf:resource="http://www.ease-crc.org/ont/SOMA-OBJ.owl"/>
        <rdfs:label xml:lang="en">Spatio-temporal role</rdfs:label>
    </owl:Class>
    


    <!-- http://www.ease-crc.org/ont/SOMA.owl#Spatula -->


    <owl:Class rdf:about="http://www.ease-crc.org/ont/SOMA.owl#Spatula">
        <rdfs:subClassOf rdf:resource="http://www.ease-crc.org/ont/SOMA.owl#Cutlery"/>
        <rdfs:subClassOf>
            <owl:Restriction>
                <owl:onProperty rdf:resource="http://www.ease-crc.org/ont/SOMA.owl#hasPhysicalComponent"/>
                <owl:someValuesFrom rdf:resource="http://www.ease-crc.org/ont/SOMA.owl#DesignedHandle"/>
            </owl:Restriction>
        </rdfs:subClassOf>
        <rdfs:subClassOf>
            <owl:Restriction>
                <owl:onProperty rdf:resource="http://www.ease-crc.org/ont/SOMA.owl#hasPhysicalComponent"/>
                <owl:someValuesFrom rdf:resource="http://www.ease-crc.org/ont/SOMA.owl#DesignedSpade"/>
            </owl:Restriction>
        </rdfs:subClassOf>
        <rdfs:isDefinedBy rdf:resource="http://www.ease-crc.org/ont/SOMA-HOME.owl"/>
    </owl:Class>
    


    <!-- http://www.ease-crc.org/ont/SOMA.owl#SphereShape -->


    <owl:Class rdf:about="http://www.ease-crc.org/ont/SOMA.owl#SphereShape">
        <rdfs:subClassOf rdf:resource="http://www.ease-crc.org/ont/SOMA.owl#ShapeRegion"/>
        <rdfs:subClassOf>
            <owl:Restriction>
                <owl:onProperty rdf:resource="http://www.ease-crc.org/ont/SOMA.owl#hasRadius"/>
                <owl:qualifiedCardinality rdf:datatype="http://www.w3.org/2001/XMLSchema#nonNegativeInteger">1</owl:qualifiedCardinality>
                <owl:onDataRange rdf:resource="http://www.w3.org/2001/XMLSchema#float"/>
            </owl:Restriction>
        </rdfs:subClassOf>
        <rdfs:comment>A round solid figure with every point on its surface equidistant from its centre.</rdfs:comment>
        <rdfs:isDefinedBy rdf:resource="http://www.ease-crc.org/ont/SOMA-OBJ.owl"/>
        <rdfs:label>Sphere shape</rdfs:label>
    </owl:Class>
    


    <!-- http://www.ease-crc.org/ont/SOMA.owl#Squeezing -->


    <owl:Class rdf:about="http://www.ease-crc.org/ont/SOMA.owl#Squeezing">
        <rdfs:subClassOf rdf:resource="http://www.ease-crc.org/ont/SOMA.owl#Actuating"/>
        <rdfs:comment>A task in which an Agent applies pressure to an object they have in their grasp.</rdfs:comment>
        <rdfs:isDefinedBy rdf:resource="http://www.ease-crc.org/ont/SOMA-ACT.owl"/>
    </owl:Class>
    


    <!-- http://www.ease-crc.org/ont/SOMA.owl#Standing -->


    <owl:Class rdf:about="http://www.ease-crc.org/ont/SOMA.owl#Standing">
        <rdfs:subClassOf rdf:resource="http://www.ease-crc.org/ont/SOMA.owl#PosturalMoving"/>
        <rdfs:comment>A motion by which an Agent arranges its body in an upright configuration. Typically, it makes sense to speak of standing for bodies where some limbs are dedicated to moving the whole body while some limbs are used for manipulation of other objects.</rdfs:comment>
        <rdfs:isDefinedBy rdf:resource="http://www.ease-crc.org/ont/SOMA-PROC.owl"/>
    </owl:Class>
    


    <!-- http://www.ease-crc.org/ont/SOMA.owl#State -->


    <owl:Class rdf:about="http://www.ease-crc.org/ont/SOMA.owl#State">
        <rdfs:isDefinedBy rdf:resource="http://www.ease-crc.org/ont/SOMA-SAY.owl"/>
    </owl:Class>
    


    <!-- http://www.ease-crc.org/ont/SOMA.owl#StateTransition -->


    <owl:Class rdf:about="http://www.ease-crc.org/ont/SOMA.owl#StateTransition">
        <rdfs:subClassOf rdf:resource="http://www.ontologydesignpatterns.org/ont/dul/DUL.owl#Transition"/>
        <rdfs:subClassOf>
            <owl:Restriction>
                <owl:onProperty rdf:resource="http://www.ease-crc.org/ont/SOMA.owl#hasInitialScene"/>
                <owl:someValuesFrom rdf:resource="http://www.ease-crc.org/ont/SOMA.owl#Scene"/>
            </owl:Restriction>
        </rdfs:subClassOf>
        <rdfs:subClassOf>
            <owl:Restriction>
                <owl:onProperty rdf:resource="http://www.ease-crc.org/ont/SOMA.owl#hasTerminalScene"/>
                <owl:someValuesFrom rdf:resource="http://www.ease-crc.org/ont/SOMA.owl#Scene"/>
            </owl:Restriction>
        </rdfs:subClassOf>
        <rdfs:subClassOf>
            <owl:Restriction>
                <owl:onProperty rdf:resource="http://www.ontologydesignpatterns.org/ont/dul/DUL.owl#includesEvent"/>
                <owl:someValuesFrom rdf:resource="http://www.ontologydesignpatterns.org/ont/dul/DUL.owl#Action"/>
            </owl:Restriction>
        </rdfs:subClassOf>
        <rdfs:subClassOf>
            <owl:Restriction>
                <owl:onProperty rdf:resource="http://www.ontologydesignpatterns.org/ont/dul/DUL.owl#satisfies"/>
                <owl:someValuesFrom rdf:resource="http://www.ease-crc.org/ont/SOMA.owl#ImageSchemaTheory"/>
            </owl:Restriction>
        </rdfs:subClassOf>
        <rdfs:comment>A transition between two states brought about by the Action of some Agent.</rdfs:comment>
        <rdfs:isDefinedBy rdf:resource="http://www.ease-crc.org/ont/SOMA-SAY.owl"/>
        <rdfs:label xml:lang="en">State transition</rdfs:label>
    </owl:Class>
    


    <!-- http://www.ease-crc.org/ont/SOMA.owl#StateType -->


    <owl:Class rdf:about="http://www.ease-crc.org/ont/SOMA.owl#StateType">
        <rdfs:subClassOf rdf:resource="http://www.ontologydesignpatterns.org/ont/dul/DUL.owl#EventType"/>
        <rdfs:subClassOf>
            <owl:Restriction>
                <owl:onProperty rdf:resource="http://www.ontologydesignpatterns.org/ont/dul/DUL.owl#classifies"/>
                <owl:allValuesFrom rdf:resource="http://www.ease-crc.org/ont/SOMA.owl#State"/>
            </owl:Restriction>
        </rdfs:subClassOf>
        <rdfs:subClassOf>
            <owl:Restriction>
                <owl:onProperty rdf:resource="http://www.ontologydesignpatterns.org/ont/dul/DUL.owl#hasPart"/>
                <owl:allValuesFrom rdf:resource="http://www.ease-crc.org/ont/SOMA.owl#StateType"/>
            </owl:Restriction>
        </rdfs:subClassOf>
        <rdfs:comment>An EventType that classifies States.</rdfs:comment>
        <rdfs:isDefinedBy rdf:resource="http://www.ease-crc.org/ont/SOMA-STATE.owl"/>
        <rdfs:label xml:lang="en">State type</rdfs:label>
    </owl:Class>
    


    <!-- http://www.ease-crc.org/ont/SOMA.owl#StaticFrictionAttribute -->


    <owl:Class rdf:about="http://www.ease-crc.org/ont/SOMA.owl#StaticFrictionAttribute">
        <rdfs:subClassOf rdf:resource="http://www.ease-crc.org/ont/SOMA.owl#FrictionAttribute"/>
        <rdfs:comment>Friction between two touching objects that do not move relative to each other.</rdfs:comment>
        <rdfs:isDefinedBy rdf:resource="http://www.ease-crc.org/ont/SOMA-OBJ.owl"/>
        <rdfs:label>Static friction attribute</rdfs:label>
    </owl:Class>
    


    <!-- http://www.ease-crc.org/ont/SOMA.owl#StatisticalReasoner -->


    <owl:Class rdf:about="http://www.ease-crc.org/ont/SOMA.owl#StatisticalReasoner">
        <rdfs:subClassOf rdf:resource="http://www.ease-crc.org/ont/SOMA.owl#Reasoner"/>
        <rdfs:isDefinedBy rdf:resource="http://www.ease-crc.org/ont/SOMA-IO.owl"/>
        <rdfs:label xml:lang="en">A Statistical Reasoner is a Reasoner that uses statistical or stochastical data to infer implicit information from explicit information. Examples are Hidden Markov Models and Neural Networks.</rdfs:label>
        <rdfs:label xml:lang="en">Statistical reasoner</rdfs:label>
    </owl:Class>
    


    <!-- http://www.ease-crc.org/ont/SOMA.owl#StatusFailure -->


    <owl:Class rdf:about="http://www.ease-crc.org/ont/SOMA.owl#StatusFailure">
        <rdfs:subClassOf rdf:resource="http://www.ontologydesignpatterns.org/ont/dul/DUL.owl#Region"/>
        <rdfs:comment>A status indicating the failure during some workflow execution.</rdfs:comment>
        <rdfs:isDefinedBy rdf:resource="http://www.ease-crc.org/ont/SOMA-WF.owl"/>
    </owl:Class>
    


    <!-- http://www.ease-crc.org/ont/SOMA.owl#StimulusRole -->


    <owl:Class rdf:about="http://www.ease-crc.org/ont/SOMA.owl#StimulusRole">
        <rdfs:subClassOf rdf:resource="http://www.ease-crc.org/ont/SOMA.owl#CausativeRole"/>
        <rdfs:comment>A role classifying an object that is perceived by some agent and thus triggers some reaction (e.g., a perception event).</rdfs:comment>
        <rdfs:isDefinedBy rdf:resource="http://www.ease-crc.org/ont/SOMA-OBJ.owl"/>
        <rdfs:label xml:lang="en">Stimulus role</rdfs:label>
    </owl:Class>
    


    <!-- http://www.ease-crc.org/ont/SOMA.owl#Stove -->


    <owl:Class rdf:about="http://www.ease-crc.org/ont/SOMA.owl#Stove">
        <rdfs:subClassOf rdf:resource="http://www.ease-crc.org/ont/SOMA.owl#Appliance"/>
        <rdfs:subClassOf>
            <owl:Restriction>
                <owl:onProperty rdf:resource="http://www.ease-crc.org/ont/SOMA.owl#hasPhysicalComponent"/>
                <owl:someValuesFrom rdf:resource="http://www.ease-crc.org/ont/SOMA.owl#Hotplate"/>
            </owl:Restriction>
        </rdfs:subClassOf>
        <rdfs:comment>An appliance for cooking or heating.</rdfs:comment>
        <rdfs:isDefinedBy rdf:resource="http://www.ease-crc.org/ont/SOMA-HOME.owl"/>
    </owl:Class>
    


    <!-- http://www.ease-crc.org/ont/SOMA.owl#StructuralDesign -->


    <owl:Class rdf:about="http://www.ease-crc.org/ont/SOMA.owl#StructuralDesign">
        <rdfs:subClassOf rdf:resource="http://www.ontologydesignpatterns.org/ont/dul/DUL.owl#Design"/>
        <rdfs:comment>A design of an object which describes its stability, strength and rigidity, and considers the way in which parts of an object are arranged. 
        </rdfs:comment>
        <rdfs:isDefinedBy rdf:resource="http://www.ease-crc.org/ont/SOMA-OBJ.owl"/>
        <rdfs:label>Structural Design</rdfs:label>
    </owl:Class>
    


    <!-- http://www.ease-crc.org/ont/SOMA.owl#Structured_Text -->


    <owl:Class rdf:about="http://www.ease-crc.org/ont/SOMA.owl#Structured_Text">
        <owl:equivalentClass>
            <owl:Class>
                <owl:intersectionOf rdf:parseType="Collection">
                    <rdf:Description rdf:about="http://www.ease-crc.org/ont/SOMA.owl#Text"/>
                    <owl:Restriction>
                        <owl:onProperty rdf:resource="http://www.ease-crc.org/ont/SOMA.owl#isGivenMeaningBy"/>
                        <owl:someValuesFrom rdf:resource="http://www.ease-crc.org/ont/SOMA.owl#FormalLanguage"/>
                    </owl:Restriction>
                </owl:intersectionOf>
            </owl:Class>
        </owl:equivalentClass>
        <rdfs:comment xml:lang="en">Any Text that adheres to some rules that are in any way more specific than natural language and that cannot be made sense of without knowing said rules.</rdfs:comment>
        <rdfs:isDefinedBy rdf:resource="http://www.ease-crc.org/ont/SOMA-IO.owl"/>
        <rdfs:label xml:lang="en">Structured text</rdfs:label>
    </owl:Class>
    


    <!-- http://www.ease-crc.org/ont/SOMA.owl#Succedence -->


    <owl:Class rdf:about="http://www.ease-crc.org/ont/SOMA.owl#Succedence">
        <rdfs:subClassOf rdf:resource="http://www.ontologydesignpatterns.org/ont/dul/DUL.owl#Relation"/>
        <rdfs:subClassOf>
            <owl:Restriction>
                <owl:onProperty>
                    <rdf:Description>
                        <owl:inverseOf rdf:resource="http://www.ease-crc.org/ont/SOMA.owl#hasSuccedence"/>
                    </rdf:Description>
                </owl:onProperty>
                <owl:someValuesFrom rdf:resource="http://www.ontologydesignpatterns.org/ont/dul/DUL.owl#Description"/>
            </owl:Restriction>
        </rdfs:subClassOf>
        <rdfs:subClassOf>
            <owl:Restriction>
                <owl:onProperty rdf:resource="http://www.ease-crc.org/ont/SOMA.owl#hasPredecessor"/>
                <owl:qualifiedCardinality rdf:datatype="http://www.w3.org/2001/XMLSchema#nonNegativeInteger">1</owl:qualifiedCardinality>
                <owl:onClass rdf:resource="http://www.ease-crc.org/ont/SOMA.owl#TaskInvocation"/>
            </owl:Restriction>
        </rdfs:subClassOf>
        <rdfs:subClassOf>
            <owl:Restriction>
                <owl:onProperty rdf:resource="http://www.ease-crc.org/ont/SOMA.owl#hasSuccessor"/>
                <owl:qualifiedCardinality rdf:datatype="http://www.w3.org/2001/XMLSchema#nonNegativeInteger">1</owl:qualifiedCardinality>
                <owl:onClass rdf:resource="http://www.ease-crc.org/ont/SOMA.owl#TaskInvocation"/>
            </owl:Restriction>
        </rdfs:subClassOf>
        <rdfs:comment>A relation that holds in some descriptive context such as a Workflow, between two TaskInvocations belonging to that same Workflow. It means that one task invocation should follow the other.

Note: a successor relation implemented as an OWL object property is sometimes enough, but not in general; in particular, when there are conditions imposed on the succession.

As a result, a reification pattern was applied here.</rdfs:comment>
        <rdfs:comment>Note: it is possible for a Succedence relation to exist between a TaskInvocation and itself; in this case, both the hasPredecessor and hasSuccessor roles are filled by the same TaskInvocation individual.

Care must be taken with this however, as a natural interpretation of this situation is an infinite loop.</rdfs:comment>
        <rdfs:isDefinedBy rdf:resource="http://www.ease-crc.org/ont/SOMA-WF.owl"/>
    </owl:Class>
    


    <!-- http://www.ease-crc.org/ont/SOMA.owl#SupportState -->


    <owl:Class rdf:about="http://www.ease-crc.org/ont/SOMA.owl#SupportState">
        <rdfs:subClassOf rdf:resource="http://www.ease-crc.org/ont/SOMA.owl#FunctionalControl"/>
        <rdfs:subClassOf>
            <owl:Restriction>
                <owl:onProperty rdf:resource="http://www.ease-crc.org/ont/SOMA.owl#isStateTypeOf"/>
                <owl:someValuesFrom>
                    <owl:Class>
                        <owl:intersectionOf rdf:parseType="Collection">
                            <rdf:Description rdf:about="http://www.ease-crc.org/ont/SOMA.owl#Supporter"/>
                            <owl:Restriction>
                                <owl:onProperty rdf:resource="http://www.ontologydesignpatterns.org/ont/dul/DUL.owl#classifies"/>
                                <owl:allValuesFrom>
                                    <owl:Restriction>
                                        <owl:onProperty rdf:resource="http://www.ease-crc.org/ont/SOMA.owl#hasDisposition"/>
                                        <owl:someValuesFrom rdf:resource="http://www.ease-crc.org/ont/SOMA.owl#Deposition"/>
                                    </owl:Restriction>
                                </owl:allValuesFrom>
                            </owl:Restriction>
                        </owl:intersectionOf>
                    </owl:Class>
                </owl:someValuesFrom>
            </owl:Restriction>
        </rdfs:subClassOf>
        <rdfs:comment>Classifies States in which an object is not able to move under gravity because of its placement relative to some other object.</rdfs:comment>
        <rdfs:isDefinedBy rdf:resource="http://www.ease-crc.org/ont/SOMA-STATE.owl"/>
        <rdfs:label xml:lang="en">Support state</rdfs:label>
    </owl:Class>
    


    <!-- http://www.ease-crc.org/ont/SOMA.owl#SupportTheory -->


    <owl:Class rdf:about="http://www.ease-crc.org/ont/SOMA.owl#SupportTheory">
        <rdfs:subClassOf rdf:resource="http://www.ease-crc.org/ont/SOMA.owl#ControlTheory"/>
        <rdfs:comment>An image schematic theory that describes the reified functional relation holding between two spatial objects x and y, such that x physically supports y in the presence of gravity; x and y need not be in contact. An example of such an expression is &quot;The bowl is on the table&quot;.

This is also known as FunctionalControlExternal in GUM (Bateman et al. 2010).

Let xL, xR be objects filling the locatum, relatum roles of this schema. Then one can infer that xL isSupportedBy xR.</rdfs:comment>
        <rdfs:isDefinedBy rdf:resource="http://www.ease-crc.org/ont/SOMA-SAY.owl"/>
        <rdfs:label xml:lang="en">Support theory</rdfs:label>
    </owl:Class>
    


    <!-- http://www.ease-crc.org/ont/SOMA.owl#SupportedObject -->


    <owl:Class rdf:about="http://www.ease-crc.org/ont/SOMA.owl#SupportedObject">
        <rdfs:subClassOf rdf:resource="http://www.ease-crc.org/ont/SOMA.owl#ConnectedObject"/>
        <rdfs:comment>An object that is supported by some supporter.</rdfs:comment>
        <rdfs:isDefinedBy rdf:resource="http://www.ease-crc.org/ont/SOMA-OBJ.owl"/>
        <rdfs:label xml:lang="en">Supported object</rdfs:label>
    </owl:Class>
    


    <!-- http://www.ease-crc.org/ont/SOMA.owl#Supporter -->


    <owl:Class rdf:about="http://www.ease-crc.org/ont/SOMA.owl#Supporter">
        <rdfs:subClassOf rdf:resource="http://www.ease-crc.org/ont/SOMA.owl#Restrictor"/>
        <rdfs:comment>A role classifying an object used to support others.</rdfs:comment>
        <rdfs:isDefinedBy rdf:resource="http://www.ease-crc.org/ont/SOMA-OBJ.owl"/>
        <rdfs:isDefinedBy rdf:resource="http://www.ease-crc.org/ont/SOMA-STATE.owl"/>
    </owl:Class>
    


    <!-- http://www.ease-crc.org/ont/SOMA.owl#Surface -->


    <owl:Class rdf:about="http://www.ease-crc.org/ont/SOMA.owl#Surface">
        <rdfs:subClassOf rdf:resource="http://www.ontologydesignpatterns.org/ont/dul/DUL.owl#PhysicalPlace"/>
        <rdfs:comment>The outside part or uppermost layer of something.</rdfs:comment>
        <rdfs:isDefinedBy rdf:resource="http://www.ease-crc.org/ont/SOMA-HOME.owl"/>
        <rdfs:isDefinedBy rdf:resource="http://www.ease-crc.org/ont/SOMA-OBJ.owl"/>
    </owl:Class>
    


    <!-- http://www.ease-crc.org/ont/SOMA.owl#Swimming -->


    <owl:Class rdf:about="http://www.ease-crc.org/ont/SOMA.owl#Swimming">
        <rdfs:subClassOf rdf:resource="http://www.ease-crc.org/ont/SOMA.owl#Locomotion"/>
        <owl:disjointWith rdf:resource="http://www.ease-crc.org/ont/SOMA.owl#Walking"/>
        <rdfs:comment>A motion of some body through water. The body provides the power for the motion.</rdfs:comment>
        <rdfs:isDefinedBy rdf:resource="http://www.ease-crc.org/ont/SOMA-PROC.owl"/>
    </owl:Class>
    


    <!-- http://www.ease-crc.org/ont/SOMA.owl#SymbolicReasoner -->


    <owl:Class rdf:about="http://www.ease-crc.org/ont/SOMA.owl#SymbolicReasoner">
        <rdfs:subClassOf rdf:resource="http://www.ease-crc.org/ont/SOMA.owl#Reasoner"/>
        <rdfs:comment xml:lang="en">A Symbolic Reasoner, is a piece of software able to infer logical consequences from a set of asserted facts or axioms.

Source: https://en.wikipedia.org/wiki/Semantic_reasoner</rdfs:comment>
        <rdfs:isDefinedBy rdf:resource="http://www.ease-crc.org/ont/SOMA-IO.owl"/>
        <rdfs:label xml:lang="en">Symbolic reasoner</rdfs:label>
    </owl:Class>
    


    <!-- http://www.ease-crc.org/ont/SOMA.owl#System -->


    <owl:Class rdf:about="http://www.ease-crc.org/ont/SOMA.owl#System">
        <rdfs:subClassOf rdf:resource="http://www.ontologydesignpatterns.org/ont/dul/DUL.owl#SocialObject"/>
        <rdfs:comment xml:lang="en">A system is a group of interacting or interrelated elements that act according to a set of rules to form a unified whole.

From Wikipedia: https://en.wikipedia.org/wiki/System</rdfs:comment>
        <rdfs:isDefinedBy rdf:resource="http://www.ease-crc.org/ont/SOMA-IO.owl"/>
        <rdfs:label xml:lang="en">System</rdfs:label>
    </owl:Class>
    


    <!-- http://www.ease-crc.org/ont/SOMA.owl#Table -->


    <owl:Class rdf:about="http://www.ease-crc.org/ont/SOMA.owl#Table">
        <rdfs:subClassOf rdf:resource="http://www.ease-crc.org/ont/SOMA.owl#DesignedFurniture"/>
        <rdfs:comment>A piece of furniture with a flat top and one or more legs.</rdfs:comment>
        <rdfs:isDefinedBy rdf:resource="http://www.ease-crc.org/ont/SOMA-HOME.owl"/>
    </owl:Class>
    


    <!-- http://www.ease-crc.org/ont/SOMA.owl#Tableware -->


    <owl:Class rdf:about="http://www.ease-crc.org/ont/SOMA.owl#Tableware">
        <rdfs:subClassOf rdf:resource="http://www.ease-crc.org/ont/SOMA.owl#DesignedTool"/>
        <rdfs:isDefinedBy rdf:resource="http://www.ease-crc.org/ont/SOMA-HOME.owl"/>
    </owl:Class>
    


    <!-- http://www.ease-crc.org/ont/SOMA.owl#Tapping -->


    <owl:Class rdf:about="http://www.ease-crc.org/ont/SOMA.owl#Tapping">
        <rdfs:subClassOf rdf:resource="http://www.ease-crc.org/ont/SOMA.owl#DirectedMotion"/>
        <rdfs:comment>A motion, usually repeated several times, for example, to probe the surface of an object.</rdfs:comment>
        <rdfs:isDefinedBy rdf:resource="http://www.ease-crc.org/ont/SOMA-PROC.owl"/>
    </owl:Class>
    


    <!-- http://www.ease-crc.org/ont/SOMA.owl#TaskInvocation -->


    <owl:Class rdf:about="http://www.ease-crc.org/ont/SOMA.owl#TaskInvocation">
        <rdfs:subClassOf rdf:resource="http://www.ontologydesignpatterns.org/ont/dul/DUL.owl#Workflow"/>
        <rdfs:subClassOf>
            <owl:Restriction>
                <owl:onProperty rdf:resource="http://www.ease-crc.org/ont/SOMA.owl#hasBinding"/>
                <owl:allValuesFrom rdf:resource="http://www.ease-crc.org/ont/SOMA.owl#FactualBinding"/>
            </owl:Restriction>
        </rdfs:subClassOf>
        <rdfs:subClassOf>
            <owl:Restriction>
                <owl:onProperty rdf:resource="http://www.ontologydesignpatterns.org/ont/dul/DUL.owl#definesTask"/>
                <owl:qualifiedCardinality rdf:datatype="http://www.w3.org/2001/XMLSchema#nonNegativeInteger">1</owl:qualifiedCardinality>
                <owl:onClass rdf:resource="http://www.ontologydesignpatterns.org/ont/dul/DUL.owl#Task"/>
            </owl:Restriction>
        </rdfs:subClassOf>
        <rdfs:comment>An elementary workflow consisting in the invocation of one single task. It is used as a descriptive context inside of which factual bindings are valid between the task&apos;s arguments and other entities (such as the &quot;local variables&quot; of a larger workflow).</rdfs:comment>
        <rdfs:isDefinedBy rdf:resource="http://www.ease-crc.org/ont/SOMA-WF.owl"/>
        <rdfs:label xml:lang="en">Task invocation</rdfs:label>
    </owl:Class>
    


    <!-- http://www.ease-crc.org/ont/SOMA.owl#Taxis -->


    <owl:Class rdf:about="http://www.ease-crc.org/ont/SOMA.owl#Taxis">
        <rdfs:subClassOf rdf:resource="http://www.ease-crc.org/ont/SOMA.owl#BodyMovement"/>
        <rdfs:comment>An innate behavioural response such as the knee-jerk reflex or the sucking reflex of human infants.</rdfs:comment>
        <rdfs:isDefinedBy rdf:resource="http://www.ease-crc.org/ont/SOMA-PROC.owl"/>
    </owl:Class>
    


    <!-- http://www.ease-crc.org/ont/SOMA.owl#Temperature -->


    <owl:Class rdf:about="http://www.ease-crc.org/ont/SOMA.owl#Temperature">
        <rdfs:subClassOf rdf:resource="http://www.ease-crc.org/ont/SOMA.owl#Intrinsic"/>
        <rdfs:subClassOf>
            <owl:Restriction>
                <owl:onProperty rdf:resource="http://www.ontologydesignpatterns.org/ont/dul/DUL.owl#hasRegion"/>
                <owl:someValuesFrom rdf:resource="http://www.ease-crc.org/ont/SOMA.owl#TemperatureRegion"/>
            </owl:Restriction>
        </rdfs:subClassOf>
        <rdfs:subClassOf>
            <owl:Restriction>
                <owl:onProperty rdf:resource="http://www.ontologydesignpatterns.org/ont/dul/DUL.owl#hasRegion"/>
                <owl:allValuesFrom rdf:resource="http://www.ease-crc.org/ont/SOMA.owl#TemperatureRegion"/>
            </owl:Restriction>
        </rdfs:subClassOf>
        <rdfs:comment>The heat present in an object.</rdfs:comment>
        <rdfs:isDefinedBy rdf:resource="http://www.ease-crc.org/ont/SOMA-OBJ.owl"/>
    </owl:Class>
    


    <!-- http://www.ease-crc.org/ont/SOMA.owl#TemperatureRegion -->


    <owl:Class rdf:about="http://www.ease-crc.org/ont/SOMA.owl#TemperatureRegion">
        <rdfs:subClassOf rdf:resource="http://www.ontologydesignpatterns.org/ont/dul/DUL.owl#Region"/>
        <rdfs:comment>Encodes the temperature of an object.</rdfs:comment>
        <rdfs:isDefinedBy rdf:resource="http://www.ease-crc.org/ont/SOMA-OBJ.owl"/>
        <rdfs:label xml:lang="en">Temperature region</rdfs:label>
    </owl:Class>
    


    <!-- http://www.ease-crc.org/ont/SOMA.owl#Tempering -->


    <owl:Class rdf:about="http://www.ease-crc.org/ont/SOMA.owl#Tempering">
        <rdfs:subClassOf rdf:resource="http://www.ease-crc.org/ont/SOMA.owl#Variability"/>
        <rdfs:subClassOf>
            <owl:Restriction>
                <owl:onProperty rdf:resource="http://www.ease-crc.org/ont/SOMA.owl#affordsSetpoint"/>
                <owl:allValuesFrom>
                    <owl:Restriction>
                        <owl:onProperty rdf:resource="http://www.ontologydesignpatterns.org/ont/dul/DUL.owl#classifies"/>
                        <owl:allValuesFrom rdf:resource="http://www.ease-crc.org/ont/SOMA.owl#Temperature"/>
                    </owl:Restriction>
                </owl:allValuesFrom>
            </owl:Restriction>
        </rdfs:subClassOf>
        <rdfs:comment>The disposition of an object (the tool) to change the temperature of others.</rdfs:comment>
        <rdfs:isDefinedBy rdf:resource="http://www.ease-crc.org/ont/SOMA-HOME.owl"/>
        <rdfs:isDefinedBy rdf:resource="http://www.ease-crc.org/ont/SOMA-OBJ.owl"/>
    </owl:Class>
    


    <!-- http://www.ease-crc.org/ont/SOMA.owl#Text -->


    <owl:Class rdf:about="http://www.ease-crc.org/ont/SOMA.owl#Text">
        <owl:equivalentClass>
            <owl:Class>
                <owl:intersectionOf rdf:parseType="Collection">
                    <rdf:Description rdf:about="http://www.ontologydesignpatterns.org/ont/dul/DUL.owl#InformationObject"/>
                    <owl:Restriction>
                        <owl:onProperty rdf:resource="http://www.ease-crc.org/ont/SOMA.owl#isGivenMeaningBy"/>
                        <owl:someValuesFrom rdf:resource="http://www.ease-crc.org/ont/SOMA.owl#Language"/>
                    </owl:Restriction>
                </owl:intersectionOf>
            </owl:Class>
        </owl:equivalentClass>
        <rdfs:comment xml:lang="en">Any Information Object defined using a Language that, when realized through a symbolic writing system, can be read and made sense of.

One may define Text as anything that can be made sense of, including e.g., Speech or Paintings.

However, the argument can be made that Speech or Paintings are not considered Text as they cannot be EXACTLY realized by a symbolic writing system: Speech may loose punctuation, Paintings their original appearance.
On the other hand, this might not be true as both could be encoded in a binary format that can be interpreted using a language (eg., mp3, png).</rdfs:comment>
        <rdfs:isDefinedBy rdf:resource="http://www.ease-crc.org/ont/SOMA-IO.owl"/>
        <rdfs:label xml:lang="en">Text</rdfs:label>
    </owl:Class>
    


    <!-- http://www.ease-crc.org/ont/SOMA.owl#ThinkAloud -->


    <owl:Class rdf:about="http://www.ease-crc.org/ont/SOMA.owl#ThinkAloud">
        <rdfs:subClassOf rdf:resource="http://www.ease-crc.org/ont/SOMA.owl#CommunicationReport"/>
        <rdfs:comment>A task in which an Agent, while in the course of performing some other task(s), reports on their own decision processes that guide this other task(s) for the benefit of an outside observer.</rdfs:comment>
        <rdfs:isDefinedBy rdf:resource="http://www.ease-crc.org/ont/SOMA-ACT.owl"/>
        <rdfs:label xml:lang="en">Think-aloud</rdfs:label>
    </owl:Class>
    


    <!-- http://www.ease-crc.org/ont/SOMA.owl#ThinkAloudActionTopic -->


    <owl:Class rdf:about="http://www.ease-crc.org/ont/SOMA.owl#ThinkAloudActionTopic">
        <rdfs:subClassOf rdf:resource="http://www.ease-crc.org/ont/SOMA.owl#ThinkAloudTopic"/>
        <rdfs:comment>A topic used when an Agent states what they are doing.</rdfs:comment>
        <rdfs:isDefinedBy rdf:resource="http://www.ease-crc.org/ont/SOMA-ACT.owl"/>
    </owl:Class>
    


    <!-- http://www.ease-crc.org/ont/SOMA.owl#ThinkAloudGeneralKnowledgeTopic -->


    <owl:Class rdf:about="http://www.ease-crc.org/ont/SOMA.owl#ThinkAloudGeneralKnowledgeTopic">
        <rdfs:subClassOf rdf:resource="http://www.ease-crc.org/ont/SOMA.owl#ThinkAloudKnowledgeTopic"/>
        <rdfs:comment>A topic used when an Agent states general knowledge they have.</rdfs:comment>
        <rdfs:isDefinedBy rdf:resource="http://www.ease-crc.org/ont/SOMA-ACT.owl"/>
    </owl:Class>
    


    <!-- http://www.ease-crc.org/ont/SOMA.owl#ThinkAloudKnowledgeTopic -->


    <owl:Class rdf:about="http://www.ease-crc.org/ont/SOMA.owl#ThinkAloudKnowledgeTopic">
        <rdfs:subClassOf rdf:resource="http://www.ease-crc.org/ont/SOMA.owl#ThinkAloudTopic"/>
        <rdfs:comment>A topic used when an Agent states some item of knowledge. This knowledge can be general, or specific to the environment and task at hand.</rdfs:comment>
        <rdfs:isDefinedBy rdf:resource="http://www.ease-crc.org/ont/SOMA-ACT.owl"/>
    </owl:Class>
    


    <!-- http://www.ease-crc.org/ont/SOMA.owl#ThinkAloudObstructionTopic -->


    <owl:Class rdf:about="http://www.ease-crc.org/ont/SOMA.owl#ThinkAloudObstructionTopic">
        <rdfs:subClassOf rdf:resource="http://www.ease-crc.org/ont/SOMA.owl#ThinkAloudTopic"/>
        <rdfs:comment>A topic used when an Agent describes some state of affairs that prevents them from performing an action.</rdfs:comment>
        <rdfs:isDefinedBy rdf:resource="http://www.ease-crc.org/ont/SOMA-ACT.owl"/>
    </owl:Class>
    


    <!-- http://www.ease-crc.org/ont/SOMA.owl#ThinkAloudOpinionTopic -->


    <owl:Class rdf:about="http://www.ease-crc.org/ont/SOMA.owl#ThinkAloudOpinionTopic">
        <rdfs:subClassOf rdf:resource="http://www.ease-crc.org/ont/SOMA.owl#ThinkAloudTopic"/>
        <rdfs:comment>A topic used when an Agent expresses an opinion about the action they perform or the environment they are in.</rdfs:comment>
        <rdfs:isDefinedBy rdf:resource="http://www.ease-crc.org/ont/SOMA-ACT.owl"/>
    </owl:Class>
    


    <!-- http://www.ease-crc.org/ont/SOMA.owl#ThinkAloudPerceptionTopic -->


    <owl:Class rdf:about="http://www.ease-crc.org/ont/SOMA.owl#ThinkAloudPerceptionTopic">
        <rdfs:subClassOf rdf:resource="http://www.ease-crc.org/ont/SOMA.owl#ThinkAloudTopic"/>
        <rdfs:comment>A topic used when an Agent describes what they currently perceive.</rdfs:comment>
        <rdfs:isDefinedBy rdf:resource="http://www.ease-crc.org/ont/SOMA-ACT.owl"/>
    </owl:Class>
    


    <!-- http://www.ease-crc.org/ont/SOMA.owl#ThinkAloudPlanTopic -->


    <owl:Class rdf:about="http://www.ease-crc.org/ont/SOMA.owl#ThinkAloudPlanTopic">
        <rdfs:subClassOf rdf:resource="http://www.ease-crc.org/ont/SOMA.owl#ThinkAloudTopic"/>
        <rdfs:comment>A topic used when an Agent describes what they intend to do. Note, this is not about describing the process through which this plan was constructed; that is covered by the MetaCognitionPlanningTopic.</rdfs:comment>
        <rdfs:isDefinedBy rdf:resource="http://www.ease-crc.org/ont/SOMA-ACT.owl"/>
    </owl:Class>
    


    <!-- http://www.ease-crc.org/ont/SOMA.owl#ThinkAloudSceneKnowledgeTopic -->


    <owl:Class rdf:about="http://www.ease-crc.org/ont/SOMA.owl#ThinkAloudSceneKnowledgeTopic">
        <rdfs:subClassOf rdf:resource="http://www.ease-crc.org/ont/SOMA.owl#ThinkAloudKnowledgeTopic"/>
        <rdfs:comment>A topic used when an Agent describes what they know about their environment, including knowledge of world states that they do not currently perceive.</rdfs:comment>
        <rdfs:isDefinedBy rdf:resource="http://www.ease-crc.org/ont/SOMA-ACT.owl"/>
    </owl:Class>
    


    <!-- http://www.ease-crc.org/ont/SOMA.owl#ThinkAloudTopic -->


    <owl:Class rdf:about="http://www.ease-crc.org/ont/SOMA.owl#ThinkAloudTopic">
        <rdfs:subClassOf rdf:resource="http://www.ease-crc.org/ont/SOMA.owl#CommunicationTopic"/>
        <rdfs:comment>A topic relevant for a think-aloud communication.</rdfs:comment>
        <rdfs:isDefinedBy rdf:resource="http://www.ease-crc.org/ont/SOMA-ACT.owl"/>
        <rdfs:label xml:lang="en">Think aloud topic</rdfs:label>
    </owl:Class>
    


    <!-- http://www.ease-crc.org/ont/SOMA.owl#Throwing -->


    <owl:Class rdf:about="http://www.ease-crc.org/ont/SOMA.owl#Throwing">
        <rdfs:subClassOf rdf:resource="http://www.ease-crc.org/ont/SOMA.owl#Actuating"/>
        <rdfs:subClassOf rdf:resource="http://www.ease-crc.org/ont/SOMA.owl#Manipulating"/>
        <rdfs:comment>A task in which an Agent imparts momentum to an object before releasing it so that it flies for some distance unsupported.</rdfs:comment>
        <rdfs:isDefinedBy rdf:resource="http://www.ease-crc.org/ont/SOMA-ACT.owl"/>
    </owl:Class>
    


    <!-- http://www.ease-crc.org/ont/SOMA.owl#TimeRole -->


    <owl:Class rdf:about="http://www.ease-crc.org/ont/SOMA.owl#TimeRole">
        <rdfs:subClassOf rdf:resource="http://www.ease-crc.org/ont/SOMA.owl#SpatioTemporalRole"/>
        <rdfs:comment>A role filled by a description of the location in time and/or duration of an event or object.</rdfs:comment>
        <rdfs:isDefinedBy rdf:resource="http://www.ease-crc.org/ont/SOMA-OBJ.owl"/>
        <rdfs:label xml:lang="en">Time role</rdfs:label>
    </owl:Class>
    


    <!-- http://www.ease-crc.org/ont/SOMA.owl#Tool -->


    <owl:Class rdf:about="http://www.ease-crc.org/ont/SOMA.owl#Tool">
        <rdfs:subClassOf rdf:resource="http://www.ease-crc.org/ont/SOMA.owl#Instrument"/>
        <rdfs:comment>A role to classify an object used to modify or actuate others.</rdfs:comment>
        <rdfs:isDefinedBy rdf:resource="http://www.ease-crc.org/ont/SOMA-OBJ.owl"/>
    </owl:Class>
    


    <!-- http://www.ease-crc.org/ont/SOMA.owl#Transient -->


    <owl:Class rdf:about="http://www.ease-crc.org/ont/SOMA.owl#Transient">
        <rdfs:subClassOf rdf:resource="http://www.ontologydesignpatterns.org/ont/dul/DUL.owl#Object"/>
        <rdfs:subClassOf>
            <owl:Restriction>
                <owl:onProperty rdf:resource="http://www.ease-crc.org/ont/SOMA.owl#transitionsFrom"/>
                <owl:someValuesFrom rdf:resource="http://www.ontologydesignpatterns.org/ont/dul/DUL.owl#Object"/>
            </owl:Restriction>
        </rdfs:subClassOf>
        <rdfs:comment>Objects may undergo changes during Processes; however, while the change Process is in operation, one cannot strictly say either the input of the Process still exists, nor that the result exists yet.

A prototypical example is making a pancake on a heater. When PancakeMix is put on the hot plate, it ceases to be PancakeMix-- already, the chemical structure of the substance gets altered-- however it is only after sufficient heating that this object becomes a Pancake.

Transients are the objects undergoing such change processes; they are no longer the initial objects fed into the process, nor are they the objects produced as results.

Instead, a Transient transitionsFrom some initial Object that was fed into a change Process. Typically, a Transient may transitionTo some resulting Object (though not always, some processes simply destroy objects).

It is also possible that a Transient transitionsBack to the initial object. An example is the catalyst in a chemical reaction; another example is a loaf of bread after a slice has been cut off.</rdfs:comment>
        <rdfs:isDefinedBy rdf:resource="http://www.ease-crc.org/ont/SOMA-OBJ.owl"/>
    </owl:Class>
    


    <!-- http://www.ease-crc.org/ont/SOMA.owl#Transporting -->


    <owl:Class rdf:about="http://www.ease-crc.org/ont/SOMA.owl#Transporting">
        <rdfs:subClassOf rdf:resource="http://www.ease-crc.org/ont/SOMA.owl#ModifyingPhysicalObject"/>
        <rdfs:comment>A task by which an Agent carries an item from a source to a destination location.</rdfs:comment>
        <rdfs:isDefinedBy rdf:resource="http://www.ease-crc.org/ont/SOMA-ACT.owl"/>
    </owl:Class>
    


    <!-- http://www.ease-crc.org/ont/SOMA.owl#Triplestore -->


    <owl:Class rdf:about="http://www.ease-crc.org/ont/SOMA.owl#Triplestore">
        <rdfs:subClassOf rdf:resource="http://www.ease-crc.org/ont/SOMA.owl#GraphDatabase"/>
        <rdfs:comment xml:lang="en">A Triplestore or RDF store is a purpose-built database for the storage and retrieval of triples through semantic queries.</rdfs:comment>
        <rdfs:isDefinedBy rdf:resource="http://www.ease-crc.org/ont/SOMA-IO.owl"/>
        <rdfs:label xml:lang="en">Triplestore</rdfs:label>
    </owl:Class>
    


    <!-- http://www.ease-crc.org/ont/SOMA.owl#Turning -->


    <owl:Class rdf:about="http://www.ease-crc.org/ont/SOMA.owl#Turning">
        <rdfs:subClassOf rdf:resource="http://www.ease-crc.org/ont/SOMA.owl#PosturalMoving"/>
        <rdfs:comment>A motion by which an agent changes which way their body faces.</rdfs:comment>
        <rdfs:isDefinedBy rdf:resource="http://www.ease-crc.org/ont/SOMA-PROC.owl"/>
    </owl:Class>
    


    <!-- http://www.ease-crc.org/ont/SOMA.owl#UnavailableSoftware -->


    <owl:Class rdf:about="http://www.ease-crc.org/ont/SOMA.owl#UnavailableSoftware">
        <rdfs:subClassOf rdf:resource="http://www.ease-crc.org/ont/SOMA.owl#SoftwareDiagnosis"/>
        <rdfs:comment>A description of a situation where some software dependency is not available.</rdfs:comment>
        <rdfs:isDefinedBy rdf:resource="http://www.ease-crc.org/ont/SOMA-IO.owl"/>
        <rdfs:label xml:lang="en">Unavailable software</rdfs:label>
    </owl:Class>
    


    <!-- http://www.ease-crc.org/ont/SOMA.owl#UndirectedMotion -->


    <owl:Class rdf:about="http://www.ease-crc.org/ont/SOMA.owl#UndirectedMotion">
        <rdfs:subClassOf rdf:resource="http://www.ease-crc.org/ont/SOMA.owl#Motion"/>
        <rdfs:comment>A Motion of a physical Entity for which a destination or path are unknown and/or considered irrelevant; the important aspect about this Motion is simply that it occurs, rather than where it is headed or how it proceeds towards it.</rdfs:comment>
        <rdfs:isDefinedBy rdf:resource="http://www.ease-crc.org/ont/SOMA-PROC.owl"/>
        <rdfs:label>Undirected motion</rdfs:label>
    </owl:Class>
    


    <!-- http://www.ease-crc.org/ont/SOMA.owl#Vaporizing -->


    <owl:Class rdf:about="http://www.ease-crc.org/ont/SOMA.owl#Vaporizing">
        <rdfs:subClassOf rdf:resource="http://www.ease-crc.org/ont/SOMA.owl#PhaseTransition"/>
        <rdfs:subClassOf>
            <owl:Restriction>
                <owl:onProperty rdf:resource="http://www.ease-crc.org/ont/SOMA.owl#isProcessTypeOf"/>
                <owl:someValuesFrom>
                    <owl:Class>
                        <owl:intersectionOf rdf:parseType="Collection">
                            <rdf:Description rdf:about="http://www.ease-crc.org/ont/SOMA.owl#AlteredObject"/>
                            <owl:Restriction>
                                <owl:onProperty rdf:resource="http://www.ontologydesignpatterns.org/ont/dul/DUL.owl#classifies"/>
                                <owl:allValuesFrom rdf:resource="http://www.ontologydesignpatterns.org/ont/dul/DUL.owl#Substance"/>
                            </owl:Restriction>
                        </owl:intersectionOf>
                    </owl:Class>
                </owl:someValuesFrom>
            </owl:Restriction>
        </rdfs:subClassOf>
        <rdfs:comment>Some material transitions from a liquid to a gaseous phase.</rdfs:comment>
        <rdfs:isDefinedBy rdf:resource="http://www.ease-crc.org/ont/SOMA-PROC.owl"/>
        <rdfs:seeAlso>Transitions from a solid to a gaseous phase are usually referred to as Sublimation.</rdfs:seeAlso>
    </owl:Class>
    


    <!-- http://www.ease-crc.org/ont/SOMA.owl#Variability -->


    <owl:Class rdf:about="http://www.ease-crc.org/ont/SOMA.owl#Variability">
        <rdfs:subClassOf rdf:resource="http://www.ease-crc.org/ont/SOMA.owl#Disposition"/>
        <rdfs:subClassOf>
            <owl:Restriction>
                <owl:onProperty rdf:resource="http://www.ease-crc.org/ont/SOMA.owl#affordsBearer"/>
                <owl:allValuesFrom rdf:resource="http://www.ease-crc.org/ont/SOMA.owl#Tool"/>
            </owl:Restriction>
        </rdfs:subClassOf>
        <rdfs:subClassOf>
            <owl:Restriction>
                <owl:onProperty rdf:resource="http://www.ease-crc.org/ont/SOMA.owl#affordsTrigger"/>
                <owl:allValuesFrom rdf:resource="http://www.ease-crc.org/ont/SOMA.owl#AlteredObject"/>
            </owl:Restriction>
        </rdfs:subClassOf>
        <rdfs:comment>The disposition of an object (the tool) to change some aspect of others.</rdfs:comment>
        <rdfs:isDefinedBy rdf:resource="http://www.ease-crc.org/ont/SOMA-OBJ.owl"/>
    </owl:Class>
    


    <!-- http://www.ease-crc.org/ont/SOMA.owl#VideoData -->


    <owl:Class rdf:about="http://www.ease-crc.org/ont/SOMA.owl#VideoData">
        <rdfs:subClassOf rdf:resource="http://www.ontologydesignpatterns.org/ont/dul/DUL.owl#InformationObject"/>
        <rdfs:comment>An information object containing data for audio-visual modalities.</rdfs:comment>
        <rdfs:isDefinedBy rdf:resource="http://www.ease-crc.org/ont/SOMA-NEEM.owl"/>
        <rdfs:label xml:lang="en">Video data</rdfs:label>
    </owl:Class>
    


    <!-- http://www.ease-crc.org/ont/SOMA.owl#Walking -->


    <owl:Class rdf:about="http://www.ease-crc.org/ont/SOMA.owl#Walking">
        <rdfs:subClassOf rdf:resource="http://www.ease-crc.org/ont/SOMA.owl#Locomotion"/>
        <rdfs:comment>An agent, under its own power, moves over some solid surface.</rdfs:comment>
        <rdfs:isDefinedBy rdf:resource="http://www.ease-crc.org/ont/SOMA-PROC.owl"/>
    </owl:Class>
    


    <!-- http://www.ease-crc.org/ont/SOMA.owl#Wall -->


    <owl:Class rdf:about="http://www.ease-crc.org/ont/SOMA.owl#Wall">
        <rdfs:subClassOf rdf:resource="http://www.ease-crc.org/ont/SOMA.owl#RoomSurface"/>
        <rdfs:comment>An upright surface of a building or room.</rdfs:comment>
        <rdfs:isDefinedBy rdf:resource="http://www.ease-crc.org/ont/SOMA-HOME.owl"/>
    </owl:Class>
    


    <!-- http://www.ease-crc.org/ont/SOMA.owl#3DPosition -->


    <owl:Class rdf:about="http://www.ease-crc.org/ont/SOMA.owl#3DPosition">
        <rdfs:subClassOf rdf:resource="http://www.ontologydesignpatterns.org/ont/dul/DUL.owl#SpaceRegion"/>
        <rdfs:subClassOf>
            <owl:Restriction>
                <owl:onProperty rdf:resource="http://www.ease-crc.org/ont/SOMA.owl#hasPositionData"/>
                <owl:qualifiedCardinality rdf:datatype="http://www.w3.org/2001/XMLSchema#nonNegativeInteger">1</owl:qualifiedCardinality>
                <owl:onDataRange rdf:resource="http://www.w3.org/2001/XMLSchema#string"/>
            </owl:Restriction>
        </rdfs:subClassOf>
        <rdfs:comment>A point in three dimensional space, given as translation.</rdfs:comment>
        <rdfs:isDefinedBy rdf:resource="http://www.ease-crc.org/ont/SOMA-OBJ.owl"/>
        <rdfs:label xml:lang="en">3D position</rdfs:label>
    </owl:Class>
    


    <!-- http://www.ease-crc.org/ont/SOMA.owl#6DPose -->


    <owl:Class rdf:about="http://www.ease-crc.org/ont/SOMA.owl#6DPose">
        <rdfs:subClassOf rdf:resource="http://www.ontologydesignpatterns.org/ont/dul/DUL.owl#SpaceRegion"/>
        <rdfs:subClassOf>
            <owl:Restriction>
                <owl:onProperty rdf:resource="http://www.ease-crc.org/ont/SOMA.owl#hasPositionData"/>
                <owl:qualifiedCardinality rdf:datatype="http://www.w3.org/2001/XMLSchema#nonNegativeInteger">1</owl:qualifiedCardinality>
                <owl:onDataRange rdf:resource="http://www.w3.org/2001/XMLSchema#string"/>
            </owl:Restriction>
        </rdfs:subClassOf>
        <rdfs:comment>A point in three dimensional space, given as translation in a reference coordinate system, and an orientation of a coordinate system centered at that point relative to the reference coordinate system.</rdfs:comment>
        <rdfs:isDefinedBy rdf:resource="http://www.ease-crc.org/ont/SOMA-OBJ.owl"/>
        <rdfs:label xml:lang="en">6D pose</rdfs:label>
    </owl:Class>
    


    <!-- http://www.ease-crc.org/ont/SOMA.owl/NonmanifestedSituation -->


    <owl:Class rdf:about="http://www.ease-crc.org/ont/SOMA.owl/NonmanifestedSituation">
        <owl:equivalentClass>
            <owl:Class>
                <owl:intersectionOf rdf:parseType="Collection">
                    <rdf:Description rdf:about="http://www.ontologydesignpatterns.org/ont/dul/DUL.owl#Situation"/>
                    <owl:Restriction>
                        <owl:onProperty rdf:resource="http://www.ease-crc.org/ont/SOMA.owl/manifestsIn"/>
                        <owl:qualifiedCardinality rdf:datatype="http://www.w3.org/2001/XMLSchema#nonNegativeInteger">0</owl:qualifiedCardinality>
                        <owl:onClass rdf:resource="http://www.ontologydesignpatterns.org/ont/dul/DUL.owl#Event"/>
                    </owl:Restriction>
                </owl:intersectionOf>
            </owl:Class>
        </owl:equivalentClass>
        <rdfs:subClassOf rdf:resource="http://www.ontologydesignpatterns.org/ont/dul/DUL.owl#Situation"/>
        <rdfs:comment>A Situation which does not manifest in any event.

The main use case for this is to represent expectations that are not met, e.g. unfulfilled post-conditions of an action. An action with unmet postconditions is then a failure.

Because of open world semantics of DL, the default assumption for a Situation individual with no &quot;manifests in&quot; relations is simply that we don&apos;t know yet whether that Situation is manifested and if so by what Event.

As such, an explicit assertion is needed to make a Situation a nonmanifested one: either declare that individual&apos;s type NonmanifestedSituation, or assert that it has 0 manifestsIn relations.</rdfs:comment>
        <rdfs:isDefinedBy rdf:resource="http://www.ease-crc.org/ont/SOMA-ACT.owl"/>
        <rdfs:label xml:lang="en">Nonmanifested situation</rdfs:label>
    </owl:Class>
    


    <!-- http://www.ontologydesignpatterns.org/ont/dul/DUL.owl#Agent -->


    <owl:Class rdf:about="http://www.ontologydesignpatterns.org/ont/dul/DUL.owl#Agent">
        <rdfs:comment xml:lang="en">Generally, agents are goal-directed entities that are able to monitor their environment to select and perform efficient means-ends actions that are available in a given situation to achieve an intended goal. Agency, therefore, implies the ability to perceive and to change the environment of the agent. Crucially, it also entails intentionality to represent the goal-state in the future, equifinal variability to be able to achieve the intended goal-state with different actions in different contexts, and rationality of actions in relation to their goal to produce the most efficient action available (Source: https://en.wikipedia.org/wiki/Agency_(psychology)).

While we follow this definition, we do so loosely: We do not require the intentionality to be sourced by the agent. E.g., a running computer program (see Software instance) can be seen as an actor and therefore participate in Actions, e.g. some Communication Action, while its intentionality has been bestowed upon it from the agents who started the program or gave an input (e.g., via a mouse click) to achieve some goal.</rdfs:comment>
        <rdfs:isDefinedBy rdf:resource="http://www.ease-crc.org/ont/SOMA-STATE.owl"/>
    </owl:Class>
    


    <!-- http://www.ontologydesignpatterns.org/ont/dul/DUL.owl#Concept -->


    <owl:Class rdf:about="http://www.ontologydesignpatterns.org/ont/dul/DUL.owl#Concept">
        <rdfs:isDefinedBy rdf:resource="http://www.ease-crc.org/ont/SOMA-WF.owl"/>
    </owl:Class>
    


    <!-- http://www.ontologydesignpatterns.org/ont/dul/DUL.owl#Description -->


    <owl:Class rdf:about="http://www.ontologydesignpatterns.org/ont/dul/DUL.owl#Description">
        <rdfs:isDefinedBy rdf:resource="http://www.ease-crc.org/ont/SOMA-PROC.owl"/>
        <rdfs:isDefinedBy rdf:resource="http://www.ease-crc.org/ont/SOMA-STATE.owl"/>
        <rdfs:isDefinedBy rdf:resource="http://www.ease-crc.org/ont/SOMA-WF.owl"/>
    </owl:Class>
    


    <!-- http://www.ontologydesignpatterns.org/ont/dul/DUL.owl#Design -->


    <owl:Class rdf:about="http://www.ontologydesignpatterns.org/ont/dul/DUL.owl#Design">
        <rdfs:isDefinedBy rdf:resource="http://www.ease-crc.org/ont/SOMA-OBJ.owl"/>
    </owl:Class>
    


    <!-- http://www.ontologydesignpatterns.org/ont/dul/DUL.owl#DesignedArtifact -->


    <owl:Class rdf:about="http://www.ontologydesignpatterns.org/ont/dul/DUL.owl#DesignedArtifact">
        <rdfs:isDefinedBy rdf:resource="http://www.ease-crc.org/ont/SOMA-HOME.owl"/>
    </owl:Class>
    


    <!-- http://www.ontologydesignpatterns.org/ont/dul/DUL.owl#DesignedSubstance -->


    <owl:Class rdf:about="http://www.ontologydesignpatterns.org/ont/dul/DUL.owl#DesignedSubstance">
        <rdfs:isDefinedBy rdf:resource="http://www.ease-crc.org/ont/SOMA-HOME.owl"/>
    </owl:Class>
    


    <!-- http://www.ontologydesignpatterns.org/ont/dul/DUL.owl#Entity -->


    <owl:Class rdf:about="http://www.ontologydesignpatterns.org/ont/dul/DUL.owl#Entity">
        <rdfs:isDefinedBy rdf:resource="http://www.ease-crc.org/ont/SOMA-WF.owl"/>
    </owl:Class>
    


    <!-- http://www.ontologydesignpatterns.org/ont/dul/DUL.owl#Event -->


    <owl:Class rdf:about="http://www.ontologydesignpatterns.org/ont/dul/DUL.owl#Event">
        <rdfs:isDefinedBy rdf:resource="http://www.ease-crc.org/ont/SOMA-STATE.owl"/>
    </owl:Class>
    


    <!-- http://www.ontologydesignpatterns.org/ont/dul/DUL.owl#EventType -->


    <owl:Class rdf:about="http://www.ontologydesignpatterns.org/ont/dul/DUL.owl#EventType">
        <rdfs:isDefinedBy rdf:resource="http://www.ease-crc.org/ont/SOMA-PROC.owl"/>
        <rdfs:isDefinedBy rdf:resource="http://www.ease-crc.org/ont/SOMA-STATE.owl"/>
    </owl:Class>
    


    <!-- http://www.ontologydesignpatterns.org/ont/dul/DUL.owl#Parameter -->


    <owl:Class rdf:about="http://www.ontologydesignpatterns.org/ont/dul/DUL.owl#Parameter">
        <rdfs:isDefinedBy rdf:resource="http://www.ease-crc.org/ont/SOMA-WF.owl"/>
    </owl:Class>
    


    <!-- http://www.ontologydesignpatterns.org/ont/dul/DUL.owl#PhysicalAgent -->


    <owl:Class rdf:about="http://www.ontologydesignpatterns.org/ont/dul/DUL.owl#PhysicalAgent">
        <rdfs:isDefinedBy rdf:resource="http://www.ease-crc.org/ont/SOMA-PROC.owl"/>
    </owl:Class>
    


    <!-- http://www.ontologydesignpatterns.org/ont/dul/DUL.owl#PhysicalArtifact -->


    <owl:Class rdf:about="http://www.ontologydesignpatterns.org/ont/dul/DUL.owl#PhysicalArtifact">
        <rdfs:isDefinedBy rdf:resource="http://www.ease-crc.org/ont/SOMA-PROC.owl"/>
    </owl:Class>
    


    <!-- http://www.ontologydesignpatterns.org/ont/dul/DUL.owl#PhysicalObject -->


    <owl:Class rdf:about="http://www.ontologydesignpatterns.org/ont/dul/DUL.owl#PhysicalObject">
        <rdfs:isDefinedBy rdf:resource="http://www.ease-crc.org/ont/SOMA-PROC.owl"/>
        <rdfs:isDefinedBy rdf:resource="http://www.ease-crc.org/ont/SOMA-STATE.owl"/>
    </owl:Class>
    


    <!-- http://www.ontologydesignpatterns.org/ont/dul/DUL.owl#Process -->


    <owl:Class rdf:about="http://www.ontologydesignpatterns.org/ont/dul/DUL.owl#Process">
        <rdfs:isDefinedBy rdf:resource="http://www.ease-crc.org/ont/SOMA-PROC.owl"/>
    </owl:Class>
    


    <!-- http://www.ontologydesignpatterns.org/ont/dul/DUL.owl#Relation -->


    <owl:Class rdf:about="http://www.ontologydesignpatterns.org/ont/dul/DUL.owl#Relation">
        <rdfs:isDefinedBy rdf:resource="http://www.ease-crc.org/ont/SOMA-WF.owl"/>
    </owl:Class>
    


    <!-- http://www.ontologydesignpatterns.org/ont/dul/DUL.owl#Role -->


    <owl:Class rdf:about="http://www.ontologydesignpatterns.org/ont/dul/DUL.owl#Role">
        <rdfs:isDefinedBy rdf:resource="http://www.ease-crc.org/ont/SOMA-PROC.owl"/>
        <rdfs:isDefinedBy rdf:resource="http://www.ease-crc.org/ont/SOMA-STATE.owl"/>
        <rdfs:isDefinedBy rdf:resource="http://www.ease-crc.org/ont/SOMA-WF.owl"/>
    </owl:Class>
    


    <!-- http://www.ontologydesignpatterns.org/ont/dul/DUL.owl#Situation -->


    <owl:Class rdf:about="http://www.ontologydesignpatterns.org/ont/dul/DUL.owl#Situation">
        <rdfs:subClassOf>
            <owl:Class>
                <owl:complementOf>
                    <owl:Class>
                        <owl:intersectionOf rdf:parseType="Collection">
                            <owl:Restriction>
                                <owl:onProperty rdf:resource="http://www.ease-crc.org/ont/SOMA.owl/manifestsIn"/>
                                <owl:someValuesFrom rdf:resource="http://www.ontologydesignpatterns.org/ont/dul/DUL.owl#Event"/>
                            </owl:Restriction>
                            <owl:Restriction>
                                <owl:onProperty rdf:resource="http://www.ease-crc.org/ont/SOMA.owl/prevents"/>
                                <owl:someValuesFrom>
                                    <owl:Restriction>
                                        <owl:onProperty rdf:resource="http://www.ease-crc.org/ont/SOMA.owl/manifestsIn"/>
                                        <owl:someValuesFrom rdf:resource="http://www.ontologydesignpatterns.org/ont/dul/DUL.owl#Event"/>
                                    </owl:Restriction>
                                </owl:someValuesFrom>
                            </owl:Restriction>
                        </owl:intersectionOf>
                    </owl:Class>
                </owl:complementOf>
            </owl:Class>
        </rdfs:subClassOf>
        <rdfs:isDefinedBy rdf:resource="http://www.ease-crc.org/ont/SOMA-PROC.owl"/>
    </owl:Class>
    


    <!-- http://www.ontologydesignpatterns.org/ont/dul/DUL.owl#Substance -->


    <owl:Class rdf:about="http://www.ontologydesignpatterns.org/ont/dul/DUL.owl#Substance">
        <rdfs:isDefinedBy rdf:resource="http://www.ease-crc.org/ont/SOMA-HOME.owl"/>
        <rdfs:isDefinedBy rdf:resource="http://www.ease-crc.org/ont/SOMA-PROC.owl"/>
    </owl:Class>
    


    <!-- http://www.ontologydesignpatterns.org/ont/dul/DUL.owl#Task -->


    <owl:Class rdf:about="http://www.ontologydesignpatterns.org/ont/dul/DUL.owl#Task">
        <rdfs:isDefinedBy rdf:resource="http://www.ease-crc.org/ont/SOMA-WF.owl"/>
    </owl:Class>
    


    <!-- http://www.ontologydesignpatterns.org/ont/dul/DUL.owl#Workflow -->


    <owl:Class rdf:about="http://www.ontologydesignpatterns.org/ont/dul/DUL.owl#Workflow">
        <rdfs:isDefinedBy rdf:resource="http://www.ease-crc.org/ont/SOMA-WF.owl"/>
    </owl:Class>
    


    <!-- 
    ///////////////////////////////////////////////////////////////////////////////////////
    //
    // Individuals
    //
    ///////////////////////////////////////////////////////////////////////////////////////
     -->


    


    <!-- http://www.ease-crc.org/ont/SOMA.owl#ExecutionState_Active -->


    <owl:NamedIndividual rdf:about="http://www.ease-crc.org/ont/SOMA.owl#ExecutionState_Active">
        <rdf:type rdf:resource="http://www.ease-crc.org/ont/SOMA.owl#ExecutionStateRegion"/>
        <rdfs:comment>The execution state of an ongoing activity.</rdfs:comment>
        <rdfs:isDefinedBy rdf:resource="http://www.ease-crc.org/ont/SOMA-ACT.owl"/>
    </owl:NamedIndividual>
    


    <!-- http://www.ease-crc.org/ont/SOMA.owl#ExecutionState_Cancelled -->


    <owl:NamedIndividual rdf:about="http://www.ease-crc.org/ont/SOMA.owl#ExecutionState_Cancelled">
        <rdf:type rdf:resource="http://www.ease-crc.org/ont/SOMA.owl#ExecutionStateRegion"/>
        <rdfs:comment>The execution state of a cancelled activity.</rdfs:comment>
        <rdfs:isDefinedBy rdf:resource="http://www.ease-crc.org/ont/SOMA-ACT.owl"/>
    </owl:NamedIndividual>
    


    <!-- http://www.ease-crc.org/ont/SOMA.owl#ExecutionState_Failed -->


    <owl:NamedIndividual rdf:about="http://www.ease-crc.org/ont/SOMA.owl#ExecutionState_Failed">
        <rdf:type rdf:resource="http://www.ease-crc.org/ont/SOMA.owl#ExecutionStateRegion"/>
        <rdfs:comment>The execution state of a failed activity.</rdfs:comment>
        <rdfs:isDefinedBy rdf:resource="http://www.ease-crc.org/ont/SOMA-ACT.owl"/>
    </owl:NamedIndividual>
    


    <!-- http://www.ease-crc.org/ont/SOMA.owl#ExecutionState_Paused -->


    <owl:NamedIndividual rdf:about="http://www.ease-crc.org/ont/SOMA.owl#ExecutionState_Paused">
        <rdf:type rdf:resource="http://www.ease-crc.org/ont/SOMA.owl#ExecutionStateRegion"/>
        <rdfs:comment>The execution state of a paused activity.</rdfs:comment>
        <rdfs:isDefinedBy rdf:resource="http://www.ease-crc.org/ont/SOMA-ACT.owl"/>
    </owl:NamedIndividual>
    


    <!-- http://www.ease-crc.org/ont/SOMA.owl#ExecutionState_Pending -->


    <owl:NamedIndividual rdf:about="http://www.ease-crc.org/ont/SOMA.owl#ExecutionState_Pending">
        <rdf:type rdf:resource="http://www.ease-crc.org/ont/SOMA.owl#ExecutionStateRegion"/>
        <rdfs:comment>The execution state of a pending activity.</rdfs:comment>
        <rdfs:isDefinedBy rdf:resource="http://www.ease-crc.org/ont/SOMA-ACT.owl"/>
    </owl:NamedIndividual>
    


    <!-- http://www.ease-crc.org/ont/SOMA.owl#ExecutionState_Succeeded -->


    <owl:NamedIndividual rdf:about="http://www.ease-crc.org/ont/SOMA.owl#ExecutionState_Succeeded">
        <rdf:type rdf:resource="http://www.ease-crc.org/ont/SOMA.owl#ExecutionStateRegion"/>
        <rdfs:comment>The execution state of a succeeded activity.</rdfs:comment>
        <rdfs:isDefinedBy rdf:resource="http://www.ease-crc.org/ont/SOMA-ACT.owl"/>
    </owl:NamedIndividual>
    


    <!-- http://www.ease-crc.org/ont/SOMA.owl#FailWFNoContinuation -->


    <owl:NamedIndividual rdf:about="http://www.ease-crc.org/ont/SOMA.owl#FailWFNoContinuation">
        <rdf:type rdf:resource="http://www.ease-crc.org/ont/SOMA.owl#StatusFailure"/>
        <rdfs:comment>A particular kind of failure: the workflow fails because there is no way to continue it, and the normal exit has not been reached.</rdfs:comment>
        <rdfs:isDefinedBy rdf:resource="http://www.ease-crc.org/ont/SOMA-WF.owl"/>
    </owl:NamedIndividual>
    


    <!-- http://www.ease-crc.org/ont/SOMA.owl#FailWFNondeterministicContinuation -->


    <owl:NamedIndividual rdf:about="http://www.ease-crc.org/ont/SOMA.owl#FailWFNondeterministicContinuation">
        <rdf:type rdf:resource="http://www.ease-crc.org/ont/SOMA.owl#StatusFailure"/>
        <rdfs:comment>A particular kind of failure: it is not clear how to continue a workflow because several possibilities exist.</rdfs:comment>
        <rdfs:isDefinedBy rdf:resource="http://www.ease-crc.org/ont/SOMA-WF.owl"/>
    </owl:NamedIndividual>
    


    <!-- http://www.ease-crc.org/ont/SOMA.owl#FailWFUninterpretableTask -->


    <owl:NamedIndividual rdf:about="http://www.ease-crc.org/ont/SOMA.owl#FailWFUninterpretableTask">
        <rdf:type rdf:resource="http://www.ease-crc.org/ont/SOMA.owl#StatusFailure"/>
        <rdfs:comment>A particular kind of failure: a task is not recognized and not associated to anything that could execute it, nor to a workflow that could detail its structure into simpler structure.</rdfs:comment>
        <rdfs:isDefinedBy rdf:resource="http://www.ease-crc.org/ont/SOMA-WF.owl"/>
    </owl:NamedIndividual>
    


    <!-- 
    ///////////////////////////////////////////////////////////////////////////////////////
    //
    // General axioms
    //
    ///////////////////////////////////////////////////////////////////////////////////////
     -->


    <owl:Axiom>
        <owl:annotatedSource>
            <owl:Class>
                <owl:intersectionOf rdf:parseType="Collection">
                    <rdf:Description rdf:about="http://www.ease-crc.org/ont/SOMA.owl#SituationTransition"/>
                    <owl:Restriction>
                        <owl:onProperty rdf:resource="http://www.ease-crc.org/ont/SOMA.owl/manifestsIn"/>
                        <owl:someValuesFrom rdf:resource="http://www.ontologydesignpatterns.org/ont/dul/DUL.owl#Event"/>
                    </owl:Restriction>
                </owl:intersectionOf>
                <rdfs:subClassOf rdf:nodeID="genid539"/>
            </owl:Class>
        </owl:annotatedSource>
        <owl:annotatedProperty rdf:resource="http://www.w3.org/2000/01/rdf-schema#subClassOf"/>
        <owl:annotatedTarget rdf:nodeID="genid539"/>
        <rdfs:comment>If a SituationTransition manifests in some Event, then it also has an initial Situation and a terminal one.</rdfs:comment>
    </owl:Axiom>
    <owl:Class rdf:nodeID="genid539">
        <owl:intersectionOf rdf:parseType="Collection">
            <owl:Restriction>
                <owl:onProperty rdf:resource="http://www.ease-crc.org/ont/SOMA.owl#hasInitialSituation"/>
                <owl:someValuesFrom rdf:resource="http://www.ontologydesignpatterns.org/ont/dul/DUL.owl#Situation"/>
            </owl:Restriction>
            <owl:Restriction>
                <owl:onProperty rdf:resource="http://www.ease-crc.org/ont/SOMA.owl#hasTerminalSituation"/>
                <owl:someValuesFrom rdf:resource="http://www.ontologydesignpatterns.org/ont/dul/DUL.owl#Situation"/>
            </owl:Restriction>
        </owl:intersectionOf>
    </owl:Class>
    <owl:Axiom>
        <owl:annotatedSource>
            <owl:Class>
                <owl:intersectionOf rdf:parseType="Collection">
                    <rdf:Description rdf:about="http://www.ease-crc.org/ont/SOMA.owl#SituationTransition"/>
                    <owl:Restriction>
                        <owl:onProperty rdf:resource="http://www.ease-crc.org/ont/SOMA.owl/manifestsIn"/>
                        <owl:someValuesFrom rdf:resource="http://www.ontologydesignpatterns.org/ont/dul/DUL.owl#Event"/>
                    </owl:Restriction>
                </owl:intersectionOf>
                <rdfs:subClassOf rdf:nodeID="genid549"/>
            </owl:Class>
        </owl:annotatedSource>
        <owl:annotatedProperty rdf:resource="http://www.w3.org/2000/01/rdf-schema#subClassOf"/>
        <owl:annotatedTarget rdf:nodeID="genid549"/>
        <rdfs:comment>A SituationTransition that manifests in some Event also includes an Action. (NOTE (MP): Typically, the Event manifesting it would be that included Action actually so perhaps we can just require that manifestations of SituationTransitions be Actions?)</rdfs:comment>
    </owl:Axiom>
    <owl:Restriction rdf:nodeID="genid549">
        <owl:onProperty rdf:resource="http://www.ontologydesignpatterns.org/ont/dul/DUL.owl#includesEvent"/>
        <owl:someValuesFrom rdf:resource="http://www.ontologydesignpatterns.org/ont/dul/DUL.owl#Action"/>
    </owl:Restriction>
    <owl:Axiom>
        <owl:annotatedSource>
            <owl:Restriction>
                <owl:onProperty rdf:resource="http://www.ease-crc.org/ont/SOMA.owl#hasInitialSituation"/>
                <owl:someValuesFrom rdf:resource="http://www.ontologydesignpatterns.org/ont/dul/DUL.owl#Situation"/>
                <rdfs:subClassOf rdf:nodeID="genid552"/>
            </owl:Restriction>
        </owl:annotatedSource>
        <owl:annotatedProperty rdf:resource="http://www.w3.org/2000/01/rdf-schema#subClassOf"/>
        <owl:annotatedTarget rdf:nodeID="genid552"/>
        <rdfs:comment>If a transition has an initial situation then it also has a manifestation.</rdfs:comment>
    </owl:Axiom>
    <owl:Restriction rdf:nodeID="genid552">
        <owl:onProperty rdf:resource="http://www.ease-crc.org/ont/SOMA.owl/manifestsIn"/>
        <owl:someValuesFrom rdf:resource="http://www.ontologydesignpatterns.org/ont/dul/DUL.owl#Event"/>
    </owl:Restriction>
    <owl:Axiom>
        <owl:annotatedSource>
            <owl:Restriction>
                <owl:onProperty rdf:resource="http://www.ease-crc.org/ont/SOMA.owl#hasTerminalSituation"/>
                <owl:someValuesFrom rdf:resource="http://www.ontologydesignpatterns.org/ont/dul/DUL.owl#Situation"/>
                <rdfs:subClassOf rdf:nodeID="genid555"/>
            </owl:Restriction>
        </owl:annotatedSource>
        <owl:annotatedProperty rdf:resource="http://www.w3.org/2000/01/rdf-schema#subClassOf"/>
        <owl:annotatedTarget rdf:nodeID="genid555"/>
        <rdfs:comment>If a transition has a terminal situation then it also has a manifestation.</rdfs:comment>
    </owl:Axiom>
    <owl:Restriction rdf:nodeID="genid555">
        <owl:onProperty rdf:resource="http://www.ease-crc.org/ont/SOMA.owl/manifestsIn"/>
        <owl:someValuesFrom rdf:resource="http://www.ontologydesignpatterns.org/ont/dul/DUL.owl#Event"/>
    </owl:Restriction>
    <owl:Restriction>
        <owl:onProperty rdf:resource="http://www.ease-crc.org/ont/SOMA.owl/manifestsIn"/>
        <owl:someValuesFrom rdf:resource="http://www.ontologydesignpatterns.org/ont/dul/DUL.owl#Event"/>
        <rdfs:subClassOf>
            <owl:Class>
                <owl:complementOf>
                    <owl:Class>
                        <owl:intersectionOf rdf:parseType="Collection">
                            <owl:Restriction>
                                <owl:onProperty rdf:resource="http://www.ontologydesignpatterns.org/ont/dul/DUL.owl#hasPrecondition"/>
                                <owl:someValuesFrom rdf:resource="http://www.ease-crc.org/ont/SOMA.owl/NonmanifestedSituation"/>
                            </owl:Restriction>
                        </owl:intersectionOf>
                    </owl:Class>
                </owl:complementOf>
            </owl:Class>
        </rdfs:subClassOf>
    </owl:Restriction>
</rdf:RDF>



<!-- Generated by the OWL API (version 5.1.20.2022-02-19T16:38:31Z) https://github.com/owlcs/owlapi/ -->


